# baseURI: http://anzsoil.org/def/au/asc/
# imports: http://purl.org/dc/elements/1.1/
# imports: http://www.w3.org/2004/02/skos/core
# prefix: asc

@prefix asc: <http://anzsoil.org/def/au/asc/> .
@prefix dc: <http://purl.org/dc/elements/1.1/> .
@prefix dcterms: <http://purl.org/dc/terms/> .
@prefix owl: <http://www.w3.org/2002/07/owl#> .
@prefix rdf: <http://www.w3.org/1999/02/22-rdf-syntax-ns#> .
@prefix rdfs: <http://www.w3.org/2000/01/rdf-schema#> .
@prefix skos: <http://www.w3.org/2004/02/skos/core#> .
@prefix xsd: <http://www.w3.org/2001/XMLSchema#> .

asc:
  a owl:Ontology ;
  dcterms:contributor <https://orcid.org/0000-0002-3884-3420> ;
  dcterms:created "2016-06-23"^^xsd:date ;
  dcterms:creator <mailto:asris@csiro.au> ;
  dcterms:description "The Australian Soil Classification provides a framework for organising knowledge about Australian soils by allocating soils to classes via a key." ;
  dcterms:license <http://creativecommons.org/licences/by/4.0> ;
  dcterms:modified "2021-11-18" ;
  dcterms:publisher <http://www.publish.csiro.au/> ;
  dcterms:rights "copyright CSIRO 2009, 2016, 2021. All rights reserved." ;
  dcterms:source "Isbell, R.F. (1996;2002;2016;2021) The Australian Soil Classification (3rd edn). CSIRO Publishing, Melbourne" ;
  dcterms:title "The Australian Soil Classification (ASC)" ;
  rdfs:seeAlso "https://www.publish.csiro.au/book/8016" ;
  owl:imports dc: ;
  owl:imports <http://www.w3.org/2004/02/skos/core> ;
.
asc:A
  a asc:Class ;
  a asc:Thickness ;
  skos:definition "< 0.1 m" ;
  skos:notation "A" ;
  skos:prefLabel "Thin" ;
.
asc:AA
  a asc:ColourClass ;
  a skos:Concept ;
  dcterms:identifier "http://anzsoil.org/def/au/asc/AA"^^xsd:anyURI ;
  skos:notation "AA" ;
  skos:prefLabel "Red" ;
.
asc:AB
  a asc:ColourClass ;
  a skos:Concept ;
  dcterms:identifier "http://anzsoil.org/def/au/asc/AB"^^xsd:anyURI ;
  skos:notation "AB" ;
  skos:prefLabel "Brown" ;
.
asc:AC
  a asc:ColourClass ;
  a skos:Concept ;
  dcterms:identifier "http://anzsoil.org/def/au/asc/AC"^^xsd:anyURI ;
  skos:notation "AC" ;
  skos:prefLabel "Yellow" ;
.
asc:AD
  a asc:ColourClass ;
  a skos:Concept ;
  dcterms:identifier "http://anzsoil.org/def/au/asc/AD"^^xsd:anyURI ;
  skos:notation "AD" ;
  skos:prefLabel "Grey" ;
.
asc:AE
  a asc:ColourClass ;
  a skos:Concept ;
  dcterms:identifier "http://anzsoil.org/def/au/asc/AE"^^xsd:anyURI ;
  skos:notation "AE" ;
  skos:prefLabel "Black" ;
.
asc:AF
  a asc:Class ;
  skos:definition "[CH] Soils in which the major part of the B2t horizon is dystrophic." ;
  skos:definition "[DE] Soils in which the major part of the B2 horizon is dystrophic." ;
  skos:definition "[FE] Soils in which the major part of the B2 horizon is dystrophic." ;
  skos:definition "[HY] Soils in which the major part of the B2 horizon is dystrophic." ;
  skos:definition "[KA] Soils in which the major part of the B2 horizon is dystrophic." ;
  skos:definition "[KU] Soils in which the major part of the B2t horizon is dystrophic." ;
  skos:definition "[SO] Soils in which the major part of the B2t horizon is dystrophic." ;
  skos:notation "AF" ;
  skos:prefLabel "Dystrophic" ;
.
asc:AG
  a asc:Class ;
  skos:definition "[CH] Soils in which the major part of the B2t horizon is mesotrophic." ;
  skos:definition "[DE] Soils in which the major part of the B2 horizon is mesotrophic." ;
  skos:definition "[FE] Soils in which the major part of the B2 horizon is mesotrophic." ;
  skos:definition "[HY] Soils in which the major part of the B2 horizon is mesotrophic." ;
  skos:definition "[KA] Soils in which the major part of the B2 horizon is mesotrophic." ;
  skos:definition "[KU] Soils in which the major part of the B2t horizon is mesotrophic." ;
  skos:definition "[SO] Soils in which the major part of the B2t horizon is mesotrophic." ;
  skos:notation "AG" ;
  skos:prefLabel "Mesotrophic" ;
.
asc:AH
  a asc:Class ;
  skos:definition "[CH] Soils in which the major part of the B2t horizon is eutrophic but the B and BC horizons are not calcareous." ;
  skos:definition "[DE] Soils in which the major part of the B2 horizon is eutrophic but the B and BC horizons are not calcareous." ;
  skos:definition "[FE] Soils in which the major part of the B2 horizon is eutrophic but the B and BC horizons are not calcareous." ;
  skos:definition "[HY] Soils in which the major part of the B2 horizon is eutrophic but the B and BC horizons are not calcareous." ;
  skos:definition "[KA] Soils in which the major part of the B2 horizon is eutrophic but the B and BC horizons are not calcareous." ;
  skos:definition "[KU] Soils in which the major part of the B2t horizon is eutrophic." ;
  skos:definition "[SO] Soils in which the major part of the B2t horizon is eutrophic but the B and BC horizons are not calcareous." ;
  skos:notation "AH" ;
  skos:prefLabel "Eutrophic" ;
.
asc:AI
  a asc:Class ;
  a skos:Concept ;
  dcterms:identifier "http://anzsoil.org/def/au/asc/AI"^^xsd:anyURI ;
  skos:definition "[DE] Other soils with a B2 horizon in which the major part is strongly acid." ;
  skos:definition "[FE] Soils with a B2 horizon in which the major part is strongly acid." ;
  skos:definition "[HY] Other soils with a B2 horizon in which the major part is strongly acid." ;
  skos:definition "[KA] Other soils with a B2 horizon in which the major part is strongly acid." ;
  skos:definition "[OR] Soils in which the major part of the organic materials is strongly acid." ;
  skos:definition "[RE] Soils in which the major part of the upper 1.0 m of the soil profile is strongly acid." ;
  skos:definition "[RU] Soils in which the major part is strongly acid." ;
  skos:definition "[TE] Soils in which the major part of the solum is strongly acid." ;
  skos:notation "AI" ;
  skos:prefLabel "Acidic  " ;
.
asc:AJ
  a asc:Class ;
  skos:definition "[DE] Soils in which the major part of the B2 horizon is strongly acid and mottled." ;
  skos:definition "[KA] Soils in which the major part of the B2 horizon is strongly acid and mottled." ;
  skos:notation "AJ" ;
  skos:prefLabel "Acidic-Mottled" ;
.
asc:AK
  a asc:Class ;
  a skos:Concept ;
  dcterms:identifier "http://anzsoil.org/def/au/asc/AK"^^xsd:anyURI ;
  skos:definition "[KA] Soils that have andic properties and have formed in basaltic tephric materials that may be visibly stratified." ;
  skos:definition "[RE] Soils which have andic properties and have formed in basaltic tephric materials that may be visibly stratified." ;
  skos:definition "[TE] Soils which have andic properties and has formed in basaltic tephric materials that may be visibly stratified." ;
  skos:notation "AK" ;
  skos:prefLabel "Andic " ;
.
asc:AL
  a asc:Class ;
  a skos:Concept ;
  skos:definition "[PO] Soils with free drainage, ie. rapidly drained. There is no restriction to through drainage in the B horizon or within the substrate. There is no perching of water within the B horizon or saturation due to a high ground water table. The B horizons are weakly coherent and porous. They are often brightly coloured, and lack evidence of seasonal reduction." ;
  skos:notation "AL" ;
  skos:prefLabel "Aeric" ;
.
asc:AM
  a asc:Class ;
  a skos:Concept ;
  skos:definition "[PO] Soils with long-term saturation in the B horizons. The saturation may be caused as in the semiaquic soils but the duration is of the order of months. The period of saturation is sufficient to reduce most iron compounds and move them out of the B horizon, hence Bh horizons are usually prominent." ;
  skos:definition "[VE] Soils with stagnant water on the soil surface and/or saturation of some part of the upper 0.5 m more or less continuously for prolonged periods in most years. The length of a 'prolonged period' is probably in the order of 2-3 continuous months. Evidence of wetness may be indicated by the presence of mottling and gley colours (chroma of 2 or less)." ;
  skos:notation "AM" ;
  skos:prefLabel "Aquic" ;
.
asc:AN
  a asc:Order ;
  a skos:Concept ;
  asc:suborder asc:HR ;
  asc:suborder asc:HS ;
  asc:suborder asc:HT ;
  asc:suborder asc:HU ;
  asc:suborder asc:HV ;
  asc:suborder asc:HW ;
  asc:suborder asc:HX ;
  asc:suborder asc:IT ;
  asc:suborder-comment """In the Garbic, Urbic and some Spolic soils it is common practice to cover the anthropic materials with a layer of soil materials as an aid to reclamation. This soil material is regarded as part of the suborder and can be used as a basis for lower category classification. In other situations sewage sludge is being used to rehabilitate mine spoil.

The Scalpic soils may also have material added to their new surface. If this is less than 0.3 m there would be, for example, a spolic phase of the Scalpic suborder; if 0.3 m or more thick the soil would classify as a Spolic suborder.

There will obviously be intergrade situations between some of the suborders. For example, it may sometimes be difficult to decide between Garbic and Urbic, Cumulic and Hortic. In these and similar situations judgement and/or knowledge of the process will be required. With the increasing emphasis on recycling, much of the garbic materials will be composted so the garbic group could become redundant.

Another likely difficult situation results when human-induced or human-accelerated erosion has removed upper soil horizons. On present thinking it would seem more appropriate for such soils to be regarded as an eroded phase of say a Sodosol, provided the original soil can be identified.

The question of soils contaminated by toxic wastes is also unresolved. They could be included in the Garbic suborder, but if the wastes are toxic to plant and animal life their host materials cannot strictly be regarded as soil. In some situations the problem could be overcome by referring to the site as a contaminated phase of the pre-existing soil. Similarly the application of liquid wastes, bore water and other irrigation waters may alter the chemical and physical properties of soil substantially. For example, salts, acids, alkalis, suspended organic matter, nutrients and toxins in applied liquids may affect the pH, salinity, sodicity and fertility of the soil. These soils could be identified as a phase of the pre-existing soils e.g. saline phase, sodic phase or alkaline phase.

Lower Categories

It is hoped that the seven suborders will provide a conceptual framework for the classification of most anthropic soils based on human-induced processes which provide particular kinds of soil parent materials. The suborders are a simplified relevant summary of an almost infinitely large range of anthropic processes and products. The need for subdivision below the suborder level is likely to be more desirable in some classes than others, but a major problem in creating lower category classes is the lack of data on the morphology and laboratory properties of anthropic soils. Most information seems to be available for the spolic soils created by mining operations. Here though it may be more appropriate to create a technical classification based on reclamation needs.

For some of the suborders, differentiae for lower categories could be based on appropriate traditional attributes used in classifying 'natural' soils, both morphologic and laboratory-determined. At present this is impractical due to the lack of an adequate representative profile data base. A related approach is to use at the great group level classes based on the other orders eg. Chromosolic, Sodosolic etc. as has been done for the Hydrosol great groups. In this approach Rudosolic Spolic Anthroposols would obviously be a very common class. A wide range of options is available for subgroup differentiae, but existing family criteria will probably be appropriate for most Anthroposols. A preliminary approach to classifying Australian minesoils based on proposed amendments to Soil Taxonomy has been made by Fitzpatrick and Hollingsworth (1994). A number of their proposed subgroups could be used in Spolic Anthroposols, and some examples are given in their paper.

Until more knowledge and experience is available, it is proposed not to formalise the classification of Anthroposols below the suborder level. Acknowledgment is due to Fanning and Fanning (1989) for a number of the concepts and terminology used in this preliminary classification of Anthroposols.""" ;
  dcterms:description """These soils result from human activities which have caused a profound modification, mixing, truncation or burial of the original soil horizons, or the creation of new soil parent materials. Note that the concept of soil used in this classification of Australian soils (see Background) also applies to the Anthroposols, and hence sealed and semi-sealed surfaces such as streets, roads etc. are regarded as 'non-soil'. Also, in depositional situations, the anthropic material must be 0.3 m or more thick where it overlies buried soils. A soil with anthropic materials less than 0.3 m thick should be classified as an anthropic phase of the underlying soil.

To qualify as soil an Anthroposol needs to possess some pedogenic features, as noted below. Key criteria in the identification of an Anthroposol are the presence of artefacts in the profile or knowledge that the soils or their parent materials have been made or altered by human action.

Anthroposols differ from other soils in that we normally know their origin with a degree of certainty, and hence we can invoke a knowledge of process rather than defined pedogenic attributes to initially classify the soil. We can then subdivide at the higher levels on the basis of type of process and nature of the product which forms the parent material of the new soil. At lower levels in the classification, conventional soil properties could be used when available, although obviously these will be limited in very young soils.""" ;
  dcterms:identifier "http://anzsoil.org/def/au/asc/AN"^^xsd:anyURI ;
  rdfs:comment """It is difficult to quantify ‘profound modification, mixing and truncation’ but this would normally exclude the usual agricultural operations (including land planning) which may change a soil from say a Chromosol to a Dermosol by mixing or removal of the upper horizons. Similarly, soils that are artificially drained or flooded are not Anthroposols but may classify as different soil orders following a permanent change in water status (see also comment in Hydrosols).

There will be instances where the question is how much truncation results in ‘profound modification’ or merely a truncated phase. It is difficult to give guidelines that will cover all circumstances, and inevitably judgement is required. Similarly, there will be instances where land reclamation and restoration in the past have been so successful that little evidence of a prior disturbance remains, and soil development gives no clue to past history. A good example of this is Podosol development on restored and revegetated coastal dunes following sand mining.""" ;
  skos:definition "Soils resulting from human activities which have led to a profound modification, truncation or burial of the original soil horizons, or the creation of new soil parent materials by a variety of mechanical means. Where burial of a pre-existing soil is involved, the anthropic materials must be 0.3 m or more thick. Pedogenic features may be the result of in situ processes (usually the minimal development of an A1 horizon, sometimes the stronger development of typical soil horizons) or the result of pedogenic processes prior to modification or placement (ie. the presence of identifiable pre-existing soil material)." ;
  skos:narrower asc:AN-HR ;
  skos:narrower asc:AN-HS ;
  skos:narrower asc:AN-HT ;
  skos:narrower asc:AN-HU ;
  skos:narrower asc:AN-HV ;
  skos:narrower asc:AN-HW ;
  skos:narrower asc:AN-HX ;
  skos:narrower asc:AN-IT ;
  skos:notation "AN" ;
  skos:prefLabel "Anthroposols" ;
.
asc:AN-HR
  a asc:Suborder ;
  asc:classifier asc:HR ;
  skos:broader asc:AN ;
  skos:notation "AN-HR" ;
  skos:prefLabel "Cumulic Anthroposol" ;
.
asc:AN-HS
  a asc:Suborder ;
  asc:classifier asc:HS ;
  skos:broader asc:AN ;
  skos:notation "AN-HS" ;
  skos:prefLabel "Hortic Anthroposol" ;
.
asc:AN-HT
  a asc:Suborder ;
  asc:classifier asc:HT ;
  skos:broader asc:AN ;
  skos:notation "AN-HT" ;
  skos:prefLabel "Garbic Anthroposol" ;
.
asc:AN-HU
  a asc:Suborder ;
  asc:classifier asc:HU ;
  skos:broader asc:AN ;
  skos:notation "AN-HU" ;
  skos:prefLabel "Urbic Anthroposol" ;
.
asc:AN-HV
  a asc:Suborder ;
  asc:classifier asc:HV ;
  skos:broader asc:AN ;
  skos:notation "AN-HV" ;
  skos:prefLabel "Dredgic Anthroposol" ;
.
asc:AN-HW
  a asc:Suborder ;
  asc:classifier asc:HW ;
  skos:broader asc:AN ;
  skos:notation "AN-HW" ;
  skos:prefLabel "Spolic Anthroposol" ;
.
asc:AN-HX
  a asc:Suborder ;
  asc:classifier asc:HX ;
  skos:broader asc:AN ;
  skos:notation "AN-HX" ;
  skos:prefLabel "Scalpic Anthroposol" ;
.
asc:AN-IT
  a asc:Suborder ;
  asc:classifier asc:IT ;
  skos:broader asc:AN ;
  skos:notation "AN-IT" ;
  skos:prefLabel "Fusic Anthroposol" ;
.
asc:AO
  a asc:Class ;
  a skos:Concept ;
  dcterms:identifier "http://anzsoil.org/def/au/asc/AO"^^xsd:anyURI ;
  skos:definition "[RU] Soils in which the profile is not or only slightly gravelly (<10% >2 mm) throughout, either loose or only weakly coherent both moist and dry, and the texture is dominantly sandy (i.e. field textures of S-LS-CS) and there is no layer with a clay content of >15% (i.e. field texture of SL+ or heavier). Aeolian cross-bedding may be present but there is little if any evidence of other stratification or buried soils." ;
  skos:definition "[TE] Soils in which the profile is not or only slightly gravelly (<20% >2mm) throughout, the soil material is either loose or only weakly coherent both moist and dry, may have aeolian cross bedding, and the texture is dominantly sandy (i.e. field textures of S-LS-CS) in >80% of the profile and no layer with a clay content of >15% (i.e. field texture of SL+)." ;
  skos:notation "AO" ;
  skos:prefLabel "Arenic " ;
.
asc:AP
  a asc:Class ;
  a skos:Concept ;
  dcterms:identifier "http://anzsoil.org/def/au/asc/AP"^^xsd:anyURI ;
  skos:definition "[CA] Soils with an argic horizon within the B horizon." ;
  skos:definition "[KA] oils with an argic horizon within the B horizon." ;
  skos:definition "[RE] Soils with an argic horizon within the B horizon." ;
  skos:definition "[RE] Soils with an argic horizon." ;
  skos:definition "[TE] Soils with an argic horizon within the solum." ;
  skos:notation "AP" ;
  skos:prefLabel "Argic " ;
.
asc:AQ
  a asc:Class ;
  skos:definition "[HY] Soils that are dominantly clay-sized to a depth of 0.5 m." ;
  skos:notation "AQ" ;
  skos:prefLabel "Argillaceous" ;
.
asc:AR
  a asc:Class ;
  a skos:Concept ;
  dcterms:identifier "http://anzsoil.org/def/au/asc/AR"^^xsd:anyURI ;
  skos:definition "[OR] Soils in which the major part of the organic materials is not calcareous but is not strongly acid." ;
  skos:definition "[RE] Other soils which are not strongly acid or calcareous." ;
  skos:definition "[RU] Soils that are not calcareous and the major part is not strongly acid." ;
  skos:definition "[TE] Soils in which the major part of the solum is not strongly acid and no part of the solum is calcareous." ;
  skos:notation "AR" ;
  skos:prefLabel "Basic  " ;
.
asc:AS
  a asc:Class ;
  a skos:Concept ;
  dcterms:identifier "http://anzsoil.org/def/au/asc/AS"^^xsd:anyURI ;
  skos:definition "[KA] Soils with a bauxitic horizon within the B horizon." ;
  skos:definition "[RE] Soils with a bauxitic horizon." ;
  skos:definition "[RU] Soils in which the gravelly materials contain a bauxitic horizon." ;
  skos:definition "[TE] Soils with a bauxitic horizon." ;
  skos:notation "AS" ;
  skos:prefLabel "Bauxitic  " ;
.
asc:AT
  a asc:Class ;
  a skos:Concept ;
  dcterms:identifier "http://anzsoil.org/def/au/asc/AT"^^xsd:anyURI ;
  skos:definition "[CH] Other soils with a conspicuously bleached A2 horizon." ;
  skos:definition "[DE] Other soils with a conspicuously bleached A2 horizon." ;
  skos:definition "[HY] Other soils with a conspicuously bleached A2 horizon." ;
  skos:definition "[KA] Other soils with a conspicuously bleached A2 horizon." ;
  skos:definition "[KU] Other soils with a conspicuously bleached A2 horizon." ;
  skos:definition "[RE] Soils with a conspicuously bleached A2 horizon." ;
  skos:definition "[TE] Soils with a conspicuously bleached A2 horizon." ;
  skos:definition "[VE] Soils with a conspicuously bleached A2 horizon." ;
  skos:notation "AT" ;
  skos:prefLabel "Bleached " ;
.
asc:AU
  a asc:Class ;
  skos:definition "[DE] Soils with a conspicuously bleached A2 horizon and a B2 horizon in which the major part is strongly acid." ;
  skos:definition "[HY] Soils with a conspicuously bleached A2 horizon and a B2 horizon in which the major part is strongly acid." ;
  skos:definition "[KA] Soils with a conspicuously bleached A2 horizon and a B2 horizon in which the major part is strongly acid." ;
  skos:notation "AU" ;
  skos:prefLabel "Bleached-Acidic" ;
.
asc:AV
  a asc:Class ;
  skos:definition "[CH] Soils with a conspicuously bleached A2 horizon and a ferric horizon within the solum." ;
  skos:definition "[DE] Soils with a conspicuously bleached A2 horizon and a ferric horizon within the solum." ;
  skos:definition "[HY] Soils with a conspicuously bleached A2 horizon and a ferric horizon within the soil profile." ;
  skos:definition "[KA] Soils with a conspicuously bleached A2 horizon and a ferric horizon within the solum." ;
  skos:definition "[KU] Soils with a conspicuously bleached A2 horizon and a ferric horizon within the solum." ;
  skos:notation "AV" ;
  skos:prefLabel "Bleached-Ferric" ;
.
asc:AW
  a asc:Class ;
  a skos:Concept ;
  dcterms:identifier "http://anzsoil.org/def/au/asc/AW"^^xsd:anyURI ;
  skos:definition "[TE] Soils with a conspicuously bleached A2 horizon, and are underlain within 0.5 m of the surface by a calcrete pan ; hard unweathered rock or other hard materials; or partially weathered or decomposed rock or saprolite." ;
  skos:notation "AW" ;
  skos:prefLabel "Bleached-Leptic" ;
.
asc:AX
  a asc:Class ;
  skos:definition "[HY] Soils with a conspicuously bleached A2 horizon and a B2 horizon in which the major part has an exchangeable Ca/Mg ratio of less than 0.1." ;
  skos:notation "AX" ;
  skos:prefLabel "Bleached-Magnesic" ;
.
asc:AY
  a asc:Class ;
  a skos:Concept ;
  dcterms:identifier "http://anzsoil.org/def/au/asc/AY"^^xsd:anyURI ;
  skos:definition "[CH] Soils with a conspicuously bleached A2 horizon and a manganic horizon within the solum." ;
  skos:definition "[DE] Soils with a conspicuously bleached A2 horizon and a manganic horizon within the solum." ;
  skos:definition "[HY] Soils with a conspicuously bleached A2 horizon and a manganic horizon within the soil profile." ;
  skos:definition "[KA] Soils with a conspicuously bleached A2 horizon and a manganic horizon within the solum." ;
  skos:definition "[KU] Soils with a conspicuously bleached A2 horizon and a manganic horizon within the solum." ;
  skos:definition "[TE] Soils with a conspicuously bleached A2 horizon and a manganic horizon within the solum." ;
  skos:notation "AY" ;
  skos:prefLabel "Bleached-Manganic" ;
.
asc:AZ
  a asc:Class ;
  skos:definition "[CH] Soils with a conspicuously bleached A2 horizon and the major part of the B2t horizon is mottled." ;
  skos:definition "[DE] Soils with a conspicuously bleached A2 horizon and the major part of the B2 horizon is mottled." ;
  skos:definition "[KA] Soils with a conspicuously bleached A2 horizon and the major part of the B2 horizon is mottled." ;
  skos:definition "[KU] Soils with a conspicuously bleached A2 horizon and the major part of the B2t horizon is mottled." ;
  skos:notation "AZ" ;
  skos:prefLabel "Bleached-Mottled" ;
.
asc:Alteration
  a owl:Class ;
  rdfs:subClassOf asc:Class ;
  skos:prefLabel "Nature of altered organic materials" ;
.
asc:B
  a asc:Class ;
  a asc:Thickness ;
  skos:altLabel "Moderately thick" ;
  skos:definition "[OR] 0.1–<0.3 m" ;
  skos:notation "B" ;
  skos:prefLabel "Medium" ;
.
asc:BA
  a asc:Class ;
  skos:definition "[CH] Soils with a conspicuously bleached A2 horizon and a B horizon in which at least the lower part is sodic." ;
  skos:definition "[DE] Soils with a conspicuously bleached A2 horizon and a B horizon in which at least the lower part is sodic." ;
  skos:definition "[HY] Soils with a conspicuously bleached A2 horizon and a B horizon in which at least the lower part is sodic." ;
  skos:definition "[KA] Soils with a conspicuously bleached A2 horizon and a B horizon in which at least the lower part is sodic." ;
  skos:definition "[KU] Soils with a conspicuously bleached A2 horizon and a B horizon in which at least the lower part is sodic." ;
  skos:notation "BA" ;
  skos:prefLabel "Bleached-Sodic" ;
.
asc:BB
  a asc:Class ;
  skos:definition "[CH] Soils with a conspicuously bleached A2 horizon overlying a B horizon in which at least 0.3m has vertic properties." ;
  skos:definition "[DE] Soils with a conspicuously bleached A2 horizon and a B horizon in which at least 0.3m has vertic properties." ;
  skos:definition "[HY] Soils with a conspicuously bleached A2 horizon and a B horizon in which at least 0.3m has vertic properties." ;
  skos:definition "[KU] Soils with a conspicuously bleached A2 horizon and a B horizon in which at least 0.3 m has vertic properties." ;
  skos:notation "BB" ;
  skos:prefLabel "Bleached-Vertic" ;
.
asc:BC
  a asc:Class ;
  a skos:Concept ;
  dcterms:identifier "http://anzsoil.org/def/au/asc/BC"^^xsd:anyURI ;
  skos:definition "[FE] Soils in which at least some part of the B or the BC horizon is calcareous." ;
  skos:definition "[HY] Soils in which at least some part of the B or the BC horizon is calcareous." ;
  skos:definition "[OR] Soils in which the major part of the organic materials is calcareous." ;
  skos:definition "[RE] Soils in which at least some part of the upper 1 m of the soil profile is calcareous." ;
  skos:definition "[RU] Soil that at least in some part are calcareous." ;
  skos:definition "[TE] Other soils in which at least some part of the solum is calcareous." ;
  skos:notation "BC" ;
  skos:prefLabel "Calcareous   " ;
.
asc:BD
  a asc:Class ;
  a skos:Concept ;
  skos:definition "[CA] Other soils with a calcareous horizon. (See carbonate classes)." ;
  skos:definition "[CH] Other soils with a calcareous horizon. (See carbonate classes)." ;
  skos:definition "[DE] Other soils with a calcareous horizon. (See carbonate classes)." ;
  skos:definition "[KA] Other soils with a calcareous horizon. (See carbonate classes)." ;
  skos:definition "[RE] Other soils with a calcareous horizon containing fine earth carbonate." ;
  skos:definition "[SO] Other soils with a calcareous horizon. (See carbonate classes)." ;
  skos:notation "BD" ;
  skos:prefLabel "Calcic" ;
.
asc:BE
  a asc:Class ;
  a skos:Concept ;
  dcterms:identifier "http://anzsoil.org/def/au/asc/BE"^^xsd:anyURI ;
  skos:definition "[RE] Soils with a peaty, humose, melacic or melanic horizon. A conspicuously bleached A2 horizon is not present." ;
  skos:definition "[TE] Soils with a peaty, humose, melacic or melanic horizon. A conspicuously bleached A2 horizon is not present." ;
  skos:notation "BE" ;
  skos:prefLabel "Chernic" ;
.
asc:BF
  a asc:Class ;
  a skos:Concept ;
  dcterms:identifier "http://anzsoil.org/def/au/asc/BF"^^xsd:anyURI ;
  skos:definition "[TE] Soils with a peaty, humose, melacic or melanic horizon, and are underlain within 0.5 m of the surface by a calcrete pan; hard unweathered rock or other hard materials; or partially weathered or decomposed rock or saprolite. An unbleached A2 horizon may be present between the dark surface horizons and the substrate material." ;
  skos:notation "BF" ;
  skos:prefLabel "Chernic-Leptic" ;
.
asc:BG
  a asc:Class ;
  skos:definition "[HY] Other soils with a <clear or abrupt textural B horizon and the pHw in the major part of the upper 0.2 m of the B2 horizon is not strongly acid." ;
  skos:definition "[HY] Other soils with a clear or abrupt textural B horizon and the pHw in the major part of the upper 0.2 m of the B2 horizon is not strongly acid." ;
  skos:notation "BG" ;
  skos:prefLabel "Chromosolic" ;
.
asc:BH
  a asc:Class ;
  skos:definition "[VE] Soils with a massive or weakly structured surface crusty horizon 30 mm or less thick, often of lighter texture (lower clay content) than the underlying pedal clay (blocky or polyhedral) which is not self-mulching." ;
  skos:notation "BH" ;
  skos:prefLabel "Crusty" ;
.
asc:BI
  a asc:Class ;
  skos:definition "[PO] Other soils with a densipan present in the A2 horizon." ;
  skos:notation "BI" ;
  skos:prefLabel "Densic" ;
.
asc:BJ
  a asc:Class ;
  a skos:Concept ;
  dcterms:identifier "http://anzsoil.org/def/au/asc/BJ"^^xsd:anyURI ;
  skos:definition "[CA] Soils that directly overlie a red-brown hardpan." ;
  skos:definition "[CH] Soils with a red-brown hardpan either within or directly underlying the B horizon." ;
  skos:definition "[DE] Soils with a red-brown hardpan either within or directly underlying the B horizon." ;
  skos:definition "[KA] Soils with a red-brown hardpan either within or directly underlying the B horizon." ;
  skos:definition "[RE] Other soils which overlie a red-brown hardpan." ;
  skos:definition "[RE] Soils that directly overlie a red-brown hardpan." ;
  skos:definition "[RU] Soils that directly overlie a red-brown hardpan." ;
  skos:definition "[SO] Soils with a red-brown hardpan either within or directly underlying the B horizon." ;
  skos:definition "[TE] Soils which overlie a red-brown hardpan." ;
  skos:definition "[VE] Soils with a red-brown hardpan either within or directly underlying the B horizon." ;
  skos:notation "BJ" ;
  skos:prefLabel "Duric " ;
.
asc:BK
  a asc:Class ;
  skos:definition "[CH] Soils in which the upper 0.2 m of the B2t horizon (or the B2t horizon if it is less than 0.2 m thick) has a strong blocky or polyhedral structure in which average ped size is usually in the range of 5 - 20 mm. There is very weak adhesion between peds (when dry it is very easy to insert a spade into the upper B2t horizon). Salt contents are usually high, resulting in weak dry strength and a bulk density of about 1.3 t m-3 or less. In some soils the B2t horizon may be weakly subplastic. A common feature (but not diagnostic) of the overlying A horizons is the presence of a band of vesicular pores near the surface or on the underside of any surface flake." ;
  skos:definition "[DE] Soils in which the upper 0.2 m of the B2 horizon (or the B2 horizon if it is less than 0.2 m thick) has a strong blocky or polyhedral structure in which average ped size is usually in the range of 5-20 mm. There is very weak adhesion between peds (when dry it is very easy to insert a spade into the upper B2 horizon). Salt contents are usually high, resulting in weak dry strength and a bulk density of about 1.3 t m-3 less. In some soils the B2 horizons may be weakly subplastic. A common feature (but not diagnostic) of the overlying A horizons is the presence of a band of vesicular pores near the surface or on the underside of any surface flake." ;
  skos:definition "[SO] Soils in which the upper 0.2 m of the B2t horizon (or the B2t horizon if it is less than 0.2 m thick) has a strong blocky or polyhedral structure in which average ped size is usually in the range of 5-20 mm. There is very weak adhesion between peds (when dry it is very easy to insert a spade into the upper B2t horizon). Salt contents are usually high, resulting in weak dry strength and a bulk density of about 1.3 t m-3 or less. In some soils the B2t horizons may be weakly subplastic. A common feature (but not diagnostic) of the overlying A horizons is the presence of a band of vesicular pores near the surface or on the underside of any surface flake." ;
  skos:notation "BK" ;
  skos:prefLabel "Pedaric" ;
.
asc:BL
  a asc:Class ;
  skos:definition "[VE] Other soils in which the major part of the solum below 0.5 m is strongly acid." ;
  skos:notation "BL" ;
  skos:prefLabel "Endoacidic" ;
.
asc:BN
  a asc:Class ;
  skos:definition "[VE] Other soils in which the upper 0.1 m of the solum is sodic." ;
  skos:notation "BN" ;
  skos:prefLabel "Episodic" ;
.
asc:BP
  a asc:Class ;
  skos:definition "[CA] Soils in which an ESP of 15 or greater occurs in some subhorizon below 0.5 m." ;
  skos:definition "[VE] Other soils in which some subhorizon of the solum below 0.5 m has an ESP of 15 or greater." ;
  skos:notation "BP" ;
  skos:prefLabel "Endohypersodic" ;
.
asc:BR
  a asc:Class ;
  skos:definition "[CA] Soils in which at least some subhorizon within the upper 0.5 m of the solum has an ESP of 15 or greater." ;
  skos:definition "[VE] Other soils in which some subsurface horizon within the upper 0.5 m of the solum has an ESP of 15 or greater." ;
  skos:notation "BR" ;
  skos:prefLabel "Epihypersodic" ;
.
asc:BT
  a asc:Class ;
  a skos:Concept ;
  skos:definition "[HY] Soils of the extratidal zone (usually supporting grassland). Tidal inundation is infrequent and achieved only by exceptional storm or cyclonic tides (above high spring tides). Freshwater inundation is seasonally common." ;
  skos:notation "BT" ;
  skos:prefLabel "Extratidal" ;
.
asc:BU
  a asc:Class ;
  a skos:Concept ;
  dcterms:identifier "http://anzsoil.org/def/au/asc/BU"^^xsd:anyURI ;
  skos:definition "[CH] Other soils with a ferric horizon within the solum." ;
  skos:definition "[DE] Other soils with a ferric horizon within the solum." ;
  skos:definition "[FE] Other soils with a ferric horizon within the solum." ;
  skos:definition "[HY] Other soils with a ferric horizon within the soil profile." ;
  skos:definition "[KA] Other soils with a ferric horizon within the solum." ;
  skos:definition "[KU] Other soils with a ferric horizon within the solum." ;
  skos:definition "[PO] Soils with a ferric horizon within the B horizon." ;
  skos:definition "[RE] Other soils with a ferric horizon." ;
  skos:definition "[RU] Soils in which the gravelly materials contain a ferric horizon." ;
  skos:definition "[SO] Soils with a ferric horizon within the solum." ;
  skos:definition "[TE] Soils with a ferric horizon." ;
  skos:definition "[VE] Soils with a ferric horizon within the solum" ;
  skos:notation "BU" ;
  skos:prefLabel "Ferric " ;
.
asc:BV
  a asc:Class ;
  skos:definition "[HY] Soils that are dominantly sand-sized to a depth of 0.5 m." ;
  skos:notation "BV" ;
  skos:prefLabel "Arenaceous" ;
.
asc:BW
  a asc:Class ;
  a skos:Concept ;
  skos:definition "[HY] Soils in which the organic materials are dominated by fibric peat." ;
  skos:definition "[OR] Soils in which the dominant organic material, by thickness, is fibric peat." ;
  skos:notation "BW" ;
  skos:prefLabel "Fibric" ;
.
asc:BX
  a asc:Class ;
  skos:definition "[RU] Soils in which the gravel consists dominantly of mostly rounded materials that have been transported by streams or by wave action." ;
  skos:notation "BX" ;
  skos:prefLabel "Fluvic" ;
.
asc:BY
  a asc:Class ;
  skos:definition "[PO] Other soils with a weakly coherent B horizon." ;
  skos:notation "BY" ;
  skos:prefLabel "Fragic" ;
.
asc:BZ
  a asc:Class ;
  skos:definition "[CA] Soils with a gypsic horizon within the B or BC horizon." ;
  skos:definition "[CH] Soils with a gypsic horizon within the B or BC horizon." ;
  skos:definition "[DE] Soils with a gypsic horizon within the B or BC horizon." ;
  skos:definition "[HY] Soils with a gypsic horizon within the upper 0.5 m of the profile." ;
  skos:definition "[RE] Soils with a gypsic horizon in the upper 1.0 m of the soil profile." ;
  skos:definition "[RE] Soils with a gypsic horizon within the upper 1.0 m of the soil profile." ;
  skos:definition "[RE} Soils with a gypsic horizon." ;
  skos:definition "[RU] Soils with a gypsic horizon that occurs within the upper 0.5 m of the profile." ;
  skos:definition "[SO] Soils with a gypsic horizon within the B or BC horizon." ;
  skos:definition "[VE] Other soils with a gypsic horizon within the B or BC horizon." ;
  skos:notation "BZ" ;
  skos:prefLabel "Gypsic" ;
.
asc:C
  a asc:Class ;
  a asc:Thickness ;
  skos:definition "[OR] 0.3–0.6 m" ;
  skos:notation "C" ;
  skos:prefLabel "Thick" ;
.
asc:CA
  a asc:Order ;
  a skos:Concept ;
  dcterms:description "The soils in this Order are usually calcareous throughout the profile, often highly so. They constitute a widespread and important group of soils in southern Australia." ;
  dcterms:identifier "http://anzsoil.org/def/au/asc/CA"^^xsd:anyURI ;
  rdfs:comment """A difficulty may arise in separating those Calcarosols that are not calcareous throughout from calcareous Kandosols and from Tenosols containing pedogenic carbonate. However, in the latter two soils it is usual for the carbonate to occur in the lower part of the B horizon, and not immediately below the A horizon. Even so, transitional cases will arise where it becomes a matter of judgement as to which order the particular soil is best placed. Similar transitions might occur between shallow Calcarosols and Arenic Rudosols overlying a layer of calcrete or limestone. Again, Calcareous Arenic Rudosols will occur where recent aeolian calcareous material has been deposited.

In landscapes dominated by wind-blown calcareous material it may be difficult to determine if the carbonates are of pedogenic origin. Deep calcareous sands, which commonly occur in this situation, are now included in the Arenosols order.

Soils with minimal soil development and dominated by coarse fragments of shells or other aquatic animals are included in Shelly Rudosols.

In dune landscapes, where these soils frequently occur, it is common to find evidence of post-European settlement deflation and layering of soil profiles caused by wind erosion and consequent deposition. Unless the surface depositional material is 0.3 m or more thick, it is ignored in the classification and treated as a phase. (see 'What do we classify?').""" ;
  skos:definition """Soils that:

1. Are either calcareous throughout the solum - or calcareous at least directly below the A1 or Ap horizon, or within a depth of 0.2 m (whichever is shallower). Carbonate accumulations must be judged to be pedogenic1, ie. are a result of soil forming processes in situ (either current or relict). Soils dominated by non-pedogenic calcareous materials such as fragments of limestone or shells are excluded. See also calcrete, and
2. Do not have deep sandy profiles that have a field texture of sand, loamy sand or clayey sand in 80% or more of the upper 1.0 m.""" ;
  skos:notation "CA" ;
  skos:prefLabel "Calcarosols" ;
.
asc:CB
  a asc:Class ;
  skos:definition "[HY] Soils that are calcareous throughout the soil profile, or at least below the A1 horizon or to a depth of 0.2 m if the A1 horizon is only weakly developed, and do not have a clear or abrupt textural B horizon." ;
  skos:definition "[HY] Soils which are calcareous throughout the soil profile, or at least below the A1 or Ap horizon or to a depth of 0.2 m if the A1 horizon is only weakly developed, and do not have a clear or abrupt textural B horizon." ;
  skos:notation "CB" ;
  skos:prefLabel "Calcarosolic" ;
.
asc:CC
  a asc:Class ;
  skos:definition "[HY] Soils in which the major part of the upper 0.5 m of the profile consists of materials dominated (>50%) by halite crystals." ;
  skos:definition "[RE] The major part of the upper 0.5 m of the soil profile consists of materials dominated (>50%) by halite crystals." ;
  skos:definition "[RU] The major part of the upper 0.5 m of the profile consists of materials dominated (>50%) by halite crystals." ;
  skos:notation "CC" ;
  skos:prefLabel "Halic" ;
.
asc:CD
  a asc:Class ;
  skos:definition "[CH] Other soils in which the major part of the B2t horizon is whole coloured." ;
  skos:definition "[DE} Soils in which the major part of the B2 horizon is whole coloured." ;
  skos:definition "[FE] Soils in which the major part of the B2 horizon is whole coloured." ;
  skos:definition "[HY] Soils in which the major part of the upper 0.5 m of the profile is whole coloured." ;
  skos:definition "[KA] Other soils in which the major part of the B2 horizon is whole coloured." ;
  skos:definition "[KU] Other soils in which the major part of the B2t horizon is whole coloured." ;
  skos:definition "[VE] Other soils in which the major part of the upper 0.5 m of the solum is whole coloured." ;
  skos:notation "CD" ;
  skos:prefLabel "Haplic" ;
.
asc:CE
  a asc:Class ;
  a skos:Concept ;
  skos:definition "[HY] Soils in which the organic materials, other than fibric peat, are dominated by hemic peat." ;
  skos:definition "[OR] Soils in which the dominant organic material, by thickness, is hemic peat." ;
  skos:notation "CE" ;
  skos:prefLabel "Hemic" ;
.
asc:CF
  a asc:Class ;
  skos:definition "[HY] Soils which are dominated by organic materials to a depth of 0.5 m." ;
  skos:notation "CF" ;
  skos:prefLabel "Histic" ;
.
asc:CG
  a asc:Class ;
  skos:definition "[PO] Soils with only a Bh horizon." ;
  skos:definition "[PO] Soils with only a Bh/Basi horizon." ;
  skos:notation "CG" ;
  skos:prefLabel "Humic" ;
.
asc:CH
  a asc:Order ;
  a skos:Concept ;
  dcterms:description "Soils with strong texture contrast between A horizons and B horizons. The latter are not strongly acid and are not sodic. The soils of this order are among the most widespread soils used for agriculture in Australia, particularly those with red subsoils." ;
  dcterms:identifier "http://anzsoil.org/def/au/asc/CH"^^xsd:anyURI ;
  rdfs:comment "In the case of those soils with strongly subplastic B horizons, care needs to be taken to ensure if they qualify for the clear or abrupt textural B horizon. As far as is presently known, such soils appear to be largely confined to the Riverine Plain of south eastern Australia." ;
  skos:definition "Soils other than Hydrosols with a clear or abrupt textural B horizon and in which the major part of the upper 0.2 m of the B2t horizon (or the major part of the entire B2t horizon if it is less than 0.2 m thick) is not sodic and not strongly acid. Soils with strongly subplastic upper B2t horizons are also included even if they are sodic." ;
  skos:notation "CH" ;
  skos:prefLabel "Chromosols" ;
.
asc:CI
  a asc:Class ;
  skos:definition "[PO] oils with a Bh/Bhs horizon." ;
  skos:notation "CI" ;
  skos:prefLabel "Humic/Humosesquic" ;
.
asc:CJ
  a asc:Class ;
  skos:definition "[PO] Soils with a Bh/Bs horizon." ;
  skos:notation "CJ" ;
  skos:prefLabel "Humic/Sesquic" ;
.
asc:CK
  a asc:Class ;
  a skos:Concept ;
  dcterms:identifier "http://anzsoil.org/def/au/asc/CK"^^xsd:anyURI ;
  skos:definition "[CH] Other soils with a humose horizon." ;
  skos:definition "[DE] Other soils with a humose horizon." ;
  skos:definition "[FE] Other soils with a humose horizon." ;
  skos:definition "[HY] Other soils with a humose horizon." ;
  skos:definition "[KA] Other soils with a humose horizon." ;
  skos:definition "[KU] Other soils with a humose horizon." ;
  skos:definition "[PO] Other soils with a humose horizon." ;
  skos:definition "[RE] Other soils with a humose horizon" ;
  skos:definition "[SO] Soils with a humose horizon." ;
  skos:definition "[TE] Soils with a humose horizon." ;
  skos:notation "CK" ;
  skos:prefLabel "Humose  " ;
.
asc:CL
  a asc:Class ;
  skos:definition "[HY] Soils with a humose horizon and a B2 horizon in which the major part has an exchangeable Ca/Mg ratio of less than 0.1." ;
  skos:notation "CL" ;
  skos:prefLabel "Humose-Magnesic" ;
.
asc:CM
  a asc:Class ;
  skos:definition "[CH] Soils with a humose horizon and the major part of the B2t horizon is mottled." ;
  skos:definition "[DE] Soils with a humose horizon and the major part of the B2 horizon is mottled." ;
  skos:definition "[KA] Soils with a humose horizon and the major part of the B2 horizon is mottled." ;
  skos:notation "CM" ;
  skos:prefLabel "Humose-Mottled" ;
.
asc:CN
  a asc:Class ;
  skos:definition "[PO] Soils with a humose horizon and a strongly coherent B horizon." ;
  skos:notation "CN" ;
  skos:prefLabel "Humose-Parapanic" ;
.
asc:CO
  a asc:Class ;
  skos:definition "[PO] Soils with only a Bhs horizon." ;
  skos:notation "CO" ;
  skos:prefLabel "Humosesquic" ;
.
asc:CP
  a asc:Class ;
  skos:definition "[CA] Soils in which the upper 0.1 m of the solum consists of more than 20% fine earth carbonate (visual estimate using a 10 x hand lens), and/or has a strong effervescence with 1 M HC1, and/or contains more than 8%2 (by analysis) of fine earth carbonate." ;
  skos:definition "[RE] Soils in which the upper 0.1 m of the soil profile consists of more than 20% fine-earth carbonate (visual estimate using a 10 x hand lens), and/or has a strong effervescence with 1 M HC1, and/or contains more than 8% 1 (by analysis) of fine-earth carbonate." ;
  skos:notation "CP" ;
  skos:prefLabel "Hypervescent" ;
.
asc:CQ
  a asc:Class ;
  a skos:Concept ;
  dcterms:identifier "http://anzsoil.org/def/au/asc/CQ"^^xsd:anyURI ;
  skos:definition "[CA] Soils with a calcareous horizon containing more than 20% of mainly soft, finely divided carbonate, and 0-20% of hard calcrete fragments and/or carbonate nodules or concretions, and/or carbonate-coated gravel." ;
  skos:definition "[CH] Soils with a calcareous horizon containing more than 20% of mainly soft, finely divided carbonate, and 0-20% of hard calcrete fragments and/or carbonate nodules or concretions, and/or carbonate-coated gravel." ;
  skos:definition "[DE] Soils with a calcareous horizon containing more than 20% of mainly soft, finely divided carbonate, and 0-20% of hard calcrete fragments and/or carbonate nodules or concretions, and/or carbonate-coated gravel." ;
  skos:definition "[KA] Soils with a calcareous horizon containing more than 20% of mainly soft, finely divided carbonate, and 0–20% of hard calcrete fragments and/or carbonate nodules or concretions, and/or carbonate-coated gravel." ;
  skos:definition "[RE] Soils with a calcareous horizon containing more than 20% of fine earth carbonate, and 0-20% of hard calcrete fragments and/or carbonate nodules or concretions, and/or carbonate-coated gravel." ;
  skos:definition "[SO] Soils with a calcareous horizon containing more than 20% of mainly soft, finely divided carbonate, and 0-20% of hard calcrete fragments and/or carbonate nodules or concretions, and/or carbonate-coated gravel." ;
  skos:definition "[TE] Other soils in which the calcareous horizon contains less than 20% of hard calcrete fragments and/or carbonate nodules or concretions." ;
  skos:notation "CQ" ;
  skos:prefLabel "Hypercalcic    " ;
.
asc:CR
  a asc:Class ;
  skos:definition "[SO] Other soils in which the major part of the upper 0.2 m of the B2t horizon is mottled and has an ESP greater than 25." ;
  skos:notation "CR" ;
  skos:prefLabel "Hypernatric" ;
.
asc:CS
  a asc:Class ;
  a skos:Concept ;
  skos:definition "[HY] Soils of the saline playa lakes (including coastal salinas and continental playas) which are usually bare and when dry are frequently halite- or gypsum-encrusted, or with a sparse cover of halophytes such as samphires. The continental playas are infrequently inundated with fresh water, but a shallow saline ground water table is usually present in all types throughout the year, mostly within 0.5 m of the surface." ;
  skos:definition "[RE] Soils that are highly saline (EC >2 dSm-1; 1:5 H2O), often salt-encrusted, frequently stratified, but do not have a permanent or seasonal water table and do not show any evidence of episodic wetting by groundwater, such as mottling." ;
  skos:definition "[RU] Soils that are highly saline (EC > 2 dSm-1; 1:5 H2O), often salt-encrusted, frequently stratified, but do not have a permanent or seasonal water table and do not show any evidence of episodic wetting by groundwater such as mottling." ;
  skos:notation "CS" ;
  skos:prefLabel "Hypersalic" ;
.
asc:CU
  a asc:Class ;
  skos:definition "[VE] Soils in which some subsurface horizon within the upper 0.5 m of the solum has an ESP of 15 or greater and the major part of the upper 0.5 m of the solum is strongly acid." ;
  skos:notation "CU" ;
  skos:prefLabel "Epihypersodic-Epiacidic" ;
.
asc:CV
  a asc:Class ;
  a skos:Concept ;
  skos:definition "[CA] Soils in which the carbonate is evident only as a slight to moderate effervescence (1M HCl), and/or contain less than 2% soft finely divided carbonate, and have less than 20% hard carbonate nodules or concretions." ;
  skos:definition "[CH] Soils in which the carbonate is evident only as a slight to moderate effervescence (1M HCl), and/or contain less than 2% soft finely divided carbonate, and have less than 20% hard carbonate nodules or concretions." ;
  skos:definition "[DE] Soils in which the carbonate is evident only as a slight to moderate effervescence (1 M HCl), and/or contain less than 2% soft finely divided carbonate, and have less than 20% hard carbonate nodules or concretions." ;
  skos:definition "[KA] Soils in which the carbonate is evident only as a slight to moderate effervescence (1M HCl), and/or contain less than 2% soft finely divided carbonate, and have less than 20% hard carbonate nodules or concretions." ;
  skos:definition "[RE] Soils in which the fine earth carbonate is evident only as a slight to moderate effervescence (1 M HCl), and/or contain less than 2% fine earth carbonate, and have less than 20% hard carbonate nodules or concretions." ;
  skos:definition "[SO] Soils in which the carbonate is evident only as a slight to moderate effervescence (1M HCl), and/or contain less than 2% soft finely divided carbonate, and have less than 20% hard carbonate nodules or concretions." ;
  skos:notation "CV" ;
  skos:prefLabel "Hypocalcic" ;
.
asc:CW
  a asc:Class ;
  a skos:Concept ;
  skos:definition "[HY] Soils of intertidal flats (often colonised by mangroves) that experience regular saline tidal inundation of mostly high frequency." ;
  skos:notation "CW" ;
  skos:prefLabel "Intertidal" ;
.
asc:CX
  a asc:Class ;
  skos:definition "[HY] Soils with a clear or abrupt textural B horizon and the major part of the upper 0.2 m of the B2 horizon is strongly acid." ;
  skos:notation "CX" ;
  skos:prefLabel "Kurosolic" ;
.
asc:CY
  a asc:Class ;
  a skos:Concept ;
  dcterms:identifier "http://anzsoil.org/def/au/asc/CY"^^xsd:anyURI ;
  skos:definition "[FE] Soils which are underlain within 0.5 m of the surface by a calcrete pan; hard unweathered rock or other hard materials; or partially weathered or decomposed rock or saprolite." ;
  skos:definition "[KA] Soils which are underlain within 0.5 m of the surface by hard unweathered rock or other hard materials; or partially weathered or decomposed rock or saprolite." ;
  skos:definition "[RU] Soils that are underlain within 0.5m of the surface by a calcrete pan; hard unweathered rock or other hard materials; or partially weathered or decomposed rock or saprolite." ;
  skos:definition "[TE] Soils which are underlain within 0.5 m of the surface by a calcrete pan; hard unweathered rock or other hard materials; or partially weathered or decomposed rock or saprolite." ;
  skos:notation "CY" ;
  skos:prefLabel "Leptic " ;
.
asc:CZ
  a asc:Class ;
  a skos:Concept ;
  dcterms:identifier "http://anzsoil.org/def/au/asc/CZ"^^xsd:anyURI ;
  skos:definition "[CA] Soils that directly overlie hard rock." ;
  skos:definition "[OR] Soils in which the organic materials directly overlie hard rock." ;
  skos:definition "[RE] Soils that directly overlie hard rock." ;
  skos:definition "[RE] Soils which overlie hard rock." ;
  skos:definition "[RU] Soils that directly overlie hard rock." ;
  skos:definition "[TE] Soils which overlie hard rock." ;
  skos:notation "CZ" ;
  skos:prefLabel "Lithic " ;
.
asc:Class
  a owl:Class ;
  rdfs:subClassOf skos:Concept ;
.
asc:Clay-content
  a owl:Class ;
  rdfs:subClassOf asc:Class ;
  skos:prefLabel "Clay content" ;
.
asc:ColourClass
  a owl:Class ;
  rdfs:label "Colour Class" ;
  rdfs:subClassOf asc:Class ;
  rdfs:subClassOf skos:Concept ;
.
asc:D
  a asc:Class ;
  a asc:Thickness ;
  skos:definition "[OR] >0.6 m" ;
  skos:notation "D" ;
  skos:prefLabel "Very thick" ;
.
asc:DA
  a asc:Class ;
  a skos:Concept ;
  dcterms:identifier "http://anzsoil.org/def/au/asc/DA"^^xsd:anyURI ;
  skos:definition "[CA] Soils with a calcareous horizon containing more than 50% of hard calcrete fragments and/or carbonate nodules or concretions and/or carbonate-coated gravel." ;
  skos:definition "[CH] Soils with a calcareous horizon containing more than 50% of hard calcrete fragments and/or carbonate nodules or concretions and/or carbonate-coated gravel." ;
  skos:definition "[DE] Soils with a calcareous horizon containing more than 50% of hard calcrete fragments and/or carbonate nodules or concretions and/or carbonate-coated gravel." ;
  skos:definition "[KA] Soils with a calcareous horizon containing more than 50% of hard calcrete fragments and/or carbonate nodules or concretions and/or carbonate-coated gravel." ;
  skos:definition "[RE] Soils with a calcareous horizon containing more than 50% of hard, calcrete fragments and/or carbonate nodules or concretions and/or carbonate-coated gravel." ;
  skos:definition "[SO] Soils with a calcareous horizon containing more than 50% of hardcalcrete fragments and/or carbonate nodules or concretions and/or carbonate-coated gravel." ;
  skos:definition "[TE] Soils in which the calcareous horizon contains more than 50% of hard calcrete fragments and/or carbonate nodules or concretions." ;
  skos:notation "DA" ;
  skos:prefLabel "Lithocalcic " ;
.
asc:DB
  a asc:Class ;
  skos:definition "[CH] Soils with an exchangeable Ca/Mg ratio of less than 0.1 in the major part of the B2t horizon." ;
  skos:definition "[DE] Soils with an exchangeable Ca/Mg ratio of less than 0.1 in the major part of the B2 horizon." ;
  skos:definition "[FE] Soils with an exchangeable Ca/Mg ratio of less than 0.1 in the major part of the B2 horizon." ;
  skos:definition "[HY] Soils with an exchangeable Ca/Mg ratio of less than 0.1 in the major part of the B2 horizon." ;
  skos:definition "[KA] Soils with an exchangeable Ca/Mg ratio of less than 0.1 in the major part of the B2 horizon." ;
  skos:definition "[KU] Other soils with an exchangeable Ca/Mg ratio of less than 0.1 in the major part of the B2t horizon." ;
  skos:definition "[SO] Soils with an exchangeable Ca/Mg ratio of less than 0.1 in the major part of the B2t horizon." ;
  skos:definition "[VE] Soils in which the major part of the B horizon has an exchangeable Ca/Mg ratio of less than 0.1." ;
  skos:notation "DB" ;
  skos:prefLabel "Magnesic" ;
.
asc:DC
  a asc:Class ;
  a skos:Concept ;
  dcterms:identifier "http://anzsoil.org/def/au/asc/DC"^^xsd:anyURI ;
  skos:definition "[CH] Other soils with a manganic horizon within the solum." ;
  skos:definition "[DE] Other soils with a manganic horizon within the solum." ;
  skos:definition "[FE] Soils with a manganic horizon within the solum." ;
  skos:definition "[HY] Other soils with a manganic horizon within the soil profile." ;
  skos:definition "[KA] Other soils with a manganic horizon within the solum." ;
  skos:definition "[KU] Other soils with a manganic horizon within the solum." ;
  skos:definition "[RE] Soils with a manganic horizon." ;
  skos:definition "[SO] Soils with a manganic horizon within the solum." ;
  skos:definition "[TE] Soils with a manganic horizon with the solum." ;
  skos:definition "[VE] Soils with a manganic horizon within the solum." ;
  skos:notation "DC" ;
  skos:prefLabel "Manganic   " ;
.
asc:DD
  a asc:Class ;
  a skos:Concept ;
  dcterms:identifier "http://anzsoil.org/def/au/asc/DD"^^xsd:anyURI ;
  skos:definition "[CA] Soils that directly overlie marl." ;
  skos:definition "[OR] Soils with a marl layer either within or immediately below the section containing the organic materials." ;
  skos:definition "[RE] Soils that directly overlie marl." ;
  skos:definition "[RE] Soils which overlie marl." ;
  skos:definition "[TE] Soils which overlie marl." ;
  skos:notation "DD" ;
  skos:prefLabel "Marly " ;
.
asc:DE
  a asc:Order ;
  a skos:Concept ;
  dcterms:description "Soils with structured B2 horizons and lacking a strong texture-contrast between the A and B horizons. Although there is some diversity within the order, it brings together a range of soils with some important properties in common." ;
  dcterms:identifier "http://anzsoil.org/def/au/asc/DE"^^xsd:anyURI ;
  rdfs:comment "Some clayey soils in the arid zone which are relatively high in salt tend to have strong, fine blocky structure. It may be difficult to decide if they are Vertosols or Dermosols because of an apparent lack of cracking and slickensides or lenticular peds. The use of shrinkage measurements such as those discussed under vertic properties will help to resolve this situation." ;
  skos:definition """Soils other than Vertosols, Hydrosols, Calcarosols and Ferrosols which:

1. Have B2 horizons that have grade of pedality greater than weak1 throughout the major part of the horizon, and
2. Do not have clear or abrupt textural B horizon.""" ;
  skos:notation "DE" ;
  skos:prefLabel "Dermosols" ;
.
asc:DF
  a asc:Class ;
  skos:definition "[VE] Soils with a massive or weak blocky (usually > 50 mm peds) A horizon, and there is no surface crusty horizon." ;
  skos:notation "DF" ;
  skos:prefLabel "Massive" ;
.
asc:DG
  a asc:Class ;
  a skos:Concept ;
  dcterms:identifier "http://anzsoil.org/def/au/asc/DG"^^xsd:anyURI ;
  skos:definition "[CH] Other soils with a melacic horizon." ;
  skos:definition "[DE] Other soils with a melacic horizon." ;
  skos:definition "[FE] Soils with a melacic horizon." ;
  skos:definition "[HY] Other soils with a melacic horizon." ;
  skos:definition "[KA] Other soils with a melacic horizon." ;
  skos:definition "[KU] Other soils with a melacic horizon." ;
  skos:definition "[PO] Other soils with a melacic horizon." ;
  skos:definition "[RE] Other soils with a melacic horizon." ;
  skos:definition "[TE] Soils with a melacic horizon." ;
  skos:notation "DG" ;
  skos:prefLabel "Melacic  " ;
.
asc:DH
  a asc:Class ;
  skos:definition "[HY] Soils with a melacic horizon and a B2 horizon in which the major part has an exchangeable Ca/Mg ratio of less than 0.1." ;
  skos:notation "DH" ;
  skos:prefLabel "Melacic-Magnesic" ;
.
asc:DI
  a asc:Class ;
  skos:definition "[CH] Soils with a melacic horizon and the major part of the B2t horizon is mottled." ;
  skos:definition "[DE] Soils with a melacic horizon and the major part of the B2 horizon is mottled" ;
  skos:definition "[KA] Soils with a melacic horizon and the major part of the B2 horizon is mottled." ;
  skos:notation "DI" ;
  skos:prefLabel "Melacic-Mottled" ;
.
asc:DJ
  a asc:Class ;
  skos:definition "[PO] Soils with a melacic horizon and a strongly coherent B horizon." ;
  skos:notation "DJ" ;
  skos:prefLabel "Melacic-Parapanic" ;
.
asc:DK
  a asc:Class ;
  a skos:Concept ;
  dcterms:identifier "http://anzsoil.org/def/au/asc/DK"^^xsd:anyURI ;
  skos:definition "[CA] Other soils with a melanic horizon." ;
  skos:definition "[CH] Other soils with a melanic horizon." ;
  skos:definition "[DE] Other soils with a melanic horizon." ;
  skos:definition "[FE] Other soils with a melanic horizon." ;
  skos:definition "[HY] Other soils with a melanic horizon." ;
  skos:definition "[KA] Other soils with a melanic horizon." ;
  skos:definition "[KU] Other soils with a melanic horizon." ;
  skos:definition "[PO] Soils with a melanic horizon." ;
  skos:definition "[RE] Other soils with a melanic horizon." ;
  skos:definition "[SO] Other soils with a melanic horizon." ;
  skos:definition "[TE] Soils with a melanic horizon." ;
  skos:notation "DK" ;
  skos:prefLabel "Melanic   " ;
.
asc:DL
  a asc:Class ;
  skos:definition "[HY] Soils with a melanic horizon and a conspicuously bleached A2 horizon." ;
  skos:notation "DL" ;
  skos:prefLabel "Melanic-Bleached" ;
.
asc:DM
  a asc:Class ;
  skos:definition "[CH] Soils with a melanic horizon and the major part of the B2t horizon is mottled." ;
  skos:definition "[DE] Soils with a melanic horizon and the major part of the B2 horizon is mottled." ;
  skos:definition "[FE] Soils with a melanic horizon and the major part of the B2 horizon is mottled." ;
  skos:definition "[KA] Soils with a melanic horizon and the major part of the B2 horizon is mottled." ;
  skos:notation "DM" ;
  skos:prefLabel "Melanic-Mottled" ;
.
asc:DN
  a asc:Class ;
  skos:definition "[CA] Soils with a melanic horizon overlying a B horizon in which at least 0.3m has vertic properties." ;
  skos:definition "[CH] Soils with a melanic horizon and a B horizon in which at least 0.3m has vertic properties." ;
  skos:definition "[DE] Soils with a melanic horizon and a B horizon in which at least 0.3m has vertic properties." ;
  skos:definition "[HY] Soils with a melanic horizon and a B horizon in which at least 0.3m has vertic properties." ;
  skos:definition "[KU] Soils with a melanic horizon and a B horizon in which at least 0.3 m has vertic properties." ;
  skos:definition "[SO] Soils with a melanic horizon and a B horizon in which at least 0.3m has vertic properties." ;
  skos:notation "DN" ;
  skos:prefLabel "Melanic-Vertic" ;
.
asc:DO
  a asc:Class ;
  skos:definition "[KA] Soils with massive to weakly structured (about 10 mm subangular blocky parting to finer granules) B horizons that are very porous with a weak consistence strength when moist. Bulk density appears to be relatively low. (See Comment below)." ;
  skos:notation "DO" ;
  skos:prefLabel "Mellic" ;
.
asc:DP
  a asc:Class ;
  skos:definition "[SO] Other soils in which the major part of the upper 0.2 m of the B2t horizon has an ESP between 15 and 25." ;
  skos:notation "DP" ;
  skos:prefLabel "Mesonatric" ;
.
asc:DQ
  a asc:Class ;
  skos:definition "[CH] Other soils in which the major part of the B2t horizon is mottled." ;
  skos:definition "[DE] Soils in which the major part of the B2 horizon is mottled." ;
  skos:definition "[FE] Soils in which the major part of the B2 horizon is mottled." ;
  skos:definition "[HY] Soils in which the major part of the upper 0.5 m of the profile is mottled." ;
  skos:definition "[KA] Other soils in which the major part of the B2 horizon is mottled." ;
  skos:definition "[KU] Other soils in which the major part of the B2t horizon is mottled." ;
  skos:definition "[VE] Soils in which the major part of the upper 0.5 m of the solum is mottled." ;
  skos:notation "DQ" ;
  skos:prefLabel "Mottled" ;
.
asc:DR
  a asc:Class ;
  a skos:Concept ;
  dcterms:identifier "http://anzsoil.org/def/au/asc/DR"^^xsd:anyURI ;
  skos:definition "[TE] Soils with all the requirements of a humose horizon except the thickness." ;
  skos:notation "DR" ;
  skos:prefLabel "Subhumose    " ;
.
asc:DT
  a asc:Class ;
  a skos:Concept ;
  skos:definition "[HY] Other soils with a seasonal or permanent water table and in which the major part of the soil profile (or the subsoil if the profile is stratified) is whole coloured." ;
  skos:notation "DT" ;
  skos:prefLabel "Oxyaquic" ;
.
asc:DU
  a asc:Class ;
  a skos:Concept ;
  dcterms:identifier "http://anzsoil.org/def/au/asc/DU"^^xsd:anyURI ;
  skos:definition "[CA] Soils which directly overlie partially weathered or decomposed rock or saprolite." ;
  skos:definition "[OR] Soils in which the organic materials directly overlie partially weathered or decomposed rock or saprolite." ;
  skos:definition "[RE] Soils which directly overlie partially weathered or decomposed rock or saprolite." ;
  skos:definition "[RE] Soils which overlie partially weathered or decomposed rock or saprolite." ;
  skos:definition "[RU] Soils that directly overlie partially weathered or decomposed rock or saprolite." ;
  skos:definition "[TE] Soils which overlie partially weathered or decomposed rock or saprolite." ;
  skos:notation "DU" ;
  skos:prefLabel "Paralithic" ;
.
asc:DV
  a asc:Class ;
  skos:definition "[PO] Soils with a strongly coherent B horizon." ;
  skos:notation "DV" ;
  skos:prefLabel "Parapanic" ;
.
asc:DW
  a asc:Class ;
  a skos:Concept ;
  dcterms:identifier "http://anzsoil.org/def/au/asc/DW"^^xsd:anyURI ;
  skos:definition "[CH] Soils with a peaty horizon." ;
  skos:definition "[HY] Other soils with a peaty horizon" ;
  skos:definition "[PO] Other soils with a peaty horizon." ;
  skos:definition "[RE] Soils with a peaty horizon." ;
  skos:definition "[TE] Soils with a peaty horizon." ;
  skos:definition "[VE] Soils with a surface peaty horizon." ;
  skos:notation "DW" ;
  skos:prefLabel "Peaty " ;
.
asc:DX
  a asc:Class ;
  skos:definition "[PO] Soils with a peaty horizon and a strongly coherent B horizon." ;
  skos:notation "DX" ;
  skos:prefLabel "Peaty-Parapanic" ;
.
asc:DY
  a asc:Class ;
  skos:definition "[CA] Soils in which the major part of the B horizon has a grade of structure that is stronger than weak." ;
  skos:notation "DY" ;
  skos:prefLabel "Pedal" ;
.
asc:DZ
  a asc:Class ;
  a skos:Concept ;
  dcterms:identifier "http://anzsoil.org/def/au/asc/DZ"^^xsd:anyURI ;
  skos:definition "[CA] Soils that directly overlie a calcrete pan." ;
  skos:definition "[CH] Soils with a B horizon that is not calcareous and which directly overlies a calcrete pan." ;
  skos:definition "[DE] Soils with a B horizon that is not calcareous and which directly overlies a calcrete pan." ;
  skos:definition "[HY] Soils that directly overlie a calcrete pan." ;
  skos:definition "[KA] Soils with a B horizon that is not calcareous and which directly overlies a calcrete pan." ;
  skos:definition "[RE] Soils that directly overlie a calcrete pan." ;
  skos:definition "[RE] Soils which overlie a hard calcrete pan." ;
  skos:definition "[RU] Soils that directly overlie a calcrete pan." ;
  skos:definition "[SO] Soils with a B horizon that is not calcareous and which directly overlies a calcrete pan." ;
  skos:definition "[TE] Soils which overlie a calcrete pan." ;
  skos:definition "[VE] Soils in which the B horizon directly overlies a calcrete pan." ;
  skos:notation "DZ" ;
  skos:prefLabel "Petrocalcic" ;
.
asc:Depth
  a owl:Class ;
  rdfs:subClassOf asc:Class ;
  skos:prefLabel "Soil depth" ;
.
asc:E
  a asc:Class ;
  a asc:Gravel-nature ;
  skos:definition "[OR] <2%" ;
  skos:notation "E" ;
  skos:prefLabel "Non-gravelly" ;
.
asc:EA
  a asc:Class ;
  a skos:Concept ;
  dcterms:identifier "http://anzsoil.org/def/au/asc/EA"^^xsd:anyURI ;
  skos:definition "[CH] Soils with a petroferric horizon within the solum." ;
  skos:definition "[DE] Soils with a B horizon either containing or directly underlain by ferricrete, a petroferric horizon, or a petroreticulate horizon." ;
  skos:definition "[HY] Soils with a petroferric horizon within the soil profile." ;
  skos:definition "[KA] Soils with a B horizon either containing or directly underlain by ferricrete, a petroferric horizon, or a petroreticulate horizon." ;
  skos:definition "[KU] Soils with a petroferric horizon within the solum." ;
  skos:definition "[RE] Other soils which overlie ferricrete, a petroferric horizon or a petroreticulate horizon." ;
  skos:definition "[RU] Other soils that directly overlie ferricrete, a petroferric horizon or a petroreticulate horizon." ;
  skos:definition "[SO] Soils with a petroferric horizon within the solum." ;
  skos:definition "[TE] Soils which overlie ferricrete, a petroferric horizon or a petroreticulate horizon." ;
  skos:notation "EA" ;
  skos:prefLabel "Petroferric" ;
.
asc:EB
  a asc:Class ;
  skos:definition "[PO] Soils with a pipey B horizon." ;
  skos:notation "EB" ;
  skos:prefLabel "Pipey" ;
.
asc:EC
  a asc:Class ;
  a skos:Concept ;
  dcterms:identifier "http://anzsoil.org/def/au/asc/EC"^^xsd:anyURI ;
  skos:definition "[KA] Soils with a thin ironpan which occurs within or directly underlying the B horizon." ;
  skos:definition "[OR] Soils with a thin ironpan below the organic materials." ;
  skos:definition "[PO] Other soils with a thin ironpan which occurs within or directly underlying the B horizon." ;
  skos:definition "[TE] Soils with a thin ironpan." ;
  skos:notation "EC" ;
  skos:prefLabel "Placic " ;
.
asc:ED
  a asc:Class ;
  a skos:Concept ;
  skos:definition "[HY] Soils with a seasonal or permanent water table and in which the major part of the soil profile (or the subsoil if the profile is stratified) is mottled." ;
  skos:notation "ED" ;
  skos:prefLabel "Redoxic" ;
.
asc:EE
  a asc:Class ;
  skos:definition "[CA} Soils in which the A horizon directly overlies a Bk horizon consisting almost entirely of soft carbonate (>80%)." ;
  skos:notation "EE" ;
  skos:prefLabel "Rendic" ;
.
asc:EF
  a asc:Class ;
  a skos:Concept ;
  dcterms:identifier "http://anzsoil.org/def/au/asc/EF"^^xsd:anyURI ;
  skos:definition "[CH] Soils with a reticulate horizon below the B2t horizon." ;
  skos:definition "[DE] Soils with a reticulate horizon below the B2 horizon." ;
  skos:definition "[HY] Soils with a reticulate horizon below the B2 horizon." ;
  skos:definition "[KA] Soils with a reticulate horizon below the B2 horizon." ;
  skos:definition "[KU] Soils with a reticulate horizon below the B2t horizon." ;
  skos:definition "[RE] Soils which overlie a reticulate horizon." ;
  skos:definition "[TE] Soils which overlie a reticulate horizon." ;
  skos:notation "EF" ;
  skos:prefLabel "Reticulate  " ;
.
asc:EG
  a asc:Class ;
  a skos:Concept ;
  skos:definition "[HY] Salinised soils caused by a rising saline water table or by saline seepage resulting from near-surface lateral movement (through flow) of water and salt from higher landscape positions. Such areas may be bare and salt-encrusted, often have a soft fluffy surface, and may or may not have a sparse cover of halophytic plants. Water table conductivity will usually be in the range of 2-50 dSm-1; soil salinity may vary widely due to capillary concentration at or near the surface, and subsequent leaching of salt by seasonal precipitation." ;
  skos:definition "[VE] Soils with a seasonal saline water table present in the upper 0.5 m of the profile (water conductivity >2 dSm-1 ). Salt efflorescence may occur on the surface soil when dry." ;
  skos:notation "EG" ;
  skos:prefLabel "Salic" ;
.
asc:EH
  a asc:Class ;
  a skos:Concept ;
  skos:definition "[HY] Soils in which the organic materials, other than fibric peat, are dominated by sapric peat." ;
  skos:definition "[OR] Soils in which the dominant organic material, by thickness, is sapric peat." ;
  skos:notation "EH" ;
  skos:prefLabel "Sapric" ;
.
asc:EI
  a asc:Class ;
  skos:definition "[VE] Soils with a surface that is moderately to strongly self-mulching; when the soil is dry the self-mulching layer should be at least 10 mm thick. Initial drying may form a thin (2-3 mm) surface flake which readily disintegrates to a mulch on further drying. This process is accelerated by mechanical disturbance." ;
  skos:notation "EI" ;
  skos:prefLabel "Self-mulching" ;
.
asc:EJ
  a asc:Class ;
  a skos:Concept ;
  skos:definition "[PO] Soils with short-term saturation in the B horizon. The saturation may be caused by impedance within the B horizon, perching of water by substrate material, or by seasonally high groundwater tables. The duration of saturation may range from several days to several weeks but is insufficient to reduce and remove significant amounts of the accumulated iron. However, there may be a greater accumulation of organic compounds and less iron in the zone of maximum saturation." ;
  skos:notation "EJ" ;
  skos:prefLabel "Semiaquic" ;
.
asc:EK
  a asc:Class ;
  skos:definition "[PO] Soils with only a Bs horizon." ;
  skos:notation "EK" ;
  skos:prefLabel "Sesquic" ;
.
asc:EL
  a asc:Class ;
  a skos:Concept ;
  skos:definition "[RU] Soils that dominantly consist of fragments of shells and other aquatic skeletons (identifiable under a 10 x hand lens and often readily visible to the naked eye)." ;
  skos:notation "EL" ;
  skos:prefLabel "Shelly" ;
.
asc:EM
  a asc:Class ;
  a skos:Concept ;
  dcterms:identifier "http://anzsoil.org/def/au/asc/EM"^^xsd:anyURI ;
  skos:definition "[HY] Soils with a hard siliceous pan in the lower A and/or upper B horizon." ;
  skos:definition "[PO] Soils with a siliceous pan directly underlying the B horizon." ;
  skos:definition "[RE] Soils which overlie a siliceous pan." ;
  skos:definition "[RU] Soils that directly overlie a siliceous pan." ;
  skos:definition "[SO] Soils with a siliceous pan in the lower A and/or upper B horizon." ;
  skos:definition "[TE] Soils which overlie a siliceous pan." ;
  skos:notation "EM" ;
  skos:prefLabel "Silpanic " ;
.
asc:EN
  a asc:Class ;
  skos:definition "[FE] Soils with an A horizon having a very fine granular structure (<2 mm) and a dry consistence strength that is weak to very weak. The horizon usually has a low bulk density and may be water repellent." ;
  skos:notation "EN" ;
  skos:prefLabel "Snuffy" ;
.
asc:EO
  a asc:Class ;
  skos:definition "[CH] Other soils with a B horizon in which at least the lower part is sodic." ;
  skos:definition "[DE] Other soils with a B horizon in which at least the lower part is sodic." ;
  skos:definition "[FE] Soils with a B2 horizon in which at least the lower part is sodic." ;
  skos:definition "[HY] Other soils with a B horizon in which at least the lower part is sodic" ;
  skos:definition "[KA] Other soils with a B horizon in which at least the lower part is sodic." ;
  skos:definition "[KU] Other soils with a B horizon in which at least the lower part is sodic." ;
  skos:notation "EO" ;
  skos:prefLabel "Sodic" ;
.
asc:EP
  a asc:Class ;
  skos:definition "[VE] Soils in which the upper 0.1 m of the solum is sodic and the major part of the upper 0.5 m of the solum is strongly acid." ;
  skos:notation "EP" ;
  skos:prefLabel "Episodic-Epiacidic" ;
.
asc:EQ
  a asc:Class ;
  skos:definition "[HY] Soils with a clear or abrupt textural B horizon which is sodic and not strongly acid in the major part of the upper 0.2 m of the B2 horizon." ;
  skos:notation "EQ" ;
  skos:prefLabel "Sodosolic" ;
.
asc:ER
  a asc:Class ;
  a skos:Concept ;
  skos:definition "[RE] Soils that consist dominantly of unconsolidated mineral materials which are distinct, not or only slightly gravelly (<10% >2 mm) sedimentary layers or buried soils but salinity is not high (EC<2 dSm-1; 1:5 H2O)." ;
  skos:definition "[RU] Soils that consist dominantly of unconsolidated mineral materials which are distinct, not or only slightly gravelly (<10% >2 mm) sedimentary layers or buried soils but salinity is not high (EC<2 dSm-1; 1:5 H2O)." ;
  skos:notation "ER" ;
  skos:prefLabel "Stratic" ;
.
asc:ES
  a asc:Class ;
  skos:definition "[SO] Other soils in which the major part of the upper 0.2 m of the B2t horizon has an ESP between 6 and <15." ;
  skos:notation "ES" ;
  skos:prefLabel "Subnatric" ;
.
asc:ET
  a asc:Class ;
  skos:definition "[CA] Other soils with a strongly subplastic B horizon." ;
  skos:definition "[CH] Soils in which the major part of the B2t horizon is strongly subplastic." ;
  skos:definition "[DE] Soils in which the major part of the B2 horizon is strongly subplastic." ;
  skos:notation "ET" ;
  skos:prefLabel "Subplastic" ;
.
asc:EU
  a asc:Class ;
  skos:definition "[HY] Soils in which sulfidic materials occur within the upper 1.5 m of the profile." ;
  skos:definition "[OR] Soils in which sulfidic materials occur within the upper 1.5 m of the profile." ;
  skos:definition "[RE] Soils in which sulfidic materials occur within the upper 1.5 m of the soil profile." ;
  skos:definition "[RU] Soils in which sulfidic materials occur within the upper 1.5 m of the profile." ;
  skos:definition "[VE] Soils in which sulfidic materials occur within the upper 1.5 m of the profile." ;
  skos:notation "EU" ;
  skos:note "[HY] Note: The sulfidic great group can be replaced by the following great groups where appropriate evidence is available:" ;
  skos:note "[OR] Note: The sulfidic Great Group can be replaced by the following Great Groups where appropriate evidence is available:" ;
  skos:note "[RE] Note that the Sulfidic Great Group can be replaced by the following Great Groups where appropriate evidence is available." ;
  skos:note "[RU] Note: The sulfidic Great Group can be replaced by the following Great Groups where appropriate evidence is available:" ;
  skos:note "[VE] Note: The sulfidic subgroup can be replaced by the following subgroups where appropriate evidence is available:" ;
  skos:prefLabel "Sulfidic" ;
.
asc:EV
  a asc:Class ;
  skos:definition "[HY] Soils in which sulfuric material (at least 0.15 m thick) occurs within the upper 1.5 m of the profile." ;
  skos:definition "[OR] Soils in which sulfuric material (at least 15 cm thick) occurs within the upper 1.5 m of the profile." ;
  skos:definition "[RE] Soils in which sulfuric material (at least 0.15 m thick) occurs within the upper 1.5 m of the soil profile." ;
  skos:definition "[RU] Soils in which sulfuric material (at least 0.15 m thick) occurs within the upper 1.5 m of the profile." ;
  skos:definition "[VE] Soils in which sulfuric material (at least 0.15 m thick) occurs within the upper 1.5 m of the profile." ;
  skos:notation "EV" ;
  skos:note "[HY] Note: The sulfuric great group can be replaced by the following [IW] great group where appropriate evidence is available:" ;
  skos:note "[OR] Note: The sulfuric Great Group can be replaced by the following [IW] Great Group where appropriate evidence is available:" ;
  skos:note "[RE] Note that the Sulfuric Great Group can be replaced by the following [IW] Great Group where appropriate evidence is available." ;
  skos:note "[RU] Note: The sulfuric Great Group can be replaced by the following [IW] Great Group where appropriate evidence is available:" ;
  skos:note "[VE] Note: The sulfuric subgroup can be replaced by the following [IW] subgroup where appropriate evidence is available:" ;
  skos:prefLabel "Sulfuric" ;
.
asc:EW
  a asc:Class ;
  a skos:Concept ;
  skos:definition "[HY] Soils of supratidal flats (normally bare of vegetation except for halophytes such as samphires), often salt-encrusted. Tidal inundation is infrequent (spring tides) but a saline water table is present at shallow depths." ;
  skos:notation "EW" ;
  skos:prefLabel "Supratidal" ;
.
asc:EX
  a asc:Class ;
  skos:definition "[CA] Other soils with a B horizon in which at least 0.3 m has vertic properties." ;
  skos:definition "[CH] Other soils with a B horizon in which at least 0.3m has vertic properties." ;
  skos:definition "[DE] Other soils with a B horizon in which at least 0.3m has vertic properties." ;
  skos:definition "[HY] Other soils with a B horizon in which at least 0.3m has vertic properties." ;
  skos:definition "[KU] Other soils with a B horizon in which at least 0.3 m has vertic properties." ;
  skos:definition "[SO] Other soils with a B horizon in which at least 0.3m has vertic properties." ;
  skos:notation "EX" ;
  skos:prefLabel "Vertic" ;
.
asc:EY
  a asc:Class ;
  skos:definition "[CH] Soils with a humose horizon and a conspicuously bleached A2 horizon." ;
  skos:definition "[HY] Soils with a humose horizon and a conspicuously bleached A2 horizon." ;
  skos:definition "[KU] Soils with a humose horizon and a conspicuously bleached A2 horizon." ;
  skos:notation "EY" ;
  skos:prefLabel "Humose-Bleached" ;
.
asc:EZ
  a asc:Class ;
  skos:definition "[HY] Soils with a melacic horizon and a conspicuously bleached A2 horizon." ;
  skos:definition "[KU] Soils with a melacic horizon and a conspicuously bleached A2 horizon." ;
  skos:notation "EZ" ;
  skos:prefLabel "Melacic-Bleached" ;
.
asc:F
  a asc:Class ;
  a asc:Gravel-nature ;
  skos:definition "[OR] 2-<10%" ;
  skos:notation "F" ;
  skos:prefLabel " Slightly gravelly" ;
.
asc:FB
  a asc:Class ;
  a skos:Concept ;
  dcterms:identifier "http://anzsoil.org/def/au/asc/FB"^^xsd:anyURI ;
  skos:definition "[CA] Soils with a calcareous horizon containing 20-50% of hard calcrete fragments and/or carbonate nodules or concretions and/or carbonate-coated gravel." ;
  skos:definition "[CH] Soils with a calcareous horizon containing 20-50% of hard calcrete fragments and/or carbonate nodules or concretions and/or carbonate-coated gravel." ;
  skos:definition "[DE] Soils with a calcareous horizon containing 20-50% of hard calcrete fragments and/or carbonate nodules or concretions and/or carbonate-coated gravel." ;
  skos:definition "[KA] Soils with a calcareous horizon containing 20–50% of hard calcrete fragments and/or carbonate nodules or concretions and/or carbonate-coated gravel." ;
  skos:definition "[RE] Soils with a calcareous horizon containing 20-50% of hard, calcrete fragments and/or carbonate nodules or concretions and/or carbonate-coated gravel." ;
  skos:definition "[SO] Soils with a calcareous horizon containing 20-50% of hard calcrete fragments and/or carbonate nodules or concretions and/or carbonate-coated gravel." ;
  skos:definition "[TE] Soils in which the calcareous horizon contains 20-50% of hard calcrete fragments and/or carbonate nodules or concretions." ;
  skos:notation "FB" ;
  skos:prefLabel "Supracalcic   " ;
.
asc:FC
  a asc:Class ;
  a skos:Concept ;
  dcterms:identifier "http://anzsoil.org/def/au/asc/FC"^^xsd:anyURI ;
  skos:definition "[RE] Soils with a melanic horizon and at least some part of the upper 1.0 m of the soil profile is calcareous." ;
  skos:definition "[TE] Soils with a melanic horizon and at least some part of the B, BC or C/B horizon (if present) is calcareous." ;
  skos:notation "FC" ;
  skos:prefLabel "Melanic-Calcareous" ;
.
asc:FD
  a asc:Class ;
  skos:definition "[HY] Other soils in which the major part of the upper 0.2 m of the B2 horizon is sodic." ;
  skos:definition "[KU] Other soils in which the major part of the upper 0.2 m of the B2t horizon is sodic." ;
  skos:notation "FD" ;
  skos:prefLabel "Natric" ;
.
asc:FE
  a asc:Order ;
  a skos:Concept ;
  dcterms:description "Soils with B2 horizons which are high in free iron oxide and lacking a strong texture-contrast between the A and B horizons." ;
  dcterms:identifier "http://anzsoil.org/def/au/asc/FE"^^xsd:anyURI ;
  rdfs:comment "These soils are almost entirely formed on either mafic or ultramafic igneous rocks, their metamorphic equivalents, or alluvium derived therefrom. Although these soils do not occupy large areas in Australia, they are widely recognised and often intensively used because of their favourable physical properties. The most common forms have B2 horizons with a strong grade of pedality; such horizons typically have polyhedral compound peds up to 10-15 mm, usually with smooth and often shiny faces, which break down readily to primary peds about 5 mm or less in size. However forms also occur with a very fine granular structure which may appear massive in place. Horizons are usually high in clay and subplastic." ;
  skos:definition """Soils other than Vertosols, Hydrosols, and Calcarosols that:

1. Have B2 horizons in which the major part has a free iron oxide content greater than 5% Fe in the fine earth fraction (<2 mm), and
2. Do not have a clear or abrupt textural B horizon or a B2 horizon in which at least 0.3 m has vertic properties.""" ;
  skos:notation "FE" ;
  skos:prefLabel "Ferrosols" ;
.
asc:FF
  a asc:Class ;
  a skos:Concept ;
  dcterms:identifier "http://anzsoil.org/def/au/asc/FF"^^xsd:anyURI ;
  skos:definition "[TE] Soils with all the requirements of a melacic horizon except the thickness." ;
  skos:notation "FF" ;
  skos:prefLabel "Submelacic     " ;
.
asc:FG
  a asc:Class ;
  a skos:Concept ;
  dcterms:identifier "http://anzsoil.org/def/au/asc/FG"^^xsd:anyURI ;
  skos:definition "[TE] Soils with all the requirements of a melanic horizon except the thickness." ;
  skos:notation "FG" ;
  skos:prefLabel "Submelanic     " ;
.
asc:FH
  a asc:Class ;
  skos:definition "[RE] Other soils that, other than the surface horizon, have a sand texture (<5% clay) throughout at least the upper 1.0 m of the soil profile." ;
  skos:notation "FH" ;
  skos:prefLabel "Palic" ;
.
asc:FJ
  a asc:Class ;
  a skos:Concept ;
  skos:definition "[CA] Soils that dominantly consist of gypsum crystals which are sand-sized or finer." ;
  skos:definition "[RE] Soils that are not highly saline (EC <2 dSm-1; 1:5 H2O) and dominantly consist of sand-sized gypsum crystals. These crystals may not feel like sands when hand texturing due to their partial dissolution in water." ;
  skos:definition "[RU] Soils that are not highly saline (EC < 2 dSm-1; 1:5 H2O) and dominantly consist of gypsum crystals which are sand-sized or finer." ;
  skos:notation "FJ" ;
  skos:prefLabel "Hypergypsic" ;
.
asc:FK
  a asc:Class ;
  a skos:Concept ;
  dcterms:identifier "http://anzsoil.org/def/au/asc/FK"^^xsd:anyURI ;
  skos:definition "[RE] Soils which have a ferric horizon and overlie a red-brown hardpan." ;
  skos:definition "[TE] Soils which have a ferric horizon and overlies a red-brown hardpan." ;
  skos:notation "FK" ;
  skos:prefLabel "Ferric-Duric" ;
.
asc:FL
  a asc:Class ;
  skos:definition "[CA] Soils in which the B horizon is strongly subplastic and the B or BC horizon contains a gypsic horizon." ;
  skos:notation "FL" ;
  skos:prefLabel "Gypsic-Subplastic" ;
.
asc:FM
  a asc:Class ;
  skos:definition "[VE] Soils in which the major part of the upper 0.5 m of the solum is calcareous and some subsurface horizon within this depth has an ESP of 15 or greater." ;
  skos:notation "FM" ;
  skos:prefLabel "Epicalcareous-Epihypersodic" ;
.
asc:FN
  a asc:Class ;
  skos:definition "[SO] Soils in which the major part of the upper 0.2 m of the B2t horizon is mottled and has an ESP between 6 and <15." ;
  skos:notation "FN" ;
  skos:prefLabel "Mottled-Subnatric" ;
.
asc:FO
  a asc:Class ;
  skos:definition "[SO] Soils in which the major part of the upper 0.2 m of the B2t horizon is mottled and has an ESP between 15 and 25." ;
  skos:notation "FO" ;
  skos:prefLabel "Mottled-Mesonatric" ;
.
asc:FP
  a asc:Class ;
  skos:definition "[SO] Other soils in which the major part of the upper 0.2 m of the B2t horizon is mottled and has an ESP greater than 25." ;
  skos:notation "FP" ;
  skos:prefLabel "Mottled-Hypernatric" ;
.
asc:FQ
  a asc:Class ;
  skos:definition "[HY] Soils with structured B2 horizons and which apart from wetness fulfil the requirements for Dermosols." ;
  skos:notation "FQ" ;
  skos:prefLabel "Dermosolic" ;
.
asc:FR
  a asc:Class ;
  skos:definition "[HY] Other soils with B2 horizons and which apart from wetness fulfil the requirements for Kandosols." ;
  skos:notation "FR" ;
  skos:prefLabel "Kandosolic" ;
.
asc:FS
  a asc:Class ;
  skos:definition "[OR] Soils with a layer (or layers) of unconsolidated mineral material within or below the organic materials but within 0.8 m of the surface." ;
  skos:notation "FS" ;
  skos:prefLabel "Terric" ;
.
asc:FU
  a asc:Class ;
  a skos:Concept ;
  dcterms:identifier "http://anzsoil.org/def/au/asc/FU"^^xsd:anyURI ;
  skos:definition "[RE] Soils with a melacic horizon and the major part of the upper 1.0 m of the soil profile is not strongly acid." ;
  skos:definition "[TE] Soils with a melacic horizon and the major part of the B horizon (if present) is not strongly acid but the B and BC or C/B horizons are not calcareous." ;
  skos:notation "FU" ;
  skos:prefLabel "Melacic-Basic  " ;
.
asc:FV
  a asc:Class ;
  a skos:Concept ;
  dcterms:identifier "http://anzsoil.org/def/au/asc/FV"^^xsd:anyURI ;
  skos:definition "[DE] Soils with a melanic horizon and the major part of the B2 horizon is strongly acid." ;
  skos:definition "[FE] Soils with a melanic horizon and the major part of the B2 horizon is strongly acid." ;
  skos:definition "[HY] Soils with a melanic horizon and the major part of the B2 horizon is strongly acid." ;
  skos:definition "[KA] Soils with a melanic horizon and the major part of the B2 horizon is strongly acid." ;
  skos:definition "[RE] Soils with a melanic horizon and the major part of the upper 1.0 m of the soil profile is strongly acid." ;
  skos:definition "[TE] Soils with a melanic horizon and the major part of the B horizon (if present) is strongly acid." ;
  skos:notation "FV" ;
  skos:prefLabel "Melanic-Acidic" ;
.
asc:FW
  a asc:Class ;
  skos:definition "[HY] Soils that are dominated by other organic-rich (non-vegetative) materials such as faunal debris to a depth of 0.5 m." ;
  skos:notation "FW" ;
  skos:prefLabel "Faunic" ;
.
asc:FX
  a asc:Class ;
  skos:definition "[HY] Soils that are dominantly silt-sized to a depth of 0.5 m." ;
  skos:notation "FX" ;
  skos:prefLabel "Lutaceous" ;
.
asc:FY
  a asc:Class ;
  skos:definition "[HY] Soils in which the major part of the upper 0.5 m of the profile is calcareous." ;
  skos:definition "[HY] Soils that are dominantly calcareous to a depth of 0.5 m." ;
  skos:definition "[VE] Other soils in which the major part of the upper 0.5 m of the solum is calcareous." ;
  skos:notation "FY" ;
  skos:prefLabel "Epicalcareous" ;
.
asc:FZ
  a asc:Class ;
  skos:definition "[VE] Other soils in which the major part of the solum below 0.5 m is calcareous." ;
  skos:notation "FZ" ;
  skos:prefLabel "Endocalcareous" ;
.
asc:Family
  a owl:Class ;
  rdfs:subClassOf skos:Concept ;
.
asc:G
  a asc:Class ;
  a asc:Gravel-nature ;
  skos:definition "[OR] 10-<20%" ;
  skos:notation "G" ;
  skos:prefLabel "Gravelly" ;
.
asc:GA
  a asc:Class ;
  skos:definition "[VE] Other soils in which the major part of the upper 0.5 m of the solum is strongly acid." ;
  skos:notation "GA" ;
  skos:prefLabel "Epiacidic" ;
.
asc:GB
  a asc:Class ;
  skos:definition "[VE] Soils in which the major part of the upper 0.5 m of the solum is calcareous and an ESP of 15 or greater occurs in some subhorizon of the solum below 0.5 m." ;
  skos:notation "GB" ;
  skos:prefLabel "Epicalcareous-Endohypersodic" ;
.
asc:GC
  a asc:Class ;
  skos:definition "[DE] Soils with a melacic horizon and a reticulate horizon which occurs below the B2 horizon." ;
  skos:notation "GC" ;
  skos:prefLabel "Melacic-Reticulate" ;
.
asc:GD
  a asc:Class ;
  skos:definition "[HY] Soils with a peaty horizon and a thin ironpan which occurs within or directly underlying the B horizon." ;
  skos:definition "[PO] Soils with a peaty horizon and a thin ironpan which occurs within or directly underlying the B horizon." ;
  skos:notation "GD" ;
  skos:prefLabel "Peaty-Placic" ;
.
asc:GE
  a asc:Class ;
  a skos:Concept ;
  dcterms:identifier "http://anzsoil.org/def/au/asc/GE"^^xsd:anyURI ;
  skos:definition "[RE] Soils which contain a ferric horizon and which overlie ferricrete, a petroferric horizon or a petroreticulate horizon." ;
  skos:definition "[RU] Soils that contain a ferric horizon and directly overlie ferricrete, a petroferric horizon or a petroreticulate horizon." ;
  skos:definition "[TE] Soils which contains a ferric horizon and directly overlies ferricrete, a petroferric horizon or a petroreticulate horizon." ;
  skos:notation "GE" ;
  skos:prefLabel "Ferric-Petroferric" ;
.
asc:GF
  a asc:Class ;
  a skos:Concept ;
  dcterms:identifier "http://anzsoil.org/def/au/asc/GF"^^xsd:anyURI ;
  skos:definition "[CA] Other soils that directly overlie unconsolidated mineral materials." ;
  skos:definition "[OR] Other soils with a layer (or layers) of unconsolidated mineral material which occurs below 0.8 m of the surface." ;
  skos:definition "[RE] Other soils that directly overlie unconsolidated mineral materials." ;
  skos:definition "[RU] Soils that directly overlie unconsolidated mineral materials." ;
  skos:definition "[TE] Soils which overlie other unconsolidated mineral materials." ;
  skos:notation "GF" ;
  skos:prefLabel "Regolithic " ;
.
asc:GG
  a asc:Class ;
  skos:definition "[VE] Soils in which the upper 0.1 m of the solum is sodic and the major part of the solum below 0.5 m is strongly acid." ;
  skos:notation "GG" ;
  skos:prefLabel "Episodic-Endoacidic" ;
.
asc:GH
  a asc:Class ;
  skos:definition "[VE] Soils in which the upper 0.1 m of the solum is sodic and the major part of the upper 0.5 m of the solum is calcareous." ;
  skos:notation "GH" ;
  skos:prefLabel "Episodic-Epicalcareous" ;
.
asc:GI
  a asc:Class ;
  skos:definition "[VE] Soils in which the upper 0.1 m of the solum is sodic and the major part of the solum below 0.5 m is calcareous." ;
  skos:notation "GI" ;
  skos:prefLabel "Episodic-Endocalcareous" ;
.
asc:GJ
  a asc:Class ;
  skos:definition "[VE] Soils in which the major part of the upper 0.5 m of the solum is calcareous and the major part of the solum below 0.5 m is strongly acid." ;
  skos:notation "GJ" ;
  skos:prefLabel "Epicalcareous-Endoacidic" ;
.
asc:GK
  a asc:Class ;
  skos:definition "[VE] Soils in which the major part of the upper 0.5 m of the solum is strongly acid and mottled." ;
  skos:notation "GK" ;
  skos:prefLabel "Epiacidic-Mottled" ;
.
asc:GL
  a asc:Class ;
  skos:definition "[VE] Soils in which the major part of the solum below 0.5 m is strongly acid and mottled." ;
  skos:notation "GL" ;
  skos:prefLabel "Endoacidic-Mottled" ;
.
asc:GM
  a asc:Class ;
  skos:definition "[VE] Soils in which the major part of the solum below 0.5 m is calcareous and some subhorizon of the solum below 0.5 m has an ESP of 15 or greater." ;
  skos:notation "GM" ;
  skos:prefLabel "Endocalcareous-Endohypersodic" ;
.
asc:GN
  a asc:Class ;
  skos:definition "[VE] Soils in which some subsurface horizon within the upper 0.5 m of the solum has an ESP of 15 or greater and the major part of the solum below 0.5 m is strongly acid." ;
  skos:notation "GN" ;
  skos:prefLabel "Epihypersodic-Endoacidic " ;
.
asc:GO
  a asc:Class ;
  skos:definition "[VE] Soils in which some subsurface horizon within the upper 0.5 m of the solum has an ESP of 15 or greater and the major part of the solum below 0.5 m is calcareous." ;
  skos:notation "GO" ;
  skos:prefLabel "Epihypersodic-Endocalcareous" ;
.
asc:GP
  a asc:Class ;
  skos:definition "[HY] Soils that have an exchangeable Ca/Mg ratio of less than 0.1 in the major part of the B2 horizon, and the major part of the upper 0.2 m of the B2 horizon is sodic." ;
  skos:definition "[KU] Soils with an exchangeable Ca/Mg ratio of less than 0.1 in the major part of the B2t horizon, and the major part of the upper 0.2 m of the B2t horizon is sodic." ;
  skos:notation "GP" ;
  skos:prefLabel "Magnesic-Natric" ;
.
asc:GQ
  a asc:Class ;
  skos:definition "[VE] Soils in which the upper 0.1 m of the solum is sodic and a gypsic horizon is present within the B or BC horizon." ;
  skos:notation "GQ" ;
  skos:prefLabel "Episodic-Gypsic" ;
.
asc:GR
  a asc:Class ;
  skos:definition "[HY] Soils which apart from wetness fulfil the requirements for Rudosols." ;
  skos:notation "GR" ;
  skos:prefLabel "Rudosolic" ;
.
asc:GS
  a asc:Class ;
  skos:definition "[VE] Soils with a pedal (stronger than weak grade, blocky or polyhedral) A horizon which is either not or only weakly self-mulching, and there is no surface crusty horizon. Some soils after wetting and drying may form a thin 5-10 mm surface flake which cracks into irregular polygons (plates) 30-100 mm diameter. These may be readily separated and removed from the underlying pedal clay." ;
  skos:notation "GS" ;
  skos:prefLabel "Epipedal" ;
.
asc:GT
  a asc:Class ;
  skos:definition "[HY] Soils which apart from wetness fulfil the requirements for Tenosols." ;
  skos:notation "GT" ;
  skos:prefLabel "Tenosolic" ;
.
asc:GU
  a asc:Class ;
  a skos:Concept ;
  dcterms:identifier "http://anzsoil.org/def/au/asc/GU"^^xsd:anyURI ;
  skos:definition "[HY] Soils with a humose horizon and at least some part of the B or BC horizon is calcareous." ;
  skos:definition "[RE] Soils with a humose horizon and at least some part of the upper 1.0 m of the soil profile is calcareous." ;
  skos:definition "[TE] Soils with a humose horizon and at least some part of the B, BC or C/B horizon (if present) is calcareous." ;
  skos:notation "GU" ;
  skos:prefLabel "Humose-Calcareous" ;
.
asc:GV
  a asc:Class ;
  a skos:Concept ;
  skos:definition "[RU] Soils that consist dominantly of unconsolidated mineral materials which are not or only slightly gravelly (<10% >2mm). Aeolian cross-bedding may be present but there is little if any evidence of other stratification or buried soils. If the soil material is sandy (ie. S-LS-CS, up to 10% clay) it is coherent." ;
  skos:notation "GV" ;
  skos:prefLabel "Lutic" ;
.
asc:GW
  a asc:Class ;
  skos:definition "[DE] Soils with a ferric horizon within the solum and a B2 horizon in which the major part is strongly acid." ;
  skos:definition "[FE] Soils with a ferric horizon within the solum and a B2 horizon in which the major part is strongly acid." ;
  skos:definition "[HY] Soils with a ferric horizon within the soil profile and a B2 horizon in which the major part is strongly acid." ;
  skos:definition "[KA] Soils with a ferric horizon within the solum and a B2 horizon in which the major part is strongly acid." ;
  skos:notation "GW" ;
  skos:prefLabel "Ferric-Acidic" ;
.
asc:GX
  a asc:Class ;
  skos:definition "[DE] Soils with a manganic horizon within the solum and a B2 horizon in which the major part is strongly acid." ;
  skos:definition "[HY] Soils with a manganic horizon within the soil profile and a B2 horizon in which the major part is strongly acid." ;
  skos:definition "[KA] Soils with a manganic horizon within the solum and a B2 horizon in which the major part is strongly acid." ;
  skos:notation "GX" ;
  skos:prefLabel "Manganic-Acidic" ;
.
asc:GY
  a asc:Class ;
  a skos:Concept ;
  dcterms:identifier "http://anzsoil.org/def/au/asc/GY"^^xsd:anyURI ;
  skos:definition "[DE] Soils with a humose horizon and the major part of the B2 horizon is strongly acid." ;
  skos:definition "[FE] Soils with a humose horizon and the major part of the B2 horizon is strongly acid." ;
  skos:definition "[HY] Soils with a humose horizon and the major part of the B2 horizon is strongly acid." ;
  skos:definition "[KA] Soils with a humose horizon and the major part of the B2 horizon is strongly acid." ;
  skos:definition "[RE] Soils with a humose horizon and the major part of the upper 1.0 m of the soil profile is strongly acid." ;
  skos:definition "[TE] Soils with a humose horizon and the major part of the B horizon (if present) is strongly acid." ;
  skos:notation "GY" ;
  skos:prefLabel "Humose-Acidic " ;
.
asc:Gravel-nature
  a owl:Class ;
  rdfs:subClassOf asc:Class ;
  skos:prefLabel "Nature of gravel" ;
.
asc:Greatgroup
  a owl:Class ;
  rdfs:label "Soil great group" ;
  rdfs:subClassOf skos:Concept ;
  rdfs:subClassOf [
      a owl:Restriction ;
      owl:allValuesFrom asc:Suborder ;
      owl:onProperty skos:broader ;
    ] ;
  rdfs:subClassOf [
      a owl:Restriction ;
      owl:cardinality "1"^^xsd:nonNegativeInteger ;
      owl:onProperty asc:classifier ;
    ] ;
.
asc:H
  a asc:Class ;
  a asc:Gravel-nature ;
  skos:definition "[OR] 20-50%" ;
  skos:notation "H" ;
  skos:prefLabel "Moderately gravelly" ;
.
asc:HA
  a asc:Class ;
  skos:definition "[DE] Soils with a melanic horizon and a B horizon in which at least the lower part is sodic." ;
  skos:notation "HA" ;
  skos:prefLabel "Melanic-Sodic" ;
.
asc:HB
  a asc:Class ;
  skos:definition "[CH] Soils in which the major part of the B2t horizon is mottled, and at least the lower part of the B horizon is sodic." ;
  skos:definition "[DE] Soils in which the major part of the B2 horizon is mottled and at least the lower part of the B horizon is sodic." ;
  skos:definition "[KA] Soils in which the major part of the B2 horizon is mottled and at least the lower part of the B horizon is sodic." ;
  skos:definition "[KU] Soils in which the major part of the B2t horizon is mottled and at least the lower part of the B horizon is sodic." ;
  skos:notation "HB" ;
  skos:prefLabel "Mottled-Sodic" ;
.
asc:HC
  a asc:Class ;
  skos:definition "[CH] Soils with a ferric horizon within the solum, and at least the lower part of the B horizon is sodic." ;
  skos:definition "[DE] Soils with a ferric horizon within the solum and a B horizon in which at least the lower part is sodic." ;
  skos:definition "[HY] Soils with a ferric horizon within the soil profile and a B horizon in which at least the lower part is sodic." ;
  skos:definition "[KA] Soils with a ferric horizon within the solum and a B horizon in which at least the lower part is sodic." ;
  skos:notation "HC" ;
  skos:prefLabel "Ferric-Sodic" ;
.
asc:HD
  a asc:Class ;
  skos:definition "[OR] Soils in which the organic materials directly overlie fragmental material such as Gravel, cobbles or stones in which the interstices are filled or partially filled with organic material." ;
  skos:notation "HD" ;
  skos:prefLabel "Rudaceous" ;
.
asc:HE
  a asc:Class ;
  skos:definition """[VE] Manganic-Endocalcareous [JI]
Soils in which the major part of the solum below 0.5 m is calcareous and the major part of the upper 0.5 m of the solum is mottled.""" ;
  skos:notation "HE" ;
  skos:prefLabel "Endocalcareous-Mottled" ;
.
asc:HF
  a asc:Class ;
  a skos:Concept ;
  dcterms:identifier "http://anzsoil.org/def/au/asc/HF"^^xsd:anyURI ;
  skos:definition "[RE] Soils which have formed in tephric materials that may be visibly stratified." ;
  skos:definition "[RU] Soils in which the gravel consists dominantly of little-weathered tephric materials." ;
  skos:definition "[TE] Soils which have formed in tephric materials that may be visibly stratified." ;
  skos:notation "HF" ;
  skos:prefLabel "Tephric " ;
.
asc:HG
  a asc:Class ;
  a skos:Concept ;
  skos:definition "[RU] Soils in which the upper 0.5 m (or less if the profile is shallower) consists dominantly of carbic materials." ;
  skos:notation "HG" ;
  skos:prefLabel "Carbic" ;
.
asc:HH
  a asc:Class ;
  a skos:Concept ;
  skos:definition "[RU] Soils that consist dominantly of unconsolidated mineral materials which are gravelly (>10% >2 mm). The gravel may occur as distinct layers, or be uniformly or irregularly distributed." ;
  skos:notation "HH" ;
  skos:prefLabel "Clastic" ;
.
asc:HI
  a asc:Class ;
  skos:definition "[RU] Soils in which the gravel consists of usually unsorted material with a wide size range. It is largely colluvial mass movement debris, including scree and talus, and landslide, mudflow and creep deposits." ;
  skos:notation "HI" ;
  skos:prefLabel "Colluvic" ;
.
asc:HJ
  a asc:Class ;
  skos:definition "[RU] Other soils in which the unconsolidated mineral materials are dominated by gravel which mostly consists of rock or mineral fragments." ;
  skos:notation "HJ" ;
  skos:prefLabel "Lithosolic" ;
.
asc:HK
  a asc:Class ;
  skos:definition "[CA] Soils in which the upper 0.1 m of the solum consists of dominantly soft, finely divided carbonate (visual estimate), and/or contains more than 40%2 (by analysis) of soft, finely divided carbonate." ;
  skos:notation "HK" ;
  skos:prefLabel "Supravescent" ;
.
asc:HL
  a asc:Class ;
  skos:definition "[HY] Other soils with sulfidic materials in the A or near surface horizons." ;
  skos:notation "HL" ;
  skos:prefLabel "Episulfidic" ;
.
asc:HM
  a asc:Class ;
  skos:definition "[HY] Soils with sulfidic materials in the A or near surface horizons and which directly overlie a calcrete pan." ;
  skos:notation "HM" ;
  skos:prefLabel "Episulfidic-Petrocalcic" ;
.
asc:HN
  a asc:Class ;
  skos:definition "[PO] Soils with a densipan present in the A2 horizon and a thin ironpan which occurs within or directly underlying the B horizon." ;
  skos:notation "HN" ;
  skos:prefLabel "Densic-Placic" ;
.
asc:HO
  a asc:Class ;
  skos:definition "[DE] Soils in which the major part of the B2 horizon is strongly acid and at least the lower part is sodic." ;
  skos:definition "[HY] Soils in which the major part of the B2 horizon is strongly acid and at least the lower part is sodic." ;
  skos:definition "[KA] Soils in which the major part of the B2 horizon is strongly acid and at least the lower part of the B horizon is sodic." ;
  skos:notation "HO" ;
  skos:prefLabel "Acidic-Sodic" ;
.
asc:HR
  a asc:Class ;
  a skos:Concept ;
  skos:definition "[AN] Soils that have been formed by applications of human-deposited materials such as mill-mud, etc. or the accumulation of shells and organic materials to form middens. (Minimum thickness of deposit or accumulation is 0.3 m)." ;
  skos:notation "HR" ;
  skos:prefLabel "Cumulic" ;
.
asc:HS
  a asc:Class ;
  a skos:Concept ;
  skos:definition "[AN] Soils that have had additions of organic residues such as organic wastes, composts, mulches, etc. that have been incorporated into the soil and obliterated pre-existing pedological features." ;
  skos:notation "HS" ;
  skos:prefLabel "Hortic" ;
.
asc:HT
  a asc:Class ;
  a skos:Concept ;
  skos:definition "[AN] Mineral soil or regolithic materials that are underlain by land fill of manufactured origin and which is predominantly of an organic nature. These materials may be of domestic or industrial origin and usually occur as artificially elevated landforms. The intent is to designate refuse from human activity high enough in organic matter to generate significant quantities of methane when placed under anaerobic conditions." ;
  skos:notation "HT" ;
  skos:prefLabel "Garbic" ;
.
asc:HU
  a asc:Class ;
  a skos:Concept ;
  skos:definition "[AN] Mineral soil or regolithic materials that are underlain by land fill of predominantly a mineral nature. The fill may be wholly of manufactured origin (glass, plastics, concrete, etc.) or contain a mixture of manufactured materials and materials of pedogenic origin. The fill usually occurs as an artificially elevated landform." ;
  skos:notation "HU" ;
  skos:prefLabel "Urbic" ;
.
asc:HV
  a asc:Class ;
  a skos:Concept ;
  skos:definition "[AN] Soils that have formed or are forming on mineral materials that have been dredged through human action from the sea or other waterways, or deposited as a slurry resulting from mining operations; eg, tailings ponds, salt ponds, coal washing residues etc. The dredged materials commonly occur as a lithologically distinctive unit overlying (buried) flood plain surfaces. Such deposits frequently occur in coastal areas, common examples being airports, golf courses and other urban developments." ;
  skos:notation "HV" ;
  skos:prefLabel "Dredgic" ;
.
asc:HW
  a asc:Class ;
  a skos:Concept ;
  skos:definition "[AN] Soils that have formed or are forming on mineral materials that have been moved by earthmoving equipment in mining, highway construction, dam building etc. The materials contain too few manufactured artefacts to qualify as urbic soils. Landscapes are human-formed, and hence may present an 'unnatural' geomorphic expression. Spolic materials are increasingly being capped by pre-existing topsoil." ;
  skos:notation "HW" ;
  skos:prefLabel "Spolic" ;
.
asc:HX
  a asc:Class ;
  a skos:Concept ;
  skos:definition "[AN] Soils that have formed or are forming on land surfaces that have been created by humans by cutting away any previously existing soil by mechanical equipment such as bulldozers and graders. Common occurrences are found along highways and hillside urban development where they are usually associated with fill areas with spolic materials. In some instances truncated remnants of the lower horizons of pre-existing soils may occur. Scalpic soil areas typically have peculiar geomorphic expressions, often with smooth and steep slopes." ;
  skos:notation "HX" ;
  skos:prefLabel "Scalpic" ;
.
asc:HY
  a asc:Order ;
  a skos:Concept ;
  asc:family-comment "The classes below are primarily for use in the Redoxic and Oxyaquic suborders, and possibly the Extratidal and Salic suborders. The criteria may be partly applicable to the Supratidal and Hypersalic suborders eg. using the terms surface soil and maximum subsoil texture. The different A horizon thickness criteria for great groups with a Clear or abrupt textural B horizon allows alignment with their adjacent but drier equivalent soil orders." ;
  asc:suborder asc:BT ;
  asc:suborder asc:CS ;
  asc:suborder asc:CW ;
  asc:suborder asc:DT ;
  asc:suborder asc:ED ;
  asc:suborder asc:EG ;
  asc:suborder asc:EW ;
  asc:suborder asc:IU ;
  asc:suborder asc:IV ;
  asc:suborder-comment """The features used in the definitions of the first seven suborders differ from those used elsewhere in the classification in that the classes are essentially based on the frequency of tidal or freshwater inundation and the nature of the soil surface. This is thought to be an appropriate approach as the key feature of Hydrosols is their wetness. The references in parenthesis to vegetation in some definitions are merely indicating accessory properties of the class which may aid identification of what are essentially wetness criteria, for example, the presence of certain mangrove species will normally indicate a regular frequency of tidal wetting. Although it may be difficult to identify the Extratidal suborder by the low frequency of tidal inundation, there is usually a distinct boundary between this zone and the often bare, salt-encrusted Supratidal zone. This boundary is commonly marked by a low (0.1 - 0.2 m) 'scarp'. The three tidal-affected Suborders of Intertidal, Supratidal and Extratidal are largely based on data from Cook and Mayo (1977).

For the purposes of soil classification, Hydrosols located within Intermittently Closed and Open Lakes and Lagoons (ICOLLS) are considered to be tidal.

Where inundation at the perimeter of larger water bodies is cyclical as a result of seiches or from variability in rainfall and runoff, it is often difficult to decide if currently submerged soils are either Subaqueous, Redoxic or Oxyaquic. Their classification will depend on conditions at the time of sampling and knowledge of the frequency and duration of any drying on exposure. With some submerged soils, evidence of prior surface soil aeration such as the development of mottles, soil structure or very low pHw suggests that the soils are not Subaqueous, i.e. subject to permanent saturation. If the period of exposure is insufficient to allow substantial soil aeration and there is no evidence of oxidation and drying, then the soils are considered to be Subaqueous.

In the Salic suborder the salinisation may or may not be human-induced. Saline water tables may arise as a result of a sequence of wetter-than-average years, or they may result from activities such as a tree clearing and/or unwise irrigation practices. With time it is likely that some of the human-induced saline soils will tend to those of the Hypersalic suborder, as evidenced in some of the saline valleys of the Western Australian wheat belt. It also follows that a wide range of soils is likely to occur in the Salic suborder.

In the Redoxic and Oxyaquic suborders water tables are normally non-saline. However exceptions may occur where these soils are underlain by sulfuric and/or sulfidic materials, as described by Walker (1972). It should be noted that the use of mottling as a diagnostic criterion in the former suborder does not necessarily imply that oxidising and reducing conditions are currently occurring in the soil in most years.""" ;
  dcterms:description """This order is designed to accommodate a range of seasonally or permanently wet soils and thus there is some diversity within the order. The key criterion is saturation of the major part of the soil profile for prolonged periods (2-3 months) in most years. Some Hydrosols are permanently submerged. The soils may or may not experience reducing conditions for all or part of the period of saturation, and thus manifestations of reduction and oxidation such as gley colours and ochrous mottles may or may not be present.

Saturation by a water table may not necessarily be caused by low soil permeability. Often site drainage will be the most important factor, while in other well-known cases tidal influence is dominant. The relevant Field Handbook drainage classes are very poorly and poorly drained.

Several major classes of soils are excluded because it is considered their other profile characteristics are of greater significance than wetness. These are the Organosols, Podosols and Vertosols. Although some Hydrosols are dominated by organic materials (see Intertidal Hydrosols below), it is thought that because of their unique nature (ie. largely consisting of mangrove debris that is regularly inundated by saline tidal waters), it is more appropriate to classify them as an organic form of Hydrosols rather than as a class of Organosols that occur in a mangrove environment.""" ;
  dcterms:identifier "http://anzsoil.org/def/au/asc/HY"^^xsd:anyURI ;
  rdfs:comment """The approach taken in this concept of 'wet' soils differs from more traditional usage in that reducing conditions are not emphasised. The rationale for the present approach is based on the assumption that saturation affects soil properties irrespective of whether or not reducing conditions are present. Obvious examples are those relating to certain physical and engineering properties, which result in limitations to the use of a soil eg. trafficability, etc.

A further reason for not making reducing conditions mandatory is the well-known difficulty in identifying such conditions, which are often of a temporal nature and sporadic in spatial distribution. It is widely recognised that the traditional use of gley colours and particular kinds of mottling are not universally indicative of a saturated condition or its duration. In particular, mottles or other segregations can be relict. Another problem in identification of reducing conditions, is the experience that various indicator dyes such as α,α-dipyridyl (Childs & Clayden 1986) may be unreliable.

It will also be apparent that the concept adopted for Hydrosols will normally exclude the pseudo (or surface water) gley class commonly distinguished in several European classification schemes. These soils have a perched water table usually caused by a slowly permeable horizon or layer within the soil profile.

A difficult question arises as to how artificially drained soils are best treated. In many cases drainage will merely lower the water table to depths which permit the successful growth of particular plants. Such depths may still be relatively shallow eg. 0.5 - 1 m, and capillary rise may result in wet soil conditions to variable heights above the new water table. Additionally, the topographic situation and/or the climatic environment may mean that drainage merely reduces the period of saturation. If drainage is such that saturation no longer occurs for appropriate periods in the relevant parts of the profile, the soil can strictly no longer be considered a Hydrosol. Possibly a 'drained' phase may be appropriate in some such circumstances.

In the case of irrigated soils, the main example is when more or less permanent flood irrigation is employed to grow rice. This would be expected to change, for example, a Chromosol to a Chromosolic Hydrosol. It should be noted that the definition of the order is deliberately somewhat equivocal in that the duration and frequency of saturation of a precise section of the profile are not specifically defined. Lack of water table data is one reason, but it is also thought that a degree of flexibility is required for the definition. It is recognised that the extent of soil wetness can seldom be assessed by a single inspection of a particular site. However, in the author's experience judicious questioning of people with local knowledge, together with the soil scientist's assessment of soil and site drainage and climatic environment, can usually achieve a satisfactory resolution of the problem.""" ;
  skos:definition "Soils other than Organosols, Podosols and Vertosols in which the major part of the soil profile is saturated for at least 2-3 months in most years." ;
  skos:narrower asc:HY-BT ;
  skos:narrower asc:HY-CS ;
  skos:narrower asc:HY-CW ;
  skos:narrower asc:HY-DT ;
  skos:narrower asc:HY-ED ;
  skos:narrower asc:HY-EG ;
  skos:narrower asc:HY-EW ;
  skos:narrower asc:HY-IU ;
  skos:narrower asc:HY-IV ;
  skos:notation "HY" ;
  skos:prefLabel "Hydrosols" ;
.
asc:HY-BT
  a asc:Suborder ;
  asc:classifier asc:BT ;
  asc:greatgroup asc:BG ;
  asc:greatgroup asc:CB ;
  asc:greatgroup asc:CX ;
  asc:greatgroup asc:EA ;
  asc:greatgroup asc:EQ ;
  asc:greatgroup asc:EU ;
  asc:greatgroup asc:EV ;
  asc:greatgroup asc:FQ ;
  asc:greatgroup asc:FR ;
  asc:greatgroup asc:GR ;
  asc:greatgroup asc:GT ;
  asc:greatgroup asc:IW ;
  asc:greatgroup asc:IX ;
  asc:greatgroup asc:IZ ;
  asc:greatgroup asc:JA ;
  asc:greatgroup asc:JC ;
  asc:greatgroup asc:JM ;
  asc:greatgroup-comment """Because of lack of data no Great Groups are presently proposed for the Subtidal and Subaqueous Hydrosols. Further studies may lead to additional great groups across all Suborders.

If a diagnostic feature in the key begins more than 1.5 m from the soil surface it may not have a significant impact on the performance of the soil. Refer to diagnostic features in the glossary for guidance on the use of such features in the classification.""" ;
  asc:greatgroup-comment "High salt contents usually tend to obliterate the original morphology, but where this can still be identified, great groups may be established on this basis." ;
  asc:subgroup-comment """No subgroups for the Subtidal, Subaqueous, Supratidal, Extratidal and Hypersalic Hydrosols are formally proposed at present because of insufficient data.

If a diagnostic feature in the key begins more than 1.5 m from the soil surface it may not have a significant impact on the performance of the soil. Refer to diagnostic features in the glossary for guidance on the use of such features in the classification.""" ;
  skos:broader asc:HY ;
  skos:notation "HY-BT" ;
  skos:prefLabel "Extratidal Hydrosol" ;
.
asc:HY-CS
  a asc:Suborder ;
  asc:classifier asc:CS ;
  asc:greatgroup asc:BZ ;
  asc:greatgroup asc:CC ;
  asc:greatgroup asc:CD ;
  asc:greatgroup asc:DQ ;
  asc:greatgroup asc:EU ;
  asc:greatgroup asc:EV ;
  asc:greatgroup asc:FY ;
  asc:greatgroup asc:IW ;
  asc:greatgroup asc:IX ;
  asc:greatgroup asc:IZ ;
  asc:greatgroup asc:JA ;
  asc:greatgroup asc:JC ;
  asc:greatgroup-comment """Because of lack of data no Great Groups are presently proposed for the Subtidal and Subaqueous Hydrosols. Further studies may lead to additional great groups across all Suborders.

If a diagnostic feature in the key begins more than 1.5 m from the soil surface it may not have a significant impact on the performance of the soil. Refer to diagnostic features in the glossary for guidance on the use of such features in the classification.""" ;
  asc:subgroup-comment """No subgroups for the Subtidal, Subaqueous, Supratidal, Extratidal and Hypersalic Hydrosols are formally proposed at present because of insufficient data.

If a diagnostic feature in the key begins more than 1.5 m from the soil surface it may not have a significant impact on the performance of the soil. Refer to diagnostic features in the glossary for guidance on the use of such features in the classification.""" ;
  skos:broader asc:HY ;
  skos:notation "HY-CS" ;
  skos:prefLabel "Hypersalic Hydrosol" ;
.
asc:HY-CW
  a asc:Suborder ;
  asc:classifier asc:CW ;
  asc:greatgroup asc:AQ ;
  asc:greatgroup asc:BV ;
  asc:greatgroup asc:CF ;
  asc:greatgroup asc:EU ;
  asc:greatgroup asc:EV ;
  asc:greatgroup asc:FW ;
  asc:greatgroup asc:FX ;
  asc:greatgroup asc:FY ;
  asc:greatgroup asc:IW ;
  asc:greatgroup asc:IX ;
  asc:greatgroup asc:IY ;
  asc:greatgroup asc:IZ ;
  asc:greatgroup asc:JA ;
  asc:greatgroup asc:JB ;
  asc:greatgroup asc:JC ;
  asc:greatgroup-comment """Because of lack of data no Great Groups are presently proposed for the Subtidal and Subaqueous Hydrosols. Further studies may lead to additional great groups across all Suborders.

If a diagnostic feature in the key begins more than 1.5 m from the soil surface it may not have a significant impact on the performance of the soil. Refer to diagnostic features in the glossary for guidance on the use of such features in the classification.""" ;
  asc:greatgroup-comment "Conventional horizon nomenclature is inapplicable to these soils, hence the use of arbitrary depth limits." ;
  asc:subgroup asc:BW ;
  asc:subgroup asc:CE ;
  asc:subgroup asc:EH ;
  asc:subgroup-comment """No subgroups for the Subtidal, Subaqueous, Supratidal, Extratidal and Hypersalic Hydrosols are formally proposed at present because of insufficient data.

If a diagnostic feature in the key begins more than 1.5 m from the soil surface it may not have a significant impact on the performance of the soil. Refer to diagnostic features in the glossary for guidance on the use of such features in the classification.""" ;
  asc:subgroup-comment "The following three subgroups will only be applicable to the Histic-Hypersulfidic and Histic-Hyposulfidic great groups." ;
  skos:broader asc:HY ;
  skos:notation "HY-CW" ;
  skos:prefLabel "Intertidal Hydrosol" ;
.
asc:HY-DT
  a asc:Suborder ;
  asc:classifier asc:DT ;
  asc:greatgroup asc:BG ;
  asc:greatgroup asc:CB ;
  asc:greatgroup asc:CX ;
  asc:greatgroup asc:EA ;
  asc:greatgroup asc:EQ ;
  asc:greatgroup asc:EU ;
  asc:greatgroup asc:EV ;
  asc:greatgroup asc:FQ ;
  asc:greatgroup asc:FR ;
  asc:greatgroup asc:GR ;
  asc:greatgroup asc:GT ;
  asc:greatgroup asc:IW ;
  asc:greatgroup asc:IX ;
  asc:greatgroup asc:IZ ;
  asc:greatgroup asc:JA ;
  asc:greatgroup asc:JC ;
  asc:greatgroup asc:JM ;
  asc:greatgroup-comment """Because of lack of data no Great Groups are presently proposed for the Subtidal and Subaqueous Hydrosols. Further studies may lead to additional great groups across all Suborders.

If a diagnostic feature in the key begins more than 1.5 m from the soil surface it may not have a significant impact on the performance of the soil. Refer to diagnostic features in the glossary for guidance on the use of such features in the classification.""" ;
  asc:greatgroup-comment "The following great groups will not all be relevant for each of these two suborders. For example, the Rudosolic great group will not be required for the Redoxic suborder." ;
  asc:subgroup asc:AF ;
  asc:subgroup asc:AG ;
  asc:subgroup asc:AH ;
  asc:subgroup asc:AI ;
  asc:subgroup asc:AT ;
  asc:subgroup asc:AU ;
  asc:subgroup asc:AV ;
  asc:subgroup asc:AX ;
  asc:subgroup asc:AY ;
  asc:subgroup asc:BA ;
  asc:subgroup asc:BB ;
  asc:subgroup asc:BC ;
  asc:subgroup asc:BU ;
  asc:subgroup asc:CK ;
  asc:subgroup asc:CL ;
  asc:subgroup asc:DB ;
  asc:subgroup asc:DC ;
  asc:subgroup asc:DG ;
  asc:subgroup asc:DH ;
  asc:subgroup asc:DK ;
  asc:subgroup asc:DL ;
  asc:subgroup asc:DN ;
  asc:subgroup asc:DW ;
  asc:subgroup asc:EF ;
  asc:subgroup asc:EM ;
  asc:subgroup asc:EO ;
  asc:subgroup asc:EX ;
  asc:subgroup asc:EY ;
  asc:subgroup asc:EZ ;
  asc:subgroup asc:FD ;
  asc:subgroup asc:FV ;
  asc:subgroup asc:GD ;
  asc:subgroup asc:GP ;
  asc:subgroup asc:GU ;
  asc:subgroup asc:GW ;
  asc:subgroup asc:GX ;
  asc:subgroup asc:GY ;
  asc:subgroup asc:HC ;
  asc:subgroup asc:HO ;
  asc:subgroup asc:IT ;
  asc:subgroup-comment "It is thought that the following subgroups will cater for most situations, although obviously some will not be relevant for particular great groups. As examples, the Acidic subgroups will not be required for the Kurosolic great groups, nor the Sodic and Natric classes for the Sodosolic great group. Although presently not listed, a Petrocalcic subgroup may be required for the Calcarosolic great group. If so, a definition is available above. Some additional subgroups will be required for the Sulfuric and Sulfidic great groups as knowledge of these soils increases eg. a possible subdivision could be based on the nature of the soil profile above the sulfuric or sulfidic materials which commonly occur as a D horizon. In the case of the Rudosolic and Tenosolic great groups, the most appropriate subgroups will be those used for the relevant suborders and great groups of Rudosols and Tenosols." ;
  asc:subgroup-comment """No subgroups for the Subtidal, Subaqueous, Supratidal, Extratidal and Hypersalic Hydrosols are formally proposed at present because of insufficient data.

If a diagnostic feature in the key begins more than 1.5 m from the soil surface it may not have a significant impact on the performance of the soil. Refer to diagnostic features in the glossary for guidance on the use of such features in the classification.""" ;
  skos:broader asc:HY ;
  skos:notation "HY-DT" ;
  skos:prefLabel "Oxyaquic Hydrosol" ;
.
asc:HY-ED
  a asc:Suborder ;
  asc:classifier asc:ED ;
  asc:greatgroup asc:BG ;
  asc:greatgroup asc:CB ;
  asc:greatgroup asc:CX ;
  asc:greatgroup asc:EA ;
  asc:greatgroup asc:EQ ;
  asc:greatgroup asc:EU ;
  asc:greatgroup asc:EV ;
  asc:greatgroup asc:FQ ;
  asc:greatgroup asc:FR ;
  asc:greatgroup asc:GR ;
  asc:greatgroup asc:GT ;
  asc:greatgroup asc:IW ;
  asc:greatgroup asc:IX ;
  asc:greatgroup asc:IZ ;
  asc:greatgroup asc:JA ;
  asc:greatgroup asc:JC ;
  asc:greatgroup asc:JM ;
  asc:greatgroup-comment """Because of lack of data no Great Groups are presently proposed for the Subtidal and Subaqueous Hydrosols. Further studies may lead to additional great groups across all Suborders.

If a diagnostic feature in the key begins more than 1.5 m from the soil surface it may not have a significant impact on the performance of the soil. Refer to diagnostic features in the glossary for guidance on the use of such features in the classification.""" ;
  asc:greatgroup-comment "The following great groups will not all be relevant for each of these two suborders. For example, the Rudosolic great group will not be required for the Redoxic suborder." ;
  asc:subgroup asc:AF ;
  asc:subgroup asc:AG ;
  asc:subgroup asc:AH ;
  asc:subgroup asc:AI ;
  asc:subgroup asc:AT ;
  asc:subgroup asc:AU ;
  asc:subgroup asc:AV ;
  asc:subgroup asc:AX ;
  asc:subgroup asc:AY ;
  asc:subgroup asc:BA ;
  asc:subgroup asc:BB ;
  asc:subgroup asc:BC ;
  asc:subgroup asc:BU ;
  asc:subgroup asc:CK ;
  asc:subgroup asc:CL ;
  asc:subgroup asc:DB ;
  asc:subgroup asc:DC ;
  asc:subgroup asc:DG ;
  asc:subgroup asc:DH ;
  asc:subgroup asc:DK ;
  asc:subgroup asc:DL ;
  asc:subgroup asc:DN ;
  asc:subgroup asc:DW ;
  asc:subgroup asc:EF ;
  asc:subgroup asc:EM ;
  asc:subgroup asc:EO ;
  asc:subgroup asc:EX ;
  asc:subgroup asc:EY ;
  asc:subgroup asc:EZ ;
  asc:subgroup asc:FD ;
  asc:subgroup asc:FV ;
  asc:subgroup asc:GD ;
  asc:subgroup asc:GP ;
  asc:subgroup asc:GU ;
  asc:subgroup asc:GW ;
  asc:subgroup asc:GX ;
  asc:subgroup asc:GY ;
  asc:subgroup asc:HC ;
  asc:subgroup asc:HO ;
  asc:subgroup asc:IT ;
  asc:subgroup-comment "It is thought that the following subgroups will cater for most situations, although obviously some will not be relevant for particular great groups. As examples, the Acidic subgroups will not be required for the Kurosolic great groups, nor the Sodic and Natric classes for the Sodosolic great group. Although presently not listed, a Petrocalcic subgroup may be required for the Calcarosolic great group. If so, a definition is available above. Some additional subgroups will be required for the Sulfuric and Sulfidic great groups as knowledge of these soils increases eg. a possible subdivision could be based on the nature of the soil profile above the sulfuric or sulfidic materials which commonly occur as a D horizon. In the case of the Rudosolic and Tenosolic great groups, the most appropriate subgroups will be those used for the relevant suborders and great groups of Rudosols and Tenosols." ;
  asc:subgroup-comment """No subgroups for the Subtidal, Subaqueous, Supratidal, Extratidal and Hypersalic Hydrosols are formally proposed at present because of insufficient data.

If a diagnostic feature in the key begins more than 1.5 m from the soil surface it may not have a significant impact on the performance of the soil. Refer to diagnostic features in the glossary for guidance on the use of such features in the classification.""" ;
  skos:broader asc:HY ;
  skos:notation "HY-ED" ;
  skos:prefLabel "Redoxic Hydrosol" ;
.
asc:HY-EG
  a asc:Suborder ;
  asc:classifier asc:EG ;
  asc:greatgroup asc:BG ;
  asc:greatgroup asc:CB ;
  asc:greatgroup asc:CX ;
  asc:greatgroup asc:EA ;
  asc:greatgroup asc:EQ ;
  asc:greatgroup asc:EU ;
  asc:greatgroup asc:EV ;
  asc:greatgroup asc:FQ ;
  asc:greatgroup asc:FR ;
  asc:greatgroup asc:GR ;
  asc:greatgroup asc:GT ;
  asc:greatgroup asc:IW ;
  asc:greatgroup asc:IX ;
  asc:greatgroup asc:IZ ;
  asc:greatgroup asc:JA ;
  asc:greatgroup asc:JC ;
  asc:greatgroup asc:JM ;
  asc:greatgroup-comment """Because of lack of data no Great Groups are presently proposed for the Subtidal and Subaqueous Hydrosols. Further studies may lead to additional great groups across all Suborders.

If a diagnostic feature in the key begins more than 1.5 m from the soil surface it may not have a significant impact on the performance of the soil. Refer to diagnostic features in the glossary for guidance on the use of such features in the classification.""" ;
  asc:greatgroup-comment "High salt contents usually tend to obliterate the original morphology, but where this can still be identified, great groups may be established on this basis." ;
  asc:subgroup asc:DZ ;
  asc:subgroup asc:HL ;
  asc:subgroup asc:HM ;
  asc:subgroup-comment """No subgroups for the Subtidal, Subaqueous, Supratidal, Extratidal and Hypersalic Hydrosols are formally proposed at present because of insufficient data.

If a diagnostic feature in the key begins more than 1.5 m from the soil surface it may not have a significant impact on the performance of the soil. Refer to diagnostic features in the glossary for guidance on the use of such features in the classification.""" ;
  asc:subgroup-comment "The following three subgroups have been identified for several great groups in the Salic suborder. Other possibly relevant subgroups may be found listed below in the subgroups for the Redoxic and Oxyaquic suborders." ;
  skos:broader asc:HY ;
  skos:notation "HY-EG" ;
  skos:prefLabel "Salic Hydrosol" ;
.
asc:HY-EW
  a asc:Suborder ;
  asc:classifier asc:EW ;
  asc:greatgroup asc:BZ ;
  asc:greatgroup asc:CD ;
  asc:greatgroup asc:DQ ;
  asc:greatgroup asc:EU ;
  asc:greatgroup asc:EV ;
  asc:greatgroup asc:FY ;
  asc:greatgroup asc:IW ;
  asc:greatgroup asc:IX ;
  asc:greatgroup asc:IZ ;
  asc:greatgroup asc:JA ;
  asc:greatgroup asc:JC ;
  asc:greatgroup-comment """Because of lack of data no Great Groups are presently proposed for the Subtidal and Subaqueous Hydrosols. Further studies may lead to additional great groups across all Suborders.

If a diagnostic feature in the key begins more than 1.5 m from the soil surface it may not have a significant impact on the performance of the soil. Refer to diagnostic features in the glossary for guidance on the use of such features in the classification.""" ;
  asc:subgroup-comment """No subgroups for the Subtidal, Subaqueous, Supratidal, Extratidal and Hypersalic Hydrosols are formally proposed at present because of insufficient data.

If a diagnostic feature in the key begins more than 1.5 m from the soil surface it may not have a significant impact on the performance of the soil. Refer to diagnostic features in the glossary for guidance on the use of such features in the classification.""" ;
  skos:broader asc:HY ;
  skos:notation "HY-EW" ;
  skos:prefLabel "Supratidal Hydrosol" ;
.
asc:HY-IU
  a asc:Suborder ;
  asc:classifier asc:IU ;
  asc:greatgroup asc:AQ ;
  asc:greatgroup asc:BV ;
  asc:greatgroup asc:CF ;
  asc:greatgroup asc:EU ;
  asc:greatgroup asc:EV ;
  asc:greatgroup asc:FW ;
  asc:greatgroup asc:FX ;
  asc:greatgroup asc:FY ;
  asc:greatgroup asc:IW ;
  asc:greatgroup asc:IX ;
  asc:greatgroup asc:IY ;
  asc:greatgroup asc:IZ ;
  asc:greatgroup asc:JA ;
  asc:greatgroup asc:JB ;
  asc:greatgroup asc:JC ;
  asc:greatgroup-comment """Because of lack of data no Great Groups are presently proposed for the Subtidal and Subaqueous Hydrosols. Further studies may lead to additional great groups across all Suborders.

If a diagnostic feature in the key begins more than 1.5 m from the soil surface it may not have a significant impact on the performance of the soil. Refer to diagnostic features in the glossary for guidance on the use of such features in the classification.""" ;
  asc:greatgroup-comment "Conventional horizon nomenclature is inapplicable to these soils, hence the use of arbitrary depth limits." ;
  asc:subgroup-comment """No subgroups for the Subtidal, Subaqueous, Supratidal, Extratidal and Hypersalic Hydrosols are formally proposed at present because of insufficient data.

If a diagnostic feature in the key begins more than 1.5 m from the soil surface it may not have a significant impact on the performance of the soil. Refer to diagnostic features in the glossary for guidance on the use of such features in the classification.""" ;
  skos:broader asc:HY ;
  skos:notation "HY-IU" ;
  skos:prefLabel "Subtidal Hydrosol" ;
.
asc:HY-IV
  a asc:Suborder ;
  asc:classifier asc:IV ;
  asc:greatgroup asc:AQ ;
  asc:greatgroup asc:BV ;
  asc:greatgroup asc:CF ;
  asc:greatgroup asc:EU ;
  asc:greatgroup asc:EV ;
  asc:greatgroup asc:FW ;
  asc:greatgroup asc:FX ;
  asc:greatgroup asc:FY ;
  asc:greatgroup asc:IW ;
  asc:greatgroup asc:IX ;
  asc:greatgroup asc:IY ;
  asc:greatgroup asc:IZ ;
  asc:greatgroup asc:JA ;
  asc:greatgroup asc:JB ;
  asc:greatgroup asc:JC ;
  asc:greatgroup-comment """Because of lack of data no Great Groups are presently proposed for the Subtidal and Subaqueous Hydrosols. Further studies may lead to additional great groups across all Suborders.

If a diagnostic feature in the key begins more than 1.5 m from the soil surface it may not have a significant impact on the performance of the soil. Refer to diagnostic features in the glossary for guidance on the use of such features in the classification.""" ;
  asc:greatgroup-comment "Conventional horizon nomenclature is inapplicable to these soils, hence the use of arbitrary depth limits." ;
  asc:subgroup-comment """No subgroups for the Subtidal, Subaqueous, Supratidal, Extratidal and Hypersalic Hydrosols are formally proposed at present because of insufficient data.

If a diagnostic feature in the key begins more than 1.5 m from the soil surface it may not have a significant impact on the performance of the soil. Refer to diagnostic features in the glossary for guidance on the use of such features in the classification.""" ;
  skos:broader asc:HY ;
  skos:notation "HY-IV" ;
  skos:prefLabel "Subaqueous Hydrosol" ;
.
asc:HZ
  a asc:Alteration ;
  a asc:Class ;
  skos:definition "[OR] ash material" ;
  skos:notation "HZ" ;
  skos:prefLabel "Ashy" ;
.
asc:I
  a asc:Class ;
  a asc:Gravel-nature ;
  skos:definition "[OR] >50%" ;
  skos:notation "I" ;
  skos:prefLabel "Very gravelly" ;
.
asc:IA
  a asc:Class ;
  a skos:Concept ;
  dcterms:identifier "http://anzsoil.org/def/au/asc/IA"^^xsd:anyURI ;
  skos:definition "[RE] Soils with a transitional horizon (C/B) occurring in fissures in the parent rock or saprolite which contains between 10 and 50% of B horizon material (including pedogenic carbonate)." ;
  skos:definition "[TE] Soils with a transitional horizon (C/B) occurring in fissures in the parent rock or saprolite which contains between 10 and 50% of B horizon material (including pedogenic carbonate)." ;
  skos:notation "IA" ;
  skos:prefLabel "Inceptic " ;
.
asc:IB
  a asc:Class ;
  skos:definition "[CA] Soils that are not calcareous in the A1 or Ap horizon, or to a depth of 0.2m if the A1 horizon is only weakly developed." ;
  skos:definition "[RE] Soils that are not calcareous in the A1 or Ap horizon, or to a depth of 0.2 m if the A1 horizon is only weakly developed." ;
  skos:notation "IB" ;
  skos:prefLabel "Epibasic" ;
.
asc:IC
  a asc:Class ;
  skos:definition "[CA] Other soils." ;
  skos:notation "IC" ;
  skos:prefLabel "Ceteric" ;
.
asc:ID
  a asc:Class ;
  a skos:Concept ;
  dcterms:identifier "http://anzsoil.org/def/au/asc/ID"^^xsd:anyURI ;
  skos:definition "[RE] Soils with all the requirements for a peaty horizon except the thickness." ;
  skos:definition "[TE] Soils with all the requirements for a peaty horizon except the thickness." ;
  skos:notation "ID" ;
  skos:prefLabel "Subpeaty   " ;
.
asc:IE
  a asc:Class ;
  skos:definition "[CH] Soils with fine earth effervescence (1M HCl) throughout the solum." ;
  skos:definition "[SO] Soils with fine earth effervescence (1M HCl) throughout the solum." ;
  skos:notation "IE" ;
  skos:prefLabel "Effervescent" ;
.
asc:IF
  a asc:Class ;
  skos:definition "[OR] Soils that are more or less freely drained and are never saturated for more than several days unless rain is falling and contain organic materials which occur as in Definition (ii) of Organosols." ;
  skos:notation "IF" ;
  skos:prefLabel "Folic" ;
.
asc:IG
  a asc:Class ;
  skos:definition "[PO] Soils with a Bhs/Bs horizon." ;
  skos:notation "IG" ;
  skos:prefLabel "Humosesquic/Sesquic" ;
.
asc:IH
  a asc:Class ;
  skos:definition "[PO] Soils with a Bh/Basi horizon." ;
  skos:notation "IH" ;
  skos:prefLabel "Humic/Alsilic" ;
.
asc:IJ
  a asc:Class ;
  skos:definition "[OR] Soils in which layers of humose, melacic and/or melanic horizon material underlie the organic materials and overlie the substrate." ;
  skos:notation "IJ" ;
  skos:prefLabel "Modic" ;
.
asc:IL
  a asc:Class ;
  a skos:Concept ;
  dcterms:identifier "http://anzsoil.org/def/au/asc/IL"^^xsd:anyURI ;
  skos:definition "[TE] Soils with a ferric or bauxitic horizon (nodules or concretions) that is at least 0.2 m thick and occupies >50% of the solum depth. The solum depth excludes cemented layers. Genetically these soils may be closely related to Podosols" ;
  skos:notation "IL" ;
  skos:prefLabel "Sesqui-Nodular" ;
.
asc:IM
  a asc:Class ;
  a skos:Concept ;
  dcterms:identifier "http://anzsoil.org/def/au/asc/IM"^^xsd:anyURI ;
  skos:definition "[TE] Soils with a horizon containing more than 20% of fine earth carbonate that is at least 0.2 m thick." ;
  skos:notation "IM" ;
  skos:prefLabel "Calcenic" ;
.
asc:IS
  a asc:Class ;
  a skos:Concept ;
  dcterms:identifier "http://anzsoil.org/def/au/asc/IS"^^xsd:anyURI ;
  skos:definition "[RE] Soils which contain a ferric horizon and which overlie a reticulate horizon." ;
  skos:definition "[TE] Soils which contain a ferric horizon and which overlie a reticulate horizon." ;
  skos:notation "IS" ;
  skos:prefLabel "Ferric-Reticulate" ;
.
asc:IT
  a asc:Class ;
  a skos:Concept ;
  skos:definition "[AN] Soils that have surface layers at least 0.3m thick that show evidence of burnt peat (often in the form of coloured ash material) and comprise ≥20% of fusic soil material." ;
  skos:definition "[HY] Soils that have been partly modified by high temperature burning of organic materials. Such soils have surface layers that comprise >20% of fusic material." ;
  skos:notation "IT" ;
  skos:prefLabel "Fusic" ;
.
asc:IU
  a asc:Class ;
  a skos:Concept ;
  skos:definition "[HY] Soils of tidal estuaries, bays and river deltas that experience permanent inundation between Mean Low Water Springs (MLWS) and 2.5 m below MLWS." ;
  skos:notation "IU" ;
  skos:prefLabel "Subtidal" ;
.
asc:IV
  a asc:Class ;
  a skos:Concept ;
  skos:definition "[HY] Soils of inland water bodies that are located between the water surface and 2.5 m below the surface." ;
  skos:notation "IV" ;
  skos:prefLabel "Subaqueous" ;
.
asc:IW
  a asc:Class ;
  skos:definition "[HY] Soils in which both monosulfidic material and sulfuric material (at least 0.15 m thick) occur within the upper 1.5 m of the profile." ;
  skos:definition "[OR] Soils in which both monosulfidic material and sulfuric material (at least 15 cm thick) occur within the upper 1.5 m of the profile." ;
  skos:definition "[RE] Soils in which both monosulfidic materials and sulfuric material (at least 0.15 m thick) occur within the upper 1.5 m of the soil profile." ;
  skos:definition "[RU] Soils in which both monosulfidic material and sulfuric material (at least 0.15 m thick) occur within the upper 1.5 m of the profile." ;
  skos:definition "[VE] Soils in which both monosulfidic material and sulfuric material (at least 0.15 m thick) occur within the upper 1.5 m of the profile." ;
  skos:notation "IW" ;
  skos:prefLabel "Monosulfidic - Sulfuric" ;
.
asc:IX
  a asc:Class ;
  skos:definition "[HY] Soils in which both monosulfidic material and hypersulfidic material occur within the upper 1.5 m of the profile." ;
  skos:definition "[OR] Soils in which both monosulfidic material and hypersulfidic material occur within the upper 1.5 m of the profile." ;
  skos:definition "[RE] Soils in which both monosulfidic material and hypersulfidic material occur within the upper 1.5 m of the soil profile." ;
  skos:definition "[RU] Soils in which both monosulfidic material and hypersulfidic material occur within the upper 1.5 m of the profile." ;
  skos:definition "[VE] Soils in which both monosulfidic material and hypersulfidic material occur within the upper 1.5 m of the profile." ;
  skos:notation "IX" ;
  skos:prefLabel "Monohypersulfidic" ;
.
asc:IY
  a asc:Class ;
  skos:definition "[HY] Soils which are dominated by organic materials to a depth of 0.5 m and which have hypersulfidic material within the upper 1.5 m of the profile." ;
  skos:notation "IY" ;
  skos:prefLabel "Histic-Hypersulfidic" ;
.
asc:IZ
  a asc:Class ;
  skos:definition "[HY] Other soils in which hypersulfidic material occurs within the upper 1.5 m of the profile." ;
  skos:definition "[OR] Other soils in which hypersulfidic material occurs within the upper 1.5 m of the profile." ;
  skos:definition "[RE] Other soils in which hypersulfidic material occurs within the upper 1.5 m of the soil profile." ;
  skos:definition "[RU] Other soils in which hypersulfidic material occurs within the upper 1.5 m of the profile." ;
  skos:definition "[VE] Other soils in which hypersulfidic material occurs within the upper 1.5 m of the profile." ;
  skos:notation "IZ" ;
  skos:prefLabel "Hypersulfidic" ;
.
asc:J
  a asc:Class ;
  a asc:Texture ;
  skos:definition "Dominated by organic materials" ;
  skos:notation "J" ;
  skos:prefLabel "Peaty" ;
.
asc:JA
  a asc:Class ;
  skos:definition "[HY] Soils in which both monosulfidic material and hyposulfidic material occur within the upper 1.5 m of the profile." ;
  skos:definition "[OR] Soils in which both monosulfidic material and hyposulfidic material occur within the upper 1.5 m of the profile." ;
  skos:definition "[RE] Soils in which both monosulfidic material and hyposulfidic material occur within the upper 1.5 m of the soil profile." ;
  skos:definition "[RU] Soils in which both monosulfidic material and hyposulfidic material occur within the upper 1.5 m of the profile." ;
  skos:definition "[VE] Soils in which both monosulfidic material and hyposulfidic material occur within the upper 1.5 m of the profile." ;
  skos:notation "JA" ;
  skos:prefLabel "Monohyposulfidic" ;
.
asc:JB
  a asc:Class ;
  skos:definition "[HY] Other soils which are dominated by organic materials to a depth of 0.5 m and which have hyposulfidic material within the upper 1.5 m of the profile." ;
  skos:notation "JB" ;
  skos:prefLabel "Histic-Hyposulfidic" ;
.
asc:JC
  a asc:Class ;
  skos:definition "[HY] Other soils with hyposulfidic material within the upper 1.5 m of the profile." ;
  skos:definition "[OR] Other soils with hyposulfidic material within the upper 1.5 m of the profile." ;
  skos:definition "[RE] Other soils with hyposulfidic material within the upper 1.5 m of the soil profile." ;
  skos:definition "[RU] Other soils with hyposulfidic material within the upper 1.5 m of the profile." ;
  skos:definition "[VE] Other soils with hyposulfidic material within the upper 1.5 m of the profile." ;
  skos:notation "JC" ;
  skos:prefLabel "Hyposulfidic" ;
.
asc:JD
  a asc:Class ;
  a skos:Concept ;
  skos:definition "[PO] Soils with long-term saturation in the B horizon and sulfuric material (at least 15 cm thick) is present in the A or B horizons." ;
  skos:notation "JD" ;
  skos:prefLabel "Aquic-Sulfuric" ;
.
asc:JE
  a asc:Class ;
  a skos:Concept ;
  skos:definition "[PO] Soils with long-term saturation in the B horizon and hypersulfidic material is present in the A or B horizons." ;
  skos:notation "JE" ;
  skos:prefLabel "Aquic-Hypersulfidic" ;
.
asc:JF
  a asc:Class ;
  skos:definition "[VE] Soils with a ferric horizon within the solum, and in which the major part of the solum below 0.5m has an ESP of 15 or greater." ;
  skos:notation "JF" ;
  skos:prefLabel "Ferric-Endohypersodic " ;
.
asc:JG
  a asc:Class ;
  skos:definition "[VE] Soils with a manganic horizon within the solum, and in which the major part of the solum below 0.5m has an ESP of 15 or greater." ;
  skos:notation "JG" ;
  skos:prefLabel "Manganic-Endohypersodic" ;
.
asc:JH
  a asc:Class ;
  skos:definition "[VE] Soils with a ferric horizon within the solum, and in which the major part of the solum below 0.5m is calcareous." ;
  skos:notation "JH" ;
  skos:prefLabel "Ferric-Endocalcareous" ;
.
asc:JI
  a asc:Class ;
  skos:definition "[VE] Soils with a manganic horizon within the solum, and in which the major part of the solum below 0.5m is calcareous." ;
  skos:notation "JI" ;
  skos:prefLabel "Manganic-Endocalcareous" ;
.
asc:JK
  a asc:Class ;
  skos:definition "[RE] The major part of the upper 0.5 m of the soil profile consists of materials with < 50% halite crystals." ;
  skos:notation "JK" ;
  skos:prefLabel "Subhalic" ;
.
asc:JL
  a asc:Class ;
  skos:definition "[RE] Soils with a layer or horizon, other than the surface horizon, that has a clayey sand or loamy sand texture (about 5-10% clay) that begins within the upper 1.0 m of the soil profile." ;
  skos:notation "JL" ;
  skos:prefLabel "Tenic" ;
.
asc:JM
  a asc:Class ;
  skos:definition "[HY] Soils which apart from wetness fulfil the requirements for Arenosols." ;
  skos:notation "JM" ;
  skos:prefLabel "Arenosolic" ;
.
asc:JN
  a asc:Class ;
  a skos:Concept ;
  skos:definition "[RE] Other soils which are calcareous throughout (at least the upper 1.0 m of the soil profile), or calcareous at least below the A1 or Ap horizon, or calcareous within a depth of 0.2 m (whichever is shallower)" ;
  skos:notation "JN" ;
  skos:prefLabel "Calsilic" ;
.
asc:JP
  a asc:Class ;
  skos:definition "[RE] Soils with a layer or horizon, other than the surface horizon, that has a light sandy loam texture (about 10-15% clay) that begins within the upper 1.0 m of the soil profile. Kandic Arenosols have affinities with Kandosols but are too sandy." ;
  skos:notation "JP" ;
  skos:prefLabel "Kandic" ;
.
asc:JQ
  a asc:Class ;
  a skos:Concept ;
  dcterms:identifier "http://anzsoil.org/def/au/asc/JQ"^^xsd:anyURI ;
  skos:definition "[RE] Soils in which the major part of the upper 1.0 m has a distinct gritty feel." ;
  skos:definition "[RU] Soils in which the major part of the upper 1.0 m has a distinct gritty feel." ;
  skos:definition "[TE] Soils in which the major part of the upper 1.0 m has a distinct gritty feel." ;
  skos:notation "JQ" ;
  skos:prefLabel "Gritty" ;
.
asc:JR
  a asc:Class ;
  skos:definition "[RE] Soils in which the major part of the upper 1.5 m of the soil profile consists of visible heavy or opaque minerals (>3%) that may also be visibly stratified (identifiable by wet panning in the field)." ;
  skos:notation "JR" ;
  skos:prefLabel "Gravic" ;
.
asc:JT
  a asc:Class ;
  a skos:Concept ;
  skos:definition "[CA] Soils which are calcareous throughout. The upper 0.1 m of the solum consists of dominantly fine earth carbonate (visual estimate) and/or contains more than 40% (by analysis) of fine earth carbonate." ;
  skos:definition "[RE] Soils which are calcareous throughout (at least the upper 1.0 m of the soil profile). The upper 0.1 m of the soil profile consists of dominantly fine earth carbonate (visual estimate) and/or contains more than 40% (by analysis) of fine earth carbonate." ;
  skos:notation "JT" ;
  skos:prefLabel "Carbonatic" ;
.
asc:JU
  a asc:Class ;
  skos:definition "[RU] Soils that directly overlie a coquina substrate." ;
  skos:notation "JU" ;
  skos:prefLabel "Coquinic" ;
.
asc:JV
  a asc:Class ;
  a skos:Concept ;
  dcterms:identifier "http://anzsoil.org/def/au/asc/JV"^^xsd:anyURI ;
  skos:definition "[TE] Soils in which a major part of the upper 1.0 m has a distinct gritty feel and overlies a siliceous pan." ;
  skos:notation "JV" ;
  skos:prefLabel "Gritty-Silpanic " ;
.
asc:JW
  a asc:Class ;
  a skos:Concept ;
  dcterms:identifier "http://anzsoil.org/def/au/asc/JW"^^xsd:anyURI ;
  skos:definition "[TE] Soils in which the major part of the upper 1.0 m has a distinct gritty feel and overlies hard rock." ;
  skos:notation "JW" ;
  skos:prefLabel "Gritty-Lithic " ;
.
asc:JX
  a asc:Class ;
  a skos:Concept ;
  dcterms:identifier "http://anzsoil.org/def/au/asc/JX"^^xsd:anyURI ;
  skos:definition "[TE] Soils in which the major part of the upper 1.0 m has a distinct gritty feel and overlies partially weathered or decomposed rock or saprolite." ;
  skos:notation "JX" ;
  skos:prefLabel "Gritty-Paralithic" ;
.
asc:JZ
  a asc:Alteration ;
  a asc:Class ;
  skos:definition "[OR] ≥20% fusic material" ;
  skos:notation "JZ" ;
  skos:prefLabel "Vitric" ;
.
asc:K
  a asc:Class ;
  a asc:Texture ;
  skos:definition "S–LS–CS (up to 10% clay)" ;
  skos:notation "K" ;
  skos:prefLabel "Sandy" ;
.
asc:KA
  a asc:Order ;
  a skos:Concept ;
  dcterms:description "This order accommodates those soils which lack strong texture contrast, have massive or only weakly structured B horizons, and are not calcareous throughout. The soils of this order range throughout the continent, often occurring locally as very large areas." ;
  dcterms:identifier "http://anzsoil.org/def/au/asc/KA"^^xsd:anyURI ;
  rdfs:comment """Because of the lack of clearly defined horizons in some of these soils (particularly the red forms) with thick sola, there can be argument as to how to identify the limits of the B2 horizon.

There may be difficulty differentiating between Kandosols and Arenosols, where texture and horizon development is weak and sandy textures dominate. Some Kandosols have very thick A and/or B1 horizons with sandy textures that overlie at > 1m deep, B2t horizons which exceed 15% clay.""" ;
  skos:definition """Soils other than Hydrosols which have all of the following:

1. B2 horizons in which the major part has a grade of pedality that is massive or weak.
2. A maximum clay content in some part of the B2 horizon which exceeds 15% (ie. heavy sandy loam [SL+] or heavier).
3. Do not have a clear or abrupt textural B horizon.
4. Are not calcareous throughout the solum, or below the A1 or Ap horizon or to a depth of 0.2 m if the A1 horizon is only weakly developed.""" ;
  skos:notation "KA" ;
  skos:prefLabel "Kandosols" ;
.
asc:KU
  a asc:Order ;
  a skos:Concept ;
  asc:colourclass asc:AA ;
  asc:colourclass asc:AB ;
  asc:colourclass asc:AC ;
  asc:colourclass asc:AD ;
  asc:colourclass asc:AE ;
  asc:colourclass-comment "The dominant colour class in the major part of the upper 0.2 m of the B2t horizon (or the major part of the entire B2t horizon if it is less than 0.2 m thick) is:" ;
  asc:family-comment "1 This refers to the most clayey field texture category." ;
  asc:family-criteria asc:A ;
  asc:family-criteria asc:B ;
  asc:family-criteria asc:C ;
  asc:family-criteria asc:D ;
  asc:family-criteria asc:E ;
  asc:family-criteria asc:F ;
  asc:family-criteria asc:G ;
  asc:family-criteria asc:H ;
  asc:family-criteria asc:I ;
  asc:family-criteria asc:J ;
  asc:family-criteria asc:K ;
  asc:family-criteria asc:L ;
  asc:family-criteria asc:M ;
  asc:family-criteria asc:N ;
  asc:family-criteria asc:NR ;
  asc:family-criteria asc:O ;
  asc:family-criteria asc:SR ;
  asc:family-criteria asc:T ;
  asc:family-criteria asc:U ;
  asc:family-criteria asc:V ;
  asc:family-criteria asc:W ;
  asc:family-criteria asc:WR ;
  asc:family-criteria asc:X ;
  asc:family-criteria asc:Y ;
  dcterms:description "Soils with strong texture contrast between A horizons and strongly acid B horizons. Many of these soils have some unusual subsoil chemical features (high magnesium, sodium and aluminium)." ;
  dcterms:identifier "http://anzsoil.org/def/au/asc/KU"^^xsd:anyURI ;
  rdfs:comment "The relevance of sodicity in strongly acid soils is open to question as in theory the presence of aluminium in such soils should counterbalance the usual deleterious effect of sodium (via dispersion) on soil physical properties. Unpublished data from many localities in Australia imply that for B horizons the critical limits of pHw 5.5 and ESP of 6 to distinguish dispersive and non-dispersive soils seems to generally work in practice, although as might be expected, some soils do not behave as predicted. For this reason, sodicity is also used in Kurosols, but at a lower hierarchical level, to cater for those soils which have an ESP > 6 and may disperse in spite of having a pHw less than 5.5. The role of the high exchangeable magnesium in many Kurosols is largely unknown." ;
  skos:definition "Soils other than Hydrosols with a clear or abrupt textural B horizon and in which the major part of the upper 0.2 m of the B2t horizon (or the major part of the entire B2t horizon if it is less than 0.2 m thick) is strongly acid." ;
  skos:narrower asc:KU-AA ;
  skos:narrower asc:KU-AB ;
  skos:narrower asc:KU-AC ;
  skos:narrower asc:KU-AD ;
  skos:narrower asc:KU-AE ;
  skos:notation "KU" ;
  skos:prefLabel "Kurosols" ;
.
asc:KU-AA
  a asc:Suborder ;
  asc:classifier asc:AA ;
  asc:greatgroup asc:AF ;
  asc:greatgroup asc:AG ;
  asc:greatgroup asc:AH ;
  asc:greatgroup asc:DB ;
  asc:greatgroup asc:EA ;
  asc:greatgroup asc:FD ;
  asc:greatgroup asc:GP ;
  asc:greatgroup-comment """These will vary somewhat among the various colour class suborders, but it is likely that the subdivisions given below will apply to most.

If a diagnostic feature in the key begins more than 1.5 m from the soil surface it may not have a significant impact on the performance of the soil. Refer to diagnostic features in the glossary for guidance on the use of such features in the classification.

A feature of the soils classified is the common occurrence of high subsoil exchangeable magnesium with or without sodium. In spite of an upper B2t horizon that is strongly acid, Mesotrophic great groups are more common than the Dystrophic forms. This is often related to relatively high magnesium values.""" ;
  asc:subgroup asc:AT ;
  asc:subgroup asc:AV ;
  asc:subgroup asc:AY ;
  asc:subgroup asc:AZ ;
  asc:subgroup asc:BA ;
  asc:subgroup asc:BB ;
  asc:subgroup asc:BU ;
  asc:subgroup asc:CD ;
  asc:subgroup asc:CK ;
  asc:subgroup asc:DC ;
  asc:subgroup asc:DG ;
  asc:subgroup asc:DK ;
  asc:subgroup asc:DN ;
  asc:subgroup asc:DQ ;
  asc:subgroup asc:EF ;
  asc:subgroup asc:EO ;
  asc:subgroup asc:EX ;
  asc:subgroup asc:EY ;
  asc:subgroup asc:EZ ;
  asc:subgroup asc:HB ;
  asc:subgroup-comment """The subgroups listed will not all be relevant for every great group. eg. Sodic classes will not be required for the Natric great groups.

If a diagnostic feature in the key begins more than 1.5 m from the soil surface it may not have a significant impact on the performance of the soil. Refer to diagnostic features in the glossary for guidance on the use of such features in the classification.

A significant proportion of the soils classified to date have mottled B2t horizons which suggests a trend to poorer internal drainage in the Kurosols compared to Chromosols.""" ;
  skos:broader asc:KU ;
  skos:notation "KU-AA" ;
  skos:prefLabel "Red Kurosol" ;
.
asc:KU-AB
  a asc:Suborder ;
  asc:classifier asc:AB ;
  asc:greatgroup asc:AF ;
  asc:greatgroup asc:AG ;
  asc:greatgroup asc:AH ;
  asc:greatgroup asc:DB ;
  asc:greatgroup asc:EA ;
  asc:greatgroup asc:FD ;
  asc:greatgroup asc:GP ;
  asc:greatgroup-comment """These will vary somewhat among the various colour class suborders, but it is likely that the subdivisions given below will apply to most.

If a diagnostic feature in the key begins more than 1.5 m from the soil surface it may not have a significant impact on the performance of the soil. Refer to diagnostic features in the glossary for guidance on the use of such features in the classification.

A feature of the soils classified is the common occurrence of high subsoil exchangeable magnesium with or without sodium. In spite of an upper B2t horizon that is strongly acid, Mesotrophic great groups are more common than the Dystrophic forms. This is often related to relatively high magnesium values.""" ;
  asc:subgroup asc:AT ;
  asc:subgroup asc:AV ;
  asc:subgroup asc:AY ;
  asc:subgroup asc:AZ ;
  asc:subgroup asc:BA ;
  asc:subgroup asc:BB ;
  asc:subgroup asc:BU ;
  asc:subgroup asc:CD ;
  asc:subgroup asc:CK ;
  asc:subgroup asc:DC ;
  asc:subgroup asc:DG ;
  asc:subgroup asc:DK ;
  asc:subgroup asc:DN ;
  asc:subgroup asc:DQ ;
  asc:subgroup asc:EF ;
  asc:subgroup asc:EO ;
  asc:subgroup asc:EX ;
  asc:subgroup asc:EY ;
  asc:subgroup asc:EZ ;
  asc:subgroup asc:HB ;
  asc:subgroup-comment """The subgroups listed will not all be relevant for every great group. eg. Sodic classes will not be required for the Natric great groups.

If a diagnostic feature in the key begins more than 1.5 m from the soil surface it may not have a significant impact on the performance of the soil. Refer to diagnostic features in the glossary for guidance on the use of such features in the classification.

A significant proportion of the soils classified to date have mottled B2t horizons which suggests a trend to poorer internal drainage in the Kurosols compared to Chromosols.""" ;
  skos:broader asc:KU ;
  skos:notation "KU-AB" ;
  skos:prefLabel "Brown Kurosol" ;
.
asc:KU-AC
  a asc:Suborder ;
  asc:classifier asc:AC ;
  asc:greatgroup asc:AF ;
  asc:greatgroup asc:AG ;
  asc:greatgroup asc:AH ;
  asc:greatgroup asc:DB ;
  asc:greatgroup asc:EA ;
  asc:greatgroup asc:FD ;
  asc:greatgroup asc:GP ;
  asc:greatgroup-comment """These will vary somewhat among the various colour class suborders, but it is likely that the subdivisions given below will apply to most.

If a diagnostic feature in the key begins more than 1.5 m from the soil surface it may not have a significant impact on the performance of the soil. Refer to diagnostic features in the glossary for guidance on the use of such features in the classification.

A feature of the soils classified is the common occurrence of high subsoil exchangeable magnesium with or without sodium. In spite of an upper B2t horizon that is strongly acid, Mesotrophic great groups are more common than the Dystrophic forms. This is often related to relatively high magnesium values.""" ;
  asc:subgroup asc:AT ;
  asc:subgroup asc:AV ;
  asc:subgroup asc:AY ;
  asc:subgroup asc:AZ ;
  asc:subgroup asc:BA ;
  asc:subgroup asc:BB ;
  asc:subgroup asc:BU ;
  asc:subgroup asc:CD ;
  asc:subgroup asc:CK ;
  asc:subgroup asc:DC ;
  asc:subgroup asc:DG ;
  asc:subgroup asc:DK ;
  asc:subgroup asc:DN ;
  asc:subgroup asc:DQ ;
  asc:subgroup asc:EF ;
  asc:subgroup asc:EO ;
  asc:subgroup asc:EX ;
  asc:subgroup asc:EY ;
  asc:subgroup asc:EZ ;
  asc:subgroup asc:HB ;
  asc:subgroup-comment """The subgroups listed will not all be relevant for every great group. eg. Sodic classes will not be required for the Natric great groups.

If a diagnostic feature in the key begins more than 1.5 m from the soil surface it may not have a significant impact on the performance of the soil. Refer to diagnostic features in the glossary for guidance on the use of such features in the classification.

A significant proportion of the soils classified to date have mottled B2t horizons which suggests a trend to poorer internal drainage in the Kurosols compared to Chromosols.""" ;
  skos:broader asc:KU ;
  skos:notation "KU-AC" ;
  skos:prefLabel "Yellow Kurosol" ;
.
asc:KU-AD
  a asc:Suborder ;
  asc:classifier asc:AD ;
  asc:greatgroup asc:AF ;
  asc:greatgroup asc:AG ;
  asc:greatgroup asc:AH ;
  asc:greatgroup asc:DB ;
  asc:greatgroup asc:EA ;
  asc:greatgroup asc:FD ;
  asc:greatgroup asc:GP ;
  asc:greatgroup-comment """These will vary somewhat among the various colour class suborders, but it is likely that the subdivisions given below will apply to most.

If a diagnostic feature in the key begins more than 1.5 m from the soil surface it may not have a significant impact on the performance of the soil. Refer to diagnostic features in the glossary for guidance on the use of such features in the classification.

A feature of the soils classified is the common occurrence of high subsoil exchangeable magnesium with or without sodium. In spite of an upper B2t horizon that is strongly acid, Mesotrophic great groups are more common than the Dystrophic forms. This is often related to relatively high magnesium values.""" ;
  asc:subgroup asc:AT ;
  asc:subgroup asc:AV ;
  asc:subgroup asc:AY ;
  asc:subgroup asc:AZ ;
  asc:subgroup asc:BA ;
  asc:subgroup asc:BB ;
  asc:subgroup asc:BU ;
  asc:subgroup asc:CD ;
  asc:subgroup asc:CK ;
  asc:subgroup asc:DC ;
  asc:subgroup asc:DG ;
  asc:subgroup asc:DK ;
  asc:subgroup asc:DN ;
  asc:subgroup asc:DQ ;
  asc:subgroup asc:EF ;
  asc:subgroup asc:EO ;
  asc:subgroup asc:EX ;
  asc:subgroup asc:EY ;
  asc:subgroup asc:EZ ;
  asc:subgroup asc:HB ;
  asc:subgroup-comment """The subgroups listed will not all be relevant for every great group. eg. Sodic classes will not be required for the Natric great groups.

If a diagnostic feature in the key begins more than 1.5 m from the soil surface it may not have a significant impact on the performance of the soil. Refer to diagnostic features in the glossary for guidance on the use of such features in the classification.

A significant proportion of the soils classified to date have mottled B2t horizons which suggests a trend to poorer internal drainage in the Kurosols compared to Chromosols.""" ;
  skos:broader asc:KU ;
  skos:notation "KU-AD" ;
  skos:prefLabel "Grey Kurosol" ;
.
asc:KU-AE
  a asc:Suborder ;
  asc:classifier asc:AE ;
  asc:greatgroup asc:AF ;
  asc:greatgroup asc:AG ;
  asc:greatgroup asc:AH ;
  asc:greatgroup asc:DB ;
  asc:greatgroup asc:EA ;
  asc:greatgroup asc:FD ;
  asc:greatgroup asc:GP ;
  asc:greatgroup-comment """These will vary somewhat among the various colour class suborders, but it is likely that the subdivisions given below will apply to most.

If a diagnostic feature in the key begins more than 1.5 m from the soil surface it may not have a significant impact on the performance of the soil. Refer to diagnostic features in the glossary for guidance on the use of such features in the classification.

A feature of the soils classified is the common occurrence of high subsoil exchangeable magnesium with or without sodium. In spite of an upper B2t horizon that is strongly acid, Mesotrophic great groups are more common than the Dystrophic forms. This is often related to relatively high magnesium values.""" ;
  asc:subgroup asc:AT ;
  asc:subgroup asc:AV ;
  asc:subgroup asc:AY ;
  asc:subgroup asc:AZ ;
  asc:subgroup asc:BA ;
  asc:subgroup asc:BB ;
  asc:subgroup asc:BU ;
  asc:subgroup asc:CD ;
  asc:subgroup asc:CK ;
  asc:subgroup asc:DC ;
  asc:subgroup asc:DG ;
  asc:subgroup asc:DK ;
  asc:subgroup asc:DN ;
  asc:subgroup asc:DQ ;
  asc:subgroup asc:EF ;
  asc:subgroup asc:EO ;
  asc:subgroup asc:EX ;
  asc:subgroup asc:EY ;
  asc:subgroup asc:EZ ;
  asc:subgroup asc:HB ;
  asc:subgroup-comment """The subgroups listed will not all be relevant for every great group. eg. Sodic classes will not be required for the Natric great groups.

If a diagnostic feature in the key begins more than 1.5 m from the soil surface it may not have a significant impact on the performance of the soil. Refer to diagnostic features in the glossary for guidance on the use of such features in the classification.

A significant proportion of the soils classified to date have mottled B2t horizons which suggests a trend to poorer internal drainage in the Kurosols compared to Chromosols.""" ;
  skos:broader asc:KU ;
  skos:notation "KU-AE" ;
  skos:prefLabel "Black Kurosol" ;
.
asc:L
  a asc:Class ;
  a asc:Texture ;
  skos:definition "SL–L (10–20% clay)" ;
  skos:notation "L" ;
  skos:prefLabel "Loamy" ;
.
asc:M
  a asc:Class ;
  a asc:Texture ;
  skos:definition "SCL–CL (20–35% clay)" ;
  skos:notation "M" ;
  skos:prefLabel "Clay loamy" ;
.
asc:N
  a asc:Class ;
  a asc:Texture ;
  skos:definition "ZL–ZCL (25–35% clay and silt 25% or more)" ;
  skos:notation "N" ;
  skos:prefLabel "Silty" ;
.
asc:NR
  a asc:Class ;
  a asc:Water-repellence ;
  skos:definition "Water absorbed in 10 seconds or less" ;
  skos:notation "NR" ;
  skos:prefLabel "Non water repellent" ;
.
asc:O
  a asc:Class ;
  a asc:Texture ;
  skos:definition "LC–MC–HC (> 35% clay)" ;
  skos:notation "O" ;
  skos:prefLabel "Clayey" ;
.
asc:OA
  a asc:Class ;
  a asc:Organic-type ;
  skos:definition "[OR] Fibric peat" ;
  skos:notation "OA" ;
  skos:prefLabel "Fibric peat" ;
.
asc:OB
  a asc:Class ;
  a asc:Organic-type ;
  skos:definition "[OR] Hemic peat" ;
  skos:notation "OB" ;
  skos:prefLabel "Hemic peat" ;
.
asc:OC
  a asc:Class ;
  a asc:Organic-type ;
  skos:definition "[OR] Sapric peat" ;
  skos:notation "OC" ;
  skos:prefLabel "Sapric peat" ;
.
asc:OD
  a asc:Class ;
  a asc:Organic-type ;
  skos:definition "[OR] Sandy peat" ;
  skos:notation "OD" ;
  skos:prefLabel "Sandy peat" ;
.
asc:OE
  a asc:Class ;
  a asc:Organic-type ;
  skos:definition "[OR] Loamy peat" ;
  skos:notation "OE" ;
  skos:prefLabel "Loamy peat" ;
.
asc:OF
  a asc:Class ;
  a asc:Organic-type ;
  skos:definition "[OR] Clayey peat" ;
  skos:notation "OF" ;
  skos:prefLabel "Clayey peat" ;
.
asc:OR
  a asc:Order ;
  a skos:Concept ;
  asc:family-comment """Texture classes specific to organic materials (and consistent with horizon definitions in the Field Handbook) describe the dominant texture of the uppermost organic materials, horizons or layers. These classes provide a useful insight to the formation processes of and inherent vulnerabilities to the uppermost organic materials.

Granular is applied if there is a layer at least 0.2 m thick that has a distinct granular or subangular blocky type of pedality (see Field Handbook). This condition occurs in some peat soils that have either naturally dried out, or have been drained or drained and cultivated, and are also known as earthy or ripened peats. In Australia it is known to occur with sapric peats, but it is uncertain if it occurs with hemic or fibric peats.

Ashy and Vitric reflect the influence of fire.""" ;
  asc:family-criteria asc:B ;
  asc:family-criteria asc:C ;
  asc:family-criteria asc:D ;
  asc:family-criteria asc:E ;
  asc:family-criteria asc:F ;
  asc:family-criteria asc:G ;
  asc:family-criteria asc:H ;
  asc:family-criteria asc:HZ ;
  asc:family-criteria asc:I ;
  asc:family-criteria asc:JZ ;
  asc:family-criteria asc:K ;
  asc:family-criteria asc:L ;
  asc:family-criteria asc:M ;
  asc:family-criteria asc:N ;
  asc:family-criteria asc:O ;
  asc:family-criteria asc:OA ;
  asc:family-criteria asc:OB ;
  asc:family-criteria asc:OC ;
  asc:family-criteria asc:OD ;
  asc:family-criteria asc:OE ;
  asc:family-criteria asc:OF ;
  asc:family-criteria asc:P ;
  asc:family-criteria asc:T ;
  asc:family-criteria asc:U ;
  asc:family-criteria asc:V ;
  asc:family-criteria asc:W ;
  asc:family-criteria asc:X ;
  asc:family-criteria asc:Y ;
  asc:family-criteria asc:Z ;
  asc:suborder asc:BW ;
  asc:suborder asc:CE ;
  asc:suborder asc:EH ;
  asc:suborder-comment """The terms fibric, hemic and sapric are essentially the same as defined in the World Reference Base (2015) and Soil Taxonomy (Soil Survey Staff 2014) and give an indication of the relative decomposition of the organic materials If the proportions of peats in a profile are such that no peat type is dominant then the peat type with the most advanced level of decomposition should be selected.

In some north Queensland seasonal swamps, thick peats can have 0.3–0.4 m of sapric over hemic and/or fibric peat. Conversely many organic moorland soils found in the remote south western wilderness area of Tasmania often grade from fibric and hemic peat through to an underlying sapric peat. When more data are available it may be necessary to modify the Suborder definitions to cater for soils where the type of peat changes with depth.""" ;
  dcterms:description "This class caters for most soils dominated by organic materials Although they are found from the wet tropics to the alpine regions, areas are mostly small except in south west Tasmania. There have been few previous attempts to subdivide these soils and substantial data are limited to Tasmania." ;
  dcterms:identifier "http://anzsoil.org/def/au/asc/OR"^^xsd:anyURI ;
  rdfs:comment "Soils with peaty horizons that do not meet the organic materials requirements of Organosols are catered for in other Orders, commonly Hydrosols. Organosols may classify as a buried soil if overlain by aeolian or fluvial deposits that may have undergone other developmental processes. If the overlying material is less than 0.3 m and can only qualify as a Rudosol, it is regarded as a depositional phase of the Organosol below." ;
  skos:definition """Soils that are not regularly inundated by saline tidal waters and either:

1. Have more than 0.4 m of organic materials within the upper 0.8 m. The required thickness may either extend down from the surface or be taken cumulatively within the upper 0.8 m; or
2. Have organic materials extending from the surface to a minimum depth of 0.1 m; these either overlie a mineral soil horizon or unconsolidated mineral material no thicker than the organic materials above, or directly overlie rock or other hard layers, partially weathered or decomposed rock or saprolite, or overlie fragmental material such as gravel, cobbles or stones in which the interstices are filled or partially filled with organic material. In some soils there may be layers of humose, melacic and/or melanic horizon material underlying the organic materials and overlying the substrate.""" ;
  skos:narrower asc:OR-BW ;
  skos:narrower asc:OR-CE ;
  skos:narrower asc:OR-EH ;
  skos:notation "OR" ;
  skos:prefLabel "Organosols" ;
.
asc:OR-BW
  a asc:Suborder ;
  asc:classifier asc:BW ;
  asc:greatgroup asc:AI ;
  asc:greatgroup asc:AR ;
  asc:greatgroup asc:BC ;
  asc:greatgroup asc:EU ;
  asc:greatgroup asc:EV ;
  asc:greatgroup asc:IF ;
  asc:greatgroup asc:IW ;
  asc:greatgroup asc:IX ;
  asc:greatgroup asc:IZ ;
  asc:greatgroup asc:JA ;
  asc:greatgroup asc:JC ;
  asc:greatgroup-comment "It is likely that not all of the great groups below will be applicable to each suborder. It is also likely that other great groups will be required as knowledge increases." ;
  asc:subgroup asc:CZ ;
  asc:subgroup asc:DD ;
  asc:subgroup asc:DU ;
  asc:subgroup asc:EC ;
  asc:subgroup asc:FS ;
  asc:subgroup asc:GF ;
  asc:subgroup asc:HD ;
  asc:subgroup asc:IJ ;
  asc:subgroup-comment """The following subgroups may not be relevant to all great groups of each suborder, and future investigations may reveal additional subgroups.

If a diagnostic feature in the key begins more than 1.5 m from the soil surface it may not have a significant impact on the performance of the soil. Refer to diagnostic features in the glossary for guidance on the use of such features in the classification.""" ;
  skos:broader asc:OR ;
  skos:notation "OR-BW" ;
  skos:prefLabel "Fibric Organosol" ;
.
asc:OR-CE
  a asc:Suborder ;
  asc:classifier asc:CE ;
  asc:greatgroup asc:AI ;
  asc:greatgroup asc:AR ;
  asc:greatgroup asc:BC ;
  asc:greatgroup asc:EU ;
  asc:greatgroup asc:EV ;
  asc:greatgroup asc:IF ;
  asc:greatgroup asc:IW ;
  asc:greatgroup asc:IX ;
  asc:greatgroup asc:IZ ;
  asc:greatgroup asc:JA ;
  asc:greatgroup asc:JC ;
  asc:greatgroup-comment "It is likely that not all of the great groups below will be applicable to each suborder. It is also likely that other great groups will be required as knowledge increases." ;
  asc:subgroup asc:CZ ;
  asc:subgroup asc:DD ;
  asc:subgroup asc:DU ;
  asc:subgroup asc:EC ;
  asc:subgroup asc:FS ;
  asc:subgroup asc:GF ;
  asc:subgroup asc:HD ;
  asc:subgroup asc:IJ ;
  asc:subgroup-comment """The following subgroups may not be relevant to all great groups of each suborder, and future investigations may reveal additional subgroups.

If a diagnostic feature in the key begins more than 1.5 m from the soil surface it may not have a significant impact on the performance of the soil. Refer to diagnostic features in the glossary for guidance on the use of such features in the classification.""" ;
  skos:broader asc:OR ;
  skos:notation "OR-BW" ;
  skos:prefLabel "Hemic Organosol" ;
.
asc:OR-EH
  a asc:Suborder ;
  asc:classifier asc:EH ;
  asc:greatgroup asc:AI ;
  asc:greatgroup asc:AR ;
  asc:greatgroup asc:BC ;
  asc:greatgroup asc:EU ;
  asc:greatgroup asc:EV ;
  asc:greatgroup asc:IF ;
  asc:greatgroup asc:IW ;
  asc:greatgroup asc:IX ;
  asc:greatgroup asc:IZ ;
  asc:greatgroup asc:JA ;
  asc:greatgroup asc:JC ;
  asc:greatgroup-comment "It is likely that not all of the great groups below will be applicable to each suborder. It is also likely that other great groups will be required as knowledge increases." ;
  asc:subgroup asc:CZ ;
  asc:subgroup asc:DD ;
  asc:subgroup asc:DU ;
  asc:subgroup asc:EC ;
  asc:subgroup asc:FS ;
  asc:subgroup asc:GF ;
  asc:subgroup asc:HD ;
  asc:subgroup asc:IJ ;
  asc:subgroup-comment """The following subgroups may not be relevant to all great groups of each suborder, and future investigations may reveal additional subgroups.

If a diagnostic feature in the key begins more than 1.5 m from the soil surface it may not have a significant impact on the performance of the soil. Refer to diagnostic features in the glossary for guidance on the use of such features in the classification.""" ;
  skos:broader asc:OR ;
  skos:notation "OR-EH" ;
  skos:prefLabel "Sapric Organosol" ;
.
asc:Order
  a owl:Class ;
  rdfs:label "Soil order" ;
  rdfs:subClassOf skos:Concept ;
  rdfs:subClassOf [
      a owl:Restriction ;
      owl:allValuesFrom asc:Suborder ;
      owl:onProperty skos:narrower ;
    ] ;
.
asc:Organic-type
  a owl:Class ;
  rdfs:subClassOf asc:Class ;
  skos:prefLabel "Type of organic materials" ;
.
asc:P
  a asc:Alteration ;
  a asc:Class ;
  skos:definition "[OR] Granular or subangular blocky type of pedality" ;
  skos:notation "P" ;
  skos:prefLabel "Granular" ;
.
asc:PO
  a asc:Order ;
  a skos:Concept ;
  asc:family-criteria asc:A ;
  asc:family-criteria asc:B ;
  asc:family-criteria asc:C ;
  asc:family-criteria asc:D ;
  asc:family-criteria asc:E ;
  asc:family-criteria asc:F ;
  asc:family-criteria asc:G ;
  asc:family-criteria asc:H ;
  asc:family-criteria asc:I ;
  asc:family-criteria asc:J ;
  asc:family-criteria asc:K ;
  asc:family-criteria asc:L ;
  asc:family-criteria asc:M ;
  asc:family-criteria asc:N ;
  asc:family-criteria asc:NR ;
  asc:family-criteria asc:O ;
  asc:family-criteria asc:SR ;
  asc:family-criteria asc:T ;
  asc:family-criteria asc:U ;
  asc:family-criteria asc:V ;
  asc:family-criteria asc:W ;
  asc:family-criteria asc:WR ;
  asc:family-criteria asc:X ;
  asc:family-criteria asc:Y ;
  asc:suborder asc:AL ;
  asc:suborder asc:AM ;
  asc:suborder asc:EJ ;
  asc:suborder asc:JD ;
  asc:suborder asc:JE ;
  asc:suborder-comment "These are based on soil and site drainage conditions. The intention is to separate soils with no short-term saturation in the B horizon, those with short-term saturation of the B horizon, and those that are saturated for long periods in the B horizon." ;
  dcterms:description "Soils with B horizons dominated by the accumulation of compounds of organic matter, aluminium and/or iron. These soils are recognised world-wide, and Australia is particularly noted for its 'giant' forms. Podosols are typically found in close proximity to the coast and on islands comprised of quartz sand." ;
  dcterms:identifier "http://anzsoil.org/def/au/asc/PO"^^xsd:anyURI ;
  rdfs:comment """Extensive revisions of the classification of Spodosols and Podzols have taken place in the USA (with world-wide input) and New Zealand. It is clear that there is considerable diversity of opinion on the desirability, nature and efficacy of chemical criteria to define Spodosols/Podzols. For this reason the present proposal for Australian 'podzols' has deliberately avoided the use of chemical diagnostic criteria.

Some Podosols with deep diagnostic B horizons may classify initially as Bleached Arenosols. Only deep examination of the soil profile can confirm the order of such soils.""" ;
  skos:definition "Soils which possess either a Bs horizon (visible dominance of iron compounds), a Bhs horizon (organic-aluminium and iron compounds), or a Bh horizon (organic-aluminium compounds). These horizons may occur singly in a profile or in combination (see Podosol diagnostic horizons)." ;
  skos:narrower asc:PO-AL ;
  skos:narrower asc:PO-AM ;
  skos:narrower asc:PO-EJ ;
  skos:narrower asc:PO-JD ;
  skos:narrower asc:PO-JE ;
  skos:notation "PO" ;
  skos:prefLabel "Podosols" ;
.
asc:PO-AL
  a asc:Suborder ;
  asc:classifier asc:AL ;
  asc:greatgroup asc:CO ;
  asc:greatgroup asc:EB ;
  asc:greatgroup asc:EK ;
  asc:greatgroup asc:IG ;
  asc:greatgroup-comment """Classes are based on observable B horizon characteristics reflecting the dominance of organic or iron compounds and their distribution in the accumulation zone. The organic accumulations can usually be recognised by their dark colours and the iron compounds by generally bright colours. Aluminium is always present, usually complexed by organic matter and therefore not usually visible, except in some horizons where large amounts of amorphous aluminium and silica (imogolite-allophane complexes) may induce a yellowish brown colouration. Yellowish brown bands in poorly-drained B horizons should not be interpreted as evidence of iron compounds without chemical verification.

In the soils classified the most common class in the Aeric suborder is the Sesquic great group, but Humic is most common in the Semiaquic and Aquic Suborders.""" ;
  asc:subgroup asc:BI ;
  asc:subgroup asc:BU ;
  asc:subgroup asc:BY ;
  asc:subgroup asc:CK ;
  asc:subgroup asc:CN ;
  asc:subgroup asc:DG ;
  asc:subgroup asc:DJ ;
  asc:subgroup asc:DK ;
  asc:subgroup asc:DV ;
  asc:subgroup asc:DW ;
  asc:subgroup asc:DX ;
  asc:subgroup asc:EC ;
  asc:subgroup asc:EM ;
  asc:subgroup asc:GD ;
  asc:subgroup asc:HN ;
  asc:subgroup-comment """Each class listed below may not be relevant for every great group of each suborder.

If a diagnostic feature in the key begins more than 1.5 m from the soil surface it may not have a significant impact on the performance of the soil. Refer to diagnostic features in the glossary for guidance on the use of such features in the classification.

The term 'parapanic' is meant to imply 'pan-like'. Note also that the A1 horizons of many Podosols may have a distinct surface layer of lighter coloured sand with clean quartz grains and discrete lumps of organic matter and charcoal, giving the layer a speckled appearance. Below this layer, a dark A1 horizon may occur. Because the great majority of Australian Podosols have a bleached A2 horizon, this attribute is not used in the classification. Similarly, the great majority have a B horizon pHw of less than 5.5, hence acidic subgroups have not been used.""" ;
  skos:broader asc:PO ;
  skos:notation "PO-AL" ;
  skos:prefLabel "Aeric Podosol" ;
.
asc:PO-AM
  a asc:Suborder ;
  asc:classifier asc:AM ;
  asc:greatgroup asc:CG ;
  asc:greatgroup asc:IH ;
  asc:greatgroup-comment """Classes are based on observable B horizon characteristics reflecting the dominance of organic or iron compounds and their distribution in the accumulation zone. The organic accumulations can usually be recognised by their dark colours and the iron compounds by generally bright colours. Aluminium is always present, usually complexed by organic matter and therefore not usually visible, except in some horizons where large amounts of amorphous aluminium and silica (imogolite-allophane complexes) may induce a yellowish brown colouration. Yellowish brown bands in poorly-drained B horizons should not be interpreted as evidence of iron compounds without chemical verification.

In the soils classified the most common class in the Aeric suborder is the Sesquic great group, but Humic is most common in the Semiaquic and Aquic Suborders.""" ;
  asc:subgroup asc:BI ;
  asc:subgroup asc:BU ;
  asc:subgroup asc:BY ;
  asc:subgroup asc:CK ;
  asc:subgroup asc:CN ;
  asc:subgroup asc:DG ;
  asc:subgroup asc:DJ ;
  asc:subgroup asc:DK ;
  asc:subgroup asc:DV ;
  asc:subgroup asc:DW ;
  asc:subgroup asc:DX ;
  asc:subgroup asc:EC ;
  asc:subgroup asc:EM ;
  asc:subgroup asc:GD ;
  asc:subgroup asc:HN ;
  asc:subgroup-comment """Each class listed below may not be relevant for every great group of each suborder.

If a diagnostic feature in the key begins more than 1.5 m from the soil surface it may not have a significant impact on the performance of the soil. Refer to diagnostic features in the glossary for guidance on the use of such features in the classification.

The term 'parapanic' is meant to imply 'pan-like'. Note also that the A1 horizons of many Podosols may have a distinct surface layer of lighter coloured sand with clean quartz grains and discrete lumps of organic matter and charcoal, giving the layer a speckled appearance. Below this layer, a dark A1 horizon may occur. Because the great majority of Australian Podosols have a bleached A2 horizon, this attribute is not used in the classification. Similarly, the great majority have a B horizon pHw of less than 5.5, hence acidic subgroups have not been used.""" ;
  skos:broader asc:PO ;
  skos:notation "PO-AM" ;
  skos:prefLabel "Aquic Podosol" ;
.
asc:PO-EJ
  a asc:Suborder ;
  asc:classifier asc:EJ ;
  asc:greatgroup asc:CG ;
  asc:greatgroup asc:CI ;
  asc:greatgroup asc:CJ ;
  asc:greatgroup asc:CO ;
  asc:greatgroup asc:EB ;
  asc:greatgroup asc:EK ;
  asc:greatgroup asc:IH ;
  asc:greatgroup-comment """Classes are based on observable B horizon characteristics reflecting the dominance of organic or iron compounds and their distribution in the accumulation zone. The organic accumulations can usually be recognised by their dark colours and the iron compounds by generally bright colours. Aluminium is always present, usually complexed by organic matter and therefore not usually visible, except in some horizons where large amounts of amorphous aluminium and silica (imogolite-allophane complexes) may induce a yellowish brown colouration. Yellowish brown bands in poorly-drained B horizons should not be interpreted as evidence of iron compounds without chemical verification.

In the soils classified the most common class in the Aeric suborder is the Sesquic great group, but Humic is most common in the Semiaquic and Aquic Suborders.""" ;
  asc:subgroup asc:BI ;
  asc:subgroup asc:BU ;
  asc:subgroup asc:BY ;
  asc:subgroup asc:CK ;
  asc:subgroup asc:CN ;
  asc:subgroup asc:DG ;
  asc:subgroup asc:DJ ;
  asc:subgroup asc:DK ;
  asc:subgroup asc:DV ;
  asc:subgroup asc:DW ;
  asc:subgroup asc:DX ;
  asc:subgroup asc:EC ;
  asc:subgroup asc:EM ;
  asc:subgroup asc:GD ;
  asc:subgroup asc:HN ;
  asc:subgroup-comment """Each class listed below may not be relevant for every great group of each suborder.

If a diagnostic feature in the key begins more than 1.5 m from the soil surface it may not have a significant impact on the performance of the soil. Refer to diagnostic features in the glossary for guidance on the use of such features in the classification.

The term 'parapanic' is meant to imply 'pan-like'. Note also that the A1 horizons of many Podosols may have a distinct surface layer of lighter coloured sand with clean quartz grains and discrete lumps of organic matter and charcoal, giving the layer a speckled appearance. Below this layer, a dark A1 horizon may occur. Because the great majority of Australian Podosols have a bleached A2 horizon, this attribute is not used in the classification. Similarly, the great majority have a B horizon pHw of less than 5.5, hence acidic subgroups have not been used.""" ;
  skos:broader asc:PO ;
  skos:notation "PO-EJ" ;
  skos:prefLabel "Semiaquic Podosol" ;
.
asc:PO-JD
  a asc:Suborder ;
  asc:classifier asc:JD ;
  asc:greatgroup asc:CG ;
  asc:greatgroup asc:IH ;
  asc:greatgroup-comment """Classes are based on observable B horizon characteristics reflecting the dominance of organic or iron compounds and their distribution in the accumulation zone. The organic accumulations can usually be recognised by their dark colours and the iron compounds by generally bright colours. Aluminium is always present, usually complexed by organic matter and therefore not usually visible, except in some horizons where large amounts of amorphous aluminium and silica (imogolite-allophane complexes) may induce a yellowish brown colouration. Yellowish brown bands in poorly-drained B horizons should not be interpreted as evidence of iron compounds without chemical verification.

In the soils classified the most common class in the Aeric suborder is the Sesquic great group, but Humic is most common in the Semiaquic and Aquic Suborders.""" ;
  asc:subgroup asc:BI ;
  asc:subgroup asc:BU ;
  asc:subgroup asc:BY ;
  asc:subgroup asc:CK ;
  asc:subgroup asc:CN ;
  asc:subgroup asc:DG ;
  asc:subgroup asc:DJ ;
  asc:subgroup asc:DK ;
  asc:subgroup asc:DV ;
  asc:subgroup asc:DW ;
  asc:subgroup asc:DX ;
  asc:subgroup asc:EC ;
  asc:subgroup asc:EM ;
  asc:subgroup asc:GD ;
  asc:subgroup asc:HN ;
  asc:subgroup-comment """Each class listed below may not be relevant for every great group of each suborder.

If a diagnostic feature in the key begins more than 1.5 m from the soil surface it may not have a significant impact on the performance of the soil. Refer to diagnostic features in the glossary for guidance on the use of such features in the classification.

The term 'parapanic' is meant to imply 'pan-like'. Note also that the A1 horizons of many Podosols may have a distinct surface layer of lighter coloured sand with clean quartz grains and discrete lumps of organic matter and charcoal, giving the layer a speckled appearance. Below this layer, a dark A1 horizon may occur. Because the great majority of Australian Podosols have a bleached A2 horizon, this attribute is not used in the classification. Similarly, the great majority have a B horizon pHw of less than 5.5, hence acidic subgroups have not been used.""" ;
  skos:broader asc:PO ;
  skos:notation "PO-JD" ;
  skos:prefLabel "Aquic-Sulfuric Podosol" ;
.
asc:PO-JE
  a asc:Suborder ;
  asc:classifier asc:JE ;
  asc:greatgroup asc:CG ;
  asc:greatgroup asc:IH ;
  asc:greatgroup-comment """Classes are based on observable B horizon characteristics reflecting the dominance of organic or iron compounds and their distribution in the accumulation zone. The organic accumulations can usually be recognised by their dark colours and the iron compounds by generally bright colours. Aluminium is always present, usually complexed by organic matter and therefore not usually visible, except in some horizons where large amounts of amorphous aluminium and silica (imogolite-allophane complexes) may induce a yellowish brown colouration. Yellowish brown bands in poorly-drained B horizons should not be interpreted as evidence of iron compounds without chemical verification.

In the soils classified the most common class in the Aeric suborder is the Sesquic great group, but Humic is most common in the Semiaquic and Aquic Suborders.""" ;
  asc:subgroup asc:BI ;
  asc:subgroup asc:BU ;
  asc:subgroup asc:BY ;
  asc:subgroup asc:CK ;
  asc:subgroup asc:CN ;
  asc:subgroup asc:DG ;
  asc:subgroup asc:DJ ;
  asc:subgroup asc:DK ;
  asc:subgroup asc:DV ;
  asc:subgroup asc:DW ;
  asc:subgroup asc:DX ;
  asc:subgroup asc:EC ;
  asc:subgroup asc:EM ;
  asc:subgroup asc:GD ;
  asc:subgroup asc:HN ;
  asc:subgroup-comment """Each class listed below may not be relevant for every great group of each suborder.

If a diagnostic feature in the key begins more than 1.5 m from the soil surface it may not have a significant impact on the performance of the soil. Refer to diagnostic features in the glossary for guidance on the use of such features in the classification.

The term 'parapanic' is meant to imply 'pan-like'. Note also that the A1 horizons of many Podosols may have a distinct surface layer of lighter coloured sand with clean quartz grains and discrete lumps of organic matter and charcoal, giving the layer a speckled appearance. Below this layer, a dark A1 horizon may occur. Because the great majority of Australian Podosols have a bleached A2 horizon, this attribute is not used in the classification. Similarly, the great majority have a B horizon pHw of less than 5.5, hence acidic subgroups have not been used.""" ;
  skos:broader asc:PO ;
  skos:notation "PO-JE" ;
  skos:prefLabel "Aquic-Hypersulfidic Podosol" ;
.
asc:Q
  a asc:Clay-content ;
  skos:definition "<45% clay" ;
  skos:notation "Q" ;
  skos:prefLabel "Fine" ;
.
asc:R
  a asc:Clay-content ;
  skos:definition "45 - 60% clay" ;
  skos:notation "R" ;
  skos:prefLabel "Medium fine" ;
.
asc:RE
  a asc:Order ;
  a skos:Concept ;
  dcterms:description """The core concept of this Order is \"deep sandy soils\".

Arenosols accommodate soils with predominantly sandy field textures (≤10% clay content), and with no horizons containing more than 15% clay within the upper 1.0 m of the profile. The presence of argic horizons are the only exception. Arenosols generally have no observable peds apart from some structural development in the A1 horizon. The upper 1.0 m of the soil profile can only contain relatively small amounts of coarse fragments or coarse, hard segregations and does not contain any hard layers such as pans or rock. Arenosols occur extensively in inland arid areas, in and adjacent to waterways, near to the coast (especially in the west), but are also present in many other parts of Australia. This Order incorporates the most widespread and abundant soils in Australia.""" ;
  dcterms:identifier "http://anzsoil.org/def/au/asc/RE"^^xsd:anyURI ;
  rdfs:comment """As B horizons are difficult to identify consistently in some Arenosols, specific mention of a B2 horizon is omitted from some Suborders. Arenosols will obviously grade to Kandosols and some difficulty may be experienced in separating them. Here Kandosols must have a clearly distinguishable, well-developed B2 horizon with more than 15% clay whereas Arenosols have less than 15% clay.

Reclassification may also be required for other sandy soils where deep examination below 1.0 m reveals deep more clayey B horizons. See How to Classify for assistance with determining whether the layer is a B or D horizon. If the layer is a D horizon, the soil remains classified as an Arenosol.

Bleached or Grey Arenosols are distinguished from Podosols by the absence of Podosol diagnostic horizons. These horizons can occur below 1.0 m deep and commonly at considerable depth. If no deep examination has been done in similar soils in similar environments, then the soil should classify as a Bleached or Grey Arenosol with a confidence level of 4. If evidence at a later date reveals the presence of Podosols diagnostic horizons at depth, the soil will need to be reclassified.

Some Arenosols may include one or more thin argic horizons (also termed lamellae) which are usually 5-10 mm thick.

Arenosols will also grade to Tenosols. This third edition of the Australian Soil Classification reflects a major change to the Tenosol Order. Many sandy soils previously classified as the colour-linked Orthic Suborders of Tenosols will now classify as Arenosols.

As the Arenosols Order includes soils with negligible development many deep sandy soils previously described as Rudosols will now classify as Arenosols.

This third edition of the Australian Soil Classification also reflects a significant change to the Calcarosol Order. Many deep sandy soils with pedogenic carbonates previously classified as Shelly, Calcic or Hypocalcic Calcarosols will now classify as Carbonatic or Calsilic Arenosols.""" ;
  skos:definition """Soils that have, within the upper 1.0 m of the soil profile:

1. A sandy field texture (i.e. a field texture of sand, loamy sand or clayey sand) in one or more layers or horizons with a combined thickness of at least 0.8 m; and
2. No layer or horizon with a clay content that exceeds 15% (i.e. heavy sandy loam [SL+] or heavier) excluding argic horizon/s; and
3. ≤10% (by visual abundance and weighted average) of coarse fragments and/or hard segregations >2 mm in size; and
4. No hard layers (cemented pans, other cemented materials, rock, saprock or saprolite that do not soften when moist1)

1this qualification has been added since publication and is not reflected in CSIRO March 2021 published edition. The purpose is to not exclude from Arenosols soils with layers in the top 1.0 m that are hard when dry but soften when moist.""" ;
  skos:notation "RE" ;
  skos:prefLabel "Arenosols" ;
.
asc:RU
  a asc:Order ;
  a skos:Concept ;
  dcterms:description "This order is designed to accommodate soils that have little, if any, pedologic organisation. They are usually young soils in the sense that soil forming factors have had little time to pedologically modify parent rocks or sediments. The component soils can obviously vary widely in terms of texture and depth; many are stratified and some are highly saline. Data on some of them are very limited." ;
  dcterms:identifier "http://anzsoil.org/def/au/asc/RU"^^xsd:anyURI ;
  rdfs:comment """By definition, these soils will grade to Tenosols, so before deciding on the order check the Tenosol definition as it will often be a matter of judgement as to which order a particular soil is best placed. Arenic (sandy) Rudosols will grade to Arenosols, although by definition will have sand less than 1.0 m deep. Hydrosols are excluded on the basis that these will normally show some pedological development eg. mottling. A particular problem with the definition and subdivision of Rudosols is the difficulty in distinguishing between soil and 'non-soil', (see also 'What do we classify?'). In many instances they are classified on the basis of the nature of AC or C horizon materials or other substrates because these are the dominating features of the profile. It also follows that there may be difficulties in deciding if a soil is best classified as an Anthroposol or be regarded as an ‘anthropic’ Rudosol because the little-altered soil parent material may be human-made.

Rudosols in arid climatic zones form under a variety of processes (i.e. dust accretion, biological surface crusts, reduced leaching and more active wind and water erosion under sparse vegetation cover). The relative significance of these processes will differ from other climatic zones.""" ;
  skos:definition "Soil with little, if any, (rudimentary) pedologic organisation apart from (a) minimal development of an Al horizon or (b) the presence of less than 10% of B horizon material (including pedogenic carbonate) in fissures in the parent rock or saprolite. The soils are apedal or only weakly structured in the A1 horizon and show no pedological colour changes apart from the darkening of an A1 horizon. There is little or no texture or colour change with depth unless stratified or buried soils are present." ;
  skos:notation "RU" ;
  skos:prefLabel "Rudosols" ;
.
asc:S
  a asc:Clay-content ;
  skos:definition ">60% clay" ;
  skos:notation "S" ;
  skos:prefLabel "Very fine" ;
.
asc:SO
  a asc:Order ;
  a skos:Concept ;
  asc:colourclass asc:AA ;
  asc:colourclass asc:AB ;
  asc:colourclass asc:AC ;
  asc:colourclass asc:AD ;
  asc:colourclass asc:AE ;
  asc:colourclass-comment "The dominant colour class in the major part of the upper 0.2 m of the B2t horizon (or the major part of the entire B2t horizon if it is less than 0.2 m thick) is:" ;
  asc:family-criteria asc:A ;
  asc:family-criteria asc:B ;
  asc:family-criteria asc:C ;
  asc:family-criteria asc:D ;
  asc:family-criteria asc:E ;
  asc:family-criteria asc:F ;
  asc:family-criteria asc:G ;
  asc:family-criteria asc:H ;
  asc:family-criteria asc:I ;
  asc:family-criteria asc:K ;
  asc:family-criteria asc:L ;
  asc:family-criteria asc:M ;
  asc:family-criteria asc:N ;
  asc:family-criteria asc:NR ;
  asc:family-criteria asc:O ;
  asc:family-criteria asc:SR ;
  asc:family-criteria asc:T ;
  asc:family-criteria asc:U ;
  asc:family-criteria asc:V ;
  asc:family-criteria asc:W ;
  asc:family-criteria asc:WR ;
  asc:family-criteria asc:X ;
  asc:family-criteria asc:Y ;
  dcterms:description "Soils with strong texture contrast between A horizons and sodic B horizons which are not strongly acid. Australia is noteworthy for the extent and diversity of sodic soils (Isbell 1995)." ;
  dcterms:identifier "http://anzsoil.org/def/au/asc/SO"^^xsd:anyURI ;
  rdfs:comment """There is convincing evidence from the Riverine Plain of south eastern Australia that soils with sodic clay B horizons (ESP 25-30) which are strongly subplastic behave very differently in terms of permeability to the more commonly found plastic sodic clay B horizons which are characterised by low to very low saturated hydraulic conductivity (McIntyre 1979). It is on this basis that subplastic sodic soils are excluded from Sodosols, because of their very different land use properties.

Strongly acid sodic soils are also excluded from Sodosols because they usually contain appreciable exchangeable aluminium (KCl extractable) and thus should be unlikely to disperse.

It is usually possible to assess, in the field, the likelihood of a soil possessing a sodic B2t horizon. Such a criterion as the presence of a bleached A2 horizon with an abrupt change to a B2t horizon which has columnar or prismatic structure is a useful but not universal guide. A high pHw value (>8.5) suggests sodicity, but the converse is not true. The soapy nature of the bolus produced in field texturing will also often suggest appreciable sodium (and/or magnesium) on the clay exchange complex.

Increasing experience in many parts of Australia is confirming that the Emerson dispersion test (Emerson 1967) and the modified version of Loveday and Pyle (1973) is a reliable guide to sodicity. It can be carried out as a preliminary test in the field, but should always be repeated under the better controlled conditions of the laboratory. In the initial test at least several fragments (each about 0.2 g or about 4 -5 mm diameter) are immersed in 100 ml of distilled water. The large water:soil ratio is necessary to remove any salt present in the aggregate. Also for this reason Emerson (1991) suggests that the classification for each test be made after 24 hours. For the remoulded test, use a 5 mm cube which can be obtained from the bolus used for determining field texture. This will be approximately in the plastic limit condition. Note that distilled water should be used to prepare the bolus.

Data from Loveday and Pyle (1973) and unpublished data available to the original author Ray Isbell suggest that a dispersive soil will usually indicate sodicity, ie. ESP of 6 or greater. The data of Murphy (1995) indicate that whereas Emerson class 1 and the more strongly dispersive soils of class 2 are a reliable indicator of sodicity, whereas class 3 is a more variable predictor. Emerson classes of 5 or greater or a Loveday and Pyle score of zero strongly suggest soils are non-sodic. There is less evidence that the dispersion tests give a reliable indication of the degree of sodicity; factors such as extent of initial slaking and initial salt content in the aggregates, and the amount of magnesium and amount and form of aluminium on the exchange complex (Emerson 1994), can also influence the rapidity of dispersion. Nevertheless, the data of Loveday and Pyle measuring dispersion after 2 hours and 20 hours showed that the rate of dispersion could be used as a guide to ESP. This relationship does not apply to the subplastic soils of the Riverine Plain where subsoils with an ESP of 25-30 do not disperse unless remoulded (Blackmore 1976). Other anomalous results occur in a small minority of normal plastic soils in which dispersion will not occur even after remoulding in spite of an ESP much greater than 6 and a pHw as high as neutral. In at least some of these non-dispersive soils the typical sodic soil morphology is present, ie. a conspicuously bleached A2 horizon abruptly overlying a B2t horizon with prismatic or columnar structure, suggesting the low hydraulic conductivity expected of a sodic B horizon.""" ;
  skos:definition "Soils with a clear or abrupt textural B horizon and in which the major part of the upper 0.2 m of the B2t horizon (or the major part of the entire B2t horizon if it is less than 0.2 m thick) is sodic and not strongly acid. Hydrosols and soils with strongly subplastic upper B2t horizons are excluded." ;
  skos:narrower asc:SO-AA ;
  skos:narrower asc:SO-AB ;
  skos:narrower asc:SO-AC ;
  skos:narrower asc:SO-AD ;
  skos:narrower asc:SO-AE ;
  skos:notation "SO" ;
  skos:prefLabel "Sodosols" ;
.
asc:SO-AA
  a asc:Suborder ;
  asc:classifier asc:AA ;
  asc:greatgroup asc:BJ ;
  asc:greatgroup asc:BK ;
  asc:greatgroup asc:CR ;
  asc:greatgroup asc:DP ;
  asc:greatgroup asc:DZ ;
  asc:greatgroup asc:EA ;
  asc:greatgroup asc:ES ;
  asc:greatgroup asc:FN ;
  asc:greatgroup asc:FO ;
  asc:greatgroup asc:FP ;
  asc:greatgroup asc:IE ;
  asc:greatgroup-comment """Some Great Group soils are much more common in certain colour Suborders than others. The Duric and Pedaric Great Groups are known only from the arid zone, the former being particularly widespread in Western Australia and the latter in western Queensland and New South Wales, and in South Australia.

If a diagnostic feature in the key begins more than 1.5 m from the soil surface it may not have a significant impact on the performance of the soil. Refer to diagnostic features in the glossary for guidance on the use of such features in the classification.""" ;
  asc:subgroup asc:AF ;
  asc:subgroup asc:AG ;
  asc:subgroup asc:AH ;
  asc:subgroup asc:BD ;
  asc:subgroup asc:BU ;
  asc:subgroup asc:BZ ;
  asc:subgroup asc:CK ;
  asc:subgroup asc:CQ ;
  asc:subgroup asc:CV ;
  asc:subgroup asc:DA ;
  asc:subgroup asc:DB ;
  asc:subgroup asc:DC ;
  asc:subgroup asc:DK ;
  asc:subgroup asc:DN ;
  asc:subgroup asc:EM ;
  asc:subgroup asc:EX ;
  asc:subgroup asc:FB ;
  asc:subgroup-comment """Not every Subgroup defined below will be required or be appropriate for each Great Group of each Suborder. Some possible attributes have not been used for various reasons, e.g. bleaching has not been used because the great majority of soils in the class probably are bleached. Structure has not been used because of the diverse range that is encountered in these particular soils.

If a diagnostic feature in the key begins more than 1.5 m from the soil surface it may not have a significant impact on the performance of the soil. Refer to diagnostic features in the glossary for guidance on the use of such features in the classification.

The calcareous classes above approximately correspond to those of Wetherby and Oades (1975) as follows: Hypocalcic - Class IV, Lithocalcic - Class III B and III C, Supracalcic - Class III B, Hypercalcic - Class III A, Calcic - Class I and IIIA. In the Lithocalcic and Supracalcic classes the coarse fragments may be >0.2 m in size and soft carbonate may or may not be present.""" ;
  skos:broader asc:SO ;
  skos:notation "SO-AA" ;
  skos:prefLabel "Red Sodosol" ;
.
asc:SO-AB
  a asc:Suborder ;
  asc:classifier asc:AB ;
  asc:greatgroup asc:BJ ;
  asc:greatgroup asc:BK ;
  asc:greatgroup asc:CR ;
  asc:greatgroup asc:DP ;
  asc:greatgroup asc:DZ ;
  asc:greatgroup asc:EA ;
  asc:greatgroup asc:ES ;
  asc:greatgroup asc:FN ;
  asc:greatgroup asc:FO ;
  asc:greatgroup asc:FP ;
  asc:greatgroup asc:IE ;
  asc:greatgroup-comment """Some Great Group soils are much more common in certain colour Suborders than others. The Duric and Pedaric Great Groups are known only from the arid zone, the former being particularly widespread in Western Australia and the latter in western Queensland and New South Wales, and in South Australia.

If a diagnostic feature in the key begins more than 1.5 m from the soil surface it may not have a significant impact on the performance of the soil. Refer to diagnostic features in the glossary for guidance on the use of such features in the classification.""" ;
  asc:subgroup asc:AF ;
  asc:subgroup asc:AG ;
  asc:subgroup asc:AH ;
  asc:subgroup asc:BD ;
  asc:subgroup asc:BU ;
  asc:subgroup asc:BZ ;
  asc:subgroup asc:CK ;
  asc:subgroup asc:CQ ;
  asc:subgroup asc:CV ;
  asc:subgroup asc:DA ;
  asc:subgroup asc:DB ;
  asc:subgroup asc:DC ;
  asc:subgroup asc:DK ;
  asc:subgroup asc:DN ;
  asc:subgroup asc:EM ;
  asc:subgroup asc:EX ;
  asc:subgroup asc:FB ;
  asc:subgroup-comment """Not every Subgroup defined below will be required or be appropriate for each Great Group of each Suborder. Some possible attributes have not been used for various reasons, e.g. bleaching has not been used because the great majority of soils in the class probably are bleached. Structure has not been used because of the diverse range that is encountered in these particular soils.

If a diagnostic feature in the key begins more than 1.5 m from the soil surface it may not have a significant impact on the performance of the soil. Refer to diagnostic features in the glossary for guidance on the use of such features in the classification.

The calcareous classes above approximately correspond to those of Wetherby and Oades (1975) as follows: Hypocalcic - Class IV, Lithocalcic - Class III B and III C, Supracalcic - Class III B, Hypercalcic - Class III A, Calcic - Class I and IIIA. In the Lithocalcic and Supracalcic classes the coarse fragments may be >0.2 m in size and soft carbonate may or may not be present.""" ;
  skos:broader asc:SO ;
  skos:notation "SO-AB" ;
  skos:prefLabel "Brown Sodosol" ;
.
asc:SO-AC
  a asc:Suborder ;
  asc:classifier asc:AC ;
  asc:greatgroup asc:BJ ;
  asc:greatgroup asc:BK ;
  asc:greatgroup asc:CR ;
  asc:greatgroup asc:DP ;
  asc:greatgroup asc:DZ ;
  asc:greatgroup asc:EA ;
  asc:greatgroup asc:ES ;
  asc:greatgroup asc:FN ;
  asc:greatgroup asc:FO ;
  asc:greatgroup asc:FP ;
  asc:greatgroup asc:IE ;
  asc:greatgroup-comment """Some Great Group soils are much more common in certain colour Suborders than others. The Duric and Pedaric Great Groups are known only from the arid zone, the former being particularly widespread in Western Australia and the latter in western Queensland and New South Wales, and in South Australia.

If a diagnostic feature in the key begins more than 1.5 m from the soil surface it may not have a significant impact on the performance of the soil. Refer to diagnostic features in the glossary for guidance on the use of such features in the classification.""" ;
  asc:subgroup asc:AF ;
  asc:subgroup asc:AG ;
  asc:subgroup asc:AH ;
  asc:subgroup asc:BD ;
  asc:subgroup asc:BU ;
  asc:subgroup asc:BZ ;
  asc:subgroup asc:CK ;
  asc:subgroup asc:CQ ;
  asc:subgroup asc:CV ;
  asc:subgroup asc:DA ;
  asc:subgroup asc:DB ;
  asc:subgroup asc:DC ;
  asc:subgroup asc:DK ;
  asc:subgroup asc:DN ;
  asc:subgroup asc:EM ;
  asc:subgroup asc:EX ;
  asc:subgroup asc:FB ;
  asc:subgroup-comment """Not every Subgroup defined below will be required or be appropriate for each Great Group of each Suborder. Some possible attributes have not been used for various reasons, e.g. bleaching has not been used because the great majority of soils in the class probably are bleached. Structure has not been used because of the diverse range that is encountered in these particular soils.

If a diagnostic feature in the key begins more than 1.5 m from the soil surface it may not have a significant impact on the performance of the soil. Refer to diagnostic features in the glossary for guidance on the use of such features in the classification.

The calcareous classes above approximately correspond to those of Wetherby and Oades (1975) as follows: Hypocalcic - Class IV, Lithocalcic - Class III B and III C, Supracalcic - Class III B, Hypercalcic - Class III A, Calcic - Class I and IIIA. In the Lithocalcic and Supracalcic classes the coarse fragments may be >0.2 m in size and soft carbonate may or may not be present.""" ;
  skos:broader asc:SO ;
  skos:notation "SO-AC" ;
  skos:prefLabel "Yellow Sodosol" ;
.
asc:SO-AD
  a asc:Suborder ;
  asc:classifier asc:AD ;
  asc:greatgroup asc:BJ ;
  asc:greatgroup asc:BK ;
  asc:greatgroup asc:CR ;
  asc:greatgroup asc:DP ;
  asc:greatgroup asc:DZ ;
  asc:greatgroup asc:EA ;
  asc:greatgroup asc:ES ;
  asc:greatgroup asc:FN ;
  asc:greatgroup asc:FO ;
  asc:greatgroup asc:FP ;
  asc:greatgroup asc:IE ;
  asc:greatgroup-comment """Some Great Group soils are much more common in certain colour Suborders than others. The Duric and Pedaric Great Groups are known only from the arid zone, the former being particularly widespread in Western Australia and the latter in western Queensland and New South Wales, and in South Australia.

If a diagnostic feature in the key begins more than 1.5 m from the soil surface it may not have a significant impact on the performance of the soil. Refer to diagnostic features in the glossary for guidance on the use of such features in the classification.""" ;
  asc:subgroup asc:AF ;
  asc:subgroup asc:AG ;
  asc:subgroup asc:AH ;
  asc:subgroup asc:BD ;
  asc:subgroup asc:BU ;
  asc:subgroup asc:BZ ;
  asc:subgroup asc:CK ;
  asc:subgroup asc:CQ ;
  asc:subgroup asc:CV ;
  asc:subgroup asc:DA ;
  asc:subgroup asc:DB ;
  asc:subgroup asc:DC ;
  asc:subgroup asc:DK ;
  asc:subgroup asc:DN ;
  asc:subgroup asc:EM ;
  asc:subgroup asc:EX ;
  asc:subgroup asc:FB ;
  asc:subgroup-comment """Not every Subgroup defined below will be required or be appropriate for each Great Group of each Suborder. Some possible attributes have not been used for various reasons, e.g. bleaching has not been used because the great majority of soils in the class probably are bleached. Structure has not been used because of the diverse range that is encountered in these particular soils.

If a diagnostic feature in the key begins more than 1.5 m from the soil surface it may not have a significant impact on the performance of the soil. Refer to diagnostic features in the glossary for guidance on the use of such features in the classification.

The calcareous classes above approximately correspond to those of Wetherby and Oades (1975) as follows: Hypocalcic - Class IV, Lithocalcic - Class III B and III C, Supracalcic - Class III B, Hypercalcic - Class III A, Calcic - Class I and IIIA. In the Lithocalcic and Supracalcic classes the coarse fragments may be >0.2 m in size and soft carbonate may or may not be present.""" ;
  skos:broader asc:SO ;
  skos:notation "SO-AD" ;
  skos:prefLabel "Grey Sodosol" ;
.
asc:SO-AE
  a asc:Suborder ;
  asc:classifier asc:AE ;
  asc:greatgroup asc:BJ ;
  asc:greatgroup asc:BK ;
  asc:greatgroup asc:CR ;
  asc:greatgroup asc:DP ;
  asc:greatgroup asc:DZ ;
  asc:greatgroup asc:EA ;
  asc:greatgroup asc:ES ;
  asc:greatgroup asc:FN ;
  asc:greatgroup asc:FO ;
  asc:greatgroup asc:FP ;
  asc:greatgroup asc:IE ;
  asc:greatgroup-comment """Some Great Group soils are much more common in certain colour Suborders than others. The Duric and Pedaric Great Groups are known only from the arid zone, the former being particularly widespread in Western Australia and the latter in western Queensland and New South Wales, and in South Australia.

If a diagnostic feature in the key begins more than 1.5 m from the soil surface it may not have a significant impact on the performance of the soil. Refer to diagnostic features in the glossary for guidance on the use of such features in the classification.""" ;
  asc:subgroup asc:AF ;
  asc:subgroup asc:AG ;
  asc:subgroup asc:AH ;
  asc:subgroup asc:BD ;
  asc:subgroup asc:BU ;
  asc:subgroup asc:BZ ;
  asc:subgroup asc:CK ;
  asc:subgroup asc:CQ ;
  asc:subgroup asc:CV ;
  asc:subgroup asc:DA ;
  asc:subgroup asc:DB ;
  asc:subgroup asc:DC ;
  asc:subgroup asc:DK ;
  asc:subgroup asc:DN ;
  asc:subgroup asc:EM ;
  asc:subgroup asc:EX ;
  asc:subgroup asc:FB ;
  asc:subgroup-comment """Not every Subgroup defined below will be required or be appropriate for each Great Group of each Suborder. Some possible attributes have not been used for various reasons, e.g. bleaching has not been used because the great majority of soils in the class probably are bleached. Structure has not been used because of the diverse range that is encountered in these particular soils.

If a diagnostic feature in the key begins more than 1.5 m from the soil surface it may not have a significant impact on the performance of the soil. Refer to diagnostic features in the glossary for guidance on the use of such features in the classification.

The calcareous classes above approximately correspond to those of Wetherby and Oades (1975) as follows: Hypocalcic - Class IV, Lithocalcic - Class III B and III C, Supracalcic - Class III B, Hypercalcic - Class III A, Calcic - Class I and IIIA. In the Lithocalcic and Supracalcic classes the coarse fragments may be >0.2 m in size and soft carbonate may or may not be present.""" ;
  skos:broader asc:SO ;
  skos:notation "SO-AE" ;
  skos:prefLabel "Black Sodosol" ;
.
asc:SR
  a asc:Water-repellence ;
  skos:definition "2 Molar ethanol takes more than 10 seconds to be absorbed into soil" ;
  skos:notation "SR" ;
  skos:prefLabel "Strongly water repellent" ;
.
asc:Suborder
  a owl:Class ;
  rdfs:label "Soil suborder" ;
  rdfs:subClassOf skos:Concept ;
  rdfs:subClassOf [
      a owl:Restriction ;
      owl:allValuesFrom asc:Order ;
      owl:onProperty skos:broader ;
    ] ;
  rdfs:subClassOf [
      a owl:Restriction ;
      owl:cardinality "1"^^xsd:nonNegativeInteger ;
      owl:onProperty asc:classifier ;
    ] ;
.
asc:T
  a asc:Class ;
  a asc:Depth ;
  skos:definition "<0.25 m" ;
  skos:notation "T" ;
  skos:prefLabel "Very shallow" ;
.
asc:TE
  a asc:Order ;
  a skos:Concept ;
  asc:colourclass asc:AA ;
  asc:colourclass asc:AB ;
  asc:colourclass asc:AC ;
  asc:colourclass asc:AD ;
  asc:colourclass asc:AE ;
  asc:colourclass-comment "The dominant colour class in the major part of the upper 0.5 m of the profile (or the entire profile if it is less than 0.5 m thick) is:" ;
  asc:greatgroup-comment "If a diagnostic feature in the key begins more than 1.5 m from the soil surface it may not have a significant impact on the performance of the soil. Refer to diagnostic features in the glossary for guidance on the use of such features in the classification." ;
  asc:subgroup-comment """These have been grouped into the various suborders, but not all subgroups will be appropriate for each great group of a particular suborder.

If a diagnostic feature in the key begins more than 1.5 m from the soil surface it may not have a significant impact on the performance of the soil. Refer to diagnostic features in the glossary for guidance on the use of such features in the classification.""" ;
  asc:suborder asc:AT ;
  asc:suborder asc:AW ;
  asc:suborder asc:BE ;
  asc:suborder asc:BF ;
  asc:suborder asc:CY ;
  asc:suborder asc:IL ;
  asc:suborder asc:IM ;
  dcterms:description "This order is designed to embrace soils with generally only weak pedologic organisation apart from the A horizons, excluding soils that have deep sandy profiles with a field texture of sand, loamy sand or clayey sand in 80% or more of the upper 1.0 m. It encompasses a rather diverse range of soils which occur in many parts of Australia." ;
  dcterms:identifier "http://anzsoil.org/def/au/asc/TE"^^xsd:anyURI ;
  rdfs:comment """It may be desirable to specify a minimum thickness for those A1 horizons which do not meet the requirements for a peaty, humose, melacic or melanic horizon. The inclusion of certain soils with conspicuously bleached A2 horizons may be questioned by some, but it is difficult to find a more appropriate place for them.

The Tenosols will differ from Rudosols by virtue of having either a more than weakly developed A1 horizon, an A2, or a weakly developed B horizon. As B horizons are difficult to identify consistently in some Tenosols, specific mention of a B horizon is omitted from some Suborders. They will obviously grade to Kandosols, and some difficulty may be experienced in separating medium-textured Tenosols from Kandosols. Here again, B horizon development is the key; Kandosols must have a clearly distinguishable, well-developed B2 horizon with more than 15% clay. Tenosols will grade to Podosols, but the latter must have a Podosol diagnostic B horizon. Tenosols also grade to Arenosols but lack the deep sandy horizons characteristic of this order. In cold, wet environments, some Tenosols with peaty A horizons will grade to Organosols.

This third edition of the Australian Soil Classification removes the Orthic term from the bleached and colour suborders.""" ;
  skos:definition """Soils that do not fit the requirements of any other soil orders and generally with one or more of the following:

1. A peaty horizon.
2. A humose, melacic or melanic horizon, or conspicuously bleached A2 horizon, which overlies a calcrete pan, hard unweathered rock or other hard materials; or partially weathered or decomposed rock or saprolite, or unconsolidated mineral materials.
3. A horizons which meet all the conditions for a peaty, humose, melacic or melanic horizon except the depth requirement, and directly overlie a calcrete pan, hard unweathered rock or other hard materials; or partially weathered or decomposed rock or saprolite, or unconsolidated mineral materials.
4. A1 horizons which have more than a weak development of structure and directly overlie a calcrete pan, hard unweathered rock or other hard materials; or partially weathered or decomposed rock or saprolite, or unconsolidated mineral materials.
5. An A2 horizon which overlies a calcrete pan, hard unweathered rock or other hard materials; or partially weathered or decomposed rock or saprolite, or unconsolidated mineral materials.
6. B2 horizon with 15% clay (SL) or less1 , or a transitional horizon (C/B) occurring in fissures in the parent rock or saprolite which contains between 10 and 50% of B horizon material (including pedogenic carbonate).
7. A ferric or bauxitic horizon >0.2 m thick.
8. A calcareous horizon >0.2 m thick.""" ;
  skos:narrower asc:TE-AT ;
  skos:narrower asc:TE-AW ;
  skos:narrower asc:TE-BE ;
  skos:narrower asc:TE-BF ;
  skos:narrower asc:TE-CY ;
  skos:narrower asc:TE-IL ;
  skos:narrower asc:TE-IM ;
  skos:notation "TE" ;
  skos:prefLabel "Tenosols" ;
.
asc:TE-AT
  a asc:Suborder ;
  a skos:Concept ;
  asc:classifier asc:AT ;
  asc:greatgroup asc:AK ;
  asc:greatgroup asc:AO ;
  asc:greatgroup asc:AP ;
  asc:greatgroup asc:AS ;
  asc:greatgroup asc:BJ ;
  asc:greatgroup asc:BU ;
  asc:greatgroup asc:CZ ;
  asc:greatgroup asc:DD ;
  asc:greatgroup asc:DU ;
  asc:greatgroup asc:DZ ;
  asc:greatgroup asc:EA ;
  asc:greatgroup asc:EF ;
  asc:greatgroup asc:EM ;
  asc:greatgroup asc:FK ;
  asc:greatgroup asc:GE ;
  asc:greatgroup asc:GF ;
  asc:greatgroup asc:HF ;
  asc:greatgroup asc:IA ;
  asc:greatgroup asc:IS ;
  asc:greatgroup asc:JQ ;
  asc:greatgroup asc:JW ;
  asc:greatgroup asc:JX ;
  asc:subgroup asc:AI ;
  asc:subgroup asc:AR ;
  asc:subgroup asc:BC ;
  asc:subgroup asc:CK ;
  asc:subgroup asc:DC ;
  asc:subgroup asc:DG ;
  asc:subgroup asc:DK ;
  asc:subgroup asc:DW ;
  asc:subgroup asc:FC ;
  asc:subgroup asc:FU ;
  asc:subgroup asc:FV ;
  asc:subgroup asc:GU ;
  asc:subgroup asc:GY ;
  dcterms:identifier "http://anzsoil.org/def/au/asc/TE-AT"^^xsd:anyURI ;
  skos:broader asc:TE ;
  skos:narrower asc:TE-AT-AK ;
  skos:narrower asc:TE-AT-AO ;
  skos:narrower asc:TE-AT-AP ;
  skos:narrower asc:TE-AT-AS ;
  skos:narrower asc:TE-AT-BJ ;
  skos:narrower asc:TE-AT-BU ;
  skos:narrower asc:TE-AT-CZ ;
  skos:narrower asc:TE-AT-DD ;
  skos:narrower asc:TE-AT-DU ;
  skos:narrower asc:TE-AT-DZ ;
  skos:narrower asc:TE-AT-EA ;
  skos:narrower asc:TE-AT-EF ;
  skos:narrower asc:TE-AT-EM ;
  skos:narrower asc:TE-AT-FK ;
  skos:narrower asc:TE-AT-GE ;
  skos:narrower asc:TE-AT-GF ;
  skos:narrower asc:TE-AT-HF ;
  skos:narrower asc:TE-AT-IA ;
  skos:narrower asc:TE-AT-IS ;
  skos:narrower asc:TE-AT-JQ ;
  skos:narrower asc:TE-AT-JW ;
  skos:narrower asc:TE-AT-JX ;
  skos:notation "TE-AT" ;
  skos:prefLabel "Bleached Tenosol" ;
.
asc:TE-AT-AK
  a asc:Greatgroup ;
  a skos:Concept ;
  asc:classifier asc:AK ;
  dcterms:identifier "http://anzsoil.org/def/au/asc/TE-AT-AK"^^xsd:anyURI ;
  skos:broader asc:TE-AT ;
  skos:prefLabel "Andic Bleached Tenosol" ;
.
asc:TE-AT-AO
  a asc:Greatgroup ;
  a skos:Concept ;
  asc:classifier asc:AO ;
  dcterms:identifier "http://anzsoil.org/def/au/asc/TE-AT-AO"^^xsd:anyURI ;
  skos:broader asc:TE-AT ;
  skos:prefLabel "Arenic Bleached Tenosol" ;
.
asc:TE-AT-AP
  a asc:Greatgroup ;
  a skos:Concept ;
  asc:classifier asc:AP ;
  dcterms:identifier "http://anzsoil.org/def/au/asc/TE-AT-AP"^^xsd:anyURI ;
  skos:broader asc:TE-AT ;
  skos:prefLabel "Argic Bleached Tenosol" ;
.
asc:TE-AT-AS
  a asc:Greatgroup ;
  a skos:Concept ;
  asc:classifier asc:AS ;
  dcterms:identifier "http://anzsoil.org/def/au/asc/TE-AT-AS"^^xsd:anyURI ;
  skos:broader asc:TE-AT ;
  skos:prefLabel "Bauxitic Bleached Tenosol" ;
.
asc:TE-AT-BJ
  a asc:Greatgroup ;
  a skos:Concept ;
  asc:classifier asc:BJ ;
  dcterms:identifier "http://anzsoil.org/def/au/asc/TE-AT-BJ"^^xsd:anyURI ;
  skos:broader asc:TE-AT ;
  skos:prefLabel "Duric Bleached Tenosol" ;
.
asc:TE-AT-BU
  a asc:Greatgroup ;
  a skos:Concept ;
  asc:classifier asc:BU ;
  dcterms:identifier "http://anzsoil.org/def/au/asc/TE-AT-BU"^^xsd:anyURI ;
  skos:broader asc:TE-AT ;
  skos:prefLabel "Ferric Bleached Tenosol" ;
.
asc:TE-AT-CZ
  a asc:Greatgroup ;
  a skos:Concept ;
  asc:classifier asc:CZ ;
  dcterms:identifier "http://anzsoil.org/def/au/asc/TE-AT-CZ"^^xsd:anyURI ;
  skos:broader asc:TE-AT ;
  skos:prefLabel "Lithic Bleached Tenosol" ;
.
asc:TE-AT-DD
  a asc:Greatgroup ;
  a skos:Concept ;
  asc:classifier asc:DD ;
  dcterms:identifier "http://anzsoil.org/def/au/asc/TE-AT-DD"^^xsd:anyURI ;
  skos:broader asc:TE-AT ;
  skos:prefLabel "Marly Bleached Tenosol" ;
.
asc:TE-AT-DU
  a asc:Greatgroup ;
  a skos:Concept ;
  asc:classifier asc:DU ;
  dcterms:identifier "http://anzsoil.org/def/au/asc/TE-AT-DU"^^xsd:anyURI ;
  skos:broader asc:TE-AT ;
  skos:prefLabel "Paralithic Bleached Tenosol" ;
.
asc:TE-AT-DZ
  a asc:Greatgroup ;
  a skos:Concept ;
  asc:classifier asc:DZ ;
  dcterms:identifier "http://anzsoil.org/def/au/asc/TE-AT-DZ"^^xsd:anyURI ;
  skos:broader asc:TE-AT ;
  skos:prefLabel "Petrocalcic Bleached Tenosol" ;
.
asc:TE-AT-EA
  a asc:Greatgroup ;
  a skos:Concept ;
  asc:classifier asc:EA ;
  dcterms:identifier "http://anzsoil.org/def/au/asc/TE-AT-EA"^^xsd:anyURI ;
  skos:broader asc:TE-AT ;
  skos:prefLabel "Petroferric Bleached Tenosol" ;
.
asc:TE-AT-EF
  a asc:Greatgroup ;
  a skos:Concept ;
  asc:classifier asc:EF ;
  dcterms:identifier "http://anzsoil.org/def/au/asc/TE-AT-EF"^^xsd:anyURI ;
  skos:broader asc:TE-AT ;
  skos:prefLabel "Reticulate Bleached Tenosol" ;
.
asc:TE-AT-EM
  a asc:Greatgroup ;
  a skos:Concept ;
  asc:classifier asc:EM ;
  dcterms:identifier "http://anzsoil.org/def/au/asc/TE-AT-EM"^^xsd:anyURI ;
  skos:broader asc:TE-AT ;
  skos:prefLabel "Silpanic Bleached Tenosol" ;
.
asc:TE-AT-FK
  a asc:Greatgroup ;
  a skos:Concept ;
  asc:classifier asc:FK ;
  dcterms:identifier "http://anzsoil.org/def/au/asc/TE-AT-FK"^^xsd:anyURI ;
  skos:broader asc:TE-AT ;
  skos:prefLabel "Ferric-Duric Bleached Tenosol" ;
.
asc:TE-AT-GE
  a asc:Greatgroup ;
  a skos:Concept ;
  asc:classifier asc:GE ;
  dcterms:identifier "http://anzsoil.org/def/au/asc/TE-AT-GE"^^xsd:anyURI ;
  skos:broader asc:TE-AT ;
  skos:prefLabel "Ferric-Petroferric Bleached Tenosol" ;
.
asc:TE-AT-GF
  a asc:Greatgroup ;
  a skos:Concept ;
  asc:classifier asc:GF ;
  dcterms:identifier "http://anzsoil.org/def/au/asc/TE-AT-GF"^^xsd:anyURI ;
  skos:broader asc:TE-AT ;
  skos:prefLabel "Regolithic Bleached Tenosol" ;
.
asc:TE-AT-HF
  a asc:Greatgroup ;
  a skos:Concept ;
  asc:classifier asc:HF ;
  dcterms:identifier "http://anzsoil.org/def/au/asc/TE-AT-HF"^^xsd:anyURI ;
  skos:broader asc:TE-AT ;
  skos:prefLabel "Tephric Bleached Tenosol" ;
.
asc:TE-AT-IA
  a asc:Greatgroup ;
  a skos:Concept ;
  asc:classifier asc:IA ;
  dcterms:identifier "http://anzsoil.org/def/au/asc/TE-AT-IA"^^xsd:anyURI ;
  skos:broader asc:TE-AT ;
  skos:prefLabel "Inceptic Bleached Tenosol" ;
.
asc:TE-AT-IS
  a asc:Greatgroup ;
  a skos:Concept ;
  asc:classifier asc:IS ;
  dcterms:identifier "http://anzsoil.org/def/au/asc/TE-AT-IS"^^xsd:anyURI ;
  skos:broader asc:TE-AT ;
  skos:prefLabel "Ferric-Reticulate Bleached Tenosol" ;
.
asc:TE-AT-JQ
  a asc:Greatgroup ;
  a skos:Concept ;
  asc:classifier asc:JQ ;
  dcterms:identifier "http://anzsoil.org/def/au/asc/TE-AT-JQ"^^xsd:anyURI ;
  skos:broader asc:TE-AT ;
  skos:prefLabel "Gritty Bleached Tenosol" ;
.
asc:TE-AT-JW
  a asc:Greatgroup ;
  a skos:Concept ;
  asc:classifier asc:JW ;
  dcterms:identifier "http://anzsoil.org/def/au/asc/TE-AT-JW"^^xsd:anyURI ;
  skos:broader asc:TE-AT ;
  skos:prefLabel "Gritty-Lithic Bleached Tenosol" ;
.
asc:TE-AT-JX
  a asc:Greatgroup ;
  a skos:Concept ;
  asc:classifier asc:JX ;
  dcterms:identifier "http://anzsoil.org/def/au/asc/TE-AT-JX"^^xsd:anyURI ;
  skos:broader asc:TE-AT ;
  skos:prefLabel "Gritty-Paralithic Bleached Tenosol" ;
.
asc:TE-AW
  a asc:Suborder ;
  a skos:Concept ;
  asc:classifier asc:AW ;
  asc:greatgroup asc:BU ;
  asc:greatgroup asc:CZ ;
  asc:greatgroup asc:DU ;
  asc:greatgroup asc:DZ ;
  asc:greatgroup asc:EA ;
  asc:greatgroup asc:EM ;
  asc:greatgroup asc:GE ;
  asc:greatgroup asc:JV ;
  asc:greatgroup asc:JW ;
  asc:greatgroup asc:JX ;
  asc:subgroup asc:AI ;
  asc:subgroup asc:AR ;
  asc:subgroup asc:BC ;
  asc:subgroup asc:CK ;
  asc:subgroup asc:DG ;
  asc:subgroup asc:DK ;
  asc:subgroup asc:DW ;
  asc:subgroup asc:FC ;
  asc:subgroup asc:FU ;
  asc:subgroup asc:FV ;
  asc:subgroup asc:GU ;
  asc:subgroup asc:GY ;
  dcterms:identifier "http://anzsoil.org/def/au/asc/TE-AW"^^xsd:anyURI ;
  skos:broader asc:TE ;
  skos:narrower asc:TE-AW-BU ;
  skos:narrower asc:TE-AW-CZ ;
  skos:narrower asc:TE-AW-DU ;
  skos:narrower asc:TE-AW-DZ ;
  skos:narrower asc:TE-AW-EA ;
  skos:narrower asc:TE-AW-EM ;
  skos:narrower asc:TE-AW-GE ;
  skos:narrower asc:TE-AW-JV ;
  skos:narrower asc:TE-AW-JW ;
  skos:narrower asc:TE-AW-JX ;
  skos:notation "TE-AW" ;
  skos:prefLabel "Bleached-Leptic Tenosol" ;
.
asc:TE-AW-BU
  a asc:Greatgroup ;
  a skos:Concept ;
  asc:classifier asc:BU ;
  dcterms:identifier "http://anzsoil.org/def/au/asc/TE-AW-BU"^^xsd:anyURI ;
  skos:broader asc:TE-AW ;
  skos:prefLabel "Ferric Bleached-Leptic Tenosol" ;
.
asc:TE-AW-CZ
  a asc:Greatgroup ;
  a skos:Concept ;
  asc:classifier asc:CZ ;
  dcterms:identifier "http://anzsoil.org/def/au/asc/TE-AW-CZ"^^xsd:anyURI ;
  skos:broader asc:TE-AW ;
  skos:prefLabel "Lithic Bleached-Leptic Tenosol" ;
.
asc:TE-AW-DU
  a asc:Greatgroup ;
  a skos:Concept ;
  asc:classifier asc:DU ;
  dcterms:identifier "http://anzsoil.org/def/au/asc/TE-AW-DU"^^xsd:anyURI ;
  skos:broader asc:TE-AW ;
  skos:prefLabel "Paralithic Bleached-Leptic Tenosol" ;
.
asc:TE-AW-DZ
  a asc:Greatgroup ;
  a skos:Concept ;
  asc:classifier asc:DZ ;
  dcterms:identifier "http://anzsoil.org/def/au/asc/TE-AW-DZ"^^xsd:anyURI ;
  skos:broader asc:TE-AW ;
  skos:prefLabel "Petrocalcic Bleached-Leptic Tenosol" ;
.
asc:TE-AW-EA
  a asc:Greatgroup ;
  a skos:Concept ;
  asc:classifier asc:EA ;
  dcterms:identifier "http://anzsoil.org/def/au/asc/TE-AW-EA"^^xsd:anyURI ;
  skos:broader asc:TE-AW ;
  skos:prefLabel "Petroferric Bleached-Leptic Tenosol" ;
.
asc:TE-AW-EM
  a asc:Greatgroup ;
  a skos:Concept ;
  asc:classifier asc:EM ;
  dcterms:identifier "http://anzsoil.org/def/au/asc/TE-AW-EM"^^xsd:anyURI ;
  skos:broader asc:TE-AW ;
  skos:prefLabel "Silpanic Bleached-Leptic Tenosol" ;
.
asc:TE-AW-GE
  a asc:Greatgroup ;
  a skos:Concept ;
  asc:classifier asc:GE ;
  dcterms:identifier "http://anzsoil.org/def/au/asc/TE-AW-GE"^^xsd:anyURI ;
  skos:broader asc:TE-AW ;
  skos:prefLabel "Ferric-Petroferric Bleached-Leptic Tenosol" ;
.
asc:TE-AW-JV
  a asc:Greatgroup ;
  a skos:Concept ;
  asc:classifier asc:JV ;
  dcterms:identifier "http://anzsoil.org/def/au/asc/TE-AW-JV"^^xsd:anyURI ;
  skos:broader asc:TE-AW ;
  skos:prefLabel "Gritty-Silpanic Bleached-Leptic Tenosol" ;
.
asc:TE-AW-JW
  a asc:Greatgroup ;
  a skos:Concept ;
  asc:classifier asc:JW ;
  dcterms:identifier "http://anzsoil.org/def/au/asc/TE-AW-JW"^^xsd:anyURI ;
  skos:broader asc:TE-AW ;
  skos:prefLabel "Gritty-Lithic Bleached-Leptic Tenosol" ;
.
asc:TE-AW-JX
  a asc:Greatgroup ;
  a skos:Concept ;
  asc:classifier asc:JX ;
  dcterms:identifier "http://anzsoil.org/def/au/asc/TE-AW-JX"^^xsd:anyURI ;
  skos:broader asc:TE-AW ;
  skos:prefLabel "Gritty-Paralithic Bleached-Leptic Tenosol" ;
.
asc:TE-BE
  a asc:Suborder ;
  a skos:Concept ;
  asc:classifier asc:BE ;
  asc:greatgroup asc:AK ;
  asc:greatgroup asc:AS ;
  asc:greatgroup asc:BU ;
  asc:greatgroup asc:CZ ;
  asc:greatgroup asc:DD ;
  asc:greatgroup asc:DU ;
  asc:greatgroup asc:DZ ;
  asc:greatgroup asc:EA ;
  asc:greatgroup asc:EC ;
  asc:greatgroup asc:EM ;
  asc:greatgroup asc:GF ;
  asc:greatgroup asc:HF ;
  asc:greatgroup asc:IA ;
  asc:subgroup asc:CK ;
  asc:subgroup asc:DG ;
  asc:subgroup asc:DK ;
  asc:subgroup asc:DW ;
  asc:subgroup asc:FC ;
  asc:subgroup asc:FU ;
  asc:subgroup asc:FV ;
  asc:subgroup asc:GU ;
  asc:subgroup asc:GY ;
  dcterms:identifier "http://anzsoil.org/def/au/asc/TE-BE"^^xsd:anyURI ;
  skos:broader asc:TE ;
  skos:narrower asc:TE-BE-AK ;
  skos:narrower asc:TE-BE-AS ;
  skos:narrower asc:TE-BE-BU ;
  skos:narrower asc:TE-BE-CZ ;
  skos:narrower asc:TE-BE-DD ;
  skos:narrower asc:TE-BE-DU ;
  skos:narrower asc:TE-BE-DZ ;
  skos:narrower asc:TE-BE-EA ;
  skos:narrower asc:TE-BE-EC ;
  skos:narrower asc:TE-BE-EM ;
  skos:narrower asc:TE-BE-GF ;
  skos:narrower asc:TE-BE-HF ;
  skos:narrower asc:TE-BE-IA ;
  skos:notation "TE-BE" ;
  skos:prefLabel "Chernic Tenosol" ;
.
asc:TE-BE-AK
  a asc:Greatgroup ;
  a skos:Concept ;
  asc:classifier asc:AK ;
  dcterms:identifier "http://anzsoil.org/def/au/asc/TE-BE-AK"^^xsd:anyURI ;
  skos:broader asc:TE-BE ;
  skos:prefLabel "Andic Chernic Tenosol" ;
.
asc:TE-BE-AS
  a asc:Greatgroup ;
  a skos:Concept ;
  asc:classifier asc:AS ;
  dcterms:identifier "http://anzsoil.org/def/au/asc/TE-BE-AS"^^xsd:anyURI ;
  skos:broader asc:TE-BE ;
  skos:prefLabel "Bauxitic Chernic Tenosol" ;
.
asc:TE-BE-BU
  a asc:Greatgroup ;
  a skos:Concept ;
  asc:classifier asc:BU ;
  dcterms:identifier "http://anzsoil.org/def/au/asc/TE-BE-BU"^^xsd:anyURI ;
  skos:broader asc:TE-BE ;
  skos:prefLabel "Ferric Chernic Tenosol" ;
.
asc:TE-BE-CZ
  a asc:Greatgroup ;
  a skos:Concept ;
  asc:classifier asc:CZ ;
  dcterms:identifier "http://anzsoil.org/def/au/asc/TE-BE-CZ"^^xsd:anyURI ;
  skos:broader asc:TE-BE ;
  skos:prefLabel "Lithic Chernic Tenosol" ;
.
asc:TE-BE-DD
  a asc:Greatgroup ;
  a skos:Concept ;
  asc:classifier asc:DD ;
  dcterms:identifier "http://anzsoil.org/def/au/asc/TE-BE-DD"^^xsd:anyURI ;
  skos:broader asc:TE-BE ;
  skos:prefLabel "Marly Chernic Tenosol" ;
.
asc:TE-BE-DU
  a asc:Greatgroup ;
  a skos:Concept ;
  asc:classifier asc:DU ;
  dcterms:identifier "http://anzsoil.org/def/au/asc/TE-BE-DU"^^xsd:anyURI ;
  skos:broader asc:TE-BE ;
  skos:prefLabel "Paralithic Chernic Tenosol" ;
.
asc:TE-BE-DZ
  a asc:Greatgroup ;
  a skos:Concept ;
  asc:classifier asc:DZ ;
  dcterms:identifier "http://anzsoil.org/def/au/asc/TE-BE-DZ"^^xsd:anyURI ;
  skos:broader asc:TE-BE ;
  skos:prefLabel "Petrocalcic Chernic Tenosol" ;
.
asc:TE-BE-EA
  a asc:Greatgroup ;
  a skos:Concept ;
  asc:classifier asc:EA ;
  dcterms:identifier "http://anzsoil.org/def/au/asc/TE-BE-EA"^^xsd:anyURI ;
  skos:broader asc:TE-BE ;
  skos:prefLabel "Petroferric Chernic Tenosol" ;
.
asc:TE-BE-EC
  a asc:Greatgroup ;
  a skos:Concept ;
  asc:classifier asc:EC ;
  dcterms:identifier "http://anzsoil.org/def/au/asc/TE-BE-EC"^^xsd:anyURI ;
  skos:broader asc:TE-BE ;
  skos:prefLabel "Placic Chernic Tenosol" ;
.
asc:TE-BE-EM
  a asc:Greatgroup ;
  a skos:Concept ;
  asc:classifier asc:EM ;
  dcterms:identifier "http://anzsoil.org/def/au/asc/TE-BE-EM"^^xsd:anyURI ;
  skos:broader asc:TE-BE ;
  skos:prefLabel "Silpanic Chernic Tenosol" ;
.
asc:TE-BE-GF
  a asc:Greatgroup ;
  a skos:Concept ;
  asc:classifier asc:GF ;
  dcterms:identifier "http://anzsoil.org/def/au/asc/TE-BE-GF"^^xsd:anyURI ;
  skos:broader asc:TE-BE ;
  skos:prefLabel "Regolithic Chernic Tenosol" ;
.
asc:TE-BE-HF
  a asc:Greatgroup ;
  a skos:Concept ;
  asc:classifier asc:HF ;
  dcterms:identifier "http://anzsoil.org/def/au/asc/TE-BE-HF"^^xsd:anyURI ;
  skos:broader asc:TE-BE ;
  skos:prefLabel "Tephric Chernic Tenosol" ;
.
asc:TE-BE-IA
  a asc:Greatgroup ;
  a skos:Concept ;
  asc:classifier asc:IA ;
  dcterms:identifier "http://anzsoil.org/def/au/asc/TE-BE-IA"^^xsd:anyURI ;
  skos:broader asc:TE-BE ;
  skos:prefLabel "Inceptic Chernic Tenosol" ;
.
asc:TE-BF
  a asc:Suborder ;
  a skos:Concept ;
  asc:classifier asc:BF ;
  asc:greatgroup asc:BJ ;
  asc:greatgroup asc:CZ ;
  asc:greatgroup asc:DU ;
  asc:greatgroup asc:DZ ;
  asc:greatgroup asc:EA ;
  asc:greatgroup asc:EM ;
  asc:greatgroup asc:GE ;
  asc:subgroup asc:CK ;
  asc:subgroup asc:DG ;
  asc:subgroup asc:DK ;
  asc:subgroup asc:DW ;
  dcterms:identifier "http://anzsoil.org/def/au/asc/TE-BF"^^xsd:anyURI ;
  skos:broader asc:TE ;
  skos:narrower asc:TE-BF-BJ ;
  skos:narrower asc:TE-BF-CZ ;
  skos:narrower asc:TE-BF-DU ;
  skos:narrower asc:TE-BF-DZ ;
  skos:narrower asc:TE-BF-EA ;
  skos:narrower asc:TE-BF-EM ;
  skos:narrower asc:TE-BF-GE ;
  skos:notation "TE-BF" ;
  skos:prefLabel "Chernic-Leptic Tenosol" ;
.
asc:TE-BF-BJ
  a asc:Greatgroup ;
  a skos:Concept ;
  asc:classifier asc:BJ ;
  dcterms:identifier "http://anzsoil.org/def/au/asc/TE-BF-BJ"^^xsd:anyURI ;
  skos:broader asc:TE-BF ;
  skos:prefLabel "Duric Chernic-Leptic Tenosol" ;
.
asc:TE-BF-CZ
  a asc:Greatgroup ;
  a skos:Concept ;
  asc:classifier asc:CZ ;
  dcterms:identifier "http://anzsoil.org/def/au/asc/TE-BF-CZ"^^xsd:anyURI ;
  skos:broader asc:TE-BF ;
  skos:prefLabel "Lithic Chernic-Leptic Tenosol" ;
.
asc:TE-BF-DU
  a asc:Greatgroup ;
  a skos:Concept ;
  asc:classifier asc:DU ;
  dcterms:identifier "http://anzsoil.org/def/au/asc/TE-BF-DU"^^xsd:anyURI ;
  skos:broader asc:TE-BF ;
  skos:prefLabel "Paralithic Chernic-Leptic Tenosol" ;
.
asc:TE-BF-DZ
  a asc:Greatgroup ;
  a skos:Concept ;
  asc:classifier asc:DZ ;
  dcterms:identifier "http://anzsoil.org/def/au/asc/TE-BF-DZ"^^xsd:anyURI ;
  skos:broader asc:TE-BF ;
  skos:prefLabel "Petrocalcic Chernic-Leptic Tenosol" ;
.
asc:TE-BF-EA
  a asc:Greatgroup ;
  a skos:Concept ;
  asc:classifier asc:EA ;
  dcterms:identifier "http://anzsoil.org/def/au/asc/TE-BF-EA"^^xsd:anyURI ;
  skos:broader asc:TE-BF ;
  skos:prefLabel "Petroferric Chernic-Leptic Tenosol" ;
.
asc:TE-BF-EM
  a asc:Greatgroup ;
  a skos:Concept ;
  asc:classifier asc:EM ;
  dcterms:identifier "http://anzsoil.org/def/au/asc/TE-BF-EM"^^xsd:anyURI ;
  skos:broader asc:TE-BF ;
  skos:prefLabel "Silpanic Chernic-Leptic Tenosol" ;
.
asc:TE-BF-GE
  a asc:Greatgroup ;
  a skos:Concept ;
  asc:classifier asc:GE ;
  dcterms:identifier "http://anzsoil.org/def/au/asc/TE-BF-GE"^^xsd:anyURI ;
  skos:broader asc:TE-BF ;
  skos:prefLabel "Ferric-Petroferric Chernic-Leptic Tenosol" ;
.
asc:TE-CY
  a asc:Suborder ;
  a skos:Concept ;
  asc:classifier asc:CY ;
  asc:greatgroup asc:BJ ;
  asc:greatgroup asc:CZ ;
  asc:greatgroup asc:DU ;
  asc:greatgroup asc:DZ ;
  asc:greatgroup asc:EA ;
  asc:greatgroup asc:EM ;
  asc:greatgroup asc:GE ;
  asc:subgroup asc:AI ;
  asc:subgroup asc:AR ;
  asc:subgroup asc:BC ;
  asc:subgroup asc:DR ;
  asc:subgroup asc:FF ;
  asc:subgroup asc:FG ;
  asc:subgroup asc:ID ;
  dcterms:identifier "http://anzsoil.org/def/au/asc/TE-CY"^^xsd:anyURI ;
  skos:broader asc:TE ;
  skos:narrower asc:TE-CY-BJ ;
  skos:narrower asc:TE-CY-CZ ;
  skos:narrower asc:TE-CY-DU ;
  skos:narrower asc:TE-CY-DZ ;
  skos:narrower asc:TE-CY-EA ;
  skos:narrower asc:TE-CY-EM ;
  skos:narrower asc:TE-CY-GE ;
  skos:notation "TE-CY" ;
  skos:prefLabel "Leptic Tenosol" ;
.
asc:TE-CY-BJ
  a asc:Greatgroup ;
  a skos:Concept ;
  asc:classifier asc:BJ ;
  dcterms:identifier "http://anzsoil.org/def/au/asc/TE-CY-BJ"^^xsd:anyURI ;
  skos:broader asc:TE-BF ;
  skos:prefLabel "Duric Leptic Tenosol" ;
.
asc:TE-CY-CZ
  a asc:Greatgroup ;
  a skos:Concept ;
  asc:classifier asc:CZ ;
  dcterms:identifier "http://anzsoil.org/def/au/asc/TE-CY-CZ"^^xsd:anyURI ;
  skos:broader asc:TE-CY ;
  skos:prefLabel "Lithic Leptic Tenosol" ;
.
asc:TE-CY-DU
  a asc:Greatgroup ;
  a skos:Concept ;
  asc:classifier asc:DU ;
  dcterms:identifier "http://anzsoil.org/def/au/asc/TE-CY-DU"^^xsd:anyURI ;
  skos:broader asc:TE-CY ;
  skos:prefLabel "Paralithic Leptic Tenosol" ;
.
asc:TE-CY-DZ
  a asc:Greatgroup ;
  a skos:Concept ;
  asc:classifier asc:DZ ;
  dcterms:identifier "http://anzsoil.org/def/au/asc/TE-CY-DZ"^^xsd:anyURI ;
  skos:broader asc:TE-CY ;
  skos:prefLabel "Petrocalcic Leptic Tenosol" ;
.
asc:TE-CY-EA
  a asc:Greatgroup ;
  a skos:Concept ;
  asc:classifier asc:EA ;
  dcterms:identifier "http://anzsoil.org/def/au/asc/TE-CY-EA"^^xsd:anyURI ;
  skos:broader asc:TE-CY ;
  skos:prefLabel "Petroferric Leptic Tenosol" ;
.
asc:TE-CY-EM
  a asc:Greatgroup ;
  a skos:Concept ;
  asc:classifier asc:EM ;
  dcterms:identifier "http://anzsoil.org/def/au/asc/TE-CY-EM"^^xsd:anyURI ;
  skos:broader asc:TE-CY ;
  skos:prefLabel "Silpanic Leptic Tenosol" ;
.
asc:TE-CY-GE
  a asc:Greatgroup ;
  a skos:Concept ;
  asc:classifier asc:GE ;
  dcterms:identifier "http://anzsoil.org/def/au/asc/TE-CY-GE"^^xsd:anyURI ;
  skos:broader asc:TE-CY ;
  skos:prefLabel "Ferric-Petroferric Leptic Tenosol" ;
.
asc:TE-IL
  a asc:Suborder ;
  a skos:Concept ;
  asc:classifier asc:IL ;
  asc:greatgroup asc:AP ;
  asc:greatgroup asc:BJ ;
  asc:greatgroup asc:CZ ;
  asc:greatgroup asc:DU ;
  asc:greatgroup asc:DZ ;
  asc:greatgroup asc:EA ;
  asc:greatgroup asc:EF ;
  asc:greatgroup asc:EM ;
  asc:greatgroup asc:GF ;
  asc:greatgroup asc:IA ;
  asc:subgroup asc:AI ;
  asc:subgroup asc:AR ;
  asc:subgroup asc:AT ;
  asc:subgroup asc:AY ;
  asc:subgroup asc:BC ;
  asc:subgroup asc:DC ;
  dcterms:identifier "http://anzsoil.org/def/au/asc/TE-IL"^^xsd:anyURI ;
  skos:broader asc:TE ;
  skos:narrower asc:TE-IL-AP ;
  skos:narrower asc:TE-IL-BJ ;
  skos:narrower asc:TE-IL-CZ ;
  skos:narrower asc:TE-IL-DU ;
  skos:narrower asc:TE-IL-DZ ;
  skos:narrower asc:TE-IL-EA ;
  skos:narrower asc:TE-IL-EF ;
  skos:narrower asc:TE-IL-EM ;
  skos:narrower asc:TE-IL-GF ;
  skos:narrower asc:TE-IL-IA ;
  skos:notation "TE-IL" ;
  skos:prefLabel "Sesqui-Nodular Tenosol" ;
.
asc:TE-IL-AP
  a asc:Greatgroup ;
  a skos:Concept ;
  asc:classifier asc:AP ;
  dcterms:identifier "http://anzsoil.org/def/au/asc/TE-IL-AP"^^xsd:anyURI ;
  skos:broader asc:TE-IL ;
  skos:prefLabel "Argic Sesqui-Nodular Tenosol" ;
.
asc:TE-IL-BJ
  a asc:Greatgroup ;
  a skos:Concept ;
  asc:classifier asc:BJ ;
  dcterms:identifier "http://anzsoil.org/def/au/asc/TE-IL-BJ"^^xsd:anyURI ;
  skos:broader asc:TE-IL ;
  skos:prefLabel "Duric Sesqui-Nodular Tenosol" ;
.
asc:TE-IL-CZ
  a asc:Greatgroup ;
  a skos:Concept ;
  asc:classifier asc:CZ ;
  dcterms:identifier "http://anzsoil.org/def/au/asc/TE-IL-CZ"^^xsd:anyURI ;
  skos:broader asc:TE-IL ;
  skos:prefLabel "Lithic Sesqui-Nodular Tenosol" ;
.
asc:TE-IL-DU
  a asc:Greatgroup ;
  a skos:Concept ;
  asc:classifier asc:DU ;
  dcterms:identifier "http://anzsoil.org/def/au/asc/TE-IL-DU"^^xsd:anyURI ;
  skos:broader asc:TE-IL ;
  skos:prefLabel "Paralithic Sesqui-Nodular Tenosol" ;
.
asc:TE-IL-DZ
  a asc:Greatgroup ;
  a skos:Concept ;
  asc:classifier asc:DZ ;
  dcterms:identifier "http://anzsoil.org/def/au/asc/TE-IL-DZ"^^xsd:anyURI ;
  skos:broader asc:TE-IL ;
  skos:prefLabel "Petrocalcic Sesqui-Nodular Tenosol" ;
.
asc:TE-IL-EA
  a asc:Greatgroup ;
  a skos:Concept ;
  asc:classifier asc:EA ;
  dcterms:identifier "http://anzsoil.org/def/au/asc/TE-IL-EA"^^xsd:anyURI ;
  skos:broader asc:TE-IL ;
  skos:prefLabel "Petroferric Sesqui-Nodular Tenosol" ;
.
asc:TE-IL-EF
  a asc:Greatgroup ;
  a skos:Concept ;
  asc:classifier asc:EF ;
  dcterms:identifier "http://anzsoil.org/def/au/asc/TE-IL-EF"^^xsd:anyURI ;
  skos:broader asc:TE-IL ;
  skos:prefLabel "Reticulate Sesqui-Nodular Tenosol" ;
.
asc:TE-IL-EM
  a asc:Greatgroup ;
  a skos:Concept ;
  asc:classifier asc:EM ;
  dcterms:identifier "http://anzsoil.org/def/au/asc/TE-IL-EM"^^xsd:anyURI ;
  skos:broader asc:TE-IL ;
  skos:prefLabel "Silpanic Sesqui-Nodular Tenosol" ;
.
asc:TE-IL-GF
  a asc:Greatgroup ;
  a skos:Concept ;
  asc:classifier asc:GF ;
  dcterms:identifier "http://anzsoil.org/def/au/asc/TE-IL-GF"^^xsd:anyURI ;
  skos:broader asc:TE-IL ;
  skos:prefLabel "Regolithic Sesqui-Nodular Tenosol" ;
.
asc:TE-IL-IA
  a asc:Greatgroup ;
  a skos:Concept ;
  asc:classifier asc:IA ;
  dcterms:identifier "http://anzsoil.org/def/au/asc/TE-IL-IA"^^xsd:anyURI ;
  skos:broader asc:TE-IL ;
  skos:prefLabel "Inceptic Sesqui-Nodular Tenosol" ;
.
asc:TE-IM
  a asc:Suborder ;
  a skos:Concept ;
  asc:classifier asc:IM ;
  asc:greatgroup asc:AK ;
  asc:greatgroup asc:AO ;
  asc:greatgroup asc:AP ;
  asc:greatgroup asc:BJ ;
  asc:greatgroup asc:BU ;
  asc:greatgroup asc:CZ ;
  asc:greatgroup asc:DU ;
  asc:greatgroup asc:DZ ;
  asc:greatgroup asc:EM ;
  asc:greatgroup asc:GF ;
  asc:greatgroup asc:HF ;
  asc:subgroup asc:CQ ;
  asc:subgroup asc:DA ;
  asc:subgroup asc:FB ;
  dcterms:identifier "http://anzsoil.org/def/au/asc/TE-IM"^^xsd:anyURI ;
  skos:broader asc:TE ;
  skos:narrower asc:TE-IM-AK ;
  skos:narrower asc:TE-IM-AO ;
  skos:narrower asc:TE-IM-AP ;
  skos:narrower asc:TE-IM-BJ ;
  skos:narrower asc:TE-IM-BU ;
  skos:narrower asc:TE-IM-CZ ;
  skos:narrower asc:TE-IM-DU ;
  skos:narrower asc:TE-IM-DZ ;
  skos:narrower asc:TE-IM-EM ;
  skos:narrower asc:TE-IM-GF ;
  skos:narrower asc:TE-IM-HF ;
  skos:notation "TE-IM" ;
  skos:prefLabel "Calcenic Tenosol" ;
.
asc:TE-IM-AK
  a asc:Greatgroup ;
  a skos:Concept ;
  asc:classifier asc:AK ;
  dcterms:identifier "http://anzsoil.org/def/au/asc/TE-IM-AK"^^xsd:anyURI ;
  skos:broader asc:TE-IM ;
  skos:prefLabel "Andic Calcenic Tenosol" ;
.
asc:TE-IM-AO
  a asc:Greatgroup ;
  a skos:Concept ;
  asc:classifier asc:AO ;
  dcterms:identifier "http://anzsoil.org/def/au/asc/TE-IM-AO"^^xsd:anyURI ;
  skos:broader asc:TE-IM ;
  skos:prefLabel "Arenic Calcenic Tenosol" ;
.
asc:TE-IM-AP
  a asc:Greatgroup ;
  a skos:Concept ;
  asc:classifier asc:AP ;
  dcterms:identifier "http://anzsoil.org/def/au/asc/TE-IM-AP"^^xsd:anyURI ;
  skos:broader asc:TE-IM ;
  skos:prefLabel "Argic Calcenic Tenosol" ;
.
asc:TE-IM-BJ
  a asc:Greatgroup ;
  a skos:Concept ;
  asc:classifier asc:BJ ;
  dcterms:identifier "http://anzsoil.org/def/au/asc/TE-IM-BJ"^^xsd:anyURI ;
  skos:broader asc:TE-IM ;
  skos:prefLabel "Duric Calcenic Tenosol" ;
.
asc:TE-IM-BU
  a asc:Greatgroup ;
  a skos:Concept ;
  asc:classifier asc:BU ;
  dcterms:identifier "http://anzsoil.org/def/au/asc/TE-IM-BU"^^xsd:anyURI ;
  skos:broader asc:TE-IM ;
  skos:prefLabel "Ferric Calcenic Tenosol" ;
.
asc:TE-IM-CZ
  a asc:Greatgroup ;
  a skos:Concept ;
  asc:classifier asc:CZ ;
  dcterms:identifier "http://anzsoil.org/def/au/asc/TE-IM-CZ"^^xsd:anyURI ;
  skos:broader asc:TE-IM ;
  skos:prefLabel "Lithic Calcenic Tenosol" ;
.
asc:TE-IM-DU
  a asc:Greatgroup ;
  a skos:Concept ;
  asc:classifier asc:DU ;
  dcterms:identifier "http://anzsoil.org/def/au/asc/TE-IM-DU"^^xsd:anyURI ;
  skos:broader asc:TE-IM ;
  skos:prefLabel "Paralithic Calcenic Tenosol" ;
.
asc:TE-IM-DZ
  a asc:Greatgroup ;
  a skos:Concept ;
  asc:classifier asc:DZ ;
  dcterms:identifier "http://anzsoil.org/def/au/asc/TE-IM-DZ"^^xsd:anyURI ;
  skos:broader asc:TE-IM ;
  skos:prefLabel "Petrocalcic Calcenic Tenosol" ;
.
asc:TE-IM-EM
  a asc:Greatgroup ;
  a skos:Concept ;
  asc:classifier asc:EM ;
  dcterms:identifier "http://anzsoil.org/def/au/asc/TE-IM-EM"^^xsd:anyURI ;
  skos:broader asc:TE-IM ;
  skos:prefLabel "Silpanic Calcenic Tenosol" ;
.
asc:TE-IM-GF
  a asc:Greatgroup ;
  a skos:Concept ;
  asc:classifier asc:GF ;
  dcterms:identifier "http://anzsoil.org/def/au/asc/TE-IM-GF"^^xsd:anyURI ;
  skos:broader asc:TE-IM ;
  skos:prefLabel "Regolithic Calcenic Tenosol" ;
.
asc:TE-IM-HF
  a asc:Greatgroup ;
  a skos:Concept ;
  asc:classifier asc:HF ;
  dcterms:identifier "http://anzsoil.org/def/au/asc/TE-IM-HF"^^xsd:anyURI ;
  skos:broader asc:TE-IM ;
  skos:prefLabel "Tephric Calcenic Tenosol" ;
.
asc:Texture
  a owl:Class ;
  rdfs:subClassOf asc:Class ;
  skos:prefLabel "Texture" ;
.
asc:Thickness
  a owl:Class ;
  rdfs:subClassOf asc:Class ;
  skos:prefLabel "Thickness" ;
.
asc:U
  a asc:Class ;
  a asc:Depth ;
  skos:definition "0.25–<0.5 m" ;
  skos:notation "U" ;
  skos:prefLabel "Shallow" ;
.
asc:V
  a asc:Class ;
  a asc:Depth ;
  skos:definition "0.5–<1.0 m" ;
  skos:notation "V" ;
  skos:prefLabel "Moderately deep" ;
.
asc:VE
  a asc:Order ;
  a skos:Concept ;
  asc:colourclass asc:AA ;
  asc:colourclass asc:AB ;
  asc:colourclass asc:AC ;
  asc:colourclass asc:AD ;
  asc:colourclass asc:AE ;
  asc:colourclass-comment """The dominant colour class in the major part of the upper 0.5 m of the B2 horizon (or the major part of the entire B2 horizon if it is less than 0.5 m thick) is:

Of the soils entered in the data base, the most common class for the first edition was Black (40%) which is probably a reflection of the agricultural importance of these soils.""" ;
  asc:family-comment "Because of the uniform clayey nature of these soils and their usual lack of distinct horizonation, several of the usual family criteria are not appropriate for Vertosols. Field texture in these soils may not be a reliable guide to actual clay content (see Field Handbook), and it may also be difficult to achieve consistent results between operators. Hence it is thought more appropriate to provide for a subdivision of actual clay content as determined by laboratory analysis. The classes used are similar to those used for clayey particle-size classes in Soil Taxonomy (Soil Survey Staff 2014). Other criteria used are gravel content of surface and A1 horizon and soil depth." ;
  asc:family-criteria asc:E ;
  asc:family-criteria asc:F ;
  asc:family-criteria asc:G ;
  asc:family-criteria asc:H ;
  asc:family-criteria asc:I ;
  asc:family-criteria asc:Q ;
  asc:family-criteria asc:R ;
  asc:family-criteria asc:S ;
  asc:family-criteria asc:T ;
  asc:family-criteria asc:U ;
  asc:family-criteria asc:V ;
  asc:family-criteria asc:W ;
  asc:family-criteria asc:X ;
  asc:family-criteria asc:Y ;
  asc:suborder asc:AM ;
  dcterms:description "Clay soils with shrink-swell properties that exhibit strong cracking when dry and at depth have slickensides and/or lenticular peds. Although many soils exhibit gilgai microrelief, this feature is not used in their definition. Australia has the greatest area and diversity of cracking clay soils of any country in the world." ;
  dcterms:identifier "http://anzsoil.org/def/au/asc/VE"^^xsd:anyURI ;
  rdfs:comment """In some clay soils it may be difficult to decide if sufficient cracks are present, or at the time of inspection the soil may be too moist to exhibit cracking. Also, in arid zone clay soils which commonly have high salt contents, the soil structure may be so fine and strong granular, or 'puffy', that it is difficult to decide if cracks are present or not. In such soils it is also obviously difficult to discern slickensides and/or lenticular peds. In yet other clay soils (up to 50% clay or more) cracks may develop but slickensides and/or lenticular peds are apparently not present.

Because cracking, slickensides and/or lenticular peds are essentially used as evidence to indicate shrink-swell behaviour, it is desirable that surrogate measurements be available if the morphological evidence is lacking or cannot be determined. See Vertic properties.""" ;
  skos:definition """Soils with the following:

1.  A clay field texture or 35% or more clay throughout the solum except for thin, surface crusty horizons 30 mm or less thick and
2. When dry, open cracks occur at some time in most years1. These are at least 5 mm wide and extend upward to the surface or to the base of any plough layer, peaty horizon, self-mulching horizon, or thin, surface crusty horizon; and
3. Slickensides and/or lenticular peds occur at some depth in the solum. 

1 Note that there is no crack frequency criterion as in the Factual Key (Northcote 1979).""" ;
  skos:narrower asc:VE-AA ;
  skos:narrower asc:VE-AB ;
  skos:narrower asc:VE-AC ;
  skos:narrower asc:VE-AD ;
  skos:narrower asc:VE-AE ;
  skos:narrower asc:VE-AM ;
  skos:notation "VE" ;
  skos:prefLabel "Vertosols" ;
.
asc:VE-AA
  a asc:Suborder ;
  asc:classifier asc:AA ;
  asc:greatgroup asc:BH ;
  asc:greatgroup asc:DF ;
  asc:greatgroup asc:DW ;
  asc:greatgroup asc:EI ;
  asc:greatgroup asc:GS ;
  asc:greatgroup-comment """These may not all apply to each suborder, in particular our knowledge of the Aquic suborder is limited.

Apart from the Peaty forms, each of the above soil surface conditions tends to reform despite cultivation or surface trampling. There may be a problem in identifying the self-mulching condition in periods of initial drying, i.e. in assessing the stability of the surface flake which forms following rainfall. If there is doubt as to whether a soil is self-mulching or has only a pedal surface, it is suggested that the latter condition be recorded, i.e. use the self-mulching great group only for those soils where the condition is not in doubt. It may be difficult to determine the surface condition if a dense grass sward is present. In this situation it will be necessary to look for a patch of bare ground, or even to kill the grass with herbicide and return at a later date. Note also that large soil units bounded by cracks are not considered to be coarse peds. It is usually necessary to examine these soils in the moist state to determine their degree of pedality.""" ;
  asc:subgroup asc:AT ;
  asc:subgroup asc:BJ ;
  asc:subgroup asc:BL ;
  asc:subgroup asc:BN ;
  asc:subgroup asc:BP ;
  asc:subgroup asc:BR ;
  asc:subgroup asc:BU ;
  asc:subgroup asc:BZ ;
  asc:subgroup asc:CD ;
  asc:subgroup asc:CU ;
  asc:subgroup asc:DB ;
  asc:subgroup asc:DC ;
  asc:subgroup asc:DQ ;
  asc:subgroup asc:DZ ;
  asc:subgroup asc:EG ;
  asc:subgroup asc:EP ;
  asc:subgroup asc:EU ;
  asc:subgroup asc:EV ;
  asc:subgroup asc:FM ;
  asc:subgroup asc:FY ;
  asc:subgroup asc:FZ ;
  asc:subgroup asc:GA ;
  asc:subgroup asc:GB ;
  asc:subgroup asc:GG ;
  asc:subgroup asc:GH ;
  asc:subgroup asc:GI ;
  asc:subgroup asc:GJ ;
  asc:subgroup asc:GK ;
  asc:subgroup asc:GL ;
  asc:subgroup asc:GM ;
  asc:subgroup asc:GN ;
  asc:subgroup asc:GO ;
  asc:subgroup asc:GQ ;
  asc:subgroup asc:HE ;
  asc:subgroup asc:IW ;
  asc:subgroup asc:IX ;
  asc:subgroup asc:IZ ;
  asc:subgroup asc:JA ;
  asc:subgroup asc:JC ;
  asc:subgroup asc:JF ;
  asc:subgroup asc:JG ;
  asc:subgroup asc:JH ;
  asc:subgroup asc:JI ;
  asc:subgroup-comment """It is thought that the following subgroups will be required for most of the suborders and great groups. Note that some of the differentiating criteria are not mutually exclusive, and thus sometimes it has been a subjective decision as to which attributes have priority in the key.

If a diagnostic feature in the key begins more than 1.5 m from the soil surface it may not have a significant impact on the performance of the soil. Refer to diagnostic features in the glossary for guidance on the use of such features in the classification.

It should be noted that all the Endoacidic soils classified are also Endohypersodic, with some also being Epihypersodic. Additionally, some Epicalcareous-Epihypersodic soils are Endoacidic at depth. It is not possible to cater for all these combinations.""" ;
  skos:broader asc:VE ;
  skos:notation "VE-AA" ;
  skos:prefLabel "Red Vertosol" ;
.
asc:VE-AB
  a asc:Suborder ;
  asc:classifier asc:AB ;
  asc:greatgroup asc:BH ;
  asc:greatgroup asc:DF ;
  asc:greatgroup asc:DW ;
  asc:greatgroup asc:EI ;
  asc:greatgroup asc:GS ;
  asc:greatgroup-comment """These may not all apply to each suborder, in particular our knowledge of the Aquic suborder is limited.

Apart from the Peaty forms, each of the above soil surface conditions tends to reform despite cultivation or surface trampling. There may be a problem in identifying the self-mulching condition in periods of initial drying, i.e. in assessing the stability of the surface flake which forms following rainfall. If there is doubt as to whether a soil is self-mulching or has only a pedal surface, it is suggested that the latter condition be recorded, i.e. use the self-mulching great group only for those soils where the condition is not in doubt. It may be difficult to determine the surface condition if a dense grass sward is present. In this situation it will be necessary to look for a patch of bare ground, or even to kill the grass with herbicide and return at a later date. Note also that large soil units bounded by cracks are not considered to be coarse peds. It is usually necessary to examine these soils in the moist state to determine their degree of pedality.""" ;
  asc:subgroup asc:AT ;
  asc:subgroup asc:BJ ;
  asc:subgroup asc:BL ;
  asc:subgroup asc:BN ;
  asc:subgroup asc:BP ;
  asc:subgroup asc:BR ;
  asc:subgroup asc:BU ;
  asc:subgroup asc:BZ ;
  asc:subgroup asc:CD ;
  asc:subgroup asc:CU ;
  asc:subgroup asc:DB ;
  asc:subgroup asc:DC ;
  asc:subgroup asc:DQ ;
  asc:subgroup asc:DZ ;
  asc:subgroup asc:EG ;
  asc:subgroup asc:EP ;
  asc:subgroup asc:EU ;
  asc:subgroup asc:EV ;
  asc:subgroup asc:FM ;
  asc:subgroup asc:FY ;
  asc:subgroup asc:FZ ;
  asc:subgroup asc:GA ;
  asc:subgroup asc:GB ;
  asc:subgroup asc:GG ;
  asc:subgroup asc:GH ;
  asc:subgroup asc:GI ;
  asc:subgroup asc:GJ ;
  asc:subgroup asc:GK ;
  asc:subgroup asc:GL ;
  asc:subgroup asc:GM ;
  asc:subgroup asc:GN ;
  asc:subgroup asc:GO ;
  asc:subgroup asc:GQ ;
  asc:subgroup asc:HE ;
  asc:subgroup asc:IW ;
  asc:subgroup asc:IX ;
  asc:subgroup asc:IZ ;
  asc:subgroup asc:JA ;
  asc:subgroup asc:JC ;
  asc:subgroup asc:JF ;
  asc:subgroup asc:JG ;
  asc:subgroup asc:JH ;
  asc:subgroup asc:JI ;
  asc:subgroup-comment """It is thought that the following subgroups will be required for most of the suborders and great groups. Note that some of the differentiating criteria are not mutually exclusive, and thus sometimes it has been a subjective decision as to which attributes have priority in the key.

If a diagnostic feature in the key begins more than 1.5 m from the soil surface it may not have a significant impact on the performance of the soil. Refer to diagnostic features in the glossary for guidance on the use of such features in the classification.

It should be noted that all the Endoacidic soils classified are also Endohypersodic, with some also being Epihypersodic. Additionally, some Epicalcareous-Epihypersodic soils are Endoacidic at depth. It is not possible to cater for all these combinations.""" ;
  skos:broader asc:VE ;
  skos:notation "VE-AB" ;
  skos:prefLabel "Brown Vertosol" ;
.
asc:VE-AC
  a asc:Suborder ;
  asc:classifier asc:AC ;
  asc:greatgroup asc:BH ;
  asc:greatgroup asc:DF ;
  asc:greatgroup asc:DW ;
  asc:greatgroup asc:EI ;
  asc:greatgroup asc:GS ;
  asc:greatgroup-comment """These may not all apply to each suborder, in particular our knowledge of the Aquic suborder is limited.

Apart from the Peaty forms, each of the above soil surface conditions tends to reform despite cultivation or surface trampling. There may be a problem in identifying the self-mulching condition in periods of initial drying, i.e. in assessing the stability of the surface flake which forms following rainfall. If there is doubt as to whether a soil is self-mulching or has only a pedal surface, it is suggested that the latter condition be recorded, i.e. use the self-mulching great group only for those soils where the condition is not in doubt. It may be difficult to determine the surface condition if a dense grass sward is present. In this situation it will be necessary to look for a patch of bare ground, or even to kill the grass with herbicide and return at a later date. Note also that large soil units bounded by cracks are not considered to be coarse peds. It is usually necessary to examine these soils in the moist state to determine their degree of pedality.""" ;
  asc:subgroup asc:AT ;
  asc:subgroup asc:BJ ;
  asc:subgroup asc:BL ;
  asc:subgroup asc:BN ;
  asc:subgroup asc:BP ;
  asc:subgroup asc:BR ;
  asc:subgroup asc:BU ;
  asc:subgroup asc:BZ ;
  asc:subgroup asc:CD ;
  asc:subgroup asc:CU ;
  asc:subgroup asc:DB ;
  asc:subgroup asc:DC ;
  asc:subgroup asc:DQ ;
  asc:subgroup asc:DZ ;
  asc:subgroup asc:EG ;
  asc:subgroup asc:EP ;
  asc:subgroup asc:EU ;
  asc:subgroup asc:EV ;
  asc:subgroup asc:FM ;
  asc:subgroup asc:FY ;
  asc:subgroup asc:FZ ;
  asc:subgroup asc:GA ;
  asc:subgroup asc:GB ;
  asc:subgroup asc:GG ;
  asc:subgroup asc:GH ;
  asc:subgroup asc:GI ;
  asc:subgroup asc:GJ ;
  asc:subgroup asc:GK ;
  asc:subgroup asc:GL ;
  asc:subgroup asc:GM ;
  asc:subgroup asc:GN ;
  asc:subgroup asc:GO ;
  asc:subgroup asc:GQ ;
  asc:subgroup asc:HE ;
  asc:subgroup asc:IW ;
  asc:subgroup asc:IX ;
  asc:subgroup asc:IZ ;
  asc:subgroup asc:JA ;
  asc:subgroup asc:JC ;
  asc:subgroup asc:JF ;
  asc:subgroup asc:JG ;
  asc:subgroup asc:JH ;
  asc:subgroup asc:JI ;
  asc:subgroup-comment """It is thought that the following subgroups will be required for most of the suborders and great groups. Note that some of the differentiating criteria are not mutually exclusive, and thus sometimes it has been a subjective decision as to which attributes have priority in the key.

If a diagnostic feature in the key begins more than 1.5 m from the soil surface it may not have a significant impact on the performance of the soil. Refer to diagnostic features in the glossary for guidance on the use of such features in the classification.

It should be noted that all the Endoacidic soils classified are also Endohypersodic, with some also being Epihypersodic. Additionally, some Epicalcareous-Epihypersodic soils are Endoacidic at depth. It is not possible to cater for all these combinations.""" ;
  skos:broader asc:VE ;
  skos:notation "VE-AC" ;
  skos:prefLabel "Yellow Vertosol" ;
.
asc:VE-AD
  a asc:Suborder ;
  asc:classifier asc:AD ;
  asc:greatgroup asc:BH ;
  asc:greatgroup asc:DF ;
  asc:greatgroup asc:DW ;
  asc:greatgroup asc:EI ;
  asc:greatgroup asc:GS ;
  asc:greatgroup-comment """These may not all apply to each suborder, in particular our knowledge of the Aquic suborder is limited.

Apart from the Peaty forms, each of the above soil surface conditions tends to reform despite cultivation or surface trampling. There may be a problem in identifying the self-mulching condition in periods of initial drying, i.e. in assessing the stability of the surface flake which forms following rainfall. If there is doubt as to whether a soil is self-mulching or has only a pedal surface, it is suggested that the latter condition be recorded, i.e. use the self-mulching great group only for those soils where the condition is not in doubt. It may be difficult to determine the surface condition if a dense grass sward is present. In this situation it will be necessary to look for a patch of bare ground, or even to kill the grass with herbicide and return at a later date. Note also that large soil units bounded by cracks are not considered to be coarse peds. It is usually necessary to examine these soils in the moist state to determine their degree of pedality.""" ;
  asc:subgroup asc:AT ;
  asc:subgroup asc:BJ ;
  asc:subgroup asc:BL ;
  asc:subgroup asc:BN ;
  asc:subgroup asc:BP ;
  asc:subgroup asc:BR ;
  asc:subgroup asc:BU ;
  asc:subgroup asc:BZ ;
  asc:subgroup asc:CD ;
  asc:subgroup asc:CU ;
  asc:subgroup asc:DB ;
  asc:subgroup asc:DC ;
  asc:subgroup asc:DQ ;
  asc:subgroup asc:DZ ;
  asc:subgroup asc:EG ;
  asc:subgroup asc:EP ;
  asc:subgroup asc:EU ;
  asc:subgroup asc:EV ;
  asc:subgroup asc:FM ;
  asc:subgroup asc:FY ;
  asc:subgroup asc:FZ ;
  asc:subgroup asc:GA ;
  asc:subgroup asc:GB ;
  asc:subgroup asc:GG ;
  asc:subgroup asc:GH ;
  asc:subgroup asc:GI ;
  asc:subgroup asc:GJ ;
  asc:subgroup asc:GK ;
  asc:subgroup asc:GL ;
  asc:subgroup asc:GM ;
  asc:subgroup asc:GN ;
  asc:subgroup asc:GO ;
  asc:subgroup asc:GQ ;
  asc:subgroup asc:HE ;
  asc:subgroup asc:IW ;
  asc:subgroup asc:IX ;
  asc:subgroup asc:IZ ;
  asc:subgroup asc:JA ;
  asc:subgroup asc:JC ;
  asc:subgroup asc:JF ;
  asc:subgroup asc:JG ;
  asc:subgroup asc:JH ;
  asc:subgroup asc:JI ;
  asc:subgroup-comment """It is thought that the following subgroups will be required for most of the suborders and great groups. Note that some of the differentiating criteria are not mutually exclusive, and thus sometimes it has been a subjective decision as to which attributes have priority in the key.

If a diagnostic feature in the key begins more than 1.5 m from the soil surface it may not have a significant impact on the performance of the soil. Refer to diagnostic features in the glossary for guidance on the use of such features in the classification.

It should be noted that all the Endoacidic soils classified are also Endohypersodic, with some also being Epihypersodic. Additionally, some Epicalcareous-Epihypersodic soils are Endoacidic at depth. It is not possible to cater for all these combinations.""" ;
  skos:broader asc:VE ;
  skos:notation "VE-AD" ;
  skos:prefLabel "Grey Vertosol" ;
.
asc:VE-AE
  a asc:Suborder ;
  asc:classifier asc:AE ;
  asc:greatgroup asc:BH ;
  asc:greatgroup asc:DF ;
  asc:greatgroup asc:DW ;
  asc:greatgroup asc:EI ;
  asc:greatgroup asc:GS ;
  asc:greatgroup-comment """These may not all apply to each suborder, in particular our knowledge of the Aquic suborder is limited.

Apart from the Peaty forms, each of the above soil surface conditions tends to reform despite cultivation or surface trampling. There may be a problem in identifying the self-mulching condition in periods of initial drying, i.e. in assessing the stability of the surface flake which forms following rainfall. If there is doubt as to whether a soil is self-mulching or has only a pedal surface, it is suggested that the latter condition be recorded, i.e. use the self-mulching great group only for those soils where the condition is not in doubt. It may be difficult to determine the surface condition if a dense grass sward is present. In this situation it will be necessary to look for a patch of bare ground, or even to kill the grass with herbicide and return at a later date. Note also that large soil units bounded by cracks are not considered to be coarse peds. It is usually necessary to examine these soils in the moist state to determine their degree of pedality.""" ;
  asc:subgroup asc:AT ;
  asc:subgroup asc:BJ ;
  asc:subgroup asc:BL ;
  asc:subgroup asc:BN ;
  asc:subgroup asc:BP ;
  asc:subgroup asc:BR ;
  asc:subgroup asc:BU ;
  asc:subgroup asc:BZ ;
  asc:subgroup asc:CD ;
  asc:subgroup asc:CU ;
  asc:subgroup asc:DB ;
  asc:subgroup asc:DC ;
  asc:subgroup asc:DQ ;
  asc:subgroup asc:DZ ;
  asc:subgroup asc:EG ;
  asc:subgroup asc:EP ;
  asc:subgroup asc:EU ;
  asc:subgroup asc:EV ;
  asc:subgroup asc:FM ;
  asc:subgroup asc:FY ;
  asc:subgroup asc:FZ ;
  asc:subgroup asc:GA ;
  asc:subgroup asc:GB ;
  asc:subgroup asc:GG ;
  asc:subgroup asc:GH ;
  asc:subgroup asc:GI ;
  asc:subgroup asc:GJ ;
  asc:subgroup asc:GK ;
  asc:subgroup asc:GL ;
  asc:subgroup asc:GM ;
  asc:subgroup asc:GN ;
  asc:subgroup asc:GO ;
  asc:subgroup asc:GQ ;
  asc:subgroup asc:HE ;
  asc:subgroup asc:IW ;
  asc:subgroup asc:IX ;
  asc:subgroup asc:IZ ;
  asc:subgroup asc:JA ;
  asc:subgroup asc:JC ;
  asc:subgroup asc:JF ;
  asc:subgroup asc:JG ;
  asc:subgroup asc:JH ;
  asc:subgroup asc:JI ;
  asc:subgroup-comment """It is thought that the following subgroups will be required for most of the suborders and great groups. Note that some of the differentiating criteria are not mutually exclusive, and thus sometimes it has been a subjective decision as to which attributes have priority in the key.

If a diagnostic feature in the key begins more than 1.5 m from the soil surface it may not have a significant impact on the performance of the soil. Refer to diagnostic features in the glossary for guidance on the use of such features in the classification.

It should be noted that all the Endoacidic soils classified are also Endohypersodic, with some also being Epihypersodic. Additionally, some Epicalcareous-Epihypersodic soils are Endoacidic at depth. It is not possible to cater for all these combinations.""" ;
  skos:broader asc:VE ;
  skos:notation "VE-AE" ;
  skos:prefLabel "Black Vertosol" ;
.
asc:VE-AM
  a asc:Suborder ;
  asc:classifier asc:AM ;
  asc:greatgroup asc:BH ;
  asc:greatgroup asc:DF ;
  asc:greatgroup asc:DW ;
  asc:greatgroup asc:EI ;
  asc:greatgroup asc:GS ;
  asc:greatgroup-comment """These may not all apply to each suborder, in particular our knowledge of the Aquic suborder is limited.

Apart from the Peaty forms, each of the above soil surface conditions tends to reform despite cultivation or surface trampling. There may be a problem in identifying the self-mulching condition in periods of initial drying, i.e. in assessing the stability of the surface flake which forms following rainfall. If there is doubt as to whether a soil is self-mulching or has only a pedal surface, it is suggested that the latter condition be recorded, i.e. use the self-mulching great group only for those soils where the condition is not in doubt. It may be difficult to determine the surface condition if a dense grass sward is present. In this situation it will be necessary to look for a patch of bare ground, or even to kill the grass with herbicide and return at a later date. Note also that large soil units bounded by cracks are not considered to be coarse peds. It is usually necessary to examine these soils in the moist state to determine their degree of pedality.""" ;
  asc:subgroup asc:AT ;
  asc:subgroup asc:BJ ;
  asc:subgroup asc:BL ;
  asc:subgroup asc:BN ;
  asc:subgroup asc:BP ;
  asc:subgroup asc:BR ;
  asc:subgroup asc:BU ;
  asc:subgroup asc:BZ ;
  asc:subgroup asc:CD ;
  asc:subgroup asc:CU ;
  asc:subgroup asc:DB ;
  asc:subgroup asc:DC ;
  asc:subgroup asc:DQ ;
  asc:subgroup asc:DZ ;
  asc:subgroup asc:EG ;
  asc:subgroup asc:EP ;
  asc:subgroup asc:EU ;
  asc:subgroup asc:EV ;
  asc:subgroup asc:FM ;
  asc:subgroup asc:FY ;
  asc:subgroup asc:FZ ;
  asc:subgroup asc:GA ;
  asc:subgroup asc:GB ;
  asc:subgroup asc:GG ;
  asc:subgroup asc:GH ;
  asc:subgroup asc:GI ;
  asc:subgroup asc:GJ ;
  asc:subgroup asc:GK ;
  asc:subgroup asc:GL ;
  asc:subgroup asc:GM ;
  asc:subgroup asc:GN ;
  asc:subgroup asc:GO ;
  asc:subgroup asc:GQ ;
  asc:subgroup asc:HE ;
  asc:subgroup asc:IW ;
  asc:subgroup asc:IX ;
  asc:subgroup asc:IZ ;
  asc:subgroup asc:JA ;
  asc:subgroup asc:JC ;
  asc:subgroup asc:JF ;
  asc:subgroup asc:JG ;
  asc:subgroup asc:JH ;
  asc:subgroup asc:JI ;
  asc:subgroup-comment """It is thought that the following subgroups will be required for most of the suborders and great groups. Note that some of the differentiating criteria are not mutually exclusive, and thus sometimes it has been a subjective decision as to which attributes have priority in the key.

If a diagnostic feature in the key begins more than 1.5 m from the soil surface it may not have a significant impact on the performance of the soil. Refer to diagnostic features in the glossary for guidance on the use of such features in the classification.

It should be noted that all the Endoacidic soils classified are also Endohypersodic, with some also being Epihypersodic. Additionally, some Epicalcareous-Epihypersodic soils are Endoacidic at depth. It is not possible to cater for all these combinations.""" ;
  skos:broader asc:VE ;
  skos:notation "VE-AM" ;
  skos:prefLabel "Aquic Vertosol" ;
.
asc:W
  a asc:Class ;
  a asc:Depth ;
  skos:definition "1.0–<1.5 m" ;
  skos:notation "W" ;
  skos:prefLabel "Deep" ;
.
asc:WR
  a asc:Class ;
  a asc:Water-repellence ;
  skos:definition "Water takes more than 10 seconds and 2 Molar ethanol takes 10 seconds or less to be absorbed into soil" ;
  skos:notation "WR" ;
  skos:prefLabel "Water repellent" ;
.
asc:Water-repellence
  a owl:Class ;
  rdfs:subClassOf asc:Class ;
  skos:prefLabel "Water repellence" ;
.
asc:X
  a asc:Class ;
  a asc:Depth ;
  skos:definition "1.5–5 m" ;
  skos:notation "X" ;
  skos:prefLabel "Very deep" ;
.
asc:Y
  a asc:Class ;
  a asc:Depth ;
  skos:definition ">5 m" ;
  skos:notation "Y" ;
  skos:prefLabel "Giant" ;
.
asc:Z
  a asc:Class ;
  skos:definition "Material absent" ;
  skos:notation "Z" ;
  skos:prefLabel "Material absent" ;
.
asc:classifier
  a owl:ObjectProperty ;
  rdfs:label "Differentiating class" ;
  rdfs:range asc:Class ;
  rdfs:subPropertyOf dcterms:relation ;
.
asc:colourclass
  a owl:ObjectProperty ;
  rdfs:domain asc:Order ;
  rdfs:label "Applicable Colour class" ;
  rdfs:range asc:ColourClass ;
  rdfs:subPropertyOf dcterms:relation ;
.
asc:colourclass-comment
  a owl:AnnotationProperty ;
  rdfs:domain asc:Order ;
  rdfs:label "Colour class comment" ;
  rdfs:subPropertyOf skos:note ;
.
asc:family-comment
  a owl:AnnotationProperty ;
  rdfs:domain asc:Order ;
  rdfs:label "Family comment" ;
  rdfs:subPropertyOf skos:note ;
.
asc:family-criteria
  a owl:ObjectProperty ;
  rdfs:domain asc:Order ;
  rdfs:label "Family criteria" ;
  rdfs:range asc:Class ;
  rdfs:subPropertyOf dcterms:relation ;
.
asc:greatgroup
  a owl:ObjectProperty ;
  rdfs:domain asc:Suborder ;
  rdfs:label "Applicable Great group" ;
  rdfs:range asc:Class ;
  rdfs:subPropertyOf dcterms:relation ;
.
asc:greatgroup-comment
  a owl:AnnotationProperty ;
  rdfs:domain asc:Order ;
  rdfs:label "Great group comment" ;
  rdfs:subPropertyOf skos:note ;
.
asc:subgroup
  a owl:ObjectProperty ;
  rdfs:domain asc:Suborder ;
  rdfs:label "Applicable Subgroup" ;
  rdfs:range asc:Class ;
  rdfs:subPropertyOf dcterms:relation ;
.
asc:subgroup-comment
  a owl:AnnotationProperty ;
  rdfs:domain asc:Order ;
  rdfs:label "Subgroup comment" ;
  rdfs:subPropertyOf skos:note ;
.
asc:suborder
  a owl:ObjectProperty ;
  rdfs:domain asc:Order ;
  rdfs:label "Applicable suborder" ;
  rdfs:range asc:Class ;
  rdfs:subPropertyOf dcterms:relation ;
.
asc:suborder-comment
  a owl:AnnotationProperty ;
  rdfs:domain asc:Order ;
  rdfs:label "Suborder comment" ;
  rdfs:subPropertyOf skos:note ;
.
dc:
  skos:definition "This version has been modified for use in TopBraid: it defines the dc namespace prefix and imports SKOS and DCTerms." ;
  skos:prefLabel "Dublin Core Metadata Element Set, Version 1.1" ;
.
<http://www.w3.org/2002/07/owl>
  skos:definition """
  This ontology partially describes the built-in classes and
  properties that together form the basis of the RDF/XML syntax of OWL 2.
  The content of this ontology is based on Tables 6.1 and 6.2
  in Section 6.4 of the OWL 2 RDF-Based Semantics specification,
  available at http://www.w3.org/TR/owl2-rdf-based-semantics/.
  Please note that those tables do not include the different annotations
  (labels, comments and rdfs:isDefinedBy links) used in this file.  
  Also note that the descriptions provided in this ontology do not
  provide a complete and correct formal description of either the syntax
  or the semantics of the introduced terms (please see the OWL 2
  recommendations for the complete and normative specifications).
  Furthermore, the information provided by this ontology may be
  misleading if not used with care. This ontology SHOULD NOT be imported
  into OWL ontologies. Importing this file into an OWL 2 DL ontology
  will cause it to become an OWL 2 Full ontology and may have other,
  unexpected, consequences.
   """ ;
  skos:prefLabel "owl" ;
.
