# baseURI: http://www.anzsoil.org/def/soil-profile
# imports: http://purl.org/dc/elements/1.1/
# imports: http://purl.org/linked-data/registry-ui#

@prefix dc: <http://purl.org/dc/elements/1.1/> .
@prefix dct: <http://purl.org/dc/terms/> .
@prefix owl: <http://www.w3.org/2002/07/owl#> .
@prefix rdf: <http://www.w3.org/1999/02/22-rdf-syntax-ns#> .
@prefix rdf123: <http://rdf123.umbc.edu/ns/> .
@prefix rdfs: <http://www.w3.org/2000/01/rdf-schema#> .
@prefix skos: <http://www.w3.org/2004/02/skos/core#> .
@prefix sp: <http://www.anzsoil.org/def/soil-profile/> .
@prefix spin: <http://spinrdf.org/spin#> .
@prefix ui: <http://purl.org/linked-data/registry-ui#> .
@prefix xsd: <http://www.w3.org/2001/XMLSchema#> .

<boundaries-between-horizons>
  rdf:type skos:Collection ;
  ui:topMemberOf <> ;
  rdfs:label "Boundaries between horizons" ;
  skos:member <horizon-boundary-distinctness> ;
  skos:member <horizon-boundary-shape> ;
.
<coarse-fragments>
  rdf:type skos:Collection ;
  dct:description "Coarse fragments are particles coarser than 2 mm. They include unattached rock fragments and other fragments such as charcoal and shells. Coarse fragments are distinguished from segregations of pedogenic origin in that they are not, or not considered to be, of pedogenic origin." ;
  ui:topMemberOf <> ;
  rdfs:label "Coarse fragments" ;
  skos:definition "Coarse fragments are particles coarser than 2 mm. They include unattached rock fragments and other fragments such as charcoal and shells. Coarse fragments are distinguished from segregations of pedogenic origin in that they are not, or not considered to be, of pedogenic origin." ;
  skos:member <coarse-fragments-abundance> ;
  skos:member <coarse-fragments-distribution> ;
  skos:member <coarse-fragments-lithology> ;
  skos:member <coarse-fragments-shape> ;
  skos:member <coarse-fragments-size> ;
  skos:member <coarse-fragments-strength> ;
  skos:prefLabel "Coarse fragments" ;
.
<coarse-fragments-abundance>
  rdf:type skos:Collection ;
  dct:description "<p><img src=\"https://bitbucket.csiro.au/projects/EIS/repos/australian-soil-vocabularies/raw/Yellow%20book/Images/Figure11.png\" /></p>"^^rdf:HTML ;
  ui:isMemberOf <coarse-fragments> ;
  rdfs:comment "N_CF_ABUN: The percentage is estimated by eye using the charts in the yellow book for comparison." ;
  rdfs:label "Abundance of coarse fragments" ;
  skos:definition "The percentage of coarse fragments." ;
  skos:member <coarse-fragments-abundance-0> ;
  skos:member <coarse-fragments-abundance-1> ;
  skos:member <coarse-fragments-abundance-2> ;
  skos:member <coarse-fragments-abundance-3> ;
  skos:member <coarse-fragments-abundance-4> ;
  skos:member <coarse-fragments-abundance-5> ;
  skos:member <coarse-fragments-abundance-6> ;
  skos:prefLabel "Abundance of coarse fragments" ;
.
<coarse-fragments-abundance-0>
  rdf:type skos:Concept ;
  dct:description "0%" ;
  ui:isMemberOf <coarse-fragments-abundance> ;
  rdfs:comment "N_CF_ABUN: The percentage is estimated by eye using the charts in the yellow book for comparison." ;
  rdfs:label "No coarse fragments" ;
  skos:definition "0%" ;
  skos:notation "0" ;
  skos:prefLabel "No coarse fragments" ;
  skos:topConceptOf <> ;
.
<coarse-fragments-abundance-1>
  rdf:type skos:Concept ;
  dct:description "<2%" ;
  ui:isMemberOf <coarse-fragments-abundance> ;
  rdfs:comment "N_CF_ABUN: The percentage is estimated by eye using the charts in the yellow book for comparison: for example very slightly fine gravelly; very few small pebbles" ;
  rdfs:label "Very slightly or very few" ;
  skos:definition "<2%" ;
  skos:notation "1" ;
  skos:prefLabel "Very slightly or very few" ;
  skos:topConceptOf <> ;
.
<coarse-fragments-abundance-2>
  rdf:type skos:Concept ;
  dct:description "2-10%" ;
  ui:isMemberOf <coarse-fragments-abundance> ;
  rdfs:comment "N_CF_ABUN: The percentage is estimated by eye using the charts in the yellow book for comparison" ;
  rdfs:label "Slightly or few" ;
  skos:definition "2-10%" ;
  skos:notation "2" ;
  skos:prefLabel "Slightly or few" ;
  skos:topConceptOf <> ;
.
<coarse-fragments-abundance-3>
  rdf:type skos:Concept ;
  dct:description "10-20%" ;
  ui:isMemberOf <coarse-fragments-abundance> ;
  rdfs:comment "N_CF_ABUN: The percentage is estimated by eye using the charts in the yellow book for comparison: for example medium gravelly; stony, common medium pebbles; common stones" ;
  rdfs:label "No qualifier or common" ;
  skos:definition "10-20%" ;
  skos:notation "3" ;
  skos:prefLabel "No qualifier or common" ;
  skos:topConceptOf <> ;
.
<coarse-fragments-abundance-4>
  rdf:type skos:Concept ;
  dct:description "20-50%" ;
  ui:isMemberOf <coarse-fragments-abundance> ;
  rdfs:comment "N_CF_ABUN: The percentage is estimated by eye using the charts in the yellow book for comparison" ;
  rdfs:label "Moderately or many" ;
  skos:definition "20-50%" ;
  skos:notation "4" ;
  skos:prefLabel "Moderately or many" ;
  skos:topConceptOf <> ;
.
<coarse-fragments-abundance-5>
  rdf:type skos:Concept ;
  dct:description "50-90%" ;
  ui:isMemberOf <coarse-fragments-abundance> ;
  rdfs:comment "N_CF_ABUN: The percentage is estimated by eye using the charts in the yellow book for comparison" ;
  rdfs:label "Very or abundant" ;
  skos:definition "50-90%" ;
  skos:notation "5" ;
  skos:prefLabel "Very or abundant" ;
  skos:topConceptOf <> ;
.
<coarse-fragments-abundance-6>
  rdf:type skos:Concept ;
  dct:description ">90%" ;
  ui:isMemberOf <coarse-fragments-abundance> ;
  rdfs:comment "N_CF_ABUN: The percentage is estimated by eye using the charts in the yellow book for comparison" ;
  rdfs:label "Extremely or very abundant" ;
  skos:definition ">90%" ;
  skos:notation "6" ;
  skos:prefLabel "Extremely or very abundant" ;
  skos:topConceptOf <> ;
.
<coarse-fragments-distribution>
  rdf:type skos:Collection ;
  dct:description "Coarse fragments may occur throughout the profile." ;
  ui:isMemberOf <coarse-fragments> ;
  rdfs:comment "C_CF_DISTRIBUTION" ;
  rdfs:label "Coarse fragments distribution" ;
  skos:definition "Coarse fragments may occur throughout the profile." ;
  skos:member <coarse-fragments-distribution-D> ;
  skos:member <coarse-fragments-distribution-R> ;
  skos:member <coarse-fragments-distribution-S> ;
  skos:member <coarse-fragments-distribution-U> ;
  skos:prefLabel "Coarse fragments distribution" ;
.
<coarse-fragments-distribution-D>
  rdf:type skos:Concept ;
  dct:description "fragments are scattered randomly throughout the soil and may be of mixed origin." ;
  ui:isMemberOf <coarse-fragments-distribution> ;
  rdfs:comment "C_CF_DISTRIBUTION" ;
  rdfs:label "Dispersed" ;
  skos:definition "fragments are scattered randomly throughout the soil and may be of mixed origin." ;
  skos:notation "D" ;
  skos:prefLabel "Dispersed" ;
  skos:topConceptOf <> ;
.
<coarse-fragments-distribution-R>
  rdf:type skos:Concept ;
  dct:description "all fragments are remnants of the underlying bedrock but their orientation is not related to the joint or bedding planes of the bedrock." ;
  ui:isMemberOf <coarse-fragments-distribution> ;
  rdfs:comment "C_CF_DISTRIBUTION" ;
  rdfs:label "Reoriented" ;
  skos:definition "all fragments are remnants of the underlying bedrock but their orientation is not related to the joint or bedding planes of the bedrock." ;
  skos:notation "R" ;
  skos:prefLabel "Reoriented" ;
  skos:topConceptOf <> ;
.
<coarse-fragments-distribution-S>
  rdf:type skos:Concept ;
  dct:description "fragments occur in bands, usually parallel with the soil surface (excluding those parallel with joint or bedding planes of the bedrock). They may include materials other than those from the underlying bedrock." ;
  ui:isMemberOf <coarse-fragments-distribution> ;
  rdfs:comment "C_CF_DISTRIBUTION" ;
  rdfs:label "Stratified" ;
  skos:definition "fragments occur in bands, usually parallel with the soil surface (excluding those parallel with joint or bedding planes of the bedrock). They may include materials other than those from the underlying bedrock." ;
  skos:notation "S" ;
  skos:prefLabel "Stratified" ;
  skos:topConceptOf <> ;
.
<coarse-fragments-distribution-U>
  rdf:type skos:Concept ;
  dct:description "all fragments are remnants of the underlying bedrock and their orientation closely parallels that of the joint or bedding planes of the bedrock." ;
  ui:isMemberOf <coarse-fragments-distribution> ;
  rdfs:comment "C_CF_DISTRIBUTION" ;
  rdfs:label "Undisturbed" ;
  skos:definition "all fragments are remnants of the underlying bedrock and their orientation closely parallels that of the joint or bedding planes of the bedrock." ;
  skos:notation "U" ;
  skos:prefLabel "Undisturbed" ;
  skos:topConceptOf <> ;
.
<coarse-fragments-lithology>
  rdf:type skos:Collection ;
  dct:description "The lithology of the coarse fragments is usually identified as coming from the substrate or from rock outcrop.   Where the lithology of the coarse fragments is different from that of the substrate material and/or rock outcrop, describe it as for lithology of substrate material only where the rock type is definitely known or is confidently presumed. Some coarse fragments are commonly encountered that are not directly related to the substrate material.   " ;
  ui:isMemberOf <coarse-fragments> ;
  rdfs:comment "C_LITHOLOGY" ;
  rdfs:label "Lithology of coarse fragments" ;
  skos:definition "The lithology of the coarse fragments is usually identified as coming from the substrate or from rock outcrop.   Where the lithology of the coarse fragments is different from that of the substrate material and/or rock outcrop, describe it as for lithology of substrate material only where the rock type is definitely known or is confidently presumed. Some coarse fragments are commonly encountered that are not directly related to the substrate material.   " ;
  skos:member <coarse-fragments-lithology-AC> ;
  skos:member <coarse-fragments-lithology-AD> ;
  skos:member <coarse-fragments-lithology-AF> ;
  skos:member <coarse-fragments-lithology-AG> ;
  skos:member <coarse-fragments-lithology-AH> ;
  skos:member <coarse-fragments-lithology-AM> ;
  skos:member <coarse-fragments-lithology-AN> ;
  skos:member <coarse-fragments-lithology-AP> ;
  skos:member <coarse-fragments-lithology-AR> ;
  skos:member <coarse-fragments-lithology-AS> ;
  skos:member <coarse-fragments-lithology-BA> ;
  skos:member <coarse-fragments-lithology-BB> ;
  skos:member <coarse-fragments-lithology-BR> ;
  skos:member <coarse-fragments-lithology-C> ;
  skos:member <coarse-fragments-lithology-CC> ;
  skos:member <coarse-fragments-lithology-CG> ;
  skos:member <coarse-fragments-lithology-CH> ;
  skos:member <coarse-fragments-lithology-CO> ;
  skos:member <coarse-fragments-lithology-CU> ;
  skos:member <coarse-fragments-lithology-DI> ;
  skos:member <coarse-fragments-lithology-DM> ;
  skos:member <coarse-fragments-lithology-DR> ;
  skos:member <coarse-fragments-lithology-FC> ;
  skos:member <coarse-fragments-lithology-GA> ;
  skos:member <coarse-fragments-lithology-GD> ;
  skos:member <coarse-fragments-lithology-GE> ;
  skos:member <coarse-fragments-lithology-GN> ;
  skos:member <coarse-fragments-lithology-GR> ;
  skos:member <coarse-fragments-lithology-GS> ;
  skos:member <coarse-fragments-lithology-GV> ;
  skos:member <coarse-fragments-lithology-GW> ;
  skos:member <coarse-fragments-lithology-GY> ;
  skos:member <coarse-fragments-lithology-HA> ;
  skos:member <coarse-fragments-lithology-HO> ;
  skos:member <coarse-fragments-lithology-IG> ;
  skos:member <coarse-fragments-lithology-IS> ;
  skos:member <coarse-fragments-lithology-JA> ;
  skos:member <coarse-fragments-lithology-KA> ;
  skos:member <coarse-fragments-lithology-KC> ;
  skos:member <coarse-fragments-lithology-KL> ;
  skos:member <coarse-fragments-lithology-KM> ;
  skos:member <coarse-fragments-lithology-KR> ;
  skos:member <coarse-fragments-lithology-KS> ;
  skos:member <coarse-fragments-lithology-LC> ;
  skos:member <coarse-fragments-lithology-LI> ;
  skos:member <coarse-fragments-lithology-M> ;
  skos:member <coarse-fragments-lithology-MB> ;
  skos:member <coarse-fragments-lithology-MD> ;
  skos:member <coarse-fragments-lithology-ME> ;
  skos:member <coarse-fragments-lithology-MG> ;
  skos:member <coarse-fragments-lithology-MI> ;
  skos:member <coarse-fragments-lithology-ML> ;
  skos:member <coarse-fragments-lithology-MS> ;
  skos:member <coarse-fragments-lithology-MU> ;
  skos:member <coarse-fragments-lithology-MY> ;
  skos:member <coarse-fragments-lithology-OT> ;
  skos:member <coarse-fragments-lithology-OW> ;
  skos:member <coarse-fragments-lithology-PC> ;
  skos:member <coarse-fragments-lithology-PE> ;
  skos:member <coarse-fragments-lithology-PG> ;
  skos:member <coarse-fragments-lithology-PH> ;
  skos:member <coarse-fragments-lithology-PL> ;
  skos:member <coarse-fragments-lithology-PO> ;
  skos:member <coarse-fragments-lithology-PU> ;
  skos:member <coarse-fragments-lithology-PY> ;
  skos:member <coarse-fragments-lithology-QP> ;
  skos:member <coarse-fragments-lithology-QS> ;
  skos:member <coarse-fragments-lithology-QU> ;
  skos:member <coarse-fragments-lithology-QZ> ;
  skos:member <coarse-fragments-lithology-R> ;
  skos:member <coarse-fragments-lithology-RB> ;
  skos:member <coarse-fragments-lithology-RH> ;
  skos:member <coarse-fragments-lithology-S> ;
  skos:member <coarse-fragments-lithology-SA> ;
  skos:member <coarse-fragments-lithology-SD> ;
  skos:member <coarse-fragments-lithology-SH> ;
  skos:member <coarse-fragments-lithology-SK> ;
  skos:member <coarse-fragments-lithology-SL> ;
  skos:member <coarse-fragments-lithology-SR> ;
  skos:member <coarse-fragments-lithology-SS> ;
  skos:member <coarse-fragments-lithology-ST> ;
  skos:member <coarse-fragments-lithology-SY> ;
  skos:member <coarse-fragments-lithology-TR> ;
  skos:member <coarse-fragments-lithology-TU> ;
  skos:member <coarse-fragments-lithology-UC> ;
  skos:member <coarse-fragments-lithology-VB> ;
  skos:member <coarse-fragments-lithology-VG> ;
  skos:member <coarse-fragments-lithology-Z> ;
  skos:member <coarse-fragments-lithology-ZS> ;
  skos:note "This concept should be expanded to include all codes from substrate material lithology.  A direct match." ;
  skos:prefLabel "Lithology of coarse fragments" ;
.
<coarse-fragments-lithology-AC>
  rdf:type skos:Concept ;
  dct:description "Alcrete (Sedimentary rock, chemical or organic)" ;
  ui:isMemberOf <coarse-fragments-lithology> ;
  rdfs:comment "C_LITHOLOGY" ;
  rdfs:label "Alcrete" ;
  skos:altLabel "Bauxite" ;
  skos:definition "Alcrete (Sedimentary rock, chemical or organic)" ;
  skos:notation "AC" ;
  skos:prefLabel "Alcrete" ;
  skos:topConceptOf <> ;
.
<coarse-fragments-lithology-AD>
  rdf:type skos:Concept ;
  dct:description "Adamellite (Igneous rock)" ;
  ui:isMemberOf <coarse-fragments-lithology> ;
  rdfs:comment "C_LITHOLOGY" ;
  rdfs:label "Adamellite" ;
  skos:definition "Adamellite (Igneous rock)" ;
  skos:notation "AD" ;
  skos:prefLabel "Adamellite" ;
  skos:topConceptOf <> ;
.
<coarse-fragments-lithology-AF>
  rdf:type skos:Concept ;
  dct:description "Ash (fine)  (Unconsolidated material)" ;
  ui:isMemberOf <coarse-fragments-lithology> ;
  rdfs:comment "C_LITHOLOGY" ;
  rdfs:label "Ash (fine)" ;
  skos:definition "Ash (fine)  (Unconsolidated material)" ;
  skos:notation "AF" ;
  skos:prefLabel "Ash (fine)" ;
  skos:topConceptOf <> ;
.
<coarse-fragments-lithology-AG>
  rdf:type skos:Concept ;
  dct:description "Agglomerate (Sedimentary rock, pyroclastic)" ;
  ui:isMemberOf <coarse-fragments-lithology> ;
  rdfs:comment "C_LITHOLOGY" ;
  rdfs:label "Agglomerate" ;
  skos:definition "Agglomerate (Sedimentary rock, pyroclastic)" ;
  skos:notation "AG" ;
  skos:prefLabel "Agglomerate" ;
  skos:topConceptOf <> ;
.
<coarse-fragments-lithology-AH>
  rdf:type skos:Concept ;
  dct:description "Anhydrite (Sedimentary rock, chemical or organic)" ;
  ui:isMemberOf <coarse-fragments-lithology> ;
  rdfs:comment "C_LITHOLOGY" ;
  rdfs:label "Anhydrite" ;
  skos:definition "Anhydrite (Sedimentary rock, chemical or organic)" ;
  skos:notation "AH" ;
  skos:prefLabel "Anhydrite" ;
  skos:topConceptOf <> ;
.
<coarse-fragments-lithology-AM>
  rdf:type skos:Concept ;
  dct:description "Amphibolite (Metamorphic rock)" ;
  ui:isMemberOf <coarse-fragments-lithology> ;
  rdfs:comment "C_LITHOLOGY" ;
  rdfs:label "Amphibolite" ;
  skos:definition "Amphibolite (Metamorphic rock)" ;
  skos:notation "AM" ;
  skos:prefLabel "Amphibolite" ;
  skos:topConceptOf <> ;
.
<coarse-fragments-lithology-AN>
  rdf:type skos:Concept ;
  dct:description "Andesite (Igneous rock)" ;
  ui:isMemberOf <coarse-fragments-lithology> ;
  rdfs:comment "C_LITHOLOGY" ;
  rdfs:label "Andesite" ;
  skos:definition "Andesite (Igneous rock)" ;
  skos:notation "AN" ;
  skos:prefLabel "Andesite" ;
  skos:topConceptOf <> ;
.
<coarse-fragments-lithology-AP>
  rdf:type skos:Concept ;
  dct:description "Aplite (Igneous rock)" ;
  ui:isMemberOf <coarse-fragments-lithology> ;
  rdfs:comment "C_LITHOLOGY" ;
  rdfs:label "Aplite" ;
  skos:definition "Aplite (Igneous rock)" ;
  skos:notation "AP" ;
  skos:prefLabel "Aplite" ;
  skos:topConceptOf <> ;
.
<coarse-fragments-lithology-AR>
  rdf:type skos:Concept ;
  dct:description "Arkose (Sedimentary rock, detrital)" ;
  ui:isMemberOf <coarse-fragments-lithology> ;
  rdfs:comment "C_LITHOLOGY" ;
  rdfs:label "Arkose" ;
  skos:definition "Arkose (Sedimentary rock, detrital)" ;
  skos:notation "AR" ;
  skos:prefLabel "Arkose" ;
  skos:topConceptOf <> ;
.
<coarse-fragments-lithology-AS>
  rdf:type skos:Concept ;
  dct:description "Ash (sandy)  (Unconsolidated material)" ;
  ui:isMemberOf <coarse-fragments-lithology> ;
  rdfs:comment "C_LITHOLOGY" ;
  rdfs:label "Ash (sandy)" ;
  skos:definition "Ash (sandy) (Unconsolidated material)" ;
  skos:notation "AS" ;
  skos:prefLabel "Ash (sandy)" ;
  skos:topConceptOf <> ;
.
<coarse-fragments-lithology-BA>
  rdf:type skos:Concept ;
  dct:description "Basalt (Igneous rock)" ;
  ui:isMemberOf <coarse-fragments-lithology> ;
  rdfs:comment "C_LITHOLOGY" ;
  rdfs:label "Basalt" ;
  skos:definition "Basalt (Igneous rock)" ;
  skos:notation "BA" ;
  skos:prefLabel "Basalt" ;
  skos:topConceptOf <> ;
.
<coarse-fragments-lithology-BB>
  rdf:type skos:Concept ;
  dct:description "Bombs (volcanic) (Unconsolidated material)" ;
  ui:isMemberOf <coarse-fragments-lithology> ;
  rdfs:comment "C_LITHOLOGY" ;
  rdfs:label "Bombs" ;
  skos:definition "Bombs (volcanic) (Unconsolidated material)" ;
  skos:notation "BB" ;
  skos:prefLabel "Bombs" ;
  skos:topConceptOf <> ;
.
<coarse-fragments-lithology-BR>
  rdf:type skos:Concept ;
  dct:description "Breccia (Sedimentary rock, detrital)" ;
  ui:isMemberOf <coarse-fragments-lithology> ;
  rdfs:comment "C_LITHOLOGY" ;
  rdfs:label "Breccia" ;
  skos:definition "Breccia (Sedimentary rock, detrital)" ;
  skos:notation "BR" ;
  skos:prefLabel "Breccia" ;
  skos:topConceptOf <> ;
.
<coarse-fragments-lithology-C>
  rdf:type skos:Concept ;
  dct:description "Clay (Unconsolidated material)" ;
  ui:isMemberOf <coarse-fragments-lithology> ;
  rdfs:comment "C_LITHOLOGY" ;
  rdfs:label "Clay" ;
  skos:definition "Clay (Unconsolidated material)" ;
  skos:notation "C" ;
  skos:prefLabel "Clay" ;
  skos:topConceptOf <> ;
.
<coarse-fragments-lithology-CC>
  rdf:type skos:Concept ;
  dct:description "Charcoal" ;
  ui:isMemberOf <coarse-fragments-lithology> ;
  rdfs:comment "C_LITHOLOGY" ;
  rdfs:label "Charcoal" ;
  skos:definition "Charcoal" ;
  skos:notation "CC" ;
  skos:prefLabel "Charcoal" ;
  skos:topConceptOf <> ;
.
<coarse-fragments-lithology-CG>
  rdf:type skos:Concept ;
  dct:description "Conglomerate (Sedimentary rock, detrital)" ;
  ui:isMemberOf <coarse-fragments-lithology> ;
  rdfs:comment "C_LITHOLOGY" ;
  rdfs:label "Conglomerate" ;
  skos:definition "Conglomerate (Sedimentary rock, detrital)" ;
  skos:notation "CG" ;
  skos:prefLabel "Conglomerate" ;
  skos:topConceptOf <> ;
.
<coarse-fragments-lithology-CH>
  rdf:type skos:Concept ;
  dct:description "Chert (Sedimentary rock, chemical or organic)" ;
  ui:isMemberOf <coarse-fragments-lithology> ;
  rdfs:comment "C_LITHOLOGY" ;
  rdfs:label "Chert" ;
  skos:definition "Chert (Sedimentary rock, chemical or organic)" ;
  skos:notation "CH" ;
  skos:prefLabel "Chert" ;
  skos:topConceptOf <> ;
.
<coarse-fragments-lithology-CO>
  rdf:type skos:Concept ;
  dct:description "Coal (Sedimentary rock, chemical or organic)" ;
  ui:isMemberOf <coarse-fragments-lithology> ;
  rdfs:comment "C_LITHOLOGY" ;
  rdfs:label "Coal" ;
  skos:definition "Coal (Sedimentary rock, chemical or organic)" ;
  skos:notation "CO" ;
  skos:prefLabel "Coal" ;
  skos:topConceptOf <> ;
.
<coarse-fragments-lithology-CU>
  rdf:type skos:Concept ;
  dct:description "Consolidated rock (Unidentified)" ;
  ui:isMemberOf <coarse-fragments-lithology> ;
  rdfs:comment "C_LITHOLOGY" ;
  rdfs:label "Consolidated rock" ;
  skos:definition "Consolidated rock (Unidentified)" ;
  skos:notation "CU" ;
  skos:prefLabel "Consolidated rock" ;
  skos:topConceptOf <> ;
.
<coarse-fragments-lithology-DI>
  rdf:type skos:Concept ;
  dct:description "Diorite (Igneous rock)" ;
  ui:isMemberOf <coarse-fragments-lithology> ;
  rdfs:comment "C_LITHOLOGY" ;
  rdfs:label "Diorite" ;
  skos:definition "Diorite (Igneous rock)" ;
  skos:notation "DI" ;
  skos:prefLabel "Diorite" ;
  skos:topConceptOf <> ;
.
<coarse-fragments-lithology-DM>
  rdf:type skos:Concept ;
  dct:description "Dolomite (Sedimentary rock, detrital)" ;
  ui:isMemberOf <coarse-fragments-lithology> ;
  rdfs:comment "C_LITHOLOGY" ;
  rdfs:label "Dolomite" ;
  skos:definition "Dolomite (Sedimentary rock, detrital)" ;
  skos:notation "DM" ;
  skos:prefLabel "Dolomite" ;
  skos:topConceptOf <> ;
.
<coarse-fragments-lithology-DR>
  rdf:type skos:Concept ;
  dct:description "Dolerite (Igneous rock)" ;
  ui:isMemberOf <coarse-fragments-lithology> ;
  rdfs:comment "C_LITHOLOGY" ;
  rdfs:label "Dolerite" ;
  skos:definition "Dolerite (Igneous rock)" ;
  skos:notation "DR" ;
  skos:prefLabel "Dolerite" ;
  skos:topConceptOf <> ;
.
<coarse-fragments-lithology-FC>
  rdf:type skos:Concept ;
  dct:description "Ferricrete (Sedimentary rock, chemical or organic)" ;
  ui:isMemberOf <coarse-fragments-lithology> ;
  rdfs:comment "C_LITHOLOGY" ;
  rdfs:label "Ferricrete" ;
  skos:definition "Ferricrete (Sedimentary rock, chemical or organic)" ;
  skos:notation "FC" ;
  skos:prefLabel "Ferricrete" ;
  skos:topConceptOf <> ;
.
<coarse-fragments-lithology-GA>
  rdf:type skos:Concept ;
  dct:description "Gabbro (Igneous rock)" ;
  ui:isMemberOf <coarse-fragments-lithology> ;
  rdfs:comment "C_LITHOLOGY" ;
  rdfs:label "Gabbro" ;
  skos:definition "Gabbro (Igneous rock)" ;
  skos:notation "GA" ;
  skos:prefLabel "Gabbro" ;
  skos:topConceptOf <> ;
.
<coarse-fragments-lithology-GD>
  rdf:type skos:Concept ;
  dct:description "Granodiorite (Igneous rock)" ;
  ui:isMemberOf <coarse-fragments-lithology> ;
  rdfs:comment "C_LITHOLOGY" ;
  rdfs:label "Granodiorite" ;
  skos:definition "Granodiorite (Igneous rock)" ;
  skos:notation "GD" ;
  skos:prefLabel "Granodiorite" ;
  skos:topConceptOf <> ;
.
<coarse-fragments-lithology-GE>
  rdf:type skos:Concept ;
  dct:description "Greenstone (Metamorphic rock)" ;
  ui:isMemberOf <coarse-fragments-lithology> ;
  rdfs:comment "C_LITHOLOGY" ;
  rdfs:label "Greenstone" ;
  skos:definition "Greenstone (Metamorphic rock)" ;
  skos:notation "GE" ;
  skos:prefLabel "Greenstone" ;
  skos:topConceptOf <> ;
.
<coarse-fragments-lithology-GN>
  rdf:type skos:Concept ;
  dct:description "Granite (Igneous rock)" ;
  ui:isMemberOf <coarse-fragments-lithology> ;
  rdfs:comment "C_LITHOLOGY" ;
  rdfs:label "Granite" ;
  skos:definition "Granite (Igneous rock)" ;
  skos:notation "GN" ;
  skos:prefLabel "Granite" ;
  skos:topConceptOf <> ;
.
<coarse-fragments-lithology-GR>
  rdf:type skos:Concept ;
  dct:description "Granulite (Metamorphic rock)" ;
  ui:isMemberOf <coarse-fragments-lithology> ;
  rdfs:comment "C_LITHOLOGY" ;
  rdfs:label "Granulite" ;
  skos:definition "Granulite (Metamorphic rock)" ;
  skos:notation "GR" ;
  skos:prefLabel "Granulite" ;
  skos:topConceptOf <> ;
.
<coarse-fragments-lithology-GS>
  rdf:type skos:Concept ;
  dct:description "Gneiss (Metamorphic rock)" ;
  ui:isMemberOf <coarse-fragments-lithology> ;
  rdfs:comment "C_LITHOLOGY" ;
  rdfs:label "Gneiss" ;
  skos:definition "Gneiss (Metamorphic rock)" ;
  skos:notation "GS" ;
  skos:prefLabel "Gneiss" ;
  skos:topConceptOf <> ;
.
<coarse-fragments-lithology-GV>
  rdf:type skos:Concept ;
  dct:description "Gravel (Unconsolidated material)" ;
  ui:isMemberOf <coarse-fragments-lithology> ;
  rdfs:comment "C_LITHOLOGY" ;
  rdfs:label "Gravel" ;
  skos:definition "Gravel (Unconsolidated material)" ;
  skos:notation "GV" ;
  skos:prefLabel "Gravel" ;
  skos:topConceptOf <> ;
.
<coarse-fragments-lithology-GW>
  rdf:type skos:Concept ;
  dct:description "Graywacke (Sedimentary rock, detrital)" ;
  ui:isMemberOf <coarse-fragments-lithology> ;
  rdfs:comment "C_LITHOLOGY" ;
  rdfs:label "Graywacke" ;
  skos:definition "Graywacke (Sedimentary rock, detrital)" ;
  skos:notation "GW" ;
  skos:prefLabel "Graywacke" ;
  skos:topConceptOf <> ;
.
<coarse-fragments-lithology-GY>
  rdf:type skos:Concept ;
  dct:description "Gypsum (Sedimentary rock, chemical or organic)" ;
  ui:isMemberOf <coarse-fragments-lithology> ;
  rdfs:comment "C_LITHOLOGY" ;
  rdfs:label "Gypsum" ;
  skos:definition "Gypsum (Sedimentary rock, chemical or organic)" ;
  skos:notation "GY" ;
  skos:prefLabel "Gypsum" ;
  skos:topConceptOf <> ;
.
<coarse-fragments-lithology-HA>
  rdf:type skos:Concept ;
  dct:description "Halite (Sedimentary rock, chemical or organic)" ;
  ui:isMemberOf <coarse-fragments-lithology> ;
  rdfs:comment "C_LITHOLOGY" ;
  rdfs:label "Halite" ;
  skos:definition "Halite (Sedimentary rock, chemical or organic)" ;
  skos:notation "HA" ;
  skos:prefLabel "Halite" ;
  skos:topConceptOf <> ;
.
<coarse-fragments-lithology-HO>
  rdf:type skos:Concept ;
  dct:description "Hornfels (Metamorphic rock)" ;
  ui:isMemberOf <coarse-fragments-lithology> ;
  rdfs:comment "C_LITHOLOGY" ;
  rdfs:label "Hornfels" ;
  skos:definition "Hornfels (Metamorphic rock)" ;
  skos:notation "HO" ;
  skos:prefLabel "Hornfels" ;
  skos:topConceptOf <> ;
.
<coarse-fragments-lithology-IG>
  rdf:type skos:Concept ;
  dct:description "Igneous rock (Unidentified)" ;
  ui:isMemberOf <coarse-fragments-lithology> ;
  rdfs:comment "C_LITHOLOGY" ;
  rdfs:label "Igneous rock" ;
  skos:definition "Igneous rock (Unidentified)" ;
  skos:notation "IG" ;
  skos:prefLabel "Igneous rock" ;
  skos:topConceptOf <> ;
.
<coarse-fragments-lithology-IS>
  rdf:type skos:Concept ;
  dct:description "Ironstone (where not considered of pedogenic origin)" ;
  ui:isMemberOf <coarse-fragments-lithology> ;
  rdfs:comment "C_LITHOLOGY" ;
  rdfs:label "Ironstone" ;
  skos:definition "Ironstone (where not considered of pedogenic origin)" ;
  skos:notation "IS" ;
  skos:prefLabel "Ironstone" ;
  skos:topConceptOf <> ;
.
<coarse-fragments-lithology-JA>
  rdf:type skos:Concept ;
  dct:description "Jasper (Sedimentary rock, chemical or organic)" ;
  ui:isMemberOf <coarse-fragments-lithology> ;
  rdfs:comment "C_LITHOLOGY" ;
  rdfs:label "Jasper" ;
  skos:definition "Jasper (Sedimentary rock, chemical or organic)" ;
  skos:notation "JA" ;
  skos:prefLabel "Jasper" ;
  skos:topConceptOf <> ;
.
<coarse-fragments-lithology-KA>
  rdf:type skos:Concept ;
  dct:description "Calcarenite (Sedimentary rock, detrital)" ;
  ui:isMemberOf <coarse-fragments-lithology> ;
  rdfs:comment "C_LITHOLOGY" ;
  rdfs:label "Calcarenite" ;
  skos:definition "Calcarenite (Sedimentary rock, detrital)" ;
  skos:notation "KA" ;
  skos:prefLabel "Calcarenite" ;
  skos:topConceptOf <> ;
.
<coarse-fragments-lithology-KC>
  rdf:type skos:Concept ;
  dct:description "Calcrete (Sedimentary rock, chemical or organic)" ;
  ui:isMemberOf <coarse-fragments-lithology> ;
  rdfs:comment "C_LITHOLOGY" ;
  rdfs:label "Calcrete" ;
  skos:definition "Calcrete (Sedimentary rock, chemical or organic)" ;
  skos:notation "KC" ;
  skos:prefLabel "Calcrete" ;
  skos:topConceptOf <> ;
.
<coarse-fragments-lithology-KL>
  rdf:type skos:Concept ;
  dct:description "Calcilutite (Sedimentary rock, detrital)" ;
  ui:isMemberOf <coarse-fragments-lithology> ;
  rdfs:comment "C_LITHOLOGY" ;
  rdfs:label "Calcilutite" ;
  skos:definition "Calcilutite (Sedimentary rock, detrital)" ;
  skos:notation "KL" ;
  skos:prefLabel "Calcilutite" ;
  skos:topConceptOf <> ;
.
<coarse-fragments-lithology-KM>
  rdf:type skos:Concept ;
  dct:description "Calcareous mudstone (Sedimentary rock, detrital)" ;
  ui:isMemberOf <coarse-fragments-lithology> ;
  rdfs:comment "C_LITHOLOGY" ;
  rdfs:label "Calcareous mudstone" ;
  skos:definition "Calcareous mudstone (Sedimentary rock, detrital)" ;
  skos:notation "KM" ;
  skos:prefLabel "Calcareous mudstone" ;
  skos:topConceptOf <> ;
.
<coarse-fragments-lithology-KR>
  rdf:type skos:Concept ;
  dct:description "Calcirudite (Sedimentary rock, detrital)" ;
  ui:isMemberOf <coarse-fragments-lithology> ;
  rdfs:comment "C_LITHOLOGY" ;
  rdfs:label "Calcirudite" ;
  skos:definition "Calcirudite (Sedimentary rock, detrital)" ;
  skos:notation "KR" ;
  skos:prefLabel "Calcirudite" ;
  skos:topConceptOf <> ;
.
<coarse-fragments-lithology-KS>
  rdf:type skos:Concept ;
  dct:description "Calcareous sand (Unconsolidated material)" ;
  ui:isMemberOf <coarse-fragments-lithology> ;
  rdfs:comment "C_LITHOLOGY" ;
  rdfs:label "Calcareous sand" ;
  skos:definition "Calcareous sand (Unconsolidated material)" ;
  skos:notation "KS" ;
  skos:prefLabel "Calcareous sand" ;
  skos:topConceptOf <> ;
.
<coarse-fragments-lithology-LC>
  rdf:type skos:Concept ;
  dct:description "Silcrete (Sedimentary rock, chemical or organic)" ;
  ui:isMemberOf <coarse-fragments-lithology> ;
  rdfs:comment "C_LITHOLOGY" ;
  rdfs:label "Silcrete" ;
  skos:definition "Silcrete (Sedimentary rock, chemical or organic)" ;
  skos:notation "LC" ;
  skos:prefLabel "Silcrete" ;
  skos:topConceptOf <> ;
.
<coarse-fragments-lithology-LI>
  rdf:type skos:Concept ;
  dct:description "Limestone (Sedimentary rock, detrital)" ;
  ui:isMemberOf <coarse-fragments-lithology> ;
  rdfs:comment "C_LITHOLOGY" ;
  rdfs:label "Limestone" ;
  skos:definition "Limestone (Sedimentary rock, detrital)" ;
  skos:notation "LI" ;
  skos:prefLabel "Limestone" ;
  skos:topConceptOf <> ;
.
<coarse-fragments-lithology-M>
  rdf:type skos:Concept ;
  dct:description "Lithology is same as the substrate material" ;
  ui:isMemberOf <coarse-fragments-lithology> ;
  rdfs:comment "C_LITHOLOGY" ;
  rdfs:label "Same as substrate material" ;
  skos:definition "Lithology is same as the substrate material" ;
  skos:notation "M" ;
  skos:prefLabel "Same as substrate material" ;
  skos:topConceptOf <> ;
.
<coarse-fragments-lithology-MB>
  rdf:type skos:Concept ;
  dct:description "Marble (Metamorphic rock)" ;
  ui:isMemberOf <coarse-fragments-lithology> ;
  rdfs:comment "C_LITHOLOGY" ;
  rdfs:label "Marble" ;
  skos:definition "Marble (Metamorphic rock)" ;
  skos:notation "MB" ;
  skos:prefLabel "Marble" ;
  skos:topConceptOf <> ;
.
<coarse-fragments-lithology-MD>
  rdf:type skos:Concept ;
  dct:description "Microdiorite (Igneous rock)" ;
  ui:isMemberOf <coarse-fragments-lithology> ;
  rdfs:comment "C_LITHOLOGY" ;
  rdfs:label "Microdiorite" ;
  skos:definition "Microdiorite (Igneous rock)" ;
  skos:notation "MD" ;
  skos:prefLabel "Microdiorite" ;
  skos:topConceptOf <> ;
.
<coarse-fragments-lithology-ME>
  rdf:type skos:Concept ;
  dct:description "Metamorphic rock (Unidentified)" ;
  ui:isMemberOf <coarse-fragments-lithology> ;
  rdfs:comment "C_LITHOLOGY" ;
  rdfs:label "Metamorphic rock" ;
  skos:definition "Metamorphic rock (Unidentified)" ;
  skos:notation "ME" ;
  skos:prefLabel "Metamorphic rock" ;
  skos:topConceptOf <> ;
.
<coarse-fragments-lithology-MG>
  rdf:type skos:Concept ;
  dct:description "Microgranite (Igneous rock)" ;
  ui:isMemberOf <coarse-fragments-lithology> ;
  rdfs:comment "C_LITHOLOGY" ;
  rdfs:label "Microgranite" ;
  skos:definition "Microgranite (Igneous rock)" ;
  skos:notation "MG" ;
  skos:prefLabel "Microgranite" ;
  skos:topConceptOf <> ;
.
<coarse-fragments-lithology-MI>
  rdf:type skos:Concept ;
  dct:description "Migmatite (Metamorphic rock)" ;
  ui:isMemberOf <coarse-fragments-lithology> ;
  rdfs:comment "C_LITHOLOGY" ;
  rdfs:label "Migmatite" ;
  skos:definition "Migmatite (Metamorphic rock)" ;
  skos:notation "MI" ;
  skos:prefLabel "Migmatite" ;
  skos:topConceptOf <> ;
.
<coarse-fragments-lithology-ML>
  rdf:type skos:Concept ;
  dct:description "Marl (Unconsolidated material)" ;
  ui:isMemberOf <coarse-fragments-lithology> ;
  rdfs:comment "C_LITHOLOGY" ;
  rdfs:label "Marl" ;
  skos:definition "Marl (Unconsolidated material)" ;
  skos:notation "ML" ;
  skos:prefLabel "Marl" ;
  skos:topConceptOf <> ;
.
<coarse-fragments-lithology-MS>
  rdf:type skos:Concept ;
  dct:description "Microsyenite (Igneous rock)" ;
  ui:isMemberOf <coarse-fragments-lithology> ;
  rdfs:comment "C_LITHOLOGY" ;
  rdfs:label "Microsyenite" ;
  skos:definition "Microsyenite (Igneous rock)" ;
  skos:notation "MS" ;
  skos:prefLabel "Microsyenite" ;
  skos:topConceptOf <> ;
.
<coarse-fragments-lithology-MU>
  rdf:type skos:Concept ;
  dct:description "Mudstone (Sedimentary rock, detrital)" ;
  ui:isMemberOf <coarse-fragments-lithology> ;
  rdfs:comment "C_LITHOLOGY" ;
  rdfs:label "Mudstone" ;
  skos:definition "Mudstone (Sedimentary rock, detrital)" ;
  skos:notation "MU" ;
  skos:prefLabel "Mudstone" ;
  skos:topConceptOf <> ;
.
<coarse-fragments-lithology-MY>
  rdf:type skos:Concept ;
  dct:description "Mylonite (Metamorphic rock)" ;
  ui:isMemberOf <coarse-fragments-lithology> ;
  rdfs:comment "C_LITHOLOGY" ;
  rdfs:label "Mylonite" ;
  skos:definition "Mylonite (Metamorphic rock)" ;
  skos:notation "MY" ;
  skos:prefLabel "Mylonite" ;
  skos:topConceptOf <> ;
.
<coarse-fragments-lithology-OT>
  rdf:type skos:Concept ;
  dct:description "Other" ;
  ui:isMemberOf <coarse-fragments-lithology> ;
  rdfs:comment "C_LITHOLOGY" ;
  rdfs:label "Other" ;
  skos:definition "Other" ;
  skos:notation "OT" ;
  skos:prefLabel "Other" ;
  skos:topConceptOf <> ;
.
<coarse-fragments-lithology-OW>
  rdf:type skos:Concept ;
  dct:description "Opalised wood" ;
  ui:isMemberOf <coarse-fragments-lithology> ;
  rdfs:comment "C_LITHOLOGY" ;
  rdfs:label "Opalised wood" ;
  skos:definition "Opalised wood" ;
  skos:notation "OW" ;
  skos:prefLabel "Opalised wood" ;
  skos:topConceptOf <> ;
.
<coarse-fragments-lithology-PC>
  rdf:type skos:Concept ;
  dct:description "Porcellanite (Sedimentary rock, chemical or organic)" ;
  ui:isMemberOf <coarse-fragments-lithology> ;
  rdfs:comment "C_LITHOLOGY" ;
  rdfs:label "Porcellanite" ;
  skos:definition "Porcellanite (Sedimentary rock, chemical or organic)" ;
  skos:notation "PC" ;
  skos:prefLabel "Porcellanite" ;
  skos:topConceptOf <> ;
.
<coarse-fragments-lithology-PE>
  rdf:type skos:Concept ;
  dct:description "Peridotite (Igneous rock)" ;
  ui:isMemberOf <coarse-fragments-lithology> ;
  rdfs:comment "C_LITHOLOGY" ;
  rdfs:label "Peridotite" ;
  skos:definition "Peridotite (Igneous rock)" ;
  skos:notation "PE" ;
  skos:prefLabel "Peridotite" ;
  skos:topConceptOf <> ;
.
<coarse-fragments-lithology-PG>
  rdf:type skos:Concept ;
  dct:description "Pegmatite (Igneous rock)" ;
  ui:isMemberOf <coarse-fragments-lithology> ;
  rdfs:comment "C_LITHOLOGY" ;
  rdfs:label "Pegmatite" ;
  skos:definition "Pegmatite (Igneous rock)" ;
  skos:notation "PG" ;
  skos:prefLabel "Pegmatite" ;
  skos:topConceptOf <> ;
.
<coarse-fragments-lithology-PH>
  rdf:type skos:Concept ;
  dct:description "Phyllite (Metamorphic rock)" ;
  ui:isMemberOf <coarse-fragments-lithology> ;
  rdfs:comment "C_LITHOLOGY" ;
  rdfs:label "Phyllite" ;
  skos:definition "Phyllite (Metamorphic rock)" ;
  skos:notation "PH" ;
  skos:prefLabel "Phyllite" ;
  skos:topConceptOf <> ;
.
<coarse-fragments-lithology-PL>
  rdf:type skos:Concept ;
  dct:description "Phonolite (Igneous rock)" ;
  ui:isMemberOf <coarse-fragments-lithology> ;
  rdfs:comment "C_LITHOLOGY" ;
  rdfs:label "Phonolite" ;
  skos:definition "Phonolite (Igneous rock)" ;
  skos:notation "PL" ;
  skos:prefLabel "Phonolite" ;
  skos:topConceptOf <> ;
.
<coarse-fragments-lithology-PO>
  rdf:type skos:Concept ;
  dct:description "Porphyry (Igneous rock)" ;
  ui:isMemberOf <coarse-fragments-lithology> ;
  rdfs:comment "C_LITHOLOGY" ;
  rdfs:label "Porphyry" ;
  skos:definition "Porphyry (Igneous rock)" ;
  skos:notation "PO" ;
  skos:prefLabel "Porphyry" ;
  skos:topConceptOf <> ;
.
<coarse-fragments-lithology-PU>
  rdf:type skos:Concept ;
  dct:description "Pumice" ;
  ui:isMemberOf <coarse-fragments-lithology> ;
  rdfs:comment "C_LITHOLOGY" ;
  rdfs:label "Pumice" ;
  skos:definition "Pumice" ;
  skos:notation "PU" ;
  skos:prefLabel "Pumice" ;
  skos:topConceptOf <> ;
.
<coarse-fragments-lithology-PY>
  rdf:type skos:Concept ;
  dct:description "Pyroxenite (Igneous rock)" ;
  ui:isMemberOf <coarse-fragments-lithology> ;
  rdfs:comment "C_LITHOLOGY" ;
  rdfs:label "Pyroxenite" ;
  skos:definition "Pyroxenite (Igneous rock)" ;
  skos:notation "PY" ;
  skos:prefLabel "Pyroxenite" ;
  skos:topConceptOf <> ;
.
<coarse-fragments-lithology-QP>
  rdf:type skos:Concept ;
  dct:description "Quartz porphyry (Igneous rock)" ;
  ui:isMemberOf <coarse-fragments-lithology> ;
  rdfs:comment "C_LITHOLOGY" ;
  rdfs:label "Quartz porphyry" ;
  skos:definition "Quartz porphyry (Igneous rock)" ;
  skos:notation "QP" ;
  skos:prefLabel "Quartz porphyry" ;
  skos:topConceptOf <> ;
.
<coarse-fragments-lithology-QS>
  rdf:type skos:Concept ;
  dct:description "Quartz sandstone (Sedimentary rock, detrital)" ;
  ui:isMemberOf <coarse-fragments-lithology> ;
  rdfs:comment "C_LITHOLOGY" ;
  rdfs:label "Quartz sandstone" ;
  skos:definition "Quartz sandstone (Sedimentary rock, detrital)" ;
  skos:notation "QS" ;
  skos:prefLabel "Quartz sandstone" ;
  skos:topConceptOf <> ;
.
<coarse-fragments-lithology-QU>
  rdf:type skos:Concept ;
  dct:description "Quartzite (Metamorphic rock)" ;
  ui:isMemberOf <coarse-fragments-lithology> ;
  rdfs:comment "C_LITHOLOGY" ;
  rdfs:label "Quartzite" ;
  skos:definition "Quartzite (Metamorphic rock)" ;
  skos:notation "QU" ;
  skos:prefLabel "Quartzite" ;
  skos:topConceptOf <> ;
.
<coarse-fragments-lithology-QZ>
  rdf:type skos:Concept ;
  dct:description "Quartz (Igneous rock)" ;
  ui:isMemberOf <coarse-fragments-lithology> ;
  rdfs:comment "C_LITHOLOGY" ;
  rdfs:label "Quartz" ;
  skos:definition "Quartz (Igneous rock)" ;
  skos:notation "QZ" ;
  skos:prefLabel "Quartz" ;
  skos:topConceptOf <> ;
.
<coarse-fragments-lithology-R>
  rdf:type skos:Concept ;
  dct:description "Lithology is same as the rock outcrop" ;
  ui:isMemberOf <coarse-fragments-lithology> ;
  rdfs:comment "C_LITHOLOGY" ;
  rdfs:label "Same as rock outcrop" ;
  skos:definition "Lithology is same as the rock outcrop" ;
  skos:notation "R" ;
  skos:prefLabel "Same as rock outcrop" ;
  skos:topConceptOf <> ;
.
<coarse-fragments-lithology-RB>
  rdf:type skos:Concept ;
  dct:description "Red-brown hardpan (Sedimentary rock, chemical or organic)" ;
  ui:isMemberOf <coarse-fragments-lithology> ;
  rdfs:comment "C_LITHOLOGY" ;
  rdfs:label "Red-brown hardpan" ;
  skos:definition "Red-brown hardpan (Sedimentary rock, chemical or organic)" ;
  skos:notation "RB" ;
  skos:prefLabel "Red-brown hardpan" ;
  skos:topConceptOf <> ;
.
<coarse-fragments-lithology-RH>
  rdf:type skos:Concept ;
  dct:description "Rhyolite (Igneous rock)" ;
  ui:isMemberOf <coarse-fragments-lithology> ;
  rdfs:comment "C_LITHOLOGY" ;
  rdfs:label "Rhyolite" ;
  skos:definition "Rhyolite (Igneous rock)" ;
  skos:notation "RH" ;
  skos:prefLabel "Rhyolite" ;
  skos:topConceptOf <> ;
.
<coarse-fragments-lithology-S>
  rdf:type skos:Concept ;
  dct:description "Sand (Unconsolidated material)" ;
  ui:isMemberOf <coarse-fragments-lithology> ;
  rdfs:comment "C_LITHOLOGY" ;
  rdfs:label "Sand" ;
  skos:definition "Sand (Unconsolidated material)" ;
  skos:notation "S" ;
  skos:prefLabel "Sand" ;
  skos:topConceptOf <> ;
.
<coarse-fragments-lithology-SA>
  rdf:type skos:Concept ;
  dct:description "Sandstone (Sedimentary rock, detrital)" ;
  ui:isMemberOf <coarse-fragments-lithology> ;
  rdfs:comment "C_LITHOLOGY" ;
  rdfs:label "Sandstone" ;
  skos:definition "Sandstone (Sedimentary rock, detrital)" ;
  skos:notation "SA" ;
  skos:prefLabel "Sandstone" ;
  skos:topConceptOf <> ;
.
<coarse-fragments-lithology-SD>
  rdf:type skos:Concept ;
  dct:description "Detrital sedimentary rock (Unidentified)" ;
  ui:isMemberOf <coarse-fragments-lithology> ;
  rdfs:comment "C_LITHOLOGY" ;
  rdfs:label "Detrital sedimentary rock" ;
  skos:definition "Detrital sedimentary rock (Unidentified)" ;
  skos:notation "SD" ;
  skos:prefLabel "Detrital sedimentary rock" ;
  skos:topConceptOf <> ;
.
<coarse-fragments-lithology-SH>
  rdf:type skos:Concept ;
  dct:description "Shale (Igneous rock)" ;
  ui:isMemberOf <coarse-fragments-lithology> ;
  rdfs:comment "C_LITHOLOGY" ;
  rdfs:label "Shale" ;
  skos:definition "Shale (Igneous rock)" ;
  skos:notation "SH" ;
  skos:prefLabel "Shale" ;
  skos:topConceptOf <> ;
.
<coarse-fragments-lithology-SK>
  rdf:type skos:Concept ;
  dct:description "Scoria (Unconsolidated material)" ;
  ui:isMemberOf <coarse-fragments-lithology> ;
  rdfs:comment "C_LITHOLOGY" ;
  rdfs:label "Scoria" ;
  skos:definition "Scoria (Unconsolidated material)" ;
  skos:notation "SK" ;
  skos:prefLabel "Scoria" ;
  skos:topConceptOf <> ;
.
<coarse-fragments-lithology-SL>
  rdf:type skos:Concept ;
  dct:description "Slate (Sedimentary rock, detrital)" ;
  ui:isMemberOf <coarse-fragments-lithology> ;
  rdfs:comment "C_LITHOLOGY" ;
  rdfs:label "Slate" ;
  skos:definition "Slate (Sedimentary rock, detrital)" ;
  skos:notation "SL" ;
  skos:prefLabel "Slate" ;
  skos:topConceptOf <> ;
.
<coarse-fragments-lithology-SR>
  rdf:type skos:Concept ;
  dct:description "Serpentinite (Igneous rock)" ;
  ui:isMemberOf <coarse-fragments-lithology> ;
  rdfs:comment "C_LITHOLOGY" ;
  rdfs:label "Serpentinite" ;
  skos:definition "Serpentinite (Igneous rock)" ;
  skos:notation "SR" ;
  skos:prefLabel "Serpentinite" ;
  skos:topConceptOf <> ;
.
<coarse-fragments-lithology-SS>
  rdf:type skos:Concept ;
  dct:description "Shells" ;
  ui:isMemberOf <coarse-fragments-lithology> ;
  rdfs:comment "C_LITHOLOGY" ;
  rdfs:label "Shells" ;
  skos:definition "Shells" ;
  skos:notation "SS" ;
  skos:prefLabel "Shells" ;
  skos:topConceptOf <> ;
.
<coarse-fragments-lithology-ST>
  rdf:type skos:Concept ;
  dct:description "Schist (Metamorphic rock)" ;
  ui:isMemberOf <coarse-fragments-lithology> ;
  rdfs:comment "C_LITHOLOGY" ;
  rdfs:label "Schist" ;
  skos:definition "Schist (Metamorphic rock)" ;
  skos:notation "ST" ;
  skos:prefLabel "Schist" ;
  skos:topConceptOf <> ;
.
<coarse-fragments-lithology-SY>
  rdf:type skos:Concept ;
  dct:description "Syenite (Metamorphic rock)" ;
  ui:isMemberOf <coarse-fragments-lithology> ;
  rdfs:comment "C_LITHOLOGY" ;
  rdfs:label "Syenite" ;
  skos:definition "Syenite (Metamorphic rock)" ;
  skos:notation "SY" ;
  skos:prefLabel "Syenite" ;
  skos:topConceptOf <> ;
.
<coarse-fragments-lithology-TR>
  rdf:type skos:Concept ;
  dct:description "Trachyte (Igneous rock)" ;
  ui:isMemberOf <coarse-fragments-lithology> ;
  rdfs:comment "C_LITHOLOGY" ;
  rdfs:label "Trachyte" ;
  skos:definition "Trachyte (Igneous rock)" ;
  skos:notation "TR" ;
  skos:prefLabel "Trachyte" ;
  skos:topConceptOf <> ;
.
<coarse-fragments-lithology-TU>
  rdf:type skos:Concept ;
  dct:description "Tuff (Igneous rock)" ;
  ui:isMemberOf <coarse-fragments-lithology> ;
  rdfs:comment "C_LITHOLOGY" ;
  rdfs:label "Tuff" ;
  skos:definition "Tuff (Igneous rock)" ;
  skos:notation "TU" ;
  skos:prefLabel "Tuff" ;
  skos:topConceptOf <> ;
.
<coarse-fragments-lithology-UC>
  rdf:type skos:Concept ;
  dct:description "Unconsolidated material (Unidentified)" ;
  ui:isMemberOf <coarse-fragments-lithology> ;
  rdfs:comment "C_LITHOLOGY" ;
  rdfs:label "Unconsolidated material" ;
  skos:definition "Unconsolidated material (Unidentified)" ;
  skos:notation "UC" ;
  skos:prefLabel "Unconsolidated material" ;
  skos:topConceptOf <> ;
.
<coarse-fragments-lithology-VB>
  rdf:type skos:Concept ;
  dct:description "Volcanic breccia (Sedimentary rock, pyroclastic)" ;
  ui:isMemberOf <coarse-fragments-lithology> ;
  rdfs:comment "C_LITHOLOGY" ;
  rdfs:label "Volcanic breccia" ;
  skos:definition "Volcanic breccia (Sedimentary rock, pyroclastic)" ;
  skos:notation "VB" ;
  skos:prefLabel "Volcanic breccia" ;
  skos:topConceptOf <> ;
.
<coarse-fragments-lithology-VG>
  rdf:type skos:Concept ;
  dct:description "Volcanic glass (Igneous rock)" ;
  ui:isMemberOf <coarse-fragments-lithology> ;
  rdfs:comment "C_LITHOLOGY" ;
  rdfs:label "Volcanic glass" ;
  skos:definition "Volcanic glass (Igneous rock)" ;
  skos:notation "VG" ;
  skos:prefLabel "Volcanic glass" ;
  skos:topConceptOf <> ;
.
<coarse-fragments-lithology-Z>
  rdf:type skos:Concept ;
  dct:description "Silt (Sedimentary rock, detrital)" ;
  ui:isMemberOf <coarse-fragments-lithology> ;
  rdfs:comment "C_LITHOLOGY" ;
  rdfs:label "Silt" ;
  skos:definition "Silt (Sedimentary rock, detrital)" ;
  skos:notation "Z" ;
  skos:prefLabel "Silt" ;
  skos:topConceptOf <> ;
.
<coarse-fragments-lithology-ZS>
  rdf:type skos:Concept ;
  dct:description "Siltstone (Unconsolidated material)" ;
  ui:isMemberOf <coarse-fragments-lithology> ;
  rdfs:comment "C_LITHOLOGY" ;
  rdfs:label "Siltstone" ;
  skos:definition "Siltstone (Unconsolidated material)" ;
  skos:notation "ZS" ;
  skos:prefLabel "Siltstone" ;
  skos:topConceptOf <> ;
.
<coarse-fragments-shape>
  rdf:type skos:Collection ;
  dct:description "The shape of coarse fragments is determined by referencing a chart that captures the roundness and sphericity." ;
  ui:isMemberOf <coarse-fragments> ;
  rdfs:comment "C_CF_SHAPE" ;
  rdfs:label "Shape of coarse fragments" ;
  skos:definition "The shape of coarse fragments is determined by referencing a chart that captures the roundness and sphericity." ;
  skos:member <coarse-fragments-shape-A> ;
  skos:member <coarse-fragments-shape-AP> ;
  skos:member <coarse-fragments-shape-AT> ;
  skos:member <coarse-fragments-shape-R> ;
  skos:member <coarse-fragments-shape-RP> ;
  skos:member <coarse-fragments-shape-RT> ;
  skos:member <coarse-fragments-shape-S> ;
  skos:member <coarse-fragments-shape-SP> ;
  skos:member <coarse-fragments-shape-ST> ;
  skos:member <coarse-fragments-shape-U> ;
  skos:member <coarse-fragments-shape-UP> ;
  skos:member <coarse-fragments-shape-UT> ;
  skos:prefLabel "Shape of coarse fragments" ;
.
<coarse-fragments-shape-A>
  rdf:type skos:Concept ;
  dct:description "Angular shape as determined from visual guide" ;
  ui:isMemberOf <coarse-fragments-shape> ;
  rdfs:comment "C_CF_SHAPE" ;
  rdfs:label "Angular" ;
  skos:definition "Angular shape as determined from visual guide" ;
  skos:notation "A" ;
  skos:prefLabel "Angular" ;
  skos:topConceptOf <> ;
.
<coarse-fragments-shape-AP>
  rdf:type skos:Concept ;
  dct:description "Angular shape as determined from visual guide" ;
  ui:isMemberOf <coarse-fragments-shape> ;
  rdfs:comment "C_CF_SHAPE" ;
  rdfs:label "Angular platy" ;
  skos:definition "Angular platy shape as determined from visual guide" ;
  skos:notation "AP" ;
  skos:prefLabel "Angular platy" ;
  skos:topConceptOf <> ;
.
<coarse-fragments-shape-AT>
  rdf:type skos:Concept ;
  dct:description "Angular tabular shape as determined from visual guide" ;
  ui:isMemberOf <coarse-fragments-shape> ;
  rdfs:comment "C_CF_SHAPE" ;
  rdfs:label "Angular tabular" ;
  skos:definition "Angular tabular shape as determined from visual guide" ;
  skos:notation "AT" ;
  skos:prefLabel "Angular tabular" ;
  skos:topConceptOf <> ;
.
<coarse-fragments-shape-R>
  rdf:type skos:Concept ;
  dct:description "Rounded shape as determined from visual guide" ;
  ui:isMemberOf <coarse-fragments-shape> ;
  rdfs:comment "C_CF_SHAPE" ;
  rdfs:label "Rounded" ;
  skos:definition "Rounded shape as determined from visual guide" ;
  skos:notation "R" ;
  skos:prefLabel "Rounded" ;
  skos:topConceptOf <> ;
.
<coarse-fragments-shape-RP>
  rdf:type skos:Concept ;
  dct:description "Rounded platy shape as determined from visual guide" ;
  ui:isMemberOf <coarse-fragments-shape> ;
  rdfs:comment "C_CF_SHAPE" ;
  rdfs:label "Rounded platy" ;
  skos:definition "Rounded platy shape as determined from visual guide" ;
  skos:notation "RP" ;
  skos:prefLabel "Rounded platy" ;
  skos:topConceptOf <> ;
.
<coarse-fragments-shape-RT>
  rdf:type skos:Concept ;
  dct:description "Rounded tabular shape as determined from visual guide" ;
  ui:isMemberOf <coarse-fragments-shape> ;
  rdfs:comment "C_CF_SHAPE" ;
  rdfs:label "Rounded tabular" ;
  skos:definition "Rounded tabular shape as determined from visual guide" ;
  skos:notation "RT" ;
  skos:prefLabel "Rounded tabular" ;
  skos:topConceptOf <> ;
.
<coarse-fragments-shape-S>
  rdf:type skos:Concept ;
  dct:description "Subangular shape as determined from visual guide" ;
  ui:isMemberOf <coarse-fragments-shape> ;
  rdfs:comment "C_CF_SHAPE" ;
  rdfs:label "Subangular" ;
  skos:definition "Subangular shape as determined from visual guide" ;
  skos:notation "S" ;
  skos:prefLabel "Subangular" ;
  skos:topConceptOf <> ;
.
<coarse-fragments-shape-SP>
  rdf:type skos:Concept ;
  dct:description "Subangular platy shape as determined from visual guide" ;
  ui:isMemberOf <coarse-fragments-shape> ;
  rdfs:comment "C_CF_SHAPE" ;
  rdfs:label "Subangular platy" ;
  skos:definition "Subangular platy shape as determined from visual guide" ;
  skos:notation "SP" ;
  skos:prefLabel "Subangular platy" ;
  skos:topConceptOf <> ;
.
<coarse-fragments-shape-ST>
  rdf:type skos:Concept ;
  dct:description "Subangular tabular shape as determined from visual guide" ;
  ui:isMemberOf <coarse-fragments-shape> ;
  rdfs:comment "C_CF_SHAPE" ;
  rdfs:label "Subangular tabular" ;
  skos:definition "Subangular tabular shape as determined from visual guide" ;
  skos:notation "ST" ;
  skos:prefLabel "Subangular tabular" ;
  skos:topConceptOf <> ;
.
<coarse-fragments-shape-U>
  rdf:type skos:Concept ;
  dct:description "Subrounded shape as determined from visual guide" ;
  ui:isMemberOf <coarse-fragments-shape> ;
  rdfs:comment "C_CF_SHAPE" ;
  rdfs:label "Subrounded" ;
  skos:definition "Subrounded shape as determined from visual guide" ;
  skos:notation "U" ;
  skos:prefLabel "Subrounded" ;
  skos:topConceptOf <> ;
.
<coarse-fragments-shape-UP>
  rdf:type skos:Concept ;
  dct:description "Subrounded platy shape as determined from visual guide" ;
  ui:isMemberOf <coarse-fragments-shape> ;
  rdfs:comment "C_CF_SHAPE" ;
  rdfs:label "Subrounded platy" ;
  skos:definition "Subrounded platy shape as determined from visual guide" ;
  skos:notation "UP" ;
  skos:prefLabel "Subrounded platy" ;
  skos:topConceptOf <> ;
.
<coarse-fragments-shape-UT>
  rdf:type skos:Concept ;
  dct:description "Subrounded tabular shape as determined from visual guide" ;
  ui:isMemberOf <coarse-fragments-shape> ;
  rdfs:comment "C_CF_SHAPE" ;
  rdfs:label "Subrounded tabular" ;
  skos:definition "Subrounded tabular shape as determined from visual guide" ;
  skos:notation "UT" ;
  skos:prefLabel "Subrounded tabular" ;
  skos:topConceptOf <> ;
.
<coarse-fragments-size>
  rdf:type skos:Collection ;
  dct:description "The scale adopted employs class boundaries at (2 × 10n/2) mm, where n is an integer. This system is an extension of that used for particles smaller than 2 mm both in the scheme of the British Standards Institution and the Massachusetts Institute of Technology  and the original Atterberg (1905) scheme on which the International Scheme was based. It is thus compatible with both the International Scheme referred to in the field texture section and the grain size criteria for substrate materials." ;
  ui:isMemberOf <coarse-fragments> ;
  rdfs:comment "N_CF_SIZE: The terms used to describe size apply to fragments of any shape: The average maximum dimension of fragments is used to determine the class interval. " ;
  rdfs:label "Size of coarse fragments" ;
  skos:definition "The scale adopted employs class boundaries at (2 × 10n/2) mm, where n is an integer. This system is an extension of that used for particles smaller than 2 mm both in the scheme of the British Standards Institution and the Massachusetts Institute of Technology  and the original Atterberg (1905) scheme on which the International Scheme was based. It is thus compatible with both the International Scheme referred to in the field texture section and the grain size criteria for substrate materials." ;
  skos:member <coarse-fragments-size-1> ;
  skos:member <coarse-fragments-size-2> ;
  skos:member <coarse-fragments-size-3> ;
  skos:member <coarse-fragments-size-4> ;
  skos:member <coarse-fragments-size-5> ;
  skos:member <coarse-fragments-size-6> ;
  skos:member <coarse-fragments-size-7> ;
  skos:prefLabel "Size of coarse fragments" ;
.
<coarse-fragments-size-1>
  rdf:type skos:Concept ;
  dct:description "2-6 mm" ;
  ui:isMemberOf <coarse-fragments-size> ;
  rdfs:comment "N_CF_SIZE: The terms used to describe size apply to fragments of any shape: The average maximum dimension of fragments is used to determine the class interval. " ;
  rdfs:label "Fine gravelly or small pebbles" ;
  skos:definition "2-6 mm" ;
  skos:notation "1" ;
  skos:prefLabel "Fine gravelly or small pebbles" ;
  skos:topConceptOf <> ;
.
<coarse-fragments-size-2>
  rdf:type skos:Concept ;
  dct:description "6-20 mm" ;
  ui:isMemberOf <coarse-fragments-size> ;
  rdfs:comment "N_CF_SIZE: The terms used to describe size apply to fragments of any shape: The average maximum dimension of fragments is used to determine the class interval. " ;
  rdfs:label "Medium gravelly or medium pebbles" ;
  skos:definition "6-20 mm" ;
  skos:notation "2" ;
  skos:prefLabel "Medium gravelly or medium pebbles" ;
  skos:topConceptOf <> ;
.
<coarse-fragments-size-3>
  rdf:type skos:Concept ;
  dct:description "20-60 mm" ;
  ui:isMemberOf <coarse-fragments-size> ;
  rdfs:comment "N_CF_SIZE: The terms used to describe size apply to fragments of any shape: The average maximum dimension of fragments is used to determine the class interval. " ;
  rdfs:label "Coarse gravelly or large pebbles" ;
  skos:definition "20-60 mm" ;
  skos:notation "3" ;
  skos:prefLabel "Coarse gravelly or large pebbles" ;
  skos:topConceptOf <> ;
.
<coarse-fragments-size-4>
  rdf:type skos:Concept ;
  dct:description "60-200 mm" ;
  ui:isMemberOf <coarse-fragments-size> ;
  rdfs:comment "N_CF_SIZE: The terms used to describe size apply to fragments of any shape: The average maximum dimension of fragments is used to determine the class interval. " ;
  rdfs:label "Cobbly or cobbles" ;
  skos:definition "60-200 mm" ;
  skos:notation "4" ;
  skos:prefLabel "Cobbly or cobbles" ;
  skos:topConceptOf <> ;
.
<coarse-fragments-size-5>
  rdf:type skos:Concept ;
  dct:description "200-600 mm" ;
  ui:isMemberOf <coarse-fragments-size> ;
  rdfs:comment "N_CF_SIZE: The terms used to describe size apply to fragments of any shape: The average maximum dimension of fragments is used to determine the class interval. " ;
  rdfs:label "Stony or stones" ;
  skos:definition "200-600 mm" ;
  skos:notation "5" ;
  skos:prefLabel "Stony or stones" ;
  skos:topConceptOf <> ;
.
<coarse-fragments-size-6>
  rdf:type skos:Concept ;
  dct:description "600-2000 mm" ;
  ui:isMemberOf <coarse-fragments-size> ;
  rdfs:comment "N_CF_SIZE: The terms used to describe size apply to fragments of any shape: The average maximum dimension of fragments is used to determine the class interval. " ;
  rdfs:label "Bouldery or boulders" ;
  skos:definition "600-2000 mm" ;
  skos:notation "6" ;
  skos:prefLabel "Bouldery or boulders" ;
  skos:topConceptOf <> ;
.
<coarse-fragments-size-7>
  rdf:type skos:Concept ;
  dct:description ">2000 mm" ;
  ui:isMemberOf <coarse-fragments-size> ;
  rdfs:comment "N_CF_SIZE: The terms used to describe size apply to fragments of any shape: The average maximum dimension of fragments is used to determine the class interval. " ;
  rdfs:label "Large boulders" ;
  skos:definition ">2000 mm" ;
  skos:notation "7" ;
  skos:prefLabel "Large boulders" ;
  skos:topConceptOf <> ;
.
<coarse-fragments-strength>
  rdf:type skos:Collection ;
  dct:description "The strength of a specimen of soil substrate material may be crudely estimated in the field by striking it with the head-end or the pick-end of a geological hammer or by trying to cut it with a knife, and then referring to Table 32 (ASLS Field Handbook). These estimates refer to the unconfined (or uniaxial) compressive strength. The strength is that of the intact material rather than that of the mass, the strength of which has generally been reduced by the development of fractures and other phenomena." ;
  ui:isMemberOf <coarse-fragments> ;
  rdfs:comment "C_CF_STRENGTH" ;
  rdfs:label "Strength of coarse fragments" ;
  skos:definition "The strength of a specimen of soil substrate material may be crudely estimated in the field by striking it with the head-end or the pick-end of a geological hammer or by trying to cut it with a knife, and then referring to Table 32 (ASLS Field Handbook). These estimates refer to the unconfined (or uniaxial) compressive strength. The strength is that of the intact material rather than that of the mass, the strength of which has generally been reduced by the development of fractures and other phenomena." ;
  skos:member <coarse-fragments-strength-M> ;
  skos:member <coarse-fragments-strength-S> ;
  skos:member <coarse-fragments-strength-VS> ;
  skos:member <coarse-fragments-strength-VW> ;
  skos:member <coarse-fragments-strength-W> ;
  skos:note "These will be exact match to material strength in substrate chapter" ;
  skos:prefLabel "Strength of coarse fragments" ;
.
<coarse-fragments-strength-M>
  rdf:type skos:Concept ;
  dct:description "50-100 MPa based on field estimate of strength class after striking or cutting the rock material - Knife:Nil or slight mark, Pick:indents shallowly, Hammer (single blow):Breaks readily into a few large and some small fragments" ;
  ui:isMemberOf <coarse-fragments-strength> ;
  rdfs:comment "C_CF_STRENGTH" ;
  rdfs:label "Moderately strong rock" ;
  skos:definition "50-100 MPa based on field estimate of strength class after striking or cutting the rock material - Knife:Nil or slight mark, Pick:indents shallowly, Hammer (single blow):Breaks readily into a few large and some small fragments" ;
  skos:notation "M" ;
  skos:prefLabel "Moderately strong rock" ;
  skos:topConceptOf <> ;
.
<coarse-fragments-strength-S>
  rdf:type skos:Concept ;
  dct:description "100-200 MPa based on field estimate of strength class after striking or cutting the rock material - Knife:Nil, Pick:Nil, Hammer (single blow):Breaks into one or two large fragments" ;
  ui:isMemberOf <coarse-fragments-strength> ;
  rdfs:comment "C_CF_STRENGTH" ;
  rdfs:label "Strong rock" ;
  skos:definition "100-200 MPa based on field estimate of strength class after striking or cutting the rock material - Knife:Nil, Pick:Nil, Hammer (single blow):Breaks into one or two large fragments" ;
  skos:notation "S" ;
  skos:prefLabel "Strong rock" ;
  skos:topConceptOf <> ;
.
<coarse-fragments-strength-VS>
  rdf:type skos:Concept ;
  dct:description ">200 MPa based on field estimate of strength class after striking or cutting the rock material - Knife:Nil, Pick:Nil, Hammer (single blow):Nil" ;
  ui:isMemberOf <coarse-fragments-strength> ;
  rdfs:comment "C_CF_STRENGTH" ;
  rdfs:label "Very strong rock" ;
  skos:definition ">200 MPa based on field estimate of strength class after striking or cutting the rock material - Knife:Nil, Pick:Nil, Hammer (single blow):Nil" ;
  skos:notation "VS" ;
  skos:prefLabel "Very strong rock" ;
  skos:topConceptOf <> ;
.
<coarse-fragments-strength-VW>
  rdf:type skos:Concept ;
  dct:description "1-25 MPa based on field estimate of strength class after striking or cutting the rock material - Knife:Deep cut, Pick:crumbles, Hammer (single blow):Flattened or powdered" ;
  ui:isMemberOf <coarse-fragments-strength> ;
  rdfs:comment "C_CF_STRENGTH" ;
  rdfs:label "Very weak rock" ;
  skos:definition "1-25 MPa based on field estimate of strength class after striking or cutting the rock material - Knife:Deep cut, Pick:crumbles, Hammer (single blow):Flattened or powdered" ;
  skos:notation "VW" ;
  skos:prefLabel "Very weak rock" ;
  skos:topConceptOf <> ;
.
<coarse-fragments-strength-W>
  rdf:type skos:Concept ;
  dct:description "25-50 MPa based on field estimate of strength class after striking or cutting the rock material - Knife:Shallow cut or scratch, Pick:indents deeply, Hammer (single blow):Shattered into many small fragments" ;
  ui:isMemberOf <coarse-fragments-strength> ;
  rdfs:comment "C_CF_STRENGTH" ;
  rdfs:label "Weak rock" ;
  skos:definition "25-50 MPa based on field estimate of strength class after striking or cutting the rock material - Knife:Shallow cut or scratch, Pick:indents deeply, Hammer (single blow):Shattered into many small fragments" ;
  skos:notation "W" ;
  skos:prefLabel "Weak rock" ;
  skos:topConceptOf <> ;
.
<colour>
  rdf:type skos:Collection ;
  dct:description """Record colours by comparing soils with colour charts using the Munsell Color system, for example the Munsell Soil Color Charts or the Revised Standard Soil Color Charts (Oyama and Takehara 1970).
Hue, value and chroma of the matrix colour are recorded, for example 10YR4/2.
Soil colours rarely match the chart colour chips perfectly. They should be matched to the chip closest in colour, or the nearest whole number in chroma where chips are not provided, for example chromas 5 and 7.
The soil colour is measured on the surface of a freshly broken aggregate of moist soil. Moisten the soil if it is dry. Record the colour when the visible moisture film disappears from the surface of the moistened broken aggregate. The aggregate should be held as close as possible to the colour chips. Take care not to smear the broken surface, as this can give an incorrect recording of the colour of the soil matrix.
Dry colours may also be recorded.""" ;
  ui:topMemberOf <> ;
  rdfs:comment "A moisture status must be recorded with the colour description" ;
  rdfs:label "Colour" ;
  skos:definition """Record colours by comparing soils with colour charts using the Munsell Color system, for example the Munsell Soil Color Charts or the Revised Standard Soil Color Charts (Oyama and Takehara 1970).
Hue, value and chroma of the matrix colour are recorded, for example 10YR4/2.
Soil colours rarely match the chart colour chips perfectly. They should be matched to the chip closest in colour, or the nearest whole number in chroma where chips are not provided, for example chromas 5 and 7.
The soil colour is measured on the surface of a freshly broken aggregate of moist soil. Moisten the soil if it is dry. Record the colour when the visible moisture film disappears from the surface of the moistened broken aggregate. The aggregate should be held as close as possible to the colour chips. Take care not to smear the broken surface, as this can give an incorrect recording of the colour of the soil matrix.
Dry colours may also be recorded.""" ;
  skos:member <colour-stat-D> ;
  skos:member <colour-stat-M> ;
  skos:prefLabel "Colour" ;
.
<colour-stat-D>
  rdf:type skos:Concept ;
  ui:isMemberOf <colour> ;
  rdfs:comment "Moisture status for colour description" ;
  rdfs:label "Dry" ;
  skos:notation "D" ;
  skos:prefLabel "Dry" ;
  skos:topConceptOf <> ;
.
<colour-stat-M>
  rdf:type skos:Concept ;
  ui:isMemberOf <colour> ;
  rdfs:comment "Moisture status for colour description" ;
  rdfs:label "Moist" ;
  skos:notation "M" ;
  skos:prefLabel "Moist" ;
  skos:topConceptOf <> ;
.
<condition-of-surface-soil-when-dry>
  rdf:type skos:Collection ;
  dct:description "Many surface soils have a characteristic appearance when dry. Because surface conditions are often relevant to the use of the soil and indicative of particular kinds of soil, every effort should be made to observe the surface condition in the dry state. The surface conditions are not necessarily mutually exclusive" ;
  ui:topMemberOf <> ;
  rdfs:label "Condition of surface soil when dry" ;
  skos:definition "Many surface soils have a characteristic appearance when dry. Because surface conditions are often relevant to the use of the soil and indicative of particular kinds of soil, every effort should be made to observe the surface condition in the dry state. The surface conditions are not necessarily mutually exclusive" ;
  skos:member <surfacecondition-C> ;
  skos:member <surfacecondition-F> ;
  skos:member <surfacecondition-G> ;
  skos:member <surfacecondition-H> ;
  skos:member <surfacecondition-L> ;
  skos:member <surfacecondition-M> ;
  skos:member <surfacecondition-O> ;
  skos:member <surfacecondition-P> ;
  skos:member <surfacecondition-R> ;
  skos:member <surfacecondition-S> ;
  skos:member <surfacecondition-T> ;
  skos:member <surfacecondition-X> ;
  skos:member <surfacecondition-Y> ;
  skos:member <surfacecondition-Z> ;
  skos:prefLabel "Condition of surface soil when dry" ;
.
<consistence>
  rdf:type skos:Collection ;
  dct:description "Consistence refers to the strength of cohesion and adhesion in soil. Strength will vary according to soil water status. Note that soil water status must be recorded with strength" ;
  ui:topMemberOf <> ;
  rdfs:label "Consistence" ;
  skos:definition "Consistence refers to the strength of cohesion and adhesion in soil. Strength will vary according to soil water status. Note that soil water status must be recorded with strength" ;
  skos:member <consistence-plasticity-degree> ;
  skos:member <consistence-plasticity-type> ;
  skos:member <consistence-stickiness> ;
  skos:member <consistence-strength> ;
  skos:narrower <consistence-plasticity-degree> ;
  skos:narrower <consistence-plasticity-type> ;
  skos:narrower <consistence-stickiness> ;
  skos:narrower <consistence-strength> ;
  skos:prefLabel "Consistence" ;
.
<consistence-plasticity-degree>
  rdf:type skos:Collection ;
  dct:description "Plasticity is the ability to change shape and retain the new shape after the stress is removed. The degree of plasticity given below applies only to normal plasticity. The degree of plasticity is determined at the soil moisture content used for field texturing, that is, just below sticky point. The soil is rolled between the palms of the hand and, if possible, 40 mm long rolls are formed. The rolls are dangled from the thumb and forefinger. Plasticity is determined on the behaviour of rolls of varying thickness." ;
  ui:isMemberOf <consistence> ;
  rdfs:comment "C_H_PLASTICITY_DEGREE" ;
  rdfs:label "Plasticity Degree" ;
  skos:broader <consistence> ;
  skos:definition "Plasticity is the ability to change shape and retain the new shape after the stress is removed. The degree of plasticity given below applies only to normal plasticity. The degree of plasticity is determined at the soil moisture content used for field texturing, that is, just below sticky point. The soil is rolled between the palms of the hand and, if possible, 40 mm long rolls are formed. The rolls are dangled from the thumb and forefinger. Plasticity is determined on the behaviour of rolls of varying thickness." ;
  skos:member <consistence-plasticity-degree-0> ;
  skos:member <consistence-plasticity-degree-1> ;
  skos:member <consistence-plasticity-degree-2> ;
  skos:member <consistence-plasticity-degree-3> ;
  skos:prefLabel "Plasticity Degree" ;
.
<consistence-plasticity-degree-0>
  rdf:type skos:Concept ;
  dct:description "Roll (40mm length x 6mm diameter) will not form." ;
  ui:isMemberOf <consistence-plasticity-degree> ;
  rdfs:label "Non plastic" ;
  skos:definition "Roll (40mm length x 6mm diameter) will not form." ;
  skos:notation "0" ;
  skos:prefLabel "Non plastic"@en ;
  skos:topConceptOf <> ;
.
<consistence-plasticity-degree-1>
  rdf:type skos:Concept ;
  dct:description """Roll (40mm length x 6mm diameter) will form and will support its own weight.
Roll (40mm length x 4mm diameter) will form but will not support its own weight.""" ;
  ui:isMemberOf <consistence-plasticity-degree> ;
  rdfs:label "Slightly plastic" ;
  skos:definition """Roll (40mm length x 6mm diameter) will form and will support its own weight.
Roll (40mm length x 4mm diameter) will form but will not support its own weight.""" ;
  skos:notation "1" ;
  skos:prefLabel "Slightly plastic"@en ;
  skos:topConceptOf <> ;
.
<consistence-plasticity-degree-2>
  rdf:type skos:Concept ;
  dct:description """Roll (40mm length x 4mm diameter) will form and will support its own weight.
Roll (40mm length x 2mm diameter) will form but will not support its own weight.""" ;
  ui:isMemberOf <consistence-plasticity-degree> ;
  rdfs:label "Moderately plastic" ;
  skos:definition """Roll (40mm length x 4mm diameter) will form and will support its own weight.
Roll (40mm length x 2mm diameter) will form but will not support its own weight.""" ;
  skos:notation "2" ;
  skos:prefLabel "Moderately plastic"@en ;
  skos:topConceptOf <> ;
.
<consistence-plasticity-degree-3>
  rdf:type skos:Concept ;
  dct:description "Roll (40mm length x 2mm diameter) will form and will support its own weight." ;
  ui:isMemberOf <consistence-plasticity-degree> ;
  rdfs:label "Very plastic" ;
  skos:definition "Roll (40mm length x 2mm diameter) will form and will support its own weight." ;
  skos:notation "3" ;
  skos:prefLabel "Very plastic"@en ;
  skos:topConceptOf <> ;
.
<consistence-plasticity-type>
  rdf:type skos:Collection ;
  dct:description "The type of plasticity refers to the degree to which the consistence and/or field texture properties of a soil suggest the amount of clay-sized particles it contains (Butler 1955). It may be identified by determining two field textures: one after an initial 1 to 2 minute working of the soil sample, and another after a prolonged 10 minute kneading. The change in field texture from the initial to the prolonged working of the soil sample indicates the type of plasticity." ;
  ui:isMemberOf <consistence> ;
  rdfs:comment "C_H_PLASTICITY_TYPE" ;
  rdfs:label "Plasticity Type" ;
  skos:broader <consistence> ;
  skos:definition "The type of plasticity refers to the degree to which the consistence and/or field texture properties of a soil suggest the amount of clay-sized particles it contains (Butler 1955). It may be identified by determining two field textures: one after an initial 1 to 2 minute working of the soil sample, and another after a prolonged 10 minute kneading. The change in field texture from the initial to the prolonged working of the soil sample indicates the type of plasticity." ;
  skos:member <consistence-plasticity-type-N> ;
  skos:member <consistence-plasticity-type-S> ;
  skos:member <consistence-plasticity-type-T> ;
  skos:member <consistence-plasticity-type-U> ;
  skos:prefLabel "Plasticity Type" ;
.
<consistence-plasticity-type-N>
  rdf:type skos:Concept ;
  dct:description "Negligible change." ;
  ui:isMemberOf <consistence-plasticity-type> ;
  rdfs:label "Normal plasticity" ;
  skos:definition "Negligible change." ;
  skos:notation "N" ;
  skos:prefLabel "Normal plasticity"@en ;
  skos:topConceptOf <> ;
.
<consistence-plasticity-type-S>
  rdf:type skos:Concept ;
  dct:description "Decreases one or more field texture groups of Northcote (1979)." ;
  ui:isMemberOf <consistence-plasticity-type> ;
  rdfs:label "Superplastic" ;
  skos:definition "Decreases one or more field texture groups of Northcote (1979)." ;
  skos:notation "S" ;
  skos:prefLabel "Superplastic"@en ;
  skos:topConceptOf <> ;
.
<consistence-plasticity-type-T>
  rdf:type skos:Concept ;
  dct:description "Increases two or more field texture groups." ;
  ui:isMemberOf <consistence-plasticity-type> ;
  rdfs:label "Strongly subplastic" ;
  skos:definition "Increases two or more field texture groups." ;
  skos:notation "T" ;
  skos:prefLabel "Strongly subplastic"@en ;
  skos:topConceptOf <> ;
.
<consistence-plasticity-type-U>
  rdf:type skos:Concept ;
  dct:description "Increases one to two field texture groups." ;
  ui:isMemberOf <consistence-plasticity-type> ;
  rdfs:label "Subplastic" ;
  skos:definition "Increases one to two field texture groups." ;
  skos:notation "U" ;
  skos:prefLabel "Subplastic"@en ;
  skos:topConceptOf <> ;
.
<consistence-stickiness>
  rdf:type skos:Collection ;
  dct:description "Stickiness is determined on wet soil by pressing the wet sample between thumb and forefinger and then observing the adherence of the soil to the fingers." ;
  ui:isMemberOf <consistence> ;
  rdfs:comment "C_H_STICKINESS" ;
  rdfs:label "Stickiness" ;
  skos:broader <consistence> ;
  skos:definition "Stickiness is determined on wet soil by pressing the wet sample between thumb and forefinger and then observing the adherence of the soil to the fingers." ;
  skos:member <consistence-stickiness-0> ;
  skos:member <consistence-stickiness-1> ;
  skos:member <consistence-stickiness-2> ;
  skos:member <consistence-stickiness-3> ;
  skos:prefLabel "Stickiness" ;
.
<consistence-stickiness-0>
  rdf:type skos:Concept ;
  dct:description "Little of no soil adheres." ;
  ui:isMemberOf <consistence-stickiness> ;
  rdfs:label "Non-sticky" ;
  skos:definition "Little or no soil adheres." ;
  skos:notation "0" ;
  skos:prefLabel "Non-sticky"@en ;
  skos:topConceptOf <> ;
.
<consistence-stickiness-1>
  rdf:type skos:Concept ;
  dct:description "Soil adheres to thumb and forefinger but is not stretched notably and comes off rather cleanly." ;
  ui:isMemberOf <consistence-stickiness> ;
  rdfs:label "Slightly sticky" ;
  skos:definition "Soil adheres to thumb and forefinger but is not stretched notably and comes off rather cleanly." ;
  skos:notation "1" ;
  skos:prefLabel "Slightly sticky"@en ;
  skos:topConceptOf <> ;
.
<consistence-stickiness-2>
  rdf:type skos:Concept ;
  dct:description "Soil adheres to thumb and forefinger and tends to stretch rather than pull free of fingers." ;
  ui:isMemberOf <consistence-stickiness> ;
  rdfs:label "Moderately sticky" ;
  skos:definition "Soil adheres to thumb and forefinger and tends to stretch rather than pull free of fingers." ;
  skos:notation "2" ;
  skos:prefLabel "Moderately sticky"@en ;
  skos:topConceptOf <> ;
.
<consistence-stickiness-3>
  rdf:type skos:Concept ;
  dct:description "Soil adheres strongly to thumb and forefinger and stretches notably." ;
  ui:isMemberOf <consistence-stickiness> ;
  rdfs:label "Very sticky" ;
  skos:definition "Soil adheres strongly to thumb and forefinger and stretches notably." ;
  skos:notation "3" ;
  skos:prefLabel "Very sticky"@en ;
  skos:topConceptOf <> ;
.
<consistence-strength>
  rdf:type skos:Collection ;
  dct:description """Strength of soil is the resistance to breaking or deformation. Strength is determined by the force just sufficient to break or deform a 20 mm diameter piece of soil when a compressive shearing force is applied between thumb and forefinger. The 20 mm piece of soil may be a ped, part of a ped, a compound ped or a fragment.

Forces 0 to 5 are equivalent to the following dry consistence classes in the ‘USDA Soil Survey Manual’ (Soil Survey Staff 1951):
0	Loose
1	Soft
2	Slightly hard
3	Hard
4	Very hard
5	Extremely hard""" ;
  ui:isMemberOf <consistence> ;
  rdfs:comment "C_STRG_CLASS" ;
  rdfs:label "Strength" ;
  skos:broader <consistence> ;
  skos:definition """Strength of soil is the resistance to breaking or deformation. Strength is determined by the force just sufficient to break or deform a 20 mm diameter piece of soil when a compressive shearing force is applied between thumb and forefinger. The 20 mm piece of soil may be a ped, part of a ped, a compound ped or a fragment.

Forces 0 to 5 are equivalent to the following dry consistence classes in the ‘USDA Soil Survey Manual’ (Soil Survey Staff 1951):
0	Loose
1	Soft
2	Slightly hard
3	Hard
4	Very hard
5	Extremely hard""" ;
  skos:member <consistence-strength-0> ;
  skos:member <consistence-strength-1> ;
  skos:member <consistence-strength-2> ;
  skos:member <consistence-strength-3> ;
  skos:member <consistence-strength-4> ;
  skos:member <consistence-strength-5> ;
  skos:member <consistence-strength-6> ;
  skos:member <consistence-strength-7> ;
  skos:prefLabel "Strength" ;
.
<consistence-strength-0>
  rdf:type skos:Concept ;
  dct:description "No force required. Separate particles such as loose sands." ;
  ui:isMemberOf <consistence-strength> ;
  rdfs:label "Loose" ;
  skos:definition "No force required. Separate particles such as loose sands." ;
  skos:notation "0" ;
  skos:prefLabel "Loose"@en ;
  skos:topConceptOf <> ;
.
<consistence-strength-1>
  rdf:type skos:Concept ;
  dct:description "Very small force, almost nil." ;
  ui:isMemberOf <consistence-strength> ;
  rdfs:label "Very weak" ;
  skos:definition "Very small force, almost nil." ;
  skos:notation "1" ;
  skos:prefLabel "Very weak"@en ;
  skos:topConceptOf <> ;
.
<consistence-strength-2>
  rdf:type skos:Concept ;
  dct:description "Small but significant force." ;
  ui:isMemberOf <consistence-strength> ;
  rdfs:label "Weak" ;
  skos:definition "Small but significant force." ;
  skos:notation "2" ;
  skos:prefLabel "Weak"@en ;
  skos:topConceptOf <> ;
.
<consistence-strength-3>
  rdf:type skos:Concept ;
  dct:description "Moderate or firm force." ;
  ui:isMemberOf <consistence-strength> ;
  rdfs:label "Firm" ;
  skos:definition "Moderate or firm force." ;
  skos:notation "3" ;
  skos:prefLabel "Firm"@en ;
  skos:topConceptOf <> ;
.
<consistence-strength-4>
  rdf:type skos:Concept ;
  dct:description "Strong force but within power of thumb and forefinger." ;
  ui:isMemberOf <consistence-strength> ;
  rdfs:label "Very Firm" ;
  skos:definition "Strong force but within power of thumb and forefinger." ;
  skos:notation "4" ;
  skos:prefLabel "Very Firm"@en ;
  skos:topConceptOf <> ;
.
<consistence-strength-5>
  rdf:type skos:Concept ;
  dct:description "Beyond power of thumb and forefinger. Crushes underfoot on hard, flat surface with small force." ;
  ui:isMemberOf <consistence-strength> ;
  rdfs:label "Strong" ;
  skos:definition "Beyond power of thumb and forefinger. Crushes underfoot on hard, flat surface with small force." ;
  skos:notation "5" ;
  skos:prefLabel "Strong"@en ;
  skos:topConceptOf <> ;
.
<consistence-strength-6>
  rdf:type skos:Concept ;
  dct:description "Crushes underfoot on hard, flat surface with full body weight applied slowly." ;
  ui:isMemberOf <consistence-strength> ;
  rdfs:label "Very Strong" ;
  skos:definition "Crushes underfoot on hard, flat surface with full body weight applied slowly." ;
  skos:notation "6" ;
  skos:prefLabel "Very Strong"@en ;
  skos:topConceptOf <> ;
.
<consistence-strength-7>
  rdf:type skos:Concept ;
  dct:description "Cannot be crushed underfoot by full body weight applied slowly." ;
  ui:isMemberOf <consistence-strength> ;
  rdfs:label "Rigid" ;
  skos:definition "Cannot be crushed underfoot by full body weight applied slowly." ;
  skos:notation "7" ;
  skos:prefLabel "Rigid"@en ;
  skos:topConceptOf <> ;
.
<cutans>
  rdf:type skos:Collection ;
  dct:description """A cutan is a modification of the texture, structure or fabric at natural surfaces in soil materials; it arises from concentration of particular soil constituents or in situ modification of the plasma. Cutans comprise any of the component substances of the soil material (Brewer 1964).
Cutans may be observed in the field (a ×10 hand lens is usually necessary) but their nature is often difficult to determine unless a thin section is made. Hence the following simple classification.""" ;
  ui:topMemberOf <> ;
  rdfs:label "Cutans" ;
  skos:definition """A cutan is a modification of the texture, structure or fabric at natural surfaces in soil materials; it arises from concentration of particular soil constituents or in situ modification of the plasma. Cutans comprise any of the component substances of the soil material (Brewer 1964).
Cutans may be observed in the field (a ×10 hand lens is usually necessary) but their nature is often difficult to determine unless a thin section is made. Hence the following simple classification.""" ;
  skos:member <cutans-abundance> ;
  skos:member <cutans-distinctness> ;
  skos:member <cutans-type> ;
  skos:prefLabel "Cutans" ;
.
<cutans-abundance>
  rdf:type skos:Collection ;
  dct:description "Abundance of cutans" ;
  ui:isMemberOf <cutans> ;
  rdfs:comment "N_CUTAN_ABUN" ;
  rdfs:label "Abundance of cutans" ;
  skos:definition "Abundance of cutans" ;
  skos:member <cutans-abundance-0> ;
  skos:member <cutans-abundance-1> ;
  skos:member <cutans-abundance-2> ;
  skos:member <cutans-abundance-3> ;
  skos:prefLabel "Abundance of cutans"@en ;
.
<cutans-abundance-0>
  rdf:type skos:Concept ;
  dct:description "0" ;
  ui:isMemberOf <cutans-abundance> ;
  rdfs:comment "N_CUTAN_ABUN" ;
  rdfs:label "No cutans" ;
  skos:definition "0" ;
  skos:notation "0" ;
  skos:prefLabel "No cutans"@en ;
  skos:topConceptOf <> ;
.
<cutans-abundance-1>
  rdf:type skos:Concept ;
  dct:description "<10% of ped faces or pore walls with cutans" ;
  ui:isMemberOf <cutans-abundance> ;
  rdfs:comment "N_CUTAN_ABUN" ;
  rdfs:label "Few" ;
  skos:definition "<10% of ped faces or pore walls with cutans" ;
  skos:notation "1" ;
  skos:prefLabel "Few"@en ;
  skos:topConceptOf <> ;
.
<cutans-abundance-2>
  rdf:type skos:Concept ;
  dct:description "10–50% of ped faces or pore walls with cutans" ;
  ui:isMemberOf <cutans-abundance> ;
  rdfs:comment "N_CUTAN_ABUN" ;
  rdfs:label "Common" ;
  skos:definition "10–50% of ped faces or pore walls with cutans" ;
  skos:notation "2" ;
  skos:prefLabel "Common"@en ;
  skos:topConceptOf <> ;
.
<cutans-abundance-3>
  rdf:type skos:Concept ;
  dct:description ">50% of ped faces or pore walls with cutans" ;
  ui:isMemberOf <cutans-abundance> ;
  rdfs:comment "N_CUTAN_ABUN" ;
  rdfs:label "Many" ;
  skos:definition ">50% of ped faces or pore walls with cutans" ;
  skos:notation "3" ;
  skos:prefLabel "Many"@en ;
  skos:topConceptOf <> ;
.
<cutans-distinctness>
  rdf:type skos:Collection ;
  dct:description "Cutan distinctness refers to the ease and certainty with which a cutan is identified. Distinctness relates to thickness and to the colour contrast with the adjacent material; it may change markedly with moisture content" ;
  ui:isMemberOf <cutans> ;
  rdfs:comment "C_CUTAN_DISTINCT" ;
  rdfs:label "Distinctness of cutans" ;
  skos:definition "Cutan distinctness refers to the ease and certainty with which a cutan is identified. Distinctness relates to thickness and to the colour contrast with the adjacent material; it may change markedly with moisture content" ;
  skos:member <cutans-distinctness-D> ;
  skos:member <cutans-distinctness-F> ;
  skos:member <cutans-distinctness-P> ;
  skos:prefLabel "Distinctness of cutans"@en ;
.
<cutans-distinctness-D>
  rdf:type skos:Concept ;
  dct:description "can be detected without magnification. Contrast with adjacent material is evident in colour, texture or other properties" ;
  ui:isMemberOf <cutans-distinctness> ;
  rdfs:comment "C_CUTAN_DISTINCT" ;
  rdfs:label "Distinct" ;
  skos:definition "can be detected without magnification. Contrast with adjacent material is evident in colour, texture or other properties" ;
  skos:notation "D" ;
  skos:prefLabel "Distinct"@en ;
  skos:topConceptOf <> ;
.
<cutans-distinctness-F>
  rdf:type skos:Concept ;
  dct:description "evident only on close examination with ×10 magnification. Little contrast with adjacent material" ;
  ui:isMemberOf <cutans-distinctness> ;
  rdfs:comment "C_CUTAN_DISTINCT" ;
  rdfs:label "Faint" ;
  skos:definition "evident only on close examination with ×10 magnification. Little contrast with adjacent material" ;
  skos:notation "F" ;
  skos:prefLabel "Faint"@en ;
  skos:topConceptOf <> ;
.
<cutans-distinctness-P>
  rdf:type skos:Concept ;
  dct:description "conspicuous without magnification when compared with a surface broken through the soil. Colour, texture or some other property contrasts sharply with properties of the adjacent material, or the feature is thick enough to be conspicuous" ;
  ui:isMemberOf <cutans-distinctness> ;
  rdfs:comment "C_CUTAN_DISTINCT" ;
  rdfs:label "Prominent" ;
  skos:definition "conspicuous without magnification when compared with a surface broken through the soil. Colour, texture or some other property contrasts sharply with properties of the adjacent material, or the feature is thick enough to be conspicuous" ;
  skos:notation "P" ;
  skos:prefLabel "Prominent"@en ;
  skos:topConceptOf <> ;
.
<cutans-type>
  rdf:type skos:Collection ;
  dct:description "Types of cutans" ;
  ui:isMemberOf <cutans> ;
  rdfs:comment "C_CUTAN_TYPE" ;
  rdfs:label "Types of cutans" ;
  skos:definition "Types of cutans" ;
  skos:member <cutans-type-C> ;
  skos:member <cutans-type-K> ;
  skos:member <cutans-type-M> ;
  skos:member <cutans-type-O> ;
  skos:member <cutans-type-S> ;
  skos:member <cutans-type-U> ;
  skos:member <cutans-type-Z> ;
  skos:prefLabel "Types of cutans"@en ;
.
<cutans-type-C>
  rdf:type skos:Concept ;
  dct:description "coatings of clay often different in colour from the matrix of the ped. They are frequently difficult to distinguish from stress cutans, which are not true coatings" ;
  ui:isMemberOf <cutans-type> ;
  rdfs:comment "C_CUTAN_TYPE" ;
  rdfs:label "Clay skins" ;
  skos:definition "coatings of clay often different in colour from the matrix of the ped. They are frequently difficult to distinguish from stress cutans, which are not true coatings" ;
  skos:notation "C" ;
  skos:prefLabel "Clay skins"@en ;
  skos:topConceptOf <> ;
.
<cutans-type-K>
  rdf:type skos:Concept ;
  dct:description "stress cutans with smooth striations or grooves" ;
  ui:isMemberOf <cutans-type> ;
  rdfs:comment "C_CUTAN_TYPE" ;
  rdfs:label "Slickensides" ;
  skos:definition "stress cutans with smooth striations or grooves" ;
  skos:notation "K" ;
  skos:prefLabel "Slickensides"@en ;
  skos:topConceptOf <> ;
.
<cutans-type-M>
  rdf:type skos:Concept ;
  dct:description "coatings of manganese oxides or hydroxides. The material may have a glazed appearance and is very dark brown to black" ;
  ui:isMemberOf <cutans-type> ;
  rdfs:comment "C_CUTAN_TYPE" ;
  rdfs:label "Mangans" ;
  skos:definition "coatings of manganese oxides or hydroxides. The material may have a glazed appearance and is very dark brown to black" ;
  skos:notation "M" ;
  skos:prefLabel "Mangans"@en ;
  skos:topConceptOf <> ;
.
<cutans-type-O>
  rdf:type skos:Concept ;
  dct:description "may be composed of iron oxides, organic matter, calcium carbonate or gypsum" ;
  ui:isMemberOf <cutans-type> ;
  rdfs:comment "C_CUTAN_TYPE" ;
  rdfs:label "Other cutans" ;
  skos:definition "may be composed of iron oxides, organic matter, calcium carbonate or gypsum" ;
  skos:notation "O" ;
  skos:prefLabel "Other cutans"@en ;
  skos:topConceptOf <> ;
.
<cutans-type-S>
  rdf:type skos:Concept ;
  dct:description "in situ modifications of natural surfaces in soil materials due to differential forces such as shearing. They are not true coatings" ;
  ui:isMemberOf <cutans-type> ;
  rdfs:comment "C_CUTAN_TYPE" ;
  rdfs:label "Stress cutans" ;
  skos:definition "in situ modifications of natural surfaces in soil materials due to differential forces such as shearing. They are not true coatings" ;
  skos:notation "S" ;
  skos:prefLabel "Stress cutans"@en ;
  skos:topConceptOf <> ;
.
<cutans-type-U>
  rdf:type skos:Concept ;
  dct:description "nature of cutans cannot be determined" ;
  ui:isMemberOf <cutans-type> ;
  rdfs:comment "C_CUTAN_TYPE" ;
  rdfs:label "Unspecified" ;
  skos:definition "nature of cutans cannot be determined" ;
  skos:notation "U" ;
  skos:prefLabel "Unspecified"@en ;
  skos:topConceptOf <> ;
.
<cutans-type-Z>
  rdf:type skos:Concept ;
  dct:description "Zero or no cutans" ;
  ui:isMemberOf <cutans-type> ;
  rdfs:comment "C_CUTAN_TYPE" ;
  rdfs:label "Zero or no cutans" ;
  skos:definition "Zero or no cutans" ;
  skos:notation "Z" ;
  skos:prefLabel "Zero or no cutans"@en ;
  skos:topConceptOf <> ;
.
<depth-of-horizons>
  rdf:type skos:Collection ;
  dct:description """The upper and lower depths, in metres, of each horizon are measured from the soil surface, excluding O horizons. O horizon depths are measured above the mineral soil surface, for example O1 0.120.10 m, O2 0.10.0 m.
A scaled horizon diagram may be useful where horizons are irregular.""" ;
  ui:topMemberOf <> ;
  rdfs:label "Depth of Horizons" ;
  skos:definition """The upper and lower depths, in metres, of each horizon are measured from the soil surface, excluding O horizons. O horizon depths are measured above the mineral soil surface, for example O1 0.120.10 m, O2 0.10.0 m.
A scaled horizon diagram may be useful where horizons are irregular.""" ;
  skos:prefLabel "Depth of Horizons" ;
.
<depth-to-r-horizon>
  rdf:type skos:Collection ;
  dct:description """Give depth to R horizon or strongly cemented pan in metres.
The purpose of recording this depth is to include in the soil description those materials that may be relatively easily moved by earth-moving equipment or may be relatively easily penetrated by roots. Strong or very strong rock or pan that may require ripping or blasting to move, and/or has little or no root penetration, is excluded""" ;
  ui:topMemberOf <> ;
  rdfs:label "Depth to R horizon or strongly cemented pan" ;
  skos:definition """Give depth to R horizon or strongly cemented pan in metres.
The purpose of recording this depth is to include in the soil description those materials that may be relatively easily moved by earth-moving equipment or may be relatively easily penetrated by roots. Strong or very strong rock or pan that may require ripping or blasting to move, and/or has little or no root penetration, is excluded""" ;
  skos:prefLabel "Depth to R horizon or strongly cemented pan" ;
.
<effervescence-H>
  rdf:type skos:Concept ;
  dct:description "moderate visible effervescence" ;
  ui:isMemberOf <effervescence-of-carbonate-in-fine-earth> ;
  rdfs:label "Highly calcareous" ;
  skos:definition "moderate visible effervescence" ;
  skos:notation "H" ;
  skos:prefLabel "Highly calcareous"@en ;
  skos:topConceptOf <> ;
.
<effervescence-M>
  rdf:type skos:Concept ;
  dct:description "audible and slightly visible effervescence" ;
  ui:isMemberOf <effervescence-of-carbonate-in-fine-earth> ;
  rdfs:label "Moderately calcareous" ;
  skos:definition "audible and slightly visible effervescence" ;
  skos:notation "M" ;
  skos:prefLabel "Moderately calcareous"@en ;
  skos:topConceptOf <> ;
.
<effervescence-N>
  rdf:type skos:Concept ;
  dct:description "no audible or visible effervescence" ;
  ui:isMemberOf <effervescence-of-carbonate-in-fine-earth> ;
  rdfs:label "Non-calcareous" ;
  skos:definition "no audible or visible effervescence" ;
  skos:notation "N" ;
  skos:prefLabel "Non-calcareous"@en ;
  skos:topConceptOf <> ;
.
<effervescence-S>
  rdf:type skos:Concept ;
  dct:description "slightly audible but no visible effervescence" ;
  ui:isMemberOf <effervescence-of-carbonate-in-fine-earth> ;
  rdfs:label "Slightly calcareous" ;
  skos:definition "slightly audible but no visible effervescence" ;
  skos:notation "S" ;
  skos:prefLabel "Slightly calcareous"@en ;
  skos:topConceptOf <> ;
.
<effervescence-V>
  rdf:type skos:Concept ;
  dct:description "strong visible effervescence" ;
  ui:isMemberOf <effervescence-of-carbonate-in-fine-earth> ;
  rdfs:label "Very highly calcareous" ;
  skos:definition "strong visible effervescence" ;
  skos:notation "V" ;
  skos:prefLabel "Very highly calcareous"@en ;
  skos:topConceptOf <> ;
.
<effervescence-of-carbonate-in-fine-earth>
  rdf:type skos:Collection ;
  dct:description "Effervescence of carbonate in fine earth using two or three drops of 1-molar HCl" ;
  ui:topMemberOf <> ;
  rdfs:label "Effervescence of carbonate in fine earth" ;
  skos:definition "Effervescence of carbonate in fine earth using two or three drops of 1-molar HCl" ;
  skos:member <effervescence-H> ;
  skos:member <effervescence-M> ;
  skos:member <effervescence-N> ;
  skos:member <effervescence-S> ;
  skos:member <effervescence-V> ;
  skos:prefLabel "Effervescence" ;
.
<fabric>
  rdf:type skos:Collection ;
  dct:description """The definition of soil fabric in Australia is incomplete. The following description is adapted from Northcote (1979).
Fabric describes the appearance of the soil material (under ×10 hand lens). Differences in fabric are associated with the presence or absence of peds, the lustre or lack of lustre of the ped surfaces, and the presence, size and arrangement of pores (voids) in the soil mass. The descriptions given below apply primarily to B horizons.""" ;
  ui:topMemberOf <> ;
  rdfs:label "Fabric" ;
  skos:definition """The definition of soil fabric in Australia is incomplete. The following description is adapted from Northcote (1979).
Fabric describes the appearance of the soil material (under ×10 hand lens). Differences in fabric are associated with the presence or absence of peds, the lustre or lack of lustre of the ped surfaces, and the presence, size and arrangement of pores (voids) in the soil mass. The descriptions given below apply primarily to B horizons.""" ;
  skos:member <fabric-E> ;
  skos:member <fabric-G> ;
  skos:member <fabric-R> ;
  skos:member <fabric-S> ;
  skos:prefLabel "Fabric" ;
.
<fabric-E>
  rdf:type skos:Concept ;
  dct:description "The soil material is coherent and characterised by the presence of pores (voids) and few, if any, peds. Ultimate soil particles (sand grains, for example) are coated with oxides and/or clays and are arranged (clumped) around the pores" ;
  ui:isMemberOf <fabric> ;
  rdfs:label "Earthy" ;
  skos:altLabel "Porous fabric" ;
  skos:definition "The soil material is coherent and characterised by the presence of pores (voids) and few, if any, peds. Ultimate soil particles (sand grains, for example) are coated with oxides and/or clays and are arranged (clumped) around the pores" ;
  skos:notation "E" ;
  skos:prefLabel "Earthy" ;
  skos:topConceptOf <> ;
.
<fabric-G>
  rdf:type skos:Concept ;
  dct:description "The soil material is coherent, with few, if any, peds. The closely packed sand grains provide the characteristic appearance of the soil mass" ;
  ui:isMemberOf <fabric> ;
  rdfs:label "Sandy (grains prominent)" ;
  skos:definition "The soil material is coherent, with few, if any, peds. The closely packed sand grains provide the characteristic appearance of the soil mass" ;
  skos:notation "G" ;
  skos:prefLabel "Sandy (grains prominent)" ;
  skos:topConceptOf <> ;
.
<fabric-R>
  rdf:type skos:Concept ;
  dct:description "Peds are evident, and characteristically more than 50% of the peds are rough-faced, that is, they have relatively porous surfaces. (Rough-faced peds generally have less clearly defined faces than smooth-faced peds and the pedality of the soil may be questioned. However, if the soil mass is pressed gently, the characteristic size and shape of the soil aggregates will confirm its pedality.) Granular peds with common or many macropores are always rough-faced, but this condition varies in other ped forms" ;
  ui:isMemberOf <fabric> ;
  rdfs:label "Rough-ped" ;
  skos:definition "Peds are evident, and characteristically more than 50% of the peds are rough-faced, that is, they have relatively porous surfaces. (Rough-faced peds generally have less clearly defined faces than smooth-faced peds and the pedality of the soil may be questioned. However, if the soil mass is pressed gently, the characteristic size and shape of the soil aggregates will confirm its pedality.) Granular peds with common or many macropores are always rough-faced, but this condition varies in other ped forms" ;
  skos:notation "R" ;
  skos:prefLabel "Rough-ped" ;
  skos:topConceptOf <> ;
.
<fabric-S>
  rdf:type skos:Concept ;
  dct:description "Peds are evident, and characteristically more than 50% of them are dense and smooth-faced, although the degree of lustre may vary." ;
  ui:isMemberOf <fabric> ;
  rdfs:label "Smooth-ped" ;
  skos:definition "Peds are evident, and characteristically more than 50% of them are dense and smooth-faced, although the degree of lustre may vary." ;
  skos:notation "S" ;
  skos:prefLabel "Smooth-ped" ;
  skos:topConceptOf <> ;
.
<field-ph>
  rdf:type skos:Collection ;
  dct:description """pH is determined in the field using a field pH kit based on the specifications of Raupach and Tucker (1959). Estimate to 0.5 of a unit. Portable pH meters may also be used.
Record depth at which pH is determined, in metres.
pH may be measured either:
•	by horizons, or
•	where horizons are thick (greater than 0.5 m) and horizon boundaries are diffuse, at selected intervals down the profile. This system gives useful data in some soils when important pH changes may occur independently of visible horizon changes, for instance the change from alkaline to strongly acid conditions in some cracking clays.""" ;
  ui:topMemberOf <> ;
  rdfs:label "Field pH" ;
  skos:definition """pH is determined in the field using a field pH kit based on the specifications of Raupach and Tucker (1959). Estimate to 0.5 of a unit. Portable pH meters may also be used.
Record depth at which pH is determined, in metres.
pH may be measured either:
•	by horizons, or
•	where horizons are thick (greater than 0.5 m) and horizon boundaries are diffuse, at selected intervals down the profile. This system gives useful data in some soils when important pH changes may occur independently of visible horizon changes, for instance the change from alkaline to strongly acid conditions in some cracking clays.""" ;
  skos:prefLabel "Field pH" ;
.
<field-texture>
  rdf:type skos:Collection ;
  dct:description "Field texture is a measure of the behaviour of a small handful of soil when moistened and kneaded into a ball and then pressed out between thumb and forefinger. The recommended field texture grades are characterised by the behaviour of the moist bolus. The approximate percentage content of clay (particles less than 0.002 mm in diameter) and silt (particles between 0.02 and 0.002 mm in diameter) are used as a guide." ;
  ui:topMemberOf <> ;
  rdfs:comment "C_H_TEXTURE; Adapted from Northcote (1979). The clay percentages must not be used to determine a field texture, that is, do not use them to convert a laboratory particle size value to a field texture grade. Similarly, do not adjust a field texture grade when laboratory particle size data become available." ;
  rdfs:label "Field texture" ;
  skos:definition "Field texture is a measure of the behaviour of a small handful of soil when moistened and kneaded into a ball and then pressed out between thumb and forefinger. The recommended field texture grades are characterised by the behaviour of the moist bolus. The approximate percentage content of clay (particles less than 0.002 mm in diameter) and silt (particles between 0.02 and 0.002 mm in diameter) are used as a guide." ;
  skos:member <field-texture-mineral> ;
  skos:member <field-texture-organic> ;
  skos:prefLabel "Field texture"@en ;
.
<field-texture-AP>
  rdf:type skos:Concept ;
  dct:description "Strongly to completely decomposed organic material. Plant remains vary from few being identifiable to completely amorphous." ;
  ui:isMemberOf <field-texture-organic> ;
  rdfs:comment "humified peat" ;
  rdfs:label "Sapric peat" ;
  skos:definition "Strongly to completely decomposed organic material. Plant remains vary from few being identifiable to completely amorphous." ;
  skos:notation "AP" ;
  skos:prefLabel "Sapric peat"@en ;
  skos:topConceptOf <> ;
.
<field-texture-CFS>
  rdf:type skos:Concept ;
  dct:description "Behaviour of moist bolus: slight coherence; sand grains of medium size; sticky when wet; many sand grains stick to fingers; will form minimal ribbon of 5–15 mm; discolours fingers with clay stain. Fine sand can be felt and often heard when manipulated. Sand grains are clearly evident under a ×10 hand lens." ;
  rdfs:comment "Approximate clay content (%): 5 - 10%" ;
  rdfs:label "Clayey fine sand" ;
  skos:broader <field-texture-CS> ;
  skos:definition "Behaviour of moist bolus: slight coherence; sand grains of medium size; sticky when wet; many sand grains stick to fingers; will form minimal ribbon of 5–15 mm; discolours fingers with clay stain. Fine sand can be felt and often heard when manipulated. Sand grains are clearly evident under a ×10 hand lens." ;
  skos:inScheme <> ;
  skos:narrower <field-texture-CFS-heavy> ;
  skos:narrower <field-texture-CFS-light> ;
  skos:notation "CFS" ;
  skos:prefLabel "Clayey fine sand"@en ;
.
<field-texture-CFS-heavy>
  rdf:type skos:Concept ;
  dct:description "Behaviour of moist bolus: slight coherence; sand grains of medium size; sticky when wet; many sand grains stick to fingers; will form minimal ribbon of 5–15 mm; discolours fingers with clay stain. Fine sand can be felt and often heard when manipulated. Sand grains are clearly evident under a ×10 hand lens." ;
  rdfs:comment "Approximate clay content (%): 5 - 10%" ;
  rdfs:label "Heavy clayey fine sand" ;
  skos:broader <field-texture-CFS> ;
  skos:broader <field-texture-CS-heavy> ;
  skos:definition "Behaviour of moist bolus: slight coherence; sand grains of medium size; sticky when wet; many sand grains stick to fingers; will form minimal ribbon of 5–15 mm; discolours fingers with clay stain. Fine sand can be felt and often heard when manipulated. Sand grains are clearly evident under a ×10 hand lens." ;
  skos:inScheme <> ;
  skos:notation "CFS+" ;
  skos:prefLabel "Heavy clayey fine sand"@en ;
.
<field-texture-CFS-light>
  rdf:type skos:Concept ;
  dct:description "Behaviour of moist bolus: slight coherence; sand grains of medium size; sticky when wet; many sand grains stick to fingers; will form minimal ribbon of 5–15 mm; discolours fingers with clay stain. Fine sand can be felt and often heard when manipulated. Sand grains are clearly evident under a ×10 hand lens." ;
  rdfs:comment "Approximate clay content (%): 5 - 10%" ;
  rdfs:label "Light clayey fine sand" ;
  skos:broader <field-texture-CFS> ;
  skos:broader <field-texture-CS-light> ;
  skos:definition "Behaviour of moist bolus: slight coherence; sand grains of medium size; sticky when wet; many sand grains stick to fingers; will form minimal ribbon of 5–15 mm; discolours fingers with clay stain. Fine sand can be felt and often heard when manipulated. Sand grains are clearly evident under a ×10 hand lens." ;
  skos:inScheme <> ;
  skos:notation "CFS-" ;
  skos:prefLabel "Light clayey fine sand"@en ;
.
<field-texture-CKS>
  rdf:type skos:Concept ;
  dct:description "Behaviour of moist bolus: slight coherence; sand grains of medium size; sticky when wet; many sand grains stick to fingers; will form minimal ribbon of 5–15 mm; discolours fingers with clay stain. Coarse sand is obviously coarse to touch. Sand grains are very readily seen with the naked eye." ;
  rdfs:comment "Approximate clay content (%): 5 - 10%" ;
  rdfs:label "Clayey coarse sand" ;
  skos:broader <field-texture-CS> ;
  skos:definition "Behaviour of moist bolus: slight coherence; sand grains of medium size; sticky when wet; many sand grains stick to fingers; will form minimal ribbon of 5–15 mm; discolours fingers with clay stain. Coarse sand is obviously coarse to touch. Sand grains are very readily seen with the naked eye." ;
  skos:inScheme <> ;
  skos:narrower <field-texture-CKS-heavy> ;
  skos:narrower <field-texture-CKS-light> ;
  skos:notation "CKS" ;
  skos:prefLabel "Clayey coarse sand"@en ;
.
<field-texture-CKS-heavy>
  rdf:type skos:Concept ;
  dct:description "Behaviour of moist bolus: slight coherence; sand grains of medium size; sticky when wet; many sand grains stick to fingers; will form minimal ribbon of 5–15 mm; discolours fingers with clay stain. Coarse sand is obviously coarse to touch. Sand grains are very readily seen with the naked eye." ;
  rdfs:comment "Approximate clay content (%): 5 - 10%" ;
  rdfs:label "Heavy clayey coarse sand" ;
  skos:broader <field-texture-CKS> ;
  skos:broader <field-texture-CS-heavy> ;
  skos:definition "Behaviour of moist bolus: slight coherence; sand grains of medium size; sticky when wet; many sand grains stick to fingers; will form minimal ribbon of 5–15 mm; discolours fingers with clay stain. Coarse sand is obviously coarse to touch. Sand grains are very readily seen with the naked eye." ;
  skos:inScheme <> ;
  skos:notation "CKS+" ;
  skos:prefLabel "Heavy clayey coarse sand"@en ;
.
<field-texture-CKS-light>
  rdf:type skos:Concept ;
  dct:description "Behaviour of moist bolus: slight coherence; sand grains of medium size; sticky when wet; many sand grains stick to fingers; will form minimal ribbon of 5–15 mm; discolours fingers with clay stain. Coarse sand is obviously coarse to touch. Sand grains are very readily seen with the naked eye." ;
  rdfs:comment "Approximate clay content (%): 5 - 10%" ;
  rdfs:label "Light clayey coarse sand" ;
  skos:broader <field-texture-CKS> ;
  skos:broader <field-texture-CS-light> ;
  skos:definition "Behaviour of moist bolus: slight coherence; sand grains of medium size; sticky when wet; many sand grains stick to fingers; will form minimal ribbon of 5–15 mm; discolours fingers with clay stain. Coarse sand is obviously coarse to touch. Sand grains are very readily seen with the naked eye." ;
  skos:inScheme <> ;
  skos:notation "CKS-" ;
  skos:prefLabel "Light clayey coarse sand"@en ;
.
<field-texture-CL>
  rdf:type skos:Concept ;
  dct:description "Behaviour of moist bolus: coherent plastic bolus, smooth to manipulate; will form ribbon of 40–50 mm." ;
  ui:isMemberOf <field-texture-mineral> ;
  rdfs:comment "Approximate clay content (%): 30 - 35%" ;
  rdfs:label "Clay Loam" ;
  skos:definition "Behaviour of moist bolus: coherent plastic bolus, smooth to manipulate; will form ribbon of 40–50 mm." ;
  skos:narrower <field-texture-CL-A> ;
  skos:narrower <field-texture-CL-I> ;
  skos:narrower <field-texture-CL-heavy> ;
  skos:narrower <field-texture-CL-light> ;
  skos:notation "CL" ;
  skos:prefLabel "Clay loam"@en ;
  skos:topConceptOf <> ;
.
<field-texture-CL-A>
  rdf:type skos:Concept ;
  dct:description "Behaviour of moist bolus: coherent plastic bolus, smooth to manipulate; will form ribbon of 40–50 mm." ;
  rdfs:comment """Approximate clay content (%): 30 - 35%
Organic and non-fibrous; dark organic stain discolours fingers; greasy feel in clayey textures and coherence in sandy textures. Fibres (excluding living roots) or plant tissue remains are not visible to naked eye and little or none visible with ×10 hand lens.""" ;
  rdfs:label "Sapric clay Loam" ;
  skos:broader <field-texture-CL> ;
  skos:definition "Behaviour of moist bolus: coherent plastic bolus, smooth to manipulate; will form ribbon of 40–50 mm." ;
  skos:inScheme <> ;
  skos:notation "CLA" ;
  skos:prefLabel "Sapric clay loam"@en ;
.
<field-texture-CL-I>
  rdf:type skos:Concept ;
  dct:description "Behaviour of moist bolus: coherent plastic bolus, smooth to manipulate; will form ribbon of 40–50 mm." ;
  rdfs:comment """Approximate clay content (%): 30 - 35%
Organic and fibrous; dark organic stain discolours fingers; greasy feel in clayey textures and coherence in sandy textures. Fibres (excluding living roots) or plant tissue remain visible to naked eye or easily visible with ×10 hand lens.""" ;
  rdfs:label "Fibric clay Loam" ;
  skos:broader <field-texture-CL> ;
  skos:definition "Behaviour of moist bolus: coherent plastic bolus, smooth to manipulate; will form ribbon of 40–50 mm." ;
  skos:inScheme <> ;
  skos:notation "CLI" ;
  skos:prefLabel "Fibric clay loam"@en ;
.
<field-texture-CL-heavy>
  rdf:type skos:Concept ;
  dct:description "Behaviour of moist bolus: coherent plastic bolus, smooth to manipulate; will form ribbon of 40–50 mm." ;
  rdfs:comment "Approximate clay content (%): 30 - 35%" ;
  rdfs:label "Heavy clay Loam" ;
  skos:broader <field-texture-CL> ;
  skos:definition "Behaviour of moist bolus: coherent plastic bolus, smooth to manipulate; will form ribbon of 40–50 mm." ;
  skos:inScheme <> ;
  skos:notation "CL+" ;
  skos:prefLabel "Heavy clay loam"@en ;
.
<field-texture-CL-light>
  rdf:type skos:Concept ;
  dct:description "Behaviour of moist bolus: coherent plastic bolus, smooth to manipulate; will form ribbon of 40–50 mm." ;
  rdfs:comment "Approximate clay content (%): 30 - 35%" ;
  rdfs:label "Light clay Loam" ;
  skos:broader <field-texture-CL> ;
  skos:definition "Behaviour of moist bolus: coherent plastic bolus, smooth to manipulate; will form ribbon of 40–50 mm." ;
  skos:inScheme <> ;
  skos:notation "CL-" ;
  skos:prefLabel "Light clay loam"@en ;
.
<field-texture-CLFS>
  rdf:type skos:Concept ;
  dct:description "Behaviour of moist bolus: coherent plastic bolus; medium-size sand grains visible in finer matrix; will form ribbon of 40–50 mm. Fine sand can be felt and often heard when manipulated. Sand grains are clearly evident under a ×10 hand lens." ;
  rdfs:comment "Approximate clay content (%): 30 - 35%" ;
  rdfs:label "Clay loam, fine sandy" ;
  skos:broader <field-texture-CLS> ;
  skos:definition "Behaviour of moist bolus: coherent plastic bolus; medium-size sand grains visible in finer matrix; will form ribbon of 40–50 mm. Fine sand can be felt and often heard when manipulated. Sand grains are clearly evident under a ×10 hand lens." ;
  skos:inScheme <> ;
  skos:narrower <field-texture-CLFS-A> ;
  skos:narrower <field-texture-CLFS-I> ;
  skos:narrower <field-texture-CLFS-heavy> ;
  skos:narrower <field-texture-CLFS-light> ;
  skos:notation "CLFS" ;
  skos:prefLabel "Clay loam, fine sandy"@en ;
.
<field-texture-CLFS-A>
  rdf:type skos:Concept ;
  dct:description "Behaviour of moist bolus: coherent plastic bolus; medium-size sand grains visible in finer matrix; will form ribbon of 40–50 mm." ;
  rdfs:comment """Approximate clay content (%): 30 - 35%
Organic and non-fibrous; dark organic stain discolours fingers; greasy feel in clayey textures and coherence in sandy textures. Fibres (excluding living roots) or plant tissue remains are not visible to naked eye and little or none visible with ×10 hand lens.""" ;
  rdfs:label "Sapric clay loam, fine sandy" ;
  skos:broader <field-texture-CLFS> ;
  skos:broader <field-texture-CLS-A> ;
  skos:definition "Behaviour of moist bolus: coherent plastic bolus; medium-size sand grains visible in finer matrix; will form ribbon of 40–50 mm." ;
  skos:inScheme <> ;
  skos:notation "CLFSA" ;
  skos:prefLabel "Sapric clay loam, fine sandy"@en ;
.
<field-texture-CLFS-I>
  rdf:type skos:Concept ;
  dct:description "Behaviour of moist bolus: coherent plastic bolus; medium-size sand grains visible in finer matrix; will form ribbon of 40–50 mm." ;
  rdfs:comment """Approximate clay content (%): 30 - 35%
Organic and fibrous; dark organic stain discolours fingers; greasy feel in clayey textures and coherence in sandy textures. Fibres (excluding living roots) or plant tissue remain visible to naked eye or easily visible with ×10 hand lens.""" ;
  rdfs:label "Fibric clay loam, fine sandy" ;
  skos:broader <field-texture-CLFS> ;
  skos:broader <field-texture-CLS-I> ;
  skos:definition "Behaviour of moist bolus: coherent plastic bolus; medium-size sand grains visible in finer matrix; will form ribbon of 40–50 mm." ;
  skos:inScheme <> ;
  skos:notation "CLFSI" ;
  skos:prefLabel "Fibric clay loam, fine sandy"@en ;
.
<field-texture-CLFS-heavy>
  rdf:type skos:Concept ;
  dct:description "Behaviour of moist bolus: coherent plastic bolus; medium-size sand grains visible in finer matrix; will form ribbon of 40–50 mm. Fine sand can be felt and often heard when manipulated. Sand grains are clearly evident under a ×10 hand lens." ;
  rdfs:comment "Approximate clay content (%): 30 - 35%" ;
  rdfs:label "Heavy clay loam, fine sandy" ;
  skos:broader <field-texture-CLFS> ;
  skos:broader <field-texture-CLS-heavy> ;
  skos:definition "Behaviour of moist bolus: coherent plastic bolus; medium-size sand grains visible in finer matrix; will form ribbon of 40–50 mm. Fine sand can be felt and often heard when manipulated. Sand grains are clearly evident under a ×10 hand lens." ;
  skos:inScheme <> ;
  skos:notation "CLFS+" ;
  skos:prefLabel "Heavy clay loam, fine sandy"@en ;
.
<field-texture-CLFS-light>
  rdf:type skos:Concept ;
  dct:description "Behaviour of moist bolus: coherent plastic bolus; medium-size sand grains visible in finer matrix; will form ribbon of 40–50 mm. Fine sand can be felt and often heard when manipulated. Sand grains are clearly evident under a ×10 hand lens." ;
  rdfs:comment "Approximate clay content (%): 30 - 35%" ;
  rdfs:label "Light clay loam, fine sandy" ;
  skos:broader <field-texture-CLFS> ;
  skos:broader <field-texture-CLS-light> ;
  skos:definition "Behaviour of moist bolus: coherent plastic bolus; medium-size sand grains visible in finer matrix; will form ribbon of 40–50 mm. Fine sand can be felt and often heard when manipulated. Sand grains are clearly evident under a ×10 hand lens." ;
  skos:inScheme <> ;
  skos:notation "CLFS-" ;
  skos:prefLabel "Light clay loam, fine sandy"@en ;
.
<field-texture-CLKS>
  rdf:type skos:Concept ;
  dct:description "Behaviour of moist bolus: coherent plastic bolus; medium-size sand grains visible in finer matrix; will form ribbon of 40–50 mm. Coarse sand is obviously coarse to touch. Sand grains are very readily seen with the naked eye." ;
  rdfs:comment "Approximate clay content (%): 30 - 35%" ;
  rdfs:label "Clay loam, coarse sandy" ;
  skos:broader <field-texture-CLS> ;
  skos:definition "Behaviour of moist bolus: coherent plastic bolus; medium-size sand grains visible in finer matrix; will form ribbon of 40–50 mm. Coarse sand is obviously coarse to touch. Sand grains are very readily seen with the naked eye." ;
  skos:inScheme <> ;
  skos:narrower <field-texture-CLKS-A> ;
  skos:narrower <field-texture-CLKS-I> ;
  skos:narrower <field-texture-CLKS-heavy> ;
  skos:narrower <field-texture-CLKS-light> ;
  skos:notation "CLKS" ;
  skos:prefLabel "Clay loam, coarse sandy"@en ;
.
<field-texture-CLKS-A>
  rdf:type skos:Concept ;
  dct:description "Behaviour of moist bolus: coherent plastic bolus; medium-size sand grains visible in finer matrix; will form ribbon of 40–50 mm." ;
  rdfs:comment """Approximate clay content (%): 30 - 35%
Organic and non-fibrous; dark organic stain discolours fingers; greasy feel in clayey textures and coherence in sandy textures. Fibres (excluding living roots) or plant tissue remains are not visible to naked eye and little or none visible with ×10 hand lens.""" ;
  rdfs:label "Sapric clay loam, coarse sandy" ;
  skos:broader <field-texture-CLKS> ;
  skos:broader <field-texture-CLS-A> ;
  skos:definition "Behaviour of moist bolus: coherent plastic bolus; medium-size sand grains visible in finer matrix; will form ribbon of 40–50 mm." ;
  skos:inScheme <> ;
  skos:notation "CLKS-A" ;
  skos:prefLabel "Sapric clay loam, coarse sandy"@en ;
.
<field-texture-CLKS-I>
  rdf:type skos:Concept ;
  dct:description "Behaviour of moist bolus: coherent plastic bolus; medium-size sand grains visible in finer matrix; will form ribbon of 40–50 mm." ;
  rdfs:comment """Approximate clay content (%): 30 - 35%
Organic and fibrous; dark organic stain discolours fingers; greasy feel in clayey textures and coherence in sandy textures. Fibres (excluding living roots) or plant tissue remain visible to naked eye or easily visible with ×10 hand lens.""" ;
  rdfs:label "Fibric clay loam, coarse sandy" ;
  skos:broader <field-texture-CLKS> ;
  skos:broader <field-texture-CLS-I> ;
  skos:definition "Behaviour of moist bolus: coherent plastic bolus; medium-size sand grains visible in finer matrix; will form ribbon of 40–50 mm." ;
  skos:inScheme <> ;
  skos:notation "CLKS-I" ;
  skos:prefLabel "Fibric clay loam, coarse sandy"@en ;
.
<field-texture-CLKS-heavy>
  rdf:type skos:Concept ;
  dct:description "Behaviour of moist bolus: coherent plastic bolus; medium-size sand grains visible in finer matrix; will form ribbon of 40–50 mm. Coarse sand is obviously coarse to touch. Sand grains are very readily seen with the naked eye." ;
  rdfs:comment "Approximate clay content (%): 30 - 35%" ;
  rdfs:label "Heavy clay loam, coarse sandy" ;
  skos:broader <field-texture-CLKS> ;
  skos:broader <field-texture-CLS-heavy> ;
  skos:definition "Behaviour of moist bolus: coherent plastic bolus; medium-size sand grains visible in finer matrix; will form ribbon of 40–50 mm. Coarse sand is obviously coarse to touch. Sand grains are very readily seen with the naked eye." ;
  skos:inScheme <> ;
  skos:notation "CLKS+" ;
  skos:prefLabel "Heavy clay loam, coarse sandy"@en ;
.
<field-texture-CLKS-light>
  rdf:type skos:Concept ;
  dct:description "Behaviour of moist bolus: coherent plastic bolus; medium-size sand grains visible in finer matrix; will form ribbon of 40–50 mm. Coarse sand is obviously coarse to touch. Sand grains are very readily seen with the naked eye." ;
  rdfs:comment "Approximate clay content (%): 30 - 35%" ;
  rdfs:label "Light clay loam, coarse sandy" ;
  skos:broader <field-texture-CLKS> ;
  skos:broader <field-texture-CLS-light> ;
  skos:definition "Behaviour of moist bolus: coherent plastic bolus; medium-size sand grains visible in finer matrix; will form ribbon of 40–50 mm. Coarse sand is obviously coarse to touch. Sand grains are very readily seen with the naked eye." ;
  skos:inScheme <> ;
  skos:notation "CLKS-" ;
  skos:prefLabel "Light clay loam, coarse sandy"@en ;
.
<field-texture-CLS>
  rdf:type skos:Concept ;
  dct:description "Behaviour of moist bolus: coherent plastic bolus; medium-size sand grains visible in finer matrix; will form ribbon of 40–50 mm." ;
  ui:isMemberOf <field-texture-mineral> ;
  rdfs:comment "Approximate clay content (%): 30 - 35%" ;
  rdfs:label "Clay loam, sandy" ;
  skos:definition "Behaviour of moist bolus: coherent plastic bolus; medium-size sand grains visible in finer matrix; will form ribbon of 40–50 mm." ;
  skos:narrower <field-texture-CLFS> ;
  skos:narrower <field-texture-CLKS> ;
  skos:narrower <field-texture-CLS-A> ;
  skos:narrower <field-texture-CLS-I> ;
  skos:narrower <field-texture-CLS-heavy> ;
  skos:narrower <field-texture-CLS-light> ;
  skos:notation "CLS" ;
  skos:prefLabel "Clay loam, sandy"@en ;
  skos:topConceptOf <> ;
.
<field-texture-CLS-A>
  rdf:type skos:Concept ;
  dct:description "Behaviour of moist bolus: coherent plastic bolus; medium-size sand grains visible in finer matrix; will form ribbon of 40–50 mm." ;
  rdfs:comment """Approximate clay content (%): 30 - 35%
Organic and non-fibrous; dark organic stain discolours fingers; greasy feel in clayey textures and coherence in sandy textures. Fibres (excluding living roots) or plant tissue remains are not visible to naked eye and little or none visible with ×10 hand lens.""" ;
  rdfs:label "Sapric clay loam, sandy" ;
  skos:broader <field-texture-CLS> ;
  skos:definition "Behaviour of moist bolus: coherent plastic bolus; medium-size sand grains visible in finer matrix; will form ribbon of 40–50 mm." ;
  skos:inScheme <> ;
  skos:narrower <field-texture-CLFS-A> ;
  skos:narrower <field-texture-CLKS-A> ;
  skos:notation "CLS-A" ;
  skos:prefLabel "Sapric clay loam, sandy"@en ;
.
<field-texture-CLS-I>
  rdf:type skos:Concept ;
  dct:description "Behaviour of moist bolus: coherent plastic bolus; medium-size sand grains visible in finer matrix; will form ribbon of 40–50 mm." ;
  rdfs:comment """Approximate clay content (%): 30 - 35%
Organic and fibrous; dark organic stain discolours fingers; greasy feel in clayey textures and coherence in sandy textures. Fibres (excluding living roots) or plant tissue remain visible to naked eye or easily visible with ×10 hand lens.""" ;
  rdfs:label "Fibric clay loam, sandy" ;
  skos:broader <field-texture-CLS> ;
  skos:definition "Behaviour of moist bolus: coherent plastic bolus; medium-size sand grains visible in finer matrix; will form ribbon of 40–50 mm." ;
  skos:inScheme <> ;
  skos:narrower <field-texture-CLFS-I> ;
  skos:narrower <field-texture-CLKS-I> ;
  skos:notation "CLS-I" ;
  skos:prefLabel "Fibric clay loam, sandy"@en ;
.
<field-texture-CLS-heavy>
  rdf:type skos:Concept ;
  dct:description "Behaviour of moist bolus: coherent plastic bolus; medium-size sand grains visible in finer matrix; will form ribbon of 40–50 mm." ;
  rdfs:comment "Approximate clay content (%): 30 - 35%" ;
  rdfs:label "Heavy clay loam, sandy" ;
  skos:broader <field-texture-CLS> ;
  skos:definition "Behaviour of moist bolus: coherent plastic bolus; medium-size sand grains visible in finer matrix; will form ribbon of 40–50 mm." ;
  skos:inScheme <> ;
  skos:narrower <field-texture-CLFS-heavy> ;
  skos:narrower <field-texture-CLKS-heavy> ;
  skos:notation "CLS+" ;
  skos:prefLabel "Heavy clay loam, sandy"@en ;
.
<field-texture-CLS-light>
  rdf:type skos:Concept ;
  dct:description "Behaviour of moist bolus: coherent plastic bolus; medium-size sand grains visible in finer matrix; will form ribbon of 40–50 mm." ;
  rdfs:comment "Approximate clay content (%): 30 - 35%" ;
  rdfs:label "Light clay loam, sandy" ;
  skos:broader <field-texture-CLS> ;
  skos:definition "Behaviour of moist bolus: coherent plastic bolus; medium-size sand grains visible in finer matrix; will form ribbon of 40–50 mm." ;
  skos:inScheme <> ;
  skos:narrower <field-texture-CLFS-light> ;
  skos:narrower <field-texture-CLKS-light> ;
  skos:notation "CLS-" ;
  skos:prefLabel "Light clay loam, sandy"@en ;
.
<field-texture-CP>
  rdf:type skos:Concept ;
  dct:description "Organic soils where: bolus has obvious fine mineral particle content, is sticky when wet, and is coherent." ;
  ui:isMemberOf <field-texture-organic> ;
  rdfs:label "Clayey peat" ;
  skos:definition "Organic soils where: bolus has obvious fine mineral particle content, is sticky when wet, and is coherent." ;
  skos:notation "CP" ;
  skos:prefLabel "Clayey peat"@en ;
  skos:topConceptOf <> ;
.
<field-texture-CS>
  rdf:type skos:Concept ;
  dct:description "Behaviour of moist bolus: slight coherence; sand grains of medium size; sticky when wet; many sand grains stick to fingers; will form minimal ribbon of 5–15 mm; discolours fingers with clay stain." ;
  ui:isMemberOf <field-texture-mineral> ;
  rdfs:comment "Approximate clay content (%): 5 - 10%" ;
  rdfs:label "Clayey sand" ;
  skos:definition "Behaviour of moist bolus: slight coherence; sand grains of medium size; sticky when wet; many sand grains stick to fingers; will form minimal ribbon of 5–15 mm; discolours fingers with clay stain." ;
  skos:narrower <field-texture-CFS> ;
  skos:narrower <field-texture-CKS> ;
  skos:narrower <field-texture-CS-heavy> ;
  skos:narrower <field-texture-CS-light> ;
  skos:notation "CS" ;
  skos:prefLabel "Clayey sand"@en ;
  skos:topConceptOf <> ;
.
<field-texture-CS-heavy>
  rdf:type skos:Concept ;
  dct:description "Behaviour of moist bolus: slight coherence; sand grains of medium size; sticky when wet; many sand grains stick to fingers; will form minimal ribbon of 5–15 mm; discolours fingers with clay stain." ;
  rdfs:comment "Approximate clay content (%): 5 - 10%" ;
  rdfs:label "Heavy clayey sand" ;
  skos:broader <field-texture-CS> ;
  skos:definition "Behaviour of moist bolus: slight coherence; sand grains of medium size; sticky when wet; many sand grains stick to fingers; will form minimal ribbon of 5–15 mm; discolours fingers with clay stain." ;
  skos:inScheme <> ;
  skos:narrower <field-texture-CFS-heavy> ;
  skos:narrower <field-texture-CKS-heavy> ;
  skos:notation "CS+" ;
  skos:prefLabel "Heavy clayey sand"@en ;
.
<field-texture-CS-light>
  rdf:type skos:Concept ;
  dct:description "Behaviour of moist bolus: slight coherence; sand grains of medium size; sticky when wet; many sand grains stick to fingers; will form minimal ribbon of 5–15 mm; discolours fingers with clay stain." ;
  rdfs:comment "Approximate clay content (%): 5 - 10%" ;
  rdfs:label "Light clayey sand" ;
  skos:broader <field-texture-CS> ;
  skos:definition "Behaviour of moist bolus: slight coherence; sand grains of medium size; sticky when wet; many sand grains stick to fingers; will form minimal ribbon of 5–15 mm; discolours fingers with clay stain." ;
  skos:inScheme <> ;
  skos:narrower <field-texture-CFS-light> ;
  skos:narrower <field-texture-CKS-light> ;
  skos:notation "CS-" ;
  skos:prefLabel "Light clayey sand"@en ;
.
<field-texture-FS>
  rdf:type skos:Concept ;
  dct:description "Behaviour of moist bolus: coherence nil to very slight, cannot be moulded; sand grains of medium size; single sand grains adhere to fingers. Fine sand can be felt and often heard when manipulated. Sand grains are clearly evident under a ×10 hand lens." ;
  rdfs:comment "Approximate clay content (%): commonly less than 5%" ;
  rdfs:label "Fine sand" ;
  skos:broader <field-texture-S> ;
  skos:definition "Behaviour of moist bolus: coherence nil to very slight, cannot be moulded; sand grains of medium size; single sand grains adhere to fingers. Fine sand can be felt and often heard when manipulated. Sand grains are clearly evident under a ×10 hand lens." ;
  skos:inScheme <> ;
  skos:narrower <field-texture-FS-A> ;
  skos:narrower <field-texture-FS-I> ;
  skos:notation "FS" ;
  skos:prefLabel "Fine sand"@en ;
.
<field-texture-FS-A>
  rdf:type skos:Concept ;
  dct:description "Behaviour of moist bolus: coherence nil to very slight, cannot be moulded; sand grains of medium size; single sand grains adhere to fingers. Fine sand can be felt and often heard when manipulated. Sand grains are clearly evident under a ×10 hand lens." ;
  rdfs:comment "Approximate clay content (%): commonly less than 5%" ;
  rdfs:label "Sapric fine sand" ;
  skos:broader <field-texture-FS> ;
  skos:broader <field-texture-S-A> ;
  skos:definition "Behaviour of moist bolus: coherence nil to very slight, cannot be moulded; sand grains of medium size; single sand grains adhere to fingers. Fine sand can be felt and often heard when manipulated. Sand grains are clearly evident under a ×10 hand lens." ;
  skos:inScheme <> ;
  skos:notation "FSA" ;
  skos:prefLabel "Sapric fine sand"@en ;
.
<field-texture-FS-I>
  rdf:type skos:Concept ;
  dct:description "Behaviour of moist bolus: coherence nil to very slight, cannot be moulded; sand grains of medium size; single sand grains adhere to fingers. Fine sand can be felt and often heard when manipulated. Sand grains are clearly evident under a ×10 hand lens." ;
  rdfs:comment "Approximate clay content (%): commonly less than 5%" ;
  rdfs:label "Fibric fine sand" ;
  skos:broader <field-texture-FS> ;
  skos:broader <field-texture-S-I> ;
  skos:definition "Behaviour of moist bolus: coherence nil to very slight, cannot be moulded; sand grains of medium size; single sand grains adhere to fingers. Fine sand can be felt and often heard when manipulated. Sand grains are clearly evident under a ×10 hand lens." ;
  skos:inScheme <> ;
  skos:notation "FSI" ;
  skos:prefLabel "Fibric fine sand"@en ;
.
<field-texture-FSCL>
  rdf:type skos:Concept ;
  dct:description "Behaviour of moist bolus: strongly coherent bolus, sandy to touch; medium-size sand grains visible in finer matrix; will form ribbon of 25–40 mm. Fine sand can be felt and often heard when manipulated. Sand grains are clearly evident under a ×10 hand lens." ;
  rdfs:comment "Approximate clay content (%): 20 - 30%" ;
  rdfs:label "Fine sandy clay loam" ;
  skos:broader <field-texture-SCL> ;
  skos:definition "Behaviour of moist bolus: strongly coherent bolus, sandy to touch; medium-size sand grains visible in finer matrix; will form ribbon of 25–40 mm. Fine sand can be felt and often heard when manipulated. Sand grains are clearly evident under a ×10 hand lens." ;
  skos:inScheme <> ;
  skos:narrower <field-texture-FSCL-A> ;
  skos:narrower <field-texture-FSCL-I> ;
  skos:narrower <field-texture-FSCL-heavy> ;
  skos:narrower <field-texture-FSCL-light> ;
  skos:notation "FSCL" ;
  skos:prefLabel "Fine sandy clay loam"@en ;
.
<field-texture-FSCL-A>
  rdf:type skos:Concept ;
  dct:description "Behaviour of moist bolus: strongly coherent bolus, sandy to touch; medium-size sand grains visible in finer matrix; will form ribbon of 25–40 mm. Fine sand can be felt and often heard when manipulated. Sand grains are clearly evident under a ×10 hand lens." ;
  rdfs:comment "Approximate clay content (%): 20 - 30%" ;
  rdfs:label "Sapric fine sandy clay loam" ;
  skos:broader <field-texture-FSCL> ;
  skos:broader <field-texture-SCL-A> ;
  skos:definition "Behaviour of moist bolus: strongly coherent bolus, sandy to touch; medium-size sand grains visible in finer matrix; will form ribbon of 25–40 mm. Fine sand can be felt and often heard when manipulated. Sand grains are clearly evident under a ×10 hand lens." ;
  skos:inScheme <> ;
  skos:notation "FSCLA" ;
  skos:prefLabel "Sapric fine sandy clay loam"@en ;
.
<field-texture-FSCL-I>
  rdf:type skos:Concept ;
  dct:description "Behaviour of moist bolus: strongly coherent bolus, sandy to touch; medium-size sand grains visible in finer matrix; will form ribbon of 25–40 mm. Fine sand can be felt and often heard when manipulated. Sand grains are clearly evident under a ×10 hand lens." ;
  rdfs:comment "Approximate clay content (%): 20 - 30%" ;
  rdfs:label "Fibric fine sandy clay loam" ;
  skos:broader <field-texture-FSCL> ;
  skos:broader <field-texture-SCL-I> ;
  skos:definition "Behaviour of moist bolus: strongly coherent bolus, sandy to touch; medium-size sand grains visible in finer matrix; will form ribbon of 25–40 mm. Fine sand can be felt and often heard when manipulated. Sand grains are clearly evident under a ×10 hand lens." ;
  skos:inScheme <> ;
  skos:notation "FSCLI" ;
  skos:prefLabel "Fibric fine sandy clay loam"@en ;
.
<field-texture-FSCL-heavy>
  rdf:type skos:Concept ;
  dct:description "Behaviour of moist bolus: strongly coherent bolus, sandy to touch; medium-size sand grains visible in finer matrix; will form ribbon of 25–40 mm. Fine sand can be felt and often heard when manipulated. Sand grains are clearly evident under a ×10 hand lens." ;
  rdfs:comment "Approximate clay content (%): 20 - 30%" ;
  rdfs:label "Heavy fine sandy clay loam" ;
  skos:broader <field-texture-FSCL> ;
  skos:broader <field-texture-SCL-heavy> ;
  skos:definition "Behaviour of moist bolus: strongly coherent bolus, sandy to touch; medium-size sand grains visible in finer matrix; will form ribbon of 25–40 mm. Fine sand can be felt and often heard when manipulated. Sand grains are clearly evident under a ×10 hand lens." ;
  skos:inScheme <> ;
  skos:notation "FSCL+" ;
  skos:prefLabel "Heavy fine sandy clay loam"@en ;
.
<field-texture-FSCL-light>
  rdf:type skos:Concept ;
  dct:description "Behaviour of moist bolus: strongly coherent bolus, sandy to touch; medium-size sand grains visible in finer matrix; will form ribbon of 25–40 mm. Fine sand can be felt and often heard when manipulated. Sand grains are clearly evident under a ×10 hand lens." ;
  rdfs:comment "Approximate clay content (%): 20 - 30%" ;
  rdfs:label "Light fine sandy clay loam" ;
  skos:broader <field-texture-FSCL> ;
  skos:broader <field-texture-SCL-light> ;
  skos:definition "Behaviour of moist bolus: strongly coherent bolus, sandy to touch; medium-size sand grains visible in finer matrix; will form ribbon of 25–40 mm. Fine sand can be felt and often heard when manipulated. Sand grains are clearly evident under a ×10 hand lens." ;
  skos:inScheme <> ;
  skos:notation "FSCL-" ;
  skos:prefLabel "Light fine sandy clay loam"@en ;
.
<field-texture-FSHC>
  rdf:type skos:Concept ;
  dct:description "Behaviour of moist bolus: smooth plastic bolus; handles like stiff plasticine; can be moulded into rods without fracture; has firm resistance to ribboning shear; will form ribbon of 75 mm or more." ;
  rdfs:comment "Approximate clay content (%): 50% or more" ;
  rdfs:label "Fine sandy heavy clay" ;
  skos:broader <field-texture-HC> ;
  skos:definition "Behaviour of moist bolus: smooth plastic bolus; handles like stiff plasticine; can be moulded into rods without fracture; has firm resistance to ribboning shear; will form ribbon of 75 mm or more." ;
  skos:inScheme <> ;
  skos:narrower <field-texture-FSHC-A> ;
  skos:narrower <field-texture-FSHC-I> ;
  skos:notation "FSHC" ;
  skos:prefLabel "Fine sandy heavy clay"@en ;
.
<field-texture-FSHC-A>
  rdf:type skos:Concept ;
  dct:description "Behaviour of moist bolus: smooth plastic bolus; handles like stiff plasticine; can be moulded into rods without fracture; has firm resistance to ribboning shear; will form ribbon of 75 mm or more." ;
  rdfs:comment "Approximate clay content (%): 50% or more" ;
  rdfs:label "Sapric fine sandy heavy clay" ;
  skos:broader <field-texture-FSHC> ;
  skos:broader <field-texture-HC-A> ;
  skos:definition "Behaviour of moist bolus: smooth plastic bolus; handles like stiff plasticine; can be moulded into rods without fracture; has firm resistance to ribboning shear; will form ribbon of 75 mm or more." ;
  skos:inScheme <> ;
  skos:notation "FSHCA" ;
  skos:prefLabel "Sapric fine sandy heavy clay"@en ;
.
<field-texture-FSHC-I>
  rdf:type skos:Concept ;
  dct:description "Behaviour of moist bolus: smooth plastic bolus; handles like stiff plasticine; can be moulded into rods without fracture; has firm resistance to ribboning shear; will form ribbon of 75 mm or more." ;
  rdfs:comment "Approximate clay content (%): 50% or more" ;
  rdfs:label "Fibric fine sandy heavy clay" ;
  skos:broader <field-texture-FSHC> ;
  skos:broader <field-texture-HC-I> ;
  skos:definition "Behaviour of moist bolus: smooth plastic bolus; handles like stiff plasticine; can be moulded into rods without fracture; has firm resistance to ribboning shear; will form ribbon of 75 mm or more." ;
  skos:inScheme <> ;
  skos:notation "FSHCI" ;
  skos:prefLabel "Fibric fine sandy heavy clay"@en ;
.
<field-texture-FSL>
  rdf:type skos:Concept ;
  dct:description "Behaviour of moist bolus: bolus coherent but very sandy to touch; will form ribbon of 15–25 mm; dominant sand grains are of medium size and are readily visible. Fine sand can be felt and often heard when manipulated. Sand grains are clearly evident under a ×10 hand lens." ;
  rdfs:comment "Approximate clay content (%): 10 - 20%" ;
  rdfs:label "Fine sandy loam" ;
  skos:broader <field-texture-SL> ;
  skos:definition "Behaviour of moist bolus: bolus coherent but very sandy to touch; will form ribbon of 15–25 mm; dominant sand grains are of medium size and are readily visible. Fine sand can be felt and often heard when manipulated. Sand grains are clearly evident under a ×10 hand lens." ;
  skos:inScheme <> ;
  skos:narrower <field-texture-FSL-A> ;
  skos:narrower <field-texture-FSL-I> ;
  skos:notation "FSL" ;
  skos:prefLabel "Fine sandy loam"@en ;
.
<field-texture-FSL-A>
  rdf:type skos:Concept ;
  dct:description "Behaviour of moist bolus: bolus coherent but very sandy to touch; will form ribbon of 15–25 mm; dominant sand grains are of medium size and are readily visible. Fine sand can be felt and often heard when manipulated. Sand grains are clearly evident under a ×10 hand lens." ;
  rdfs:comment "Approximate clay content (%): 10 - 20%" ;
  rdfs:label "Sapric fine sandy loam" ;
  skos:broader <field-texture-FSL> ;
  skos:broader <field-texture-SL-A> ;
  skos:definition "Behaviour of moist bolus: bolus coherent but very sandy to touch; will form ribbon of 15–25 mm; dominant sand grains are of medium size and are readily visible. Fine sand can be felt and often heard when manipulated. Sand grains are clearly evident under a ×10 hand lens." ;
  skos:inScheme <> ;
  skos:notation "FSLA" ;
  skos:prefLabel "Sapric fine sandy loam"@en ;
.
<field-texture-FSL-I>
  rdf:type skos:Concept ;
  dct:description "Behaviour of moist bolus: bolus coherent but very sandy to touch; will form ribbon of 15–25 mm; dominant sand grains are of medium size and are readily visible. Fine sand can be felt and often heard when manipulated. Sand grains are clearly evident under a ×10 hand lens." ;
  rdfs:comment "Approximate clay content (%): 10 - 20%" ;
  rdfs:label "Fibric fine sandy loam" ;
  skos:broader <field-texture-FSL> ;
  skos:broader <field-texture-SL-I> ;
  skos:definition "Behaviour of moist bolus: bolus coherent but very sandy to touch; will form ribbon of 15–25 mm; dominant sand grains are of medium size and are readily visible. Fine sand can be felt and often heard when manipulated. Sand grains are clearly evident under a ×10 hand lens." ;
  skos:inScheme <> ;
  skos:notation "FSLI" ;
  skos:prefLabel "Fibric fine sandy loam"@en ;
.
<field-texture-FSLC>
  rdf:type skos:Concept ;
  dct:description "Behaviour of moist bolus: plastic bolus; smooth to touch; slight resistance to shearing between thumb and forefinger; will form ribbon of 50–75 mm." ;
  rdfs:comment "Approximate clay content (%): 35 - 40%" ;
  rdfs:label "Fine sandy light clay" ;
  skos:broader <field-texture-LC> ;
  skos:definition "Behaviour of moist bolus: plastic bolus; smooth to touch; slight resistance to shearing between thumb and forefinger; will form ribbon of 50–75 mm." ;
  skos:inScheme <> ;
  skos:narrower <field-texture-FSLC-A> ;
  skos:narrower <field-texture-FSLC-I> ;
  skos:notation "FSLC" ;
  skos:prefLabel "Fine sandy light clay"@en ;
.
<field-texture-FSLC-A>
  rdf:type skos:Concept ;
  dct:description "Behaviour of moist bolus: plastic bolus; smooth to touch; slight resistance to shearing between thumb and forefinger; will form ribbon of 50–75 mm." ;
  rdfs:comment "Approximate clay content (%): 35 - 40%" ;
  rdfs:label "Sapric fine sandy light clay" ;
  skos:broader <field-texture-FSLC> ;
  skos:broader <field-texture-LC-A> ;
  skos:definition "Behaviour of moist bolus: plastic bolus; smooth to touch; slight resistance to shearing between thumb and forefinger; will form ribbon of 50–75 mm." ;
  skos:inScheme <> ;
  skos:notation "FSLCA" ;
  skos:prefLabel "Sapric fine sandy light clay"@en ;
.
<field-texture-FSLC-I>
  rdf:type skos:Concept ;
  dct:description "Behaviour of moist bolus: plastic bolus; smooth to touch; slight resistance to shearing between thumb and forefinger; will form ribbon of 50–75 mm." ;
  rdfs:comment "Approximate clay content (%): 35 - 40%" ;
  rdfs:label "Fibric fine sandy light clay" ;
  skos:broader <field-texture-FSLC> ;
  skos:broader <field-texture-LC-I> ;
  skos:definition "Behaviour of moist bolus: plastic bolus; smooth to touch; slight resistance to shearing between thumb and forefinger; will form ribbon of 50–75 mm." ;
  skos:inScheme <> ;
  skos:notation "FSLCI" ;
  skos:prefLabel "Fibric fine sandy light clay"@en ;
.
<field-texture-FSLMC>
  rdf:type skos:Concept ;
  dct:description "Behaviour of moist bolus: plastic bolus; smooth to touch; slight to moderate resistance to ribboning shear; will form ribbon of about 75 mm." ;
  rdfs:comment "Approximate clay content (%): 40 - 45%" ;
  rdfs:label "Fine sandy light medium clay" ;
  skos:broader <field-texture-LMC> ;
  skos:definition "Behaviour of moist bolus: plastic bolus; smooth to touch; slight to moderate resistance to ribboning shear; will form ribbon of about 75 mm." ;
  skos:inScheme <> ;
  skos:narrower <field-texture-FSLMC-A> ;
  skos:narrower <field-texture-FSLMC-I> ;
  skos:notation "FSLMC" ;
  skos:prefLabel "Fine sandy light medium clay"@en ;
.
<field-texture-FSLMC-A>
  rdf:type skos:Concept ;
  dct:description "Behaviour of moist bolus: plastic bolus; smooth to touch; slight to moderate resistance to ribboning shear; will form ribbon of about 75 mm." ;
  rdfs:comment "Approximate clay content (%): 40 - 45%" ;
  rdfs:label "Sapric fine sandy light medium clay" ;
  skos:broader <field-texture-FSLMC> ;
  skos:broader <field-texture-LMC-A> ;
  skos:definition "Behaviour of moist bolus: plastic bolus; smooth to touch; slight to moderate resistance to ribboning shear; will form ribbon of about 75 mm." ;
  skos:inScheme <> ;
  skos:notation "FSLMCA" ;
  skos:prefLabel "Sapric fine sandy light medium clay"@en ;
.
<field-texture-FSLMC-I>
  rdf:type skos:Concept ;
  dct:description "Behaviour of moist bolus: plastic bolus; smooth to touch; slight to moderate resistance to ribboning shear; will form ribbon of about 75 mm." ;
  rdfs:comment "Approximate clay content (%): 40 - 45%" ;
  rdfs:label "Fibric fine sandy light medium clay" ;
  skos:broader <field-texture-FSLMC> ;
  skos:broader <field-texture-LMC-I> ;
  skos:definition "Behaviour of moist bolus: plastic bolus; smooth to touch; slight to moderate resistance to ribboning shear; will form ribbon of about 75 mm." ;
  skos:inScheme <> ;
  skos:notation "FSLMCI" ;
  skos:prefLabel "Fibric fine sandy light medium clay"@en ;
.
<field-texture-FSMC>
  rdf:type skos:Concept ;
  dct:description "Behaviour of moist bolus: smooth plastic bolus; handles like plasticine and can be moulded into rods without fracture; has moderate resistance to ribboning shear; will form ribbon of 75 mm or more." ;
  rdfs:comment "Approximate clay content (%): 45 - 55%" ;
  rdfs:label "Fine sandy medium clay" ;
  skos:broader <field-texture-MC> ;
  skos:definition "Behaviour of moist bolus: smooth plastic bolus; handles like plasticine and can be moulded into rods without fracture; has moderate resistance to ribboning shear; will form ribbon of 75 mm or more." ;
  skos:inScheme <> ;
  skos:narrower <field-texture-FSMC-A> ;
  skos:narrower <field-texture-FSMC-I> ;
  skos:notation "FSMC" ;
  skos:prefLabel "Fine sandy medium clay"@en ;
.
<field-texture-FSMC-A>
  rdf:type skos:Concept ;
  dct:description "Behaviour of moist bolus: smooth plastic bolus; handles like plasticine and can be moulded into rods without fracture; has moderate resistance to ribboning shear; will form ribbon of 75 mm or more." ;
  rdfs:comment "Approximate clay content (%): 45 - 55%" ;
  rdfs:label "Sapric fine sandy medium clay" ;
  skos:broader <field-texture-FSMC> ;
  skos:broader <field-texture-MC-A> ;
  skos:definition "Behaviour of moist bolus: smooth plastic bolus; handles like plasticine and can be moulded into rods without fracture; has moderate resistance to ribboning shear; will form ribbon of 75 mm or more." ;
  skos:inScheme <> ;
  skos:notation "FSMCA" ;
  skos:prefLabel "Sapric fine sandy medium clay"@en ;
.
<field-texture-FSMC-I>
  rdf:type skos:Concept ;
  dct:description "Behaviour of moist bolus: smooth plastic bolus; handles like plasticine and can be moulded into rods without fracture; has moderate resistance to ribboning shear; will form ribbon of 75 mm or more." ;
  rdfs:comment "Approximate clay content (%): 45 - 55%" ;
  rdfs:label "Fibric fine sandy medium clay" ;
  skos:broader <field-texture-FSMC> ;
  skos:broader <field-texture-MC-I> ;
  skos:definition "Behaviour of moist bolus: smooth plastic bolus; handles like plasticine and can be moulded into rods without fracture; has moderate resistance to ribboning shear; will form ribbon of 75 mm or more." ;
  skos:inScheme <> ;
  skos:notation "FSMCI" ;
  skos:prefLabel "Fibric fine sandy medium clay"@en ;
.
<field-texture-FSMHC>
  rdf:type skos:Concept ;
  dct:description "Behaviour of moist bolus: smooth plastic bolus; handles like plasticine; can be moulded into rods without fracture; has moderate to firm resistance to ribboning shear; will form ribbon of 75 mm or more." ;
  rdfs:comment "Approximate clay content (%): 50% or more" ;
  rdfs:label "Fine sandy medium heavy clay" ;
  skos:broader <field-texture-MHC> ;
  skos:definition "Behaviour of moist bolus: smooth plastic bolus; handles like plasticine; can be moulded into rods without fracture; has moderate to firm resistance to ribboning shear; will form ribbon of 75 mm or more." ;
  skos:inScheme <> ;
  skos:narrower <field-texture-FSMHC-A> ;
  skos:narrower <field-texture-FSMHC-I> ;
  skos:notation "FSMHC" ;
  skos:prefLabel "Fine sandy medium heavy clay"@en ;
.
<field-texture-FSMHC-A>
  rdf:type skos:Concept ;
  dct:description "Behaviour of moist bolus: smooth plastic bolus; handles like plasticine; can be moulded into rods without fracture; has moderate to firm resistance to ribboning shear; will form ribbon of 75 mm or more." ;
  rdfs:comment "Approximate clay content (%): 50% or more" ;
  rdfs:label "Sapric fine sandy medium heavy clay" ;
  skos:broader <field-texture-FSMHC> ;
  skos:broader <field-texture-MHC-A> ;
  skos:definition "Behaviour of moist bolus: smooth plastic bolus; handles like plasticine; can be moulded into rods without fracture; has moderate to firm resistance to ribboning shear; will form ribbon of 75 mm or more." ;
  skos:inScheme <> ;
  skos:notation "FSMHCA" ;
  skos:prefLabel "Sapric fine sandy medium heavy clay"@en ;
.
<field-texture-FSMHC-I>
  rdf:type skos:Concept ;
  dct:description "Behaviour of moist bolus: smooth plastic bolus; handles like plasticine; can be moulded into rods without fracture; has moderate to firm resistance to ribboning shear; will form ribbon of 75 mm or more." ;
  rdfs:comment "Approximate clay content (%): 50% or more" ;
  rdfs:label "Fibric fine sandy medium heavy clay" ;
  skos:broader <field-texture-FSMHC> ;
  skos:broader <field-texture-MHC-I> ;
  skos:definition "Behaviour of moist bolus: smooth plastic bolus; handles like plasticine; can be moulded into rods without fracture; has moderate to firm resistance to ribboning shear; will form ribbon of 75 mm or more." ;
  skos:inScheme <> ;
  skos:notation "FSMHCI" ;
  skos:prefLabel "Fibric fine sandy medium heavy clay"@en ;
.
<field-texture-GP>
  rdf:type skos:Concept ;
  dct:description "Dominantly decomposed organic material, which has dried irreversibly to fine granules through exposure and drying and/or cultivation. Granules are approximately 1–2 mm in diameter and have granular or subangular blocky structure." ;
  ui:isMemberOf <field-texture-organic> ;
  rdfs:comment "On drying, peat may change irreversibly." ;
  rdfs:label "Granular peat" ;
  skos:definition "Dominantly decomposed organic material, which has dried irreversibly to fine granules through exposure and drying and/or cultivation. Granules are approximately 1–2 mm in diameter and have granular or subangular blocky structure." ;
  skos:notation "GP" ;
  skos:prefLabel "Granular peat"@en ;
  skos:topConceptOf <> ;
.
<field-texture-HC>
  rdf:type skos:Concept ;
  dct:description "Behaviour of moist bolus: smooth plastic bolus; handles like stiff plasticine; can be moulded into rods without fracture; has firm resistance to ribboning shear; will form ribbon of 75 mm or more." ;
  ui:isMemberOf <field-texture-mineral> ;
  rdfs:comment "Approximate clay content (%): 50% or more" ;
  rdfs:label "Heavy clay" ;
  skos:definition "Behaviour of moist bolus: smooth plastic bolus; handles like stiff plasticine; can be moulded into rods without fracture; has firm resistance to ribboning shear; will form ribbon of 75 mm or more." ;
  skos:narrower <field-texture-FSHC> ;
  skos:narrower <field-texture-HC-A> ;
  skos:narrower <field-texture-HC-I> ;
  skos:narrower <field-texture-KSHC> ;
  skos:narrower <field-texture-SHC> ;
  skos:narrower <field-texture-ZHC> ;
  skos:notation "HC" ;
  skos:prefLabel "Heavy clay"@en ;
  skos:topConceptOf <> ;
.
<field-texture-HC-A>
  rdf:type skos:Concept ;
  dct:description "Behaviour of moist bolus: smooth plastic bolus; handles like stiff plasticine; can be moulded into rods without fracture; has firm resistance to ribboning shear; will form ribbon of 75 mm or more." ;
  rdfs:comment "Approximate clay content (%): 50% or more" ;
  rdfs:label "Sapric heavy clay" ;
  skos:broader <field-texture-HC> ;
  skos:definition "Behaviour of moist bolus: smooth plastic bolus; handles like stiff plasticine; can be moulded into rods without fracture; has firm resistance to ribboning shear; will form ribbon of 75 mm or more." ;
  skos:inScheme <> ;
  skos:narrower <field-texture-FSHC-A> ;
  skos:narrower <field-texture-KSHC-A> ;
  skos:narrower <field-texture-SHC-A> ;
  skos:narrower <field-texture-ZHC-A> ;
  skos:notation "HCA" ;
  skos:prefLabel "Sapric heavy clay"@en ;
.
<field-texture-HC-I>
  rdf:type skos:Concept ;
  dct:description "Behaviour of moist bolus: smooth plastic bolus; handles like stiff plasticine; can be moulded into rods without fracture; has firm resistance to ribboning shear; will form ribbon of 75 mm or more." ;
  rdfs:comment "Approximate clay content (%): 50% or more" ;
  rdfs:label "Fibric heavy clay" ;
  skos:broader <field-texture-HC> ;
  skos:definition "Behaviour of moist bolus: smooth plastic bolus; handles like stiff plasticine; can be moulded into rods without fracture; has firm resistance to ribboning shear; will form ribbon of 75 mm or more." ;
  skos:inScheme <> ;
  skos:narrower <field-texture-FSHC-I> ;
  skos:narrower <field-texture-KSHC-I> ;
  skos:narrower <field-texture-SHC-I> ;
  skos:narrower <field-texture-ZHC-I> ;
  skos:notation "HCI" ;
  skos:prefLabel "Fibric heavy clay"@en ;
.
<field-texture-HP>
  rdf:type skos:Concept ;
  dct:description "Moderately to well decomposed organic material. Plant remains vary from most being difficult to identify to most being unidentifiable. It is intermediate in degree of decomposition between the less decomposed fibric peat and the more decomposed sapric peat." ;
  ui:isMemberOf <field-texture-organic> ;
  rdfs:comment "Semi-fibrous peat" ;
  rdfs:label "Hemic peat" ;
  skos:definition "Moderately to well decomposed organic material. Plant remains vary from most being difficult to identify to most being unidentifiable. It is intermediate in degree of decomposition between the less decomposed fibric peat and the more decomposed sapric peat." ;
  skos:notation "HP" ;
  skos:prefLabel "Hemic peat"@en ;
  skos:topConceptOf <> ;
.
<field-texture-IP>
  rdf:type skos:Concept ;
  dct:description "Undecomposed or weakly decomposed organic material. Plant remains are distinct and readily identifiable." ;
  ui:isMemberOf <field-texture-organic> ;
  rdfs:comment "Fibrous peat" ;
  rdfs:label "Fibric peat" ;
  skos:definition "Undecomposed or weakly decomposed organic material. Plant remains are distinct and readily identifiable." ;
  skos:notation "IP" ;
  skos:prefLabel "Fibric peat"@en ;
  skos:topConceptOf <> ;
.
<field-texture-KS>
  rdf:type skos:Concept ;
  dct:description "Behaviour of moist bolus: coherence nil to very slight, cannot be moulded; sand grains of medium size; single sand grains adhere to fingers. Coarse sand is obviously coarse to touch. Sand grains are very readily seen with the naked eye." ;
  rdfs:comment "Approximate clay content (%): commonly less than 5%" ;
  rdfs:label "Coarse sand" ;
  skos:broader <field-texture-S> ;
  skos:definition "Behaviour of moist bolus: coherence nil to very slight, cannot be moulded; sand grains of medium size; single sand grains adhere to fingers. Coarse sand is obviously coarse to touch. Sand grains are very readily seen with the naked eye." ;
  skos:inScheme <> ;
  skos:narrower <field-texture-KS-A> ;
  skos:narrower <field-texture-KS-I> ;
  skos:notation "KS" ;
  skos:prefLabel "Coarse sand"@en ;
.
<field-texture-KS-A>
  rdf:type skos:Concept ;
  dct:description "Behaviour of moist bolus: coherence nil to very slight, cannot be moulded; sand grains of medium size; single sand grains adhere to fingers. Coarse sand is obviously coarse to touch. Sand grains are very readily seen with the naked eye." ;
  rdfs:comment "Approximate clay content (%): commonly less than 5%" ;
  rdfs:label "Sapric coarse sand" ;
  skos:broader <field-texture-KS> ;
  skos:broader <field-texture-S-A> ;
  skos:definition "Behaviour of moist bolus: coherence nil to very slight, cannot be moulded; sand grains of medium size; single sand grains adhere to fingers. Coarse sand is obviously coarse to touch. Sand grains are very readily seen with the naked eye." ;
  skos:inScheme <> ;
  skos:notation "KSA" ;
  skos:prefLabel "Sapric coarse sand"@en ;
.
<field-texture-KS-I>
  rdf:type skos:Concept ;
  dct:description "Behaviour of moist bolus: coherence nil to very slight, cannot be moulded; sand grains of medium size; single sand grains adhere to fingers. Coarse sand is obviously coarse to touch. Sand grains are very readily seen with the naked eye." ;
  rdfs:comment "Approximate clay content (%): commonly less than 5%" ;
  rdfs:label "Fibric coarse sand" ;
  skos:broader <field-texture-KS> ;
  skos:broader <field-texture-S-I> ;
  skos:definition "Behaviour of moist bolus: coherence nil to very slight, cannot be moulded; sand grains of medium size; single sand grains adhere to fingers. Coarse sand is obviously coarse to touch. Sand grains are very readily seen with the naked eye." ;
  skos:inScheme <> ;
  skos:notation "KSI" ;
  skos:prefLabel "Fibric coarse sand"@en ;
.
<field-texture-KSCL>
  rdf:type skos:Concept ;
  dct:description "Behaviour of moist bolus: strongly coherent bolus, sandy to touch; medium-size sand grains visible in finer matrix; will form ribbon of 25–40 mm. Coarse sand is obviously coarse to touch. Sand grains are very readily seen with the naked eye." ;
  rdfs:comment "Approximate clay content (%): 20 - 30%" ;
  rdfs:label "Coarse sandy clay loam" ;
  skos:broader <field-texture-SCL> ;
  skos:definition "Behaviour of moist bolus: strongly coherent bolus, sandy to touch; medium-size sand grains visible in finer matrix; will form ribbon of 25–40 mm. Coarse sand is obviously coarse to touch. Sand grains are very readily seen with the naked eye." ;
  skos:inScheme <> ;
  skos:narrower <field-texture-KSCL-A> ;
  skos:narrower <field-texture-KSCL-I> ;
  skos:narrower <field-texture-KSCL-heavy> ;
  skos:narrower <field-texture-KSCL-light> ;
  skos:notation "KSCL" ;
  skos:prefLabel "Coarse sandy clay loam"@en ;
.
<field-texture-KSCL-A>
  rdf:type skos:Concept ;
  dct:description "Behaviour of moist bolus: strongly coherent bolus, sandy to touch; medium-size sand grains visible in finer matrix; will form ribbon of 25–40 mm. Coarse sand is obviously coarse to touch. Sand grains are very readily seen with the naked eye." ;
  rdfs:comment "Approximate clay content (%): 20 - 30%" ;
  rdfs:label "Sapric coarse sandy clay loam" ;
  skos:broader <field-texture-KSCL> ;
  skos:broader <field-texture-SCL-A> ;
  skos:definition "Behaviour of moist bolus: strongly coherent bolus, sandy to touch; medium-size sand grains visible in finer matrix; will form ribbon of 25–40 mm. Coarse sand is obviously coarse to touch. Sand grains are very readily seen with the naked eye." ;
  skos:inScheme <> ;
  skos:notation "KSCLA" ;
  skos:prefLabel "Sapric coarse sandy clay loam"@en ;
.
<field-texture-KSCL-I>
  rdf:type skos:Concept ;
  dct:description "Behaviour of moist bolus: strongly coherent bolus, sandy to touch; medium-size sand grains visible in finer matrix; will form ribbon of 25–40 mm. Coarse sand is obviously coarse to touch. Sand grains are very readily seen with the naked eye." ;
  rdfs:comment "Approximate clay content (%): 20 - 30%" ;
  rdfs:label "Fibric coarse sandy clay loam" ;
  skos:broader <field-texture-KSCL> ;
  skos:broader <field-texture-SCL-I> ;
  skos:definition "Behaviour of moist bolus: strongly coherent bolus, sandy to touch; medium-size sand grains visible in finer matrix; will form ribbon of 25–40 mm. Coarse sand is obviously coarse to touch. Sand grains are very readily seen with the naked eye." ;
  skos:inScheme <> ;
  skos:notation "KSCLI" ;
  skos:prefLabel "Fibric coarse sandy clay loam"@en ;
.
<field-texture-KSCL-heavy>
  rdf:type skos:Concept ;
  dct:description "Behaviour of moist bolus: strongly coherent bolus, sandy to touch; medium-size sand grains visible in finer matrix; will form ribbon of 25–40 mm. Coarse sand is obviously coarse to touch. Sand grains are very readily seen with the naked eye." ;
  rdfs:comment "Approximate clay content (%): 20 - 30%" ;
  rdfs:label "Heavy coarse sandy clay loam" ;
  skos:broader <field-texture-KSCL> ;
  skos:broader <field-texture-SCL-heavy> ;
  skos:definition "Behaviour of moist bolus: strongly coherent bolus, sandy to touch; medium-size sand grains visible in finer matrix; will form ribbon of 25–40 mm. Coarse sand is obviously coarse to touch. Sand grains are very readily seen with the naked eye." ;
  skos:inScheme <> ;
  skos:notation "KSCL+" ;
  skos:prefLabel "Heavy coarse sandy clay loam"@en ;
.
<field-texture-KSCL-light>
  rdf:type skos:Concept ;
  dct:description "Behaviour of moist bolus: strongly coherent bolus, sandy to touch; medium-size sand grains visible in finer matrix; will form ribbon of 25–40 mm. Coarse sand is obviously coarse to touch. Sand grains are very readily seen with the naked eye." ;
  rdfs:comment "Approximate clay content (%): 20 - 30%" ;
  rdfs:label "Light coarse sandy clay loam" ;
  skos:broader <field-texture-KSCL> ;
  skos:broader <field-texture-SCL-light> ;
  skos:definition "Behaviour of moist bolus: strongly coherent bolus, sandy to touch; medium-size sand grains visible in finer matrix; will form ribbon of 25–40 mm. Coarse sand is obviously coarse to touch. Sand grains are very readily seen with the naked eye." ;
  skos:inScheme <> ;
  skos:notation "KSCL-" ;
  skos:prefLabel "Light coarse sandy clay loam"@en ;
.
<field-texture-KSHC>
  rdf:type skos:Concept ;
  dct:description "Behaviour of moist bolus: smooth plastic bolus; handles like stiff plasticine; can be moulded into rods without fracture; has firm resistance to ribboning shear; will form ribbon of 75 mm or more." ;
  rdfs:comment "Approximate clay content (%): 50% or more" ;
  rdfs:label "Coarse sandy heavy clay" ;
  skos:broader <field-texture-HC> ;
  skos:definition "Behaviour of moist bolus: smooth plastic bolus; handles like stiff plasticine; can be moulded into rods without fracture; has firm resistance to ribboning shear; will form ribbon of 75 mm or more." ;
  skos:inScheme <> ;
  skos:narrower <field-texture-KSHC-A> ;
  skos:narrower <field-texture-KSHC-I> ;
  skos:notation "KSHC" ;
  skos:prefLabel "Coarse sandy heavy clay"@en ;
.
<field-texture-KSHC-A>
  rdf:type skos:Concept ;
  dct:description "Behaviour of moist bolus: smooth plastic bolus; handles like stiff plasticine; can be moulded into rods without fracture; has firm resistance to ribboning shear; will form ribbon of 75 mm or more." ;
  rdfs:comment "Approximate clay content (%): 50% or more" ;
  rdfs:label "Sapric coarse sandy heavy clay" ;
  skos:broader <field-texture-HC-A> ;
  skos:broader <field-texture-KSHC> ;
  skos:definition "Behaviour of moist bolus: smooth plastic bolus; handles like stiff plasticine; can be moulded into rods without fracture; has firm resistance to ribboning shear; will form ribbon of 75 mm or more." ;
  skos:inScheme <> ;
  skos:notation "KSHCA" ;
  skos:prefLabel "Sapric coarse sandy heavy clay"@en ;
.
<field-texture-KSHC-I>
  rdf:type skos:Concept ;
  dct:description "Behaviour of moist bolus: smooth plastic bolus; handles like stiff plasticine; can be moulded into rods without fracture; has firm resistance to ribboning shear; will form ribbon of 75 mm or more." ;
  rdfs:comment "Approximate clay content (%): 50% or more" ;
  rdfs:label "Fibric coarse sandy heavy clay" ;
  skos:broader <field-texture-HC-I> ;
  skos:broader <field-texture-KSHC> ;
  skos:definition "Behaviour of moist bolus: smooth plastic bolus; handles like stiff plasticine; can be moulded into rods without fracture; has firm resistance to ribboning shear; will form ribbon of 75 mm or more." ;
  skos:inScheme <> ;
  skos:notation "KSHCI" ;
  skos:prefLabel "Fibric coarse sandy heavy clay"@en ;
.
<field-texture-KSL>
  rdf:type skos:Concept ;
  dct:description "Behaviour of moist bolus: bolus coherent but very sandy to touch; will form ribbon of 15–25 mm; dominant sand grains are of medium size and are readily visible. Coarse sand is obviously coarse to touch. Sand grains are very readily seen with the naked eye." ;
  rdfs:comment "Approximate clay content (%): 10 - 20%" ;
  rdfs:label "Coarse sandy loam" ;
  skos:broader <field-texture-SL> ;
  skos:definition "Behaviour of moist bolus: bolus coherent but very sandy to touch; will form ribbon of 15–25 mm; dominant sand grains are of medium size and are readily visible. Coarse sand is obviously coarse to touch. Sand grains are very readily seen with the naked eye." ;
  skos:inScheme <> ;
  skos:narrower <field-texture-KSL-A> ;
  skos:narrower <field-texture-KSL-I> ;
  skos:notation "KSL" ;
  skos:prefLabel "Coarse sandy loam"@en ;
.
<field-texture-KSL-A>
  rdf:type skos:Concept ;
  dct:description "Behaviour of moist bolus: bolus coherent but very sandy to touch; will form ribbon of 15–25 mm; dominant sand grains are of medium size and are readily visible. Coarse sand is obviously coarse to touch. Sand grains are very readily seen with the naked eye." ;
  rdfs:comment "Approximate clay content (%): 10 - 20%" ;
  rdfs:label "Sapric coarse sandy loam" ;
  skos:broader <field-texture-KSL> ;
  skos:broader <field-texture-SL-A> ;
  skos:definition "Behaviour of moist bolus: bolus coherent but very sandy to touch; will form ribbon of 15–25 mm; dominant sand grains are of medium size and are readily visible. Coarse sand is obviously coarse to touch. Sand grains are very readily seen with the naked eye." ;
  skos:inScheme <> ;
  skos:notation "KSLA" ;
  skos:prefLabel "Sapric coarse sandy loam"@en ;
.
<field-texture-KSL-I>
  rdf:type skos:Concept ;
  dct:description "Behaviour of moist bolus: bolus coherent but very sandy to touch; will form ribbon of 15–25 mm; dominant sand grains are of medium size and are readily visible. Coarse sand is obviously coarse to touch. Sand grains are very readily seen with the naked eye." ;
  rdfs:comment "Approximate clay content (%): 10 - 20%" ;
  rdfs:label "Fibric coarse sandy loam" ;
  skos:broader <field-texture-KSL> ;
  skos:broader <field-texture-SL-I> ;
  skos:definition "Behaviour of moist bolus: bolus coherent but very sandy to touch; will form ribbon of 15–25 mm; dominant sand grains are of medium size and are readily visible. Coarse sand is obviously coarse to touch. Sand grains are very readily seen with the naked eye." ;
  skos:inScheme <> ;
  skos:notation "KSLI" ;
  skos:prefLabel "Fibric coarse sandy loam"@en ;
.
<field-texture-KSLC>
  rdf:type skos:Concept ;
  dct:description "Behaviour of moist bolus: plastic bolus; smooth to touch; slight resistance to shearing between thumb and forefinger; will form ribbon of 50–75 mm." ;
  rdfs:comment "Approximate clay content (%): 35 - 40%" ;
  rdfs:label "Coarse sandy light clay" ;
  skos:broader <field-texture-LC> ;
  skos:definition "Behaviour of moist bolus: plastic bolus; smooth to touch; slight resistance to shearing between thumb and forefinger; will form ribbon of 50–75 mm." ;
  skos:inScheme <> ;
  skos:narrower <field-texture-KSLC-A> ;
  skos:narrower <field-texture-KSLC-I> ;
  skos:notation "KSLC" ;
  skos:prefLabel "Coarse sandy light clay"@en ;
.
<field-texture-KSLC-A>
  rdf:type skos:Concept ;
  dct:description "Behaviour of moist bolus: plastic bolus; smooth to touch; slight resistance to shearing between thumb and forefinger; will form ribbon of 50–75 mm." ;
  rdfs:comment "Approximate clay content (%): 35 - 40%" ;
  rdfs:label "Sapric coarse sandy light clay" ;
  skos:broader <field-texture-KSLC> ;
  skos:broader <field-texture-LC-A> ;
  skos:definition "Behaviour of moist bolus: plastic bolus; smooth to touch; slight resistance to shearing between thumb and forefinger; will form ribbon of 50–75 mm." ;
  skos:inScheme <> ;
  skos:notation "KSLCA" ;
  skos:prefLabel "Sapric coarse sandy light clay"@en ;
.
<field-texture-KSLC-I>
  rdf:type skos:Concept ;
  dct:description "Behaviour of moist bolus: plastic bolus; smooth to touch; slight resistance to shearing between thumb and forefinger; will form ribbon of 50–75 mm." ;
  rdfs:comment "Approximate clay content (%): 35 - 40%" ;
  rdfs:label "Fibric coarse sandy light clay" ;
  skos:broader <field-texture-KSLC> ;
  skos:broader <field-texture-LC-I> ;
  skos:definition "Behaviour of moist bolus: plastic bolus; smooth to touch; slight resistance to shearing between thumb and forefinger; will form ribbon of 50–75 mm." ;
  skos:inScheme <> ;
  skos:notation "KSLCI" ;
  skos:prefLabel "Fibric coarse sandy light clay"@en ;
.
<field-texture-KSLMC>
  rdf:type skos:Concept ;
  dct:description "Behaviour of moist bolus: plastic bolus; smooth to touch; slight to moderate resistance to ribboning shear; will form ribbon of about 75 mm." ;
  rdfs:comment "Approximate clay content (%): 40 - 45%" ;
  rdfs:label "Coarse sandy light medium clay" ;
  skos:broader <field-texture-LMC> ;
  skos:definition "Behaviour of moist bolus: plastic bolus; smooth to touch; slight to moderate resistance to ribboning shear; will form ribbon of about 75 mm." ;
  skos:inScheme <> ;
  skos:narrower <field-texture-KSLMC-A> ;
  skos:narrower <field-texture-KSLMC-I> ;
  skos:notation "KSLMC" ;
  skos:prefLabel "Coarse sandy light medium clay"@en ;
.
<field-texture-KSLMC-A>
  rdf:type skos:Concept ;
  dct:description "Behaviour of moist bolus: plastic bolus; smooth to touch; slight to moderate resistance to ribboning shear; will form ribbon of about 75 mm." ;
  rdfs:comment "Approximate clay content (%): 40 - 45%" ;
  rdfs:label "Sapric coarse sandy light medium clay" ;
  skos:broader <field-texture-KSLMC> ;
  skos:broader <field-texture-LMC-A> ;
  skos:definition "Behaviour of moist bolus: plastic bolus; smooth to touch; slight to moderate resistance to ribboning shear; will form ribbon of about 75 mm." ;
  skos:inScheme <> ;
  skos:notation "KSLMCA" ;
  skos:prefLabel "Sapric coarse sandy light medium clay"@en ;
.
<field-texture-KSLMC-I>
  rdf:type skos:Concept ;
  dct:description "Behaviour of moist bolus: plastic bolus; smooth to touch; slight to moderate resistance to ribboning shear; will form ribbon of about 75 mm." ;
  rdfs:comment "Approximate clay content (%): 40 - 45%" ;
  rdfs:label "Fibric coarse sandy light medium clay" ;
  skos:broader <field-texture-KSLMC> ;
  skos:broader <field-texture-LMC-I> ;
  skos:definition "Behaviour of moist bolus: plastic bolus; smooth to touch; slight to moderate resistance to ribboning shear; will form ribbon of about 75 mm." ;
  skos:inScheme <> ;
  skos:notation "KSLMCI" ;
  skos:prefLabel "Fibric coarse sandy light medium clay"@en ;
.
<field-texture-KSMC>
  rdf:type skos:Concept ;
  dct:description "Behaviour of moist bolus: smooth plastic bolus; handles like plasticine and can be moulded into rods without fracture; has moderate resistance to ribboning shear; will form ribbon of 75 mm or more." ;
  rdfs:comment "Approximate clay content (%): 45 - 55%" ;
  rdfs:label "Coarse sandy medium clay" ;
  skos:broader <field-texture-MC> ;
  skos:definition "Behaviour of moist bolus: smooth plastic bolus; handles like plasticine and can be moulded into rods without fracture; has moderate resistance to ribboning shear; will form ribbon of 75 mm or more." ;
  skos:inScheme <> ;
  skos:narrower <field-texture-KSMC-A> ;
  skos:narrower <field-texture-KSMC-I> ;
  skos:notation "KSMC" ;
  skos:prefLabel "Coarse sandy medium clay"@en ;
.
<field-texture-KSMC-A>
  rdf:type skos:Concept ;
  dct:description "Behaviour of moist bolus: smooth plastic bolus; handles like plasticine and can be moulded into rods without fracture; has moderate resistance to ribboning shear; will form ribbon of 75 mm or more." ;
  rdfs:comment "Approximate clay content (%): 45 - 55%" ;
  rdfs:label "Sapric coarse sandy medium clay" ;
  skos:broader <field-texture-KSMC> ;
  skos:broader <field-texture-MC-A> ;
  skos:definition "Behaviour of moist bolus: smooth plastic bolus; handles like plasticine and can be moulded into rods without fracture; has moderate resistance to ribboning shear; will form ribbon of 75 mm or more." ;
  skos:inScheme <> ;
  skos:notation "KSMCA" ;
  skos:prefLabel "Sapric coarse sandy medium clay"@en ;
.
<field-texture-KSMC-I>
  rdf:type skos:Concept ;
  dct:description "Behaviour of moist bolus: smooth plastic bolus; handles like plasticine and can be moulded into rods without fracture; has moderate resistance to ribboning shear; will form ribbon of 75 mm or more." ;
  rdfs:comment "Approximate clay content (%): 45 - 55%" ;
  rdfs:label "Fibric coarse sandy medium clay" ;
  skos:broader <field-texture-KSMC> ;
  skos:broader <field-texture-MC-I> ;
  skos:definition "Behaviour of moist bolus: smooth plastic bolus; handles like plasticine and can be moulded into rods without fracture; has moderate resistance to ribboning shear; will form ribbon of 75 mm or more." ;
  skos:inScheme <> ;
  skos:notation "KSMCI" ;
  skos:prefLabel "Fibric coarse sandy medium clay"@en ;
.
<field-texture-KSMHC>
  rdf:type skos:Concept ;
  dct:description "Behaviour of moist bolus: smooth plastic bolus; handles like plasticine; can be moulded into rods without fracture; has moderate to firm resistance to ribboning shear; will form ribbon of 75 mm or more." ;
  rdfs:comment "Approximate clay content (%): 50% or more" ;
  rdfs:label "Coarse sandy medium heavy clay" ;
  skos:broader <field-texture-MHC> ;
  skos:definition "Behaviour of moist bolus: smooth plastic bolus; handles like plasticine; can be moulded into rods without fracture; has moderate to firm resistance to ribboning shear; will form ribbon of 75 mm or more." ;
  skos:inScheme <> ;
  skos:narrower <field-texture-KSMHC-A> ;
  skos:narrower <field-texture-KSMHC-I> ;
  skos:notation "KSMHC" ;
  skos:prefLabel "Coarse sandy medium heavy clay"@en ;
.
<field-texture-KSMHC-A>
  rdf:type skos:Concept ;
  dct:description "Behaviour of moist bolus: smooth plastic bolus; handles like plasticine; can be moulded into rods without fracture; has moderate to firm resistance to ribboning shear; will form ribbon of 75 mm or more." ;
  rdfs:comment "Approximate clay content (%): 50% or more" ;
  rdfs:label "Sapric coarse sandy medium heavy clay" ;
  skos:broader <field-texture-KSMHC> ;
  skos:broader <field-texture-MHC-A> ;
  skos:definition "Behaviour of moist bolus: smooth plastic bolus; handles like plasticine; can be moulded into rods without fracture; has moderate to firm resistance to ribboning shear; will form ribbon of 75 mm or more." ;
  skos:inScheme <> ;
  skos:notation "KSMHCA" ;
  skos:prefLabel "Sapric coarse sandy medium heavy clay"@en ;
.
<field-texture-KSMHC-I>
  rdf:type skos:Concept ;
  dct:description "Behaviour of moist bolus: smooth plastic bolus; handles like plasticine; can be moulded into rods without fracture; has moderate to firm resistance to ribboning shear; will form ribbon of 75 mm or more." ;
  rdfs:comment "Approximate clay content (%): 50% or more" ;
  rdfs:label "Fibric coarse sandy medium heavy clay" ;
  skos:broader <field-texture-KSMHC> ;
  skos:broader <field-texture-MHC-I> ;
  skos:definition "Behaviour of moist bolus: smooth plastic bolus; handles like plasticine; can be moulded into rods without fracture; has moderate to firm resistance to ribboning shear; will form ribbon of 75 mm or more." ;
  skos:inScheme <> ;
  skos:notation "KSMHCI" ;
  skos:prefLabel "Fibric coarse sandy medium heavy clay"@en ;
.
<field-texture-L>
  rdf:type skos:Concept ;
  dct:description "Behaviour of moist bolus: bolus coherent and rather spongy; smooth feel when manipulated but with no obvious sandiness or ‘silkiness’; may be somewhat greasy to the touch if much organic matter present; will form ribbon of about 25 mm." ;
  ui:isMemberOf <field-texture-mineral> ;
  rdfs:comment "Approximate clay content (%): about 25%" ;
  rdfs:label "Loam" ;
  skos:definition "Behaviour of moist bolus: bolus coherent and rather spongy; smooth feel when manipulated but with no obvious sandiness or ‘silkiness’; may be somewhat greasy to the touch if much organic matter present; will form ribbon of about 25 mm." ;
  skos:narrower <field-texture-L-A> ;
  skos:narrower <field-texture-L-I> ;
  skos:notation "L" ;
  skos:prefLabel "Loam"@en ;
  skos:topConceptOf <> ;
.
<field-texture-L-A>
  rdf:type skos:Concept ;
  dct:description "Behaviour of moist bolus: bolus coherent and rather spongy; smooth feel when manipulated but with no obvious sandiness or ‘silkiness’; may be somewhat greasy to the touch if much organic matter present; will form ribbon of about 25 mm." ;
  rdfs:comment """Approximate clay content (%): about 25%
Organic and non-fibrous; dark organic stain discolours fingers; greasy feel in clayey textures and coherence in sandy textures. Fibres (excluding living roots) or plant tissue remains are not visible to naked eye and little or none visible with ×10 hand lens.""" ;
  rdfs:label "Sapric loam" ;
  skos:broader <field-texture-L> ;
  skos:definition "Behaviour of moist bolus: bolus coherent and rather spongy; smooth feel when manipulated but with no obvious sandiness or ‘silkiness’; may be somewhat greasy to the touch if much organic matter present; will form ribbon of about 25 mm." ;
  skos:inScheme <> ;
  skos:notation "LA" ;
  skos:prefLabel "Sapric loam"@en ;
.
<field-texture-L-I>
  rdf:type skos:Concept ;
  dct:description "Behaviour of moist bolus: bolus coherent and rather spongy; smooth feel when manipulated but with no obvious sandiness or ‘silkiness’; may be somewhat greasy to the touch if much organic matter present; will form ribbon of about 25 mm." ;
  rdfs:comment """Approximate clay content (%): about 25%
Organic and fibrous; dark organic stain discolours fingers; greasy feel in clayey textures and coherence in sandy textures. Fibres (excluding living roots) or plant tissue remain visible to naked eye or easily visible with ×10 hand lens.""" ;
  rdfs:label "Fibric loam" ;
  skos:broader <field-texture-L> ;
  skos:definition "Behaviour of moist bolus: bolus coherent and rather spongy; smooth feel when manipulated but with no obvious sandiness or ‘silkiness’; may be somewhat greasy to the touch if much organic matter present; will form ribbon of about 25 mm." ;
  skos:inScheme <> ;
  skos:notation "LI" ;
  skos:prefLabel "Fibric loam"@en ;
.
<field-texture-LC>
  rdf:type skos:Concept ;
  dct:description "Behaviour of moist bolus: plastic bolus; smooth to touch; slight resistance to shearing between thumb and forefinger; will form ribbon of 50–75 mm." ;
  ui:isMemberOf <field-texture-mineral> ;
  rdfs:comment "Approximate clay content (%): 35 - 40%" ;
  rdfs:label "Light clay" ;
  skos:definition "Behaviour of moist bolus: plastic bolus; smooth to touch; slight resistance to shearing between thumb and forefinger; will form ribbon of 50–75 mm." ;
  skos:narrower <field-texture-FSLC> ;
  skos:narrower <field-texture-KSLC> ;
  skos:narrower <field-texture-LC-A> ;
  skos:narrower <field-texture-LC-I> ;
  skos:narrower <field-texture-SLC> ;
  skos:narrower <field-texture-ZLC> ;
  skos:notation "LC" ;
  skos:prefLabel "Light clay"@en ;
  skos:topConceptOf <> ;
.
<field-texture-LC-A>
  rdf:type skos:Concept ;
  dct:description "Behaviour of moist bolus: plastic bolus; smooth to touch; slight resistance to shearing between thumb and forefinger; will form ribbon of 50–75 mm." ;
  rdfs:comment "Approximate clay content (%): 35 - 40%" ;
  rdfs:label "Sapric light clay" ;
  skos:broader <field-texture-LC> ;
  skos:definition "Behaviour of moist bolus: plastic bolus; smooth to touch; slight resistance to shearing between thumb and forefinger; will form ribbon of 50–75 mm." ;
  skos:inScheme <> ;
  skos:narrower <field-texture-FSLC-A> ;
  skos:narrower <field-texture-KSLC-A> ;
  skos:narrower <field-texture-SLC-A> ;
  skos:narrower <field-texture-ZLC-A> ;
  skos:notation "LCA" ;
  skos:prefLabel "Sapric light clay"@en ;
.
<field-texture-LC-I>
  rdf:type skos:Concept ;
  dct:description "Behaviour of moist bolus: plastic bolus; smooth to touch; slight resistance to shearing between thumb and forefinger; will form ribbon of 50–75 mm." ;
  rdfs:comment "Approximate clay content (%): 35 - 40%" ;
  rdfs:label "Fibric light clay" ;
  skos:broader <field-texture-LC> ;
  skos:definition "Behaviour of moist bolus: plastic bolus; smooth to touch; slight resistance to shearing between thumb and forefinger; will form ribbon of 50–75 mm." ;
  skos:inScheme <> ;
  skos:narrower <field-texture-FSLC-I> ;
  skos:narrower <field-texture-KSLC-I> ;
  skos:narrower <field-texture-SLC-I> ;
  skos:narrower <field-texture-ZLC-I> ;
  skos:notation "LCI" ;
  skos:prefLabel "Fibric light clay"@en ;
.
<field-texture-LFS>
  rdf:type skos:Concept ;
  dct:description "Behaviour of moist bolus: slight coherence; sand grains of medium size; can be sheared between thumb and forefinger to give minimal ribbon of about 5 mm. Fine sand can be felt and often heard when manipulated. Sand grains are clearly evident under a ×10 hand lens." ;
  rdfs:comment "Approximate clay content (%): about 5%" ;
  rdfs:label "Loamy fine sand" ;
  skos:broader <field-texture-LS> ;
  skos:definition "Behaviour of moist bolus: slight coherence; sand grains of medium size; can be sheared between thumb and forefinger to give minimal ribbon of about 5 mm. Fine sand can be felt and often heard when manipulated. Sand grains are clearly evident under a ×10 hand lens." ;
  skos:inScheme <> ;
  skos:narrower <field-texture-LFS-A> ;
  skos:narrower <field-texture-LFS-I> ;
  skos:notation "LFS" ;
  skos:prefLabel "Loamy fine sand"@en ;
.
<field-texture-LFS-A>
  rdf:type skos:Concept ;
  dct:description "Behaviour of moist bolus: slight coherence; sand grains of medium size; can be sheared between thumb and forefinger to give minimal ribbon of about 5 mm." ;
  rdfs:comment """Approximate clay content (%): about 5%
Organic and non-fibrous; dark organic stain discolours fingers; greasy feel in clayey textures and coherence in sandy textures. Fibres (excluding living roots) or plant tissue remains are not visible to naked eye and little or none visible with ×10 hand lens.""" ;
  rdfs:label "Sapric loamy fine sand" ;
  skos:broader <field-texture-LFS> ;
  skos:broader <field-texture-LS-A> ;
  skos:definition "Behaviour of moist bolus: slight coherence; sand grains of medium size; can be sheared between thumb and forefinger to give minimal ribbon of about 5 mm." ;
  skos:inScheme <> ;
  skos:notation "LFSA" ;
  skos:prefLabel "Sapric loamy fine sand"@en ;
.
<field-texture-LFS-I>
  rdf:type skos:Concept ;
  dct:description "Behaviour of moist bolus: slight coherence; sand grains of medium size; can be sheared between thumb and forefinger to give minimal ribbon of about 5 mm." ;
  rdfs:comment """Approximate clay content (%): about 5%
Organic and fibrous; dark organic stain discolours fingers; greasy feel in clayey textures and coherence in sandy textures. Fibres (excluding living roots) or plant tissue remain visible to naked eye or easily visible with ×10 hand lens.""" ;
  rdfs:label "Fibric loamy fine sand" ;
  skos:broader <field-texture-LFS> ;
  skos:broader <field-texture-LS-I> ;
  skos:definition "Behaviour of moist bolus: slight coherence; sand grains of medium size; can be sheared between thumb and forefinger to give minimal ribbon of about 5 mm." ;
  skos:inScheme <> ;
  skos:notation "LFSI" ;
  skos:prefLabel "Fibric loamy fine sand"@en ;
.
<field-texture-LKS>
  rdf:type skos:Concept ;
  dct:description "Behaviour of moist bolus: slight coherence; sand grains of medium size; can be sheared between thumb and forefinger to give minimal ribbon of about 5 mm. Coarse sand is obviously coarse to touch. Sand grains are very readily seen with the naked eye." ;
  rdfs:comment "Approximate clay content (%): about 5%" ;
  rdfs:label "Loamy coarse sand" ;
  skos:broader <field-texture-LS> ;
  skos:definition "Behaviour of moist bolus: slight coherence; sand grains of medium size; can be sheared between thumb and forefinger to give minimal ribbon of about 5 mm. Coarse sand is obviously coarse to touch. Sand grains are very readily seen with the naked eye." ;
  skos:inScheme <> ;
  skos:narrower <field-texture-LKS-A> ;
  skos:narrower <field-texture-LKS-I> ;
  skos:notation "LKS" ;
  skos:prefLabel "Loamy coarse sand"@en ;
.
<field-texture-LKS-A>
  rdf:type skos:Concept ;
  dct:description "Behaviour of moist bolus: slight coherence; sand grains of medium size; can be sheared between thumb and forefinger to give minimal ribbon of about 5 mm." ;
  rdfs:comment """Approximate clay content (%): about 5%
Organic and non-fibrous; dark organic stain discolours fingers; greasy feel in clayey textures and coherence in sandy textures. Fibres (excluding living roots) or plant tissue remains are not visible to naked eye and little or none visible with ×10 hand lens.""" ;
  rdfs:label "Sapric loamy coarse sand" ;
  skos:broader <field-texture-LKS> ;
  skos:broader <field-texture-LS-A> ;
  skos:definition "Behaviour of moist bolus: slight coherence; sand grains of medium size; can be sheared between thumb and forefinger to give minimal ribbon of about 5 mm." ;
  skos:inScheme <> ;
  skos:notation "LKSA" ;
  skos:prefLabel "Sapric loamy coarse sand"@en ;
.
<field-texture-LKS-I>
  rdf:type skos:Concept ;
  dct:description "Behaviour of moist bolus: slight coherence; sand grains of medium size; can be sheared between thumb and forefinger to give minimal ribbon of about 5 mm." ;
  rdfs:comment """Approximate clay content (%): about 5%
Organic and fibrous; dark organic stain discolours fingers; greasy feel in clayey textures and coherence in sandy textures. Fibres (excluding living roots) or plant tissue remain visible to naked eye or easily visible with ×10 hand lens.""" ;
  rdfs:label "Fibric loamy coarse sand" ;
  skos:broader <field-texture-LKS> ;
  skos:broader <field-texture-LS-I> ;
  skos:definition "Behaviour of moist bolus: slight coherence; sand grains of medium size; can be sheared between thumb and forefinger to give minimal ribbon of about 5 mm." ;
  skos:inScheme <> ;
  skos:notation "LKSI" ;
  skos:prefLabel "Fibric loamy coarse sand"@en ;
.
<field-texture-LMC>
  rdf:type skos:Concept ;
  dct:description "Behaviour of moist bolus: plastic bolus; smooth to touch; slight to moderate resistance to ribboning shear; will form ribbon of about 75 mm." ;
  ui:isMemberOf <field-texture-mineral> ;
  rdfs:comment "Approximate clay content (%): 40 - 45%" ;
  rdfs:label "Light medium clay" ;
  skos:definition "Behaviour of moist bolus: plastic bolus; smooth to touch; slight to moderate resistance to ribboning shear; will form ribbon of about 75 mm." ;
  skos:narrower <field-texture-FSLMC> ;
  skos:narrower <field-texture-KSLMC> ;
  skos:narrower <field-texture-LMC-A> ;
  skos:narrower <field-texture-LMC-I> ;
  skos:narrower <field-texture-SLMC> ;
  skos:narrower <field-texture-ZLMC> ;
  skos:notation "LMC" ;
  skos:prefLabel "Light medium clay"@en ;
  skos:topConceptOf <> ;
.
<field-texture-LMC-A>
  rdf:type skos:Concept ;
  dct:description "Behaviour of moist bolus: plastic bolus; smooth to touch; slight to moderate resistance to ribboning shear; will form ribbon of about 75 mm." ;
  rdfs:comment "Approximate clay content (%): 40 - 45%" ;
  rdfs:label "Sapric light medium clay" ;
  skos:broader <field-texture-LMC> ;
  skos:definition "Behaviour of moist bolus: plastic bolus; smooth to touch; slight to moderate resistance to ribboning shear; will form ribbon of about 75 mm." ;
  skos:inScheme <> ;
  skos:narrower <field-texture-FSLMC-A> ;
  skos:narrower <field-texture-KSLMC-A> ;
  skos:narrower <field-texture-SLMC-A> ;
  skos:narrower <field-texture-ZLMC-A> ;
  skos:notation "LMCA" ;
  skos:prefLabel "Sapric light medium clay"@en ;
.
<field-texture-LMC-I>
  rdf:type skos:Concept ;
  dct:description "Behaviour of moist bolus: plastic bolus; smooth to touch; slight to moderate resistance to ribboning shear; will form ribbon of about 75 mm." ;
  rdfs:comment "Approximate clay content (%): 40 - 45%" ;
  rdfs:label "Fibric light medium clay" ;
  skos:broader <field-texture-LMC> ;
  skos:definition "Behaviour of moist bolus: plastic bolus; smooth to touch; slight to moderate resistance to ribboning shear; will form ribbon of about 75 mm." ;
  skos:inScheme <> ;
  skos:narrower <field-texture-FSLMC-I> ;
  skos:narrower <field-texture-KSLMC-I> ;
  skos:narrower <field-texture-SLMC-I> ;
  skos:narrower <field-texture-ZLMC-I> ;
  skos:notation "LMCI" ;
  skos:prefLabel "Fibric light medium clay"@en ;
.
<field-texture-LP>
  rdf:type skos:Concept ;
  dct:description "Organic soils where: bolus has obvious mineral particle content but no obvious sandiness to touch and is smooth, non-sticky when wet, and weakly coherent." ;
  ui:isMemberOf <field-texture-organic> ;
  rdfs:label "Loamy peat" ;
  skos:definition "Organic soils where: bolus has obvious mineral particle content but no obvious sandiness to touch and is smooth, non-sticky when wet, and weakly coherent." ;
  skos:notation "LP" ;
  skos:prefLabel "Loamy peat"@en ;
  skos:topConceptOf <> ;
.
<field-texture-LS>
  rdf:type skos:Concept ;
  dct:description "Behaviour of moist bolus: slight coherence; sand grains of medium size; can be sheared between thumb and forefinger to give minimal ribbon of about 5 mm." ;
  ui:isMemberOf <field-texture-mineral> ;
  rdfs:comment "Approximate clay content (%): about 5%" ;
  rdfs:label "Loamy sand" ;
  skos:definition "Behaviour of moist bolus: slight coherence; sand grains of medium size; can be sheared between thumb and forefinger to give minimal ribbon of about 5 mm." ;
  skos:narrower <field-texture-LFS> ;
  skos:narrower <field-texture-LKS> ;
  skos:narrower <field-texture-LS-A> ;
  skos:narrower <field-texture-LS-I> ;
  skos:notation "LS" ;
  skos:prefLabel "Loamy sand"@en ;
  skos:topConceptOf <> ;
.
<field-texture-LS-A>
  rdf:type skos:Concept ;
  dct:description "Behaviour of moist bolus: slight coherence; sand grains of medium size; can be sheared between thumb and forefinger to give minimal ribbon of about 5 mm." ;
  rdfs:comment """Approximate clay content (%): about 5%
Organic and non-fibrous; dark organic stain discolours fingers; greasy feel in clayey textures and coherence in sandy textures. Fibres (excluding living roots) or plant tissue remains are not visible to naked eye and little or none visible with ×10 hand lens.""" ;
  rdfs:label "Sapric loamy sand" ;
  skos:broader <field-texture-LS> ;
  skos:definition "Behaviour of moist bolus: slight coherence; sand grains of medium size; can be sheared between thumb and forefinger to give minimal ribbon of about 5 mm." ;
  skos:inScheme <> ;
  skos:narrower <field-texture-LFS-A> ;
  skos:narrower <field-texture-LKS-A> ;
  skos:notation "LSA" ;
  skos:prefLabel "Sapric loamy sand"@en ;
.
<field-texture-LS-I>
  rdf:type skos:Concept ;
  dct:description "Behaviour of moist bolus: slight coherence; sand grains of medium size; can be sheared between thumb and forefinger to give minimal ribbon of about 5 mm." ;
  rdfs:comment """Approximate clay content (%): about 5%
Organic and fibrous; dark organic stain discolours fingers; greasy feel in clayey textures and coherence in sandy textures. Fibres (excluding living roots) or plant tissue remain visible to naked eye or easily visible with ×10 hand lens.""" ;
  rdfs:label "Fibric loamy sand" ;
  skos:broader <field-texture-LS> ;
  skos:definition "Behaviour of moist bolus: slight coherence; sand grains of medium size; can be sheared between thumb and forefinger to give minimal ribbon of about 5 mm." ;
  skos:inScheme <> ;
  skos:narrower <field-texture-LFS-I> ;
  skos:narrower <field-texture-LKS-I> ;
  skos:notation "LSI" ;
  skos:prefLabel "Fibric loamy sand"@en ;
.
<field-texture-MC>
  rdf:type skos:Concept ;
  dct:description "Behaviour of moist bolus: smooth plastic bolus; handles like plasticine and can be moulded into rods without fracture; has moderate resistance to ribboning shear; will form ribbon of 75 mm or more." ;
  ui:isMemberOf <field-texture-mineral> ;
  rdfs:comment "Approximate clay content (%): 45 - 55%" ;
  rdfs:label "Medium clay" ;
  skos:definition "Behaviour of moist bolus: smooth plastic bolus; handles like plasticine and can be moulded into rods without fracture; has moderate resistance to ribboning shear; will form ribbon of 75 mm or more." ;
  skos:narrower <field-texture-FSMC> ;
  skos:narrower <field-texture-KSMC> ;
  skos:narrower <field-texture-MC-A> ;
  skos:narrower <field-texture-MC-I> ;
  skos:narrower <field-texture-SMC> ;
  skos:narrower <field-texture-ZMC> ;
  skos:notation "MC" ;
  skos:prefLabel "Medium clay"@en ;
  skos:topConceptOf <> ;
.
<field-texture-MC-A>
  rdf:type skos:Concept ;
  dct:description "Behaviour of moist bolus: smooth plastic bolus; handles like plasticine and can be moulded into rods without fracture; has moderate resistance to ribboning shear; will form ribbon of 75 mm or more." ;
  rdfs:comment "Approximate clay content (%): 45 - 55%" ;
  rdfs:label "Sapric medium clay" ;
  skos:broader <field-texture-MC> ;
  skos:definition "Behaviour of moist bolus: smooth plastic bolus; handles like plasticine and can be moulded into rods without fracture; has moderate resistance to ribboning shear; will form ribbon of 75 mm or more." ;
  skos:inScheme <> ;
  skos:narrower <field-texture-FSMC-A> ;
  skos:narrower <field-texture-KSMC-A> ;
  skos:narrower <field-texture-SMC-A> ;
  skos:narrower <field-texture-ZMC-A> ;
  skos:notation "MCA" ;
  skos:prefLabel "Sapric medium clay"@en ;
.
<field-texture-MC-I>
  rdf:type skos:Concept ;
  dct:description "Behaviour of moist bolus: smooth plastic bolus; handles like plasticine and can be moulded into rods without fracture; has moderate resistance to ribboning shear; will form ribbon of 75 mm or more." ;
  rdfs:comment "Approximate clay content (%): 45 - 55%" ;
  rdfs:label "Fibric medium clay" ;
  skos:broader <field-texture-MC> ;
  skos:definition "Behaviour of moist bolus: smooth plastic bolus; handles like plasticine and can be moulded into rods without fracture; has moderate resistance to ribboning shear; will form ribbon of 75 mm or more." ;
  skos:inScheme <> ;
  skos:narrower <field-texture-FSMC-I> ;
  skos:narrower <field-texture-KSMC-I> ;
  skos:narrower <field-texture-SMC-I> ;
  skos:narrower <field-texture-ZMC-I> ;
  skos:notation "MCI" ;
  skos:prefLabel "Fibric medium clay"@en ;
.
<field-texture-MHC>
  rdf:type skos:Concept ;
  dct:description "Behaviour of moist bolus: smooth plastic bolus; handles like plasticine; can be moulded into rods without fracture; has moderate to firm resistance to ribboning shear; will form ribbon of 75 mm or more." ;
  ui:isMemberOf <field-texture-mineral> ;
  rdfs:comment "Approximate clay content (%): 50% or more" ;
  rdfs:label "Medium heavy clay" ;
  skos:definition "Behaviour of moist bolus: smooth plastic bolus; handles like plasticine; can be moulded into rods without fracture; has moderate to firm resistance to ribboning shear; will form ribbon of 75 mm or more." ;
  skos:narrower <field-texture-FSMHC> ;
  skos:narrower <field-texture-KSMHC> ;
  skos:narrower <field-texture-MHC-A> ;
  skos:narrower <field-texture-MHC-I> ;
  skos:narrower <field-texture-SMHC> ;
  skos:narrower <field-texture-ZMHC> ;
  skos:notation "MHC" ;
  skos:prefLabel "Medium heavy clay"@en ;
  skos:topConceptOf <> ;
.
<field-texture-MHC-A>
  rdf:type skos:Concept ;
  dct:description "Behaviour of moist bolus: smooth plastic bolus; handles like plasticine; can be moulded into rods without fracture; has moderate to firm resistance to ribboning shear; will form ribbon of 75 mm or more." ;
  rdfs:comment "Approximate clay content (%): 50% or more" ;
  rdfs:label "Sapric medium heavy clay" ;
  skos:broader <field-texture-MHC> ;
  skos:broader <field-texture-MHC-A> ;
  skos:definition "Behaviour of moist bolus: smooth plastic bolus; handles like plasticine; can be moulded into rods without fracture; has moderate to firm resistance to ribboning shear; will form ribbon of 75 mm or more." ;
  skos:inScheme <> ;
  skos:narrower <field-texture-FSMHC-A> ;
  skos:narrower <field-texture-KSMHC-A> ;
  skos:narrower <field-texture-MHC-A> ;
  skos:narrower <field-texture-SMHC-A> ;
  skos:narrower <field-texture-ZMHC-A> ;
  skos:notation "MHCA" ;
  skos:prefLabel "Sapric medium heavy clay"@en ;
.
<field-texture-MHC-I>
  rdf:type skos:Concept ;
  dct:description "Behaviour of moist bolus: smooth plastic bolus; handles like plasticine; can be moulded into rods without fracture; has moderate to firm resistance to ribboning shear; will form ribbon of 75 mm or more." ;
  rdfs:comment "Approximate clay content (%): 50% or more" ;
  rdfs:label "Fibric medium heavy clay" ;
  skos:broader <field-texture-MHC> ;
  skos:broader <field-texture-MHC-I> ;
  skos:definition "Behaviour of moist bolus: smooth plastic bolus; handles like plasticine; can be moulded into rods without fracture; has moderate to firm resistance to ribboning shear; will form ribbon of 75 mm or more." ;
  skos:inScheme <> ;
  skos:narrower <field-texture-FSMHC-I> ;
  skos:narrower <field-texture-KSMHC-I> ;
  skos:narrower <field-texture-MHC-I> ;
  skos:narrower <field-texture-SMHC-I> ;
  skos:narrower <field-texture-ZMHC-I> ;
  skos:notation "MHCI" ;
  skos:prefLabel "Fibric medium heavy clay"@en ;
.
<field-texture-S>
  rdf:type skos:Concept ;
  dct:description "Behaviour of moist bolus: coherence nil to very slight, cannot be moulded; sand grains of medium size; single sand grains adhere to fingers." ;
  ui:isMemberOf <field-texture-mineral> ;
  rdfs:comment "Approximate clay content (%): commonly less than 5%" ;
  rdfs:label "Sand" ;
  skos:definition "Behaviour of moist bolus: coherence nil to very slight, cannot be moulded; sand grains of medium size; single sand grains adhere to fingers." ;
  skos:narrower <field-texture-FS> ;
  skos:narrower <field-texture-KS> ;
  skos:narrower <field-texture-S-A> ;
  skos:narrower <field-texture-S-I> ;
  skos:notation "S" ;
  skos:prefLabel "Sand"@en ;
  skos:topConceptOf <> ;
.
<field-texture-S-A>
  rdf:type skos:Concept ;
  dct:description "Behaviour of moist bolus: coherence nil to very slight, cannot be moulded; sand grains of medium size; single sand grains adhere to fingers." ;
  rdfs:comment """Approximate clay content (%): commonly less than 5%
Organic and non-fibrous; dark organic stain discolours fingers; greasy feel in clayey textures and coherence in sandy textures. Fibres (excluding living roots) or plant tissue remains are not visible to naked eye and little or none visible with ×10 hand lens.""" ;
  rdfs:label "Sapric sand" ;
  skos:broader <field-texture-S> ;
  skos:definition "Behaviour of moist bolus: coherence nil to very slight, cannot be moulded; sand grains of medium size; single sand grains adhere to fingers." ;
  skos:inScheme <> ;
  skos:narrower <field-texture-FS-A> ;
  skos:narrower <field-texture-KS-A> ;
  skos:notation "SA" ;
  skos:prefLabel "Sapric sand"@en ;
.
<field-texture-S-I>
  rdf:type skos:Concept ;
  dct:description "Behaviour of moist bolus: coherence nil to very slight, cannot be moulded; sand grains of medium size; single sand grains adhere to fingers." ;
  rdfs:comment """Approximate clay content (%): commonly less than 5%
Organic and fibrous; dark organic stain discolours fingers; greasy feel in clayey textures and coherence in sandy textures. Fibres (excluding living roots) or plant tissue remain visible to naked eye or easily visible with ×10 hand lens.""" ;
  rdfs:label "Fibric sand" ;
  skos:broader <field-texture-S> ;
  skos:definition "Behaviour of moist bolus: coherence nil to very slight, cannot be moulded; sand grains of medium size; single sand grains adhere to fingers." ;
  skos:inScheme <> ;
  skos:narrower <field-texture-FS-I> ;
  skos:narrower <field-texture-KS-I> ;
  skos:notation "SI" ;
  skos:prefLabel "Fibric sand"@en ;
.
<field-texture-SCL>
  rdf:type skos:Concept ;
  dct:description "Behaviour of moist bolus: strongly coherent bolus, sandy to touch; medium-size sand grains visible in finer matrix; will form ribbon of 25–40 mm." ;
  ui:isMemberOf <field-texture-mineral> ;
  rdfs:comment "Approximate clay content (%): 20 - 30%" ;
  rdfs:label "Sandy clay loam" ;
  skos:definition "Behaviour of moist bolus: strongly coherent bolus, sandy to touch; medium-size sand grains visible in finer matrix; will form ribbon of 25–40 mm." ;
  skos:narrower <field-texture-FSCL> ;
  skos:narrower <field-texture-KSCL> ;
  skos:narrower <field-texture-SCL-A> ;
  skos:narrower <field-texture-SCL-I> ;
  skos:narrower <field-texture-SCL-heavy> ;
  skos:narrower <field-texture-SCL-light> ;
  skos:notation "SCL" ;
  skos:prefLabel "Sandy clay loam"@en ;
  skos:topConceptOf <> ;
.
<field-texture-SCL-A>
  rdf:type skos:Concept ;
  dct:description "Behaviour of moist bolus: strongly coherent bolus, sandy to touch; medium-size sand grains visible in finer matrix; will form ribbon of 25–40 mm." ;
  rdfs:comment "Approximate clay content (%): 20 - 30%" ;
  rdfs:label "Sapric sandy clay loam" ;
  skos:broader <field-texture-SCL> ;
  skos:definition "Behaviour of moist bolus: strongly coherent bolus, sandy to touch; medium-size sand grains visible in finer matrix; will form ribbon of 25–40 mm." ;
  skos:inScheme <> ;
  skos:narrower <field-texture-FSCL-A> ;
  skos:narrower <field-texture-KSCL-A> ;
  skos:notation "SCLA" ;
  skos:prefLabel "Sapric sandy clay loam"@en ;
.
<field-texture-SCL-I>
  rdf:type skos:Concept ;
  dct:description "Behaviour of moist bolus: strongly coherent bolus, sandy to touch; medium-size sand grains visible in finer matrix; will form ribbon of 25–40 mm." ;
  rdfs:comment "Approximate clay content (%): 20 - 30%" ;
  rdfs:label "Fibric sandy clay loam" ;
  skos:broader <field-texture-SCL> ;
  skos:definition "Behaviour of moist bolus: strongly coherent bolus, sandy to touch; medium-size sand grains visible in finer matrix; will form ribbon of 25–40 mm." ;
  skos:inScheme <> ;
  skos:narrower <field-texture-FSCL-I> ;
  skos:narrower <field-texture-KSCL-I> ;
  skos:notation "SCLI" ;
  skos:prefLabel "Fibric sandy clay loam"@en ;
.
<field-texture-SCL-heavy>
  rdf:type skos:Concept ;
  dct:description "Behaviour of moist bolus: strongly coherent bolus, sandy to touch; medium-size sand grains visible in finer matrix; will form ribbon of 25–40 mm." ;
  rdfs:comment "Approximate clay content (%): 20 - 30%" ;
  rdfs:label "Heavy sandy clay loam" ;
  skos:broader <field-texture-SCL> ;
  skos:definition "Behaviour of moist bolus: strongly coherent bolus, sandy to touch; medium-size sand grains visible in finer matrix; will form ribbon of 25–40 mm." ;
  skos:inScheme <> ;
  skos:narrower <field-texture-FSCL-heavy> ;
  skos:narrower <field-texture-KSCL-heavy> ;
  skos:notation "SCL+" ;
  skos:prefLabel "Heavy sandy clay loam"@en ;
.
<field-texture-SCL-light>
  rdf:type skos:Concept ;
  dct:description "Behaviour of moist bolus: strongly coherent bolus, sandy to touch; medium-size sand grains visible in finer matrix; will form ribbon of 25–40 mm." ;
  rdfs:comment "Approximate clay content (%): 20 - 30%" ;
  rdfs:label "Light sandy clay loam" ;
  skos:broader <field-texture-SCL> ;
  skos:definition "Behaviour of moist bolus: strongly coherent bolus, sandy to touch; medium-size sand grains visible in finer matrix; will form ribbon of 25–40 mm." ;
  skos:inScheme <> ;
  skos:narrower <field-texture-FSCL-light> ;
  skos:narrower <field-texture-KSCL-light> ;
  skos:notation "SCL-" ;
  skos:prefLabel "Light sandy clay loam"@en ;
.
<field-texture-SHC>
  rdf:type skos:Concept ;
  dct:description "Behaviour of moist bolus: smooth plastic bolus; handles like stiff plasticine; can be moulded into rods without fracture; has firm resistance to ribboning shear; will form ribbon of 75 mm or more." ;
  rdfs:comment "Approximate clay content (%): 50% or more" ;
  rdfs:label "Sandy heavy clay" ;
  skos:broader <field-texture-HC> ;
  skos:definition "Behaviour of moist bolus: smooth plastic bolus; handles like stiff plasticine; can be moulded into rods without fracture; has firm resistance to ribboning shear; will form ribbon of 75 mm or more." ;
  skos:inScheme <> ;
  skos:narrower <field-texture-SHC-A> ;
  skos:narrower <field-texture-SHC-I> ;
  skos:notation "SHC" ;
  skos:prefLabel "Sandy heavy clay"@en ;
.
<field-texture-SHC-A>
  rdf:type skos:Concept ;
  dct:description "Behaviour of moist bolus: smooth plastic bolus; handles like stiff plasticine; can be moulded into rods without fracture; has firm resistance to ribboning shear; will form ribbon of 75 mm or more." ;
  rdfs:comment "Approximate clay content (%): 50% or more" ;
  rdfs:label "Sapric sandy heavy clay" ;
  skos:broader <field-texture-HC-A> ;
  skos:broader <field-texture-SHC> ;
  skos:definition "Behaviour of moist bolus: smooth plastic bolus; handles like stiff plasticine; can be moulded into rods without fracture; has firm resistance to ribboning shear; will form ribbon of 75 mm or more." ;
  skos:inScheme <> ;
  skos:notation "SHCA" ;
  skos:prefLabel "Sapric sandy heavy clay"@en ;
.
<field-texture-SHC-I>
  rdf:type skos:Concept ;
  dct:description "Behaviour of moist bolus: smooth plastic bolus; handles like stiff plasticine; can be moulded into rods without fracture; has firm resistance to ribboning shear; will form ribbon of 75 mm or more." ;
  rdfs:comment "Approximate clay content (%): 50% or more" ;
  rdfs:label "Fibric sandy heavy clay" ;
  skos:broader <field-texture-HC-I> ;
  skos:broader <field-texture-SHC> ;
  skos:definition "Behaviour of moist bolus: smooth plastic bolus; handles like stiff plasticine; can be moulded into rods without fracture; has firm resistance to ribboning shear; will form ribbon of 75 mm or more." ;
  skos:inScheme <> ;
  skos:notation "SHCI" ;
  skos:prefLabel "Fibric sandy heavy clay"@en ;
.
<field-texture-SL>
  rdf:type skos:Concept ;
  dct:description "Behaviour of moist bolus: bolus coherent but very sandy to touch; will form ribbon of 15–25 mm; dominant sand grains are of medium size and are readily visible." ;
  ui:isMemberOf <field-texture-mineral> ;
  rdfs:comment "Approximate clay content (%): 10 - 20%" ;
  rdfs:label "Sandy loam" ;
  skos:definition "Behaviour of moist bolus: bolus coherent but very sandy to touch; will form ribbon of 15–25 mm; dominant sand grains are of medium size and are readily visible." ;
  skos:narrower <field-texture-FSL> ;
  skos:narrower <field-texture-KSL> ;
  skos:narrower <field-texture-SL-A> ;
  skos:narrower <field-texture-SL-I> ;
  skos:notation "SL" ;
  skos:prefLabel "Sandy loam"@en ;
  skos:topConceptOf <> ;
.
<field-texture-SL-A>
  rdf:type skos:Concept ;
  dct:description "Behaviour of moist bolus: bolus coherent but very sandy to touch; will form ribbon of 15–25 mm; dominant sand grains are of medium size and are readily visible." ;
  rdfs:comment "Approximate clay content (%): 10 - 20%" ;
  rdfs:label "Sapric sandy loam" ;
  skos:broader <field-texture-SL> ;
  skos:definition "Behaviour of moist bolus: bolus coherent but very sandy to touch; will form ribbon of 15–25 mm; dominant sand grains are of medium size and are readily visible." ;
  skos:inScheme <> ;
  skos:narrower <field-texture-FSL-A> ;
  skos:narrower <field-texture-KSL-A> ;
  skos:notation "SLA" ;
  skos:prefLabel "Sapric sandy loam"@en ;
.
<field-texture-SL-I>
  rdf:type skos:Concept ;
  dct:description "Behaviour of moist bolus: bolus coherent but very sandy to touch; will form ribbon of 15–25 mm; dominant sand grains are of medium size and are readily visible." ;
  rdfs:comment "Approximate clay content (%): 10 - 20%" ;
  rdfs:label "Fibric sandy loam" ;
  skos:broader <field-texture-SL> ;
  skos:definition "Behaviour of moist bolus: bolus coherent but very sandy to touch; will form ribbon of 15–25 mm; dominant sand grains are of medium size and are readily visible." ;
  skos:inScheme <> ;
  skos:narrower <field-texture-FSL-I> ;
  skos:narrower <field-texture-KSL-I> ;
  skos:notation "SLI" ;
  skos:prefLabel "Fibric sandy loam"@en ;
.
<field-texture-SLC>
  rdf:type skos:Concept ;
  dct:description "Behaviour of moist bolus: plastic bolus; smooth to touch; slight resistance to shearing between thumb and forefinger; will form ribbon of 50–75 mm." ;
  rdfs:comment "Approximate clay content (%): 35 - 40%" ;
  rdfs:label "Sandy light clay" ;
  skos:broader <field-texture-LC> ;
  skos:definition "Behaviour of moist bolus: plastic bolus; smooth to touch; slight resistance to shearing between thumb and forefinger; will form ribbon of 50–75 mm." ;
  skos:inScheme <> ;
  skos:narrower <field-texture-SLC-A> ;
  skos:narrower <field-texture-SLC-I> ;
  skos:notation "SLC" ;
  skos:prefLabel "Sandy light clay"@en ;
.
<field-texture-SLC-A>
  rdf:type skos:Concept ;
  dct:description "Behaviour of moist bolus: plastic bolus; smooth to touch; slight resistance to shearing between thumb and forefinger; will form ribbon of 50–75 mm." ;
  rdfs:comment "Approximate clay content (%): 35 - 40%" ;
  rdfs:label "Sapric sandy light clay" ;
  skos:broader <field-texture-LC-A> ;
  skos:broader <field-texture-SLC> ;
  skos:definition "Behaviour of moist bolus: plastic bolus; smooth to touch; slight resistance to shearing between thumb and forefinger; will form ribbon of 50–75 mm." ;
  skos:inScheme <> ;
  skos:notation "SLCA" ;
  skos:prefLabel "Sapric sandy light clay"@en ;
.
<field-texture-SLC-I>
  rdf:type skos:Concept ;
  dct:description "Behaviour of moist bolus: plastic bolus; smooth to touch; slight resistance to shearing between thumb and forefinger; will form ribbon of 50–75 mm." ;
  rdfs:comment "Approximate clay content (%): 35 - 40%" ;
  rdfs:label "Fibric sandy light clay" ;
  skos:broader <field-texture-LC-I> ;
  skos:broader <field-texture-SLC> ;
  skos:definition "Behaviour of moist bolus: plastic bolus; smooth to touch; slight resistance to shearing between thumb and forefinger; will form ribbon of 50–75 mm." ;
  skos:inScheme <> ;
  skos:notation "SLCI" ;
  skos:prefLabel "Fibric sandy light clay"@en ;
.
<field-texture-SLMC>
  rdf:type skos:Concept ;
  dct:description "Behaviour of moist bolus: plastic bolus; smooth to touch; slight to moderate resistance to ribboning shear; will form ribbon of about 75 mm." ;
  rdfs:comment "Approximate clay content (%): 40 - 45%" ;
  rdfs:label "Sandy light medium clay" ;
  skos:broader <field-texture-LMC> ;
  skos:definition "Behaviour of moist bolus: plastic bolus; smooth to touch; slight to moderate resistance to ribboning shear; will form ribbon of about 75 mm." ;
  skos:inScheme <> ;
  skos:narrower <field-texture-SLMC-A> ;
  skos:narrower <field-texture-SLMC-I> ;
  skos:notation "SLMC" ;
  skos:prefLabel "Sandy light medium clay"@en ;
.
<field-texture-SLMC-A>
  rdf:type skos:Concept ;
  dct:description "Behaviour of moist bolus: plastic bolus; smooth to touch; slight to moderate resistance to ribboning shear; will form ribbon of about 75 mm." ;
  rdfs:comment "Approximate clay content (%): 40 - 45%" ;
  rdfs:label "Sapric sandy light medium clay" ;
  skos:broader <field-texture-LMC-A> ;
  skos:broader <field-texture-SLMC> ;
  skos:definition "Behaviour of moist bolus: plastic bolus; smooth to touch; slight to moderate resistance to ribboning shear; will form ribbon of about 75 mm." ;
  skos:inScheme <> ;
  skos:notation "SLMCA" ;
  skos:prefLabel "Sapric sandy light medium clay"@en ;
.
<field-texture-SLMC-I>
  rdf:type skos:Concept ;
  dct:description "Behaviour of moist bolus: plastic bolus; smooth to touch; slight to moderate resistance to ribboning shear; will form ribbon of about 75 mm." ;
  rdfs:comment "Approximate clay content (%): 40 - 45%" ;
  rdfs:label "Fibric sandy light medium clay" ;
  skos:broader <field-texture-LMC-I> ;
  skos:broader <field-texture-SLMC> ;
  skos:definition "Behaviour of moist bolus: plastic bolus; smooth to touch; slight to moderate resistance to ribboning shear; will form ribbon of about 75 mm." ;
  skos:inScheme <> ;
  skos:notation "SLMCI" ;
  skos:prefLabel "Fibric sandy light medium clay"@en ;
.
<field-texture-SMC>
  rdf:type skos:Concept ;
  dct:description "Behaviour of moist bolus: smooth plastic bolus; handles like plasticine and can be moulded into rods without fracture; has moderate resistance to ribboning shear; will form ribbon of 75 mm or more." ;
  rdfs:comment "Approximate clay content (%): 45 - 55%" ;
  rdfs:label "Sandy medium clay" ;
  skos:broader <field-texture-MC> ;
  skos:definition "Behaviour of moist bolus: smooth plastic bolus; handles like plasticine and can be moulded into rods without fracture; has moderate resistance to ribboning shear; will form ribbon of 75 mm or more." ;
  skos:inScheme <> ;
  skos:narrower <field-texture-SMC-A> ;
  skos:narrower <field-texture-SMC-I> ;
  skos:notation "SMC" ;
  skos:prefLabel "Sandy medium clay"@en ;
.
<field-texture-SMC-A>
  rdf:type skos:Concept ;
  dct:description "Behaviour of moist bolus: smooth plastic bolus; handles like plasticine and can be moulded into rods without fracture; has moderate resistance to ribboning shear; will form ribbon of 75 mm or more." ;
  rdfs:comment "Approximate clay content (%): 45 - 55%" ;
  rdfs:label "Sapric sandy medium clay" ;
  skos:broader <field-texture-MC-A> ;
  skos:broader <field-texture-SMC> ;
  skos:definition "Behaviour of moist bolus: smooth plastic bolus; handles like plasticine and can be moulded into rods without fracture; has moderate resistance to ribboning shear; will form ribbon of 75 mm or more." ;
  skos:inScheme <> ;
  skos:notation "SMCA" ;
  skos:prefLabel "Sapric sandy medium clay"@en ;
.
<field-texture-SMC-I>
  rdf:type skos:Concept ;
  dct:description "Behaviour of moist bolus: smooth plastic bolus; handles like plasticine and can be moulded into rods without fracture; has moderate resistance to ribboning shear; will form ribbon of 75 mm or more." ;
  rdfs:comment "Approximate clay content (%): 45 - 55%" ;
  rdfs:label "Fibric sandy medium clay" ;
  skos:broader <field-texture-MC-I> ;
  skos:broader <field-texture-SMC> ;
  skos:definition "Behaviour of moist bolus: smooth plastic bolus; handles like plasticine and can be moulded into rods without fracture; has moderate resistance to ribboning shear; will form ribbon of 75 mm or more." ;
  skos:inScheme <> ;
  skos:notation "SMCI" ;
  skos:prefLabel "Fibric sandy medium clay"@en ;
.
<field-texture-SMHC>
  rdf:type skos:Concept ;
  dct:description "Behaviour of moist bolus: smooth plastic bolus; handles like plasticine; can be moulded into rods without fracture; has moderate to firm resistance to ribboning shear; will form ribbon of 75 mm or more." ;
  rdfs:comment "Approximate clay content (%): 50% or more" ;
  rdfs:label "Sandy medium heavy clay" ;
  skos:broader <field-texture-MHC> ;
  skos:definition "Behaviour of moist bolus: smooth plastic bolus; handles like plasticine; can be moulded into rods without fracture; has moderate to firm resistance to ribboning shear; will form ribbon of 75 mm or more." ;
  skos:inScheme <> ;
  skos:narrower <field-texture-SMHC-A> ;
  skos:narrower <field-texture-SMHC-I> ;
  skos:notation "SMHC" ;
  skos:prefLabel "Sandy medium heavy clay"@en ;
.
<field-texture-SMHC-A>
  rdf:type skos:Concept ;
  dct:description "Behaviour of moist bolus: smooth plastic bolus; handles like plasticine; can be moulded into rods without fracture; has moderate to firm resistance to ribboning shear; will form ribbon of 75 mm or more." ;
  rdfs:comment "Approximate clay content (%): 50% or more" ;
  rdfs:label "Sapric sandy medium heavy clay" ;
  skos:broader <field-texture-MHC-A> ;
  skos:broader <field-texture-SMHC> ;
  skos:definition "Behaviour of moist bolus: smooth plastic bolus; handles like plasticine; can be moulded into rods without fracture; has moderate to firm resistance to ribboning shear; will form ribbon of 75 mm or more." ;
  skos:inScheme <> ;
  skos:notation "SMHCA" ;
  skos:prefLabel "Sapric sandy medium heavy clay"@en ;
.
<field-texture-SMHC-I>
  rdf:type skos:Concept ;
  dct:description "Behaviour of moist bolus: smooth plastic bolus; handles like plasticine; can be moulded into rods without fracture; has moderate to firm resistance to ribboning shear; will form ribbon of 75 mm or more." ;
  rdfs:comment "Approximate clay content (%): 50% or more" ;
  rdfs:label "Fibric sandy medium heavy clay" ;
  skos:broader <field-texture-MHC-I> ;
  skos:broader <field-texture-SMHC> ;
  skos:definition "Behaviour of moist bolus: smooth plastic bolus; handles like plasticine; can be moulded into rods without fracture; has moderate to firm resistance to ribboning shear; will form ribbon of 75 mm or more." ;
  skos:inScheme <> ;
  skos:notation "SMHCI" ;
  skos:prefLabel "Fibric sandy medium heavy clay"@en ;
.
<field-texture-SP>
  rdf:type skos:Concept ;
  dct:description "Organic soil where: bolus is sandy to touch." ;
  ui:isMemberOf <field-texture-organic> ;
  rdfs:label "Sandy peat" ;
  skos:definition "Organic soil where: bolus is sandy to touch." ;
  skos:notation "SP" ;
  skos:prefLabel "Sandy peat"@en ;
  skos:topConceptOf <> ;
.
<field-texture-ZCL>
  rdf:type skos:Concept ;
  dct:description "Behaviour of moist bolus: coherent smooth bolus, plastic and often silky to the touch; will form ribbon of 40–50 mm." ;
  ui:isMemberOf <field-texture-mineral> ;
  rdfs:comment "Approximate clay content (%): 30 - 35% and with silt 25% or more" ;
  rdfs:label "Silty clay loam" ;
  skos:definition "Behaviour of moist bolus: coherent smooth bolus, plastic and often silky to the touch; will form ribbon of 40–50 mm." ;
  skos:narrower <field-texture-ZCL-A> ;
  skos:narrower <field-texture-ZCL-I> ;
  skos:narrower <field-texture-ZCL-heavy> ;
  skos:narrower <field-texture-ZCL-light> ;
  skos:notation "ZCL" ;
  skos:prefLabel "Silty clay loam"@en ;
  skos:topConceptOf <> ;
.
<field-texture-ZCL-A>
  rdf:type skos:Concept ;
  dct:description "Behaviour of moist bolus: coherent smooth bolus, plastic and often silky to the touch; will form ribbon of 40–50 mm." ;
  rdfs:comment "Approximate clay content (%): 30 - 35% and with silt 25% or more" ;
  rdfs:label "Sapric silty clay loam" ;
  skos:broader <field-texture-ZCL> ;
  skos:definition "Behaviour of moist bolus: coherent smooth bolus, plastic and often silky to the touch; will form ribbon of 40–50 mm." ;
  skos:inScheme <> ;
  skos:notation "ZCLA" ;
  skos:prefLabel "Sapric silty clay loam"@en ;
.
<field-texture-ZCL-I>
  rdf:type skos:Concept ;
  dct:description "Behaviour of moist bolus: coherent smooth bolus, plastic and often silky to the touch; will form ribbon of 40–50 mm." ;
  rdfs:comment "Approximate clay content (%): 30 - 35% and with silt 25% or more" ;
  rdfs:label "Fibric silty clay loam" ;
  skos:broader <field-texture-ZCL> ;
  skos:definition "Behaviour of moist bolus: coherent smooth bolus, plastic and often silky to the touch; will form ribbon of 40–50 mm." ;
  skos:inScheme <> ;
  skos:notation "ZCLI" ;
  skos:prefLabel "Fibric silty clay loam"@en ;
.
<field-texture-ZCL-heavy>
  rdf:type skos:Concept ;
  dct:description "Behaviour of moist bolus: coherent smooth bolus, plastic and often silky to the touch; will form ribbon of 40–50 mm." ;
  rdfs:comment "Approximate clay content (%): 30 - 35% and with silt 25% or more" ;
  rdfs:label "Heavy silty clay loam" ;
  skos:broader <field-texture-ZCL> ;
  skos:definition "Behaviour of moist bolus: coherent smooth bolus, plastic and often silky to the touch; will form ribbon of 40–50 mm." ;
  skos:inScheme <> ;
  skos:notation "ZCL+" ;
  skos:prefLabel "Heavy silty clay loam"@en ;
.
<field-texture-ZCL-light>
  rdf:type skos:Concept ;
  dct:description "Behaviour of moist bolus: coherent smooth bolus, plastic and often silky to the touch; will form ribbon of 40–50 mm." ;
  rdfs:comment "Approximate clay content (%): 30 - 35% and with silt 25% or more" ;
  rdfs:label "Light silty clay loam" ;
  skos:broader <field-texture-ZCL> ;
  skos:definition "Behaviour of moist bolus: coherent smooth bolus, plastic and often silky to the touch; will form ribbon of 40–50 mm." ;
  skos:inScheme <> ;
  skos:notation "ZCL-" ;
  skos:prefLabel "Light silty clay loam"@en ;
.
<field-texture-ZHC>
  rdf:type skos:Concept ;
  dct:description "Behaviour of moist bolus: smooth plastic bolus; handles like stiff plasticine; can be moulded into rods without fracture; has firm resistance to ribboning shear; will form ribbon of 75 mm or more." ;
  rdfs:comment "Approximate clay content (%): 50% or more" ;
  rdfs:label "Silty heavy clay" ;
  skos:broader <field-texture-HC> ;
  skos:definition "Behaviour of moist bolus: smooth plastic bolus; handles like stiff plasticine; can be moulded into rods without fracture; has firm resistance to ribboning shear; will form ribbon of 75 mm or more." ;
  skos:inScheme <> ;
  skos:narrower <field-texture-ZHC-A> ;
  skos:narrower <field-texture-ZHC-I> ;
  skos:notation "ZHC" ;
  skos:prefLabel "Silty heavy clay"@en ;
.
<field-texture-ZHC-A>
  rdf:type skos:Concept ;
  dct:description "Behaviour of moist bolus: smooth plastic bolus; handles like stiff plasticine; can be moulded into rods without fracture; has firm resistance to ribboning shear; will form ribbon of 75 mm or more." ;
  rdfs:comment "Approximate clay content (%): 50% or more" ;
  rdfs:label "Sapric silty heavy clay" ;
  skos:broader <field-texture-HC-A> ;
  skos:broader <field-texture-ZHC> ;
  skos:definition "Behaviour of moist bolus: smooth plastic bolus; handles like stiff plasticine; can be moulded into rods without fracture; has firm resistance to ribboning shear; will form ribbon of 75 mm or more." ;
  skos:inScheme <> ;
  skos:notation "ZHCA" ;
  skos:prefLabel "Sapric silty heavy clay"@en ;
.
<field-texture-ZHC-I>
  rdf:type skos:Concept ;
  dct:description "Behaviour of moist bolus: smooth plastic bolus; handles like stiff plasticine; can be moulded into rods without fracture; has firm resistance to ribboning shear; will form ribbon of 75 mm or more." ;
  rdfs:comment "Approximate clay content (%): 50% or more" ;
  rdfs:label "Fibric silty heavy clay" ;
  skos:broader <field-texture-HC-I> ;
  skos:broader <field-texture-ZHC> ;
  skos:definition "Behaviour of moist bolus: smooth plastic bolus; handles like stiff plasticine; can be moulded into rods without fracture; has firm resistance to ribboning shear; will form ribbon of 75 mm or more." ;
  skos:inScheme <> ;
  skos:notation "ZHCI" ;
  skos:prefLabel "Fibric silty heavy clay"@en ;
.
<field-texture-ZL>
  rdf:type skos:Concept ;
  dct:description "Behaviour of moist bolus: coherent bolus; very smooth to often silky when manipulated; will form ribbon of about 25 mm." ;
  ui:isMemberOf <field-texture-mineral> ;
  rdfs:comment "Approximate clay content (%): about 25% and with silt 25% or more." ;
  rdfs:label "Silty loam" ;
  skos:definition "Behaviour of moist bolus: coherent bolus; very smooth to often silky when manipulated; will form ribbon of about 25 mm." ;
  skos:narrower <field-texture-ZL-A> ;
  skos:narrower <field-texture-ZL-I> ;
  skos:notation "ZL" ;
  skos:prefLabel "Silty loam"@en ;
  skos:topConceptOf <> ;
.
<field-texture-ZL-A>
  rdf:type skos:Concept ;
  dct:description "Behaviour of moist bolus: coherent bolus; very smooth to often silky when manipulated; will form ribbon of about 25 mm." ;
  rdfs:comment "Approximate clay content (%): about 25% and with silt 25% or more." ;
  rdfs:label "Sapric silty loam" ;
  skos:broader <field-texture-ZL> ;
  skos:definition "Behaviour of moist bolus: coherent bolus; very smooth to often silky when manipulated; will form ribbon of about 25 mm." ;
  skos:inScheme <> ;
  skos:notation "ZLA" ;
  skos:prefLabel "Sapric silty loam"@en ;
.
<field-texture-ZL-I>
  rdf:type skos:Concept ;
  dct:description "Behaviour of moist bolus: coherent bolus; very smooth to often silky when manipulated; will form ribbon of about 25 mm." ;
  rdfs:comment "Approximate clay content (%): about 25% and with silt 25% or more." ;
  rdfs:label "Fibric silty loam" ;
  skos:broader <field-texture-ZL> ;
  skos:definition "Behaviour of moist bolus: coherent bolus; very smooth to often silky when manipulated; will form ribbon of about 25 mm." ;
  skos:inScheme <> ;
  skos:notation "ZLI" ;
  skos:prefLabel "Fibric silty loam"@en ;
.
<field-texture-ZLC>
  rdf:type skos:Concept ;
  dct:description "Behaviour of moist bolus: plastic bolus; smooth to touch; slight resistance to shearing between thumb and forefinger; will form ribbon of 50–75 mm." ;
  rdfs:comment "Approximate clay content (%): 35 - 40%" ;
  rdfs:label "Silty light clay" ;
  skos:broader <field-texture-LC> ;
  skos:definition "Behaviour of moist bolus: plastic bolus; smooth to touch; slight resistance to shearing between thumb and forefinger; will form ribbon of 50–75 mm." ;
  skos:inScheme <> ;
  skos:narrower <field-texture-ZLC-A> ;
  skos:narrower <field-texture-ZLC-I> ;
  skos:notation "ZLC" ;
  skos:prefLabel "Silty light clay"@en ;
.
<field-texture-ZLC-A>
  rdf:type skos:Concept ;
  dct:description "Behaviour of moist bolus: plastic bolus; smooth to touch; slight resistance to shearing between thumb and forefinger; will form ribbon of 50–75 mm." ;
  rdfs:comment "Approximate clay content (%): 35 - 40%" ;
  rdfs:label "Sapric silty light clay" ;
  skos:broader <field-texture-LC-A> ;
  skos:broader <field-texture-ZLC> ;
  skos:definition "Behaviour of moist bolus: plastic bolus; smooth to touch; slight resistance to shearing between thumb and forefinger; will form ribbon of 50–75 mm." ;
  skos:inScheme <> ;
  skos:notation "ZLCA" ;
  skos:prefLabel "Sapric silty light clay"@en ;
.
<field-texture-ZLC-I>
  rdf:type skos:Concept ;
  dct:description "Behaviour of moist bolus: plastic bolus; smooth to touch; slight resistance to shearing between thumb and forefinger; will form ribbon of 50–75 mm." ;
  rdfs:comment "Approximate clay content (%): 35 - 40%" ;
  rdfs:label "Fibric silty light clay" ;
  skos:broader <field-texture-LC-I> ;
  skos:broader <field-texture-ZLC> ;
  skos:definition "Behaviour of moist bolus: plastic bolus; smooth to touch; slight resistance to shearing between thumb and forefinger; will form ribbon of 50–75 mm." ;
  skos:inScheme <> ;
  skos:notation "ZLCI" ;
  skos:prefLabel "Fibric silty light clay"@en ;
.
<field-texture-ZLMC>
  rdf:type skos:Concept ;
  dct:description "Behaviour of moist bolus: plastic bolus; smooth to touch; slight to moderate resistance to ribboning shear; will form ribbon of about 75 mm." ;
  rdfs:comment "Approximate clay content (%): 40 - 45%" ;
  rdfs:label "Silty light medium clay" ;
  skos:broader <field-texture-LMC> ;
  skos:definition "Behaviour of moist bolus: plastic bolus; smooth to touch; slight to moderate resistance to ribboning shear; will form ribbon of about 75 mm." ;
  skos:inScheme <> ;
  skos:narrower <field-texture-ZLMC-A> ;
  skos:narrower <field-texture-ZLMC-I> ;
  skos:notation "ZLMC" ;
  skos:prefLabel "Silty light medium clay"@en ;
.
<field-texture-ZLMC-A>
  rdf:type skos:Concept ;
  dct:description "Behaviour of moist bolus: plastic bolus; smooth to touch; slight to moderate resistance to ribboning shear; will form ribbon of about 75 mm." ;
  rdfs:comment "Approximate clay content (%): 40 - 45%" ;
  rdfs:label "Sapric silty light medium clay" ;
  skos:broader <field-texture-LMC-A> ;
  skos:broader <field-texture-ZLMC> ;
  skos:definition "Behaviour of moist bolus: plastic bolus; smooth to touch; slight to moderate resistance to ribboning shear; will form ribbon of about 75 mm." ;
  skos:inScheme <> ;
  skos:notation "ZLMCA" ;
  skos:prefLabel "Sapric silty light medium clay"@en ;
.
<field-texture-ZLMC-I>
  rdf:type skos:Concept ;
  dct:description "Behaviour of moist bolus: plastic bolus; smooth to touch; slight to moderate resistance to ribboning shear; will form ribbon of about 75 mm." ;
  rdfs:comment "Approximate clay content (%): 40 - 45%" ;
  rdfs:label "Fibric silty light medium clay" ;
  skos:broader <field-texture-LMC-I> ;
  skos:broader <field-texture-ZLMC> ;
  skos:definition "Behaviour of moist bolus: plastic bolus; smooth to touch; slight to moderate resistance to ribboning shear; will form ribbon of about 75 mm." ;
  skos:inScheme <> ;
  skos:notation "ZLMCI" ;
  skos:prefLabel "Fibric silty light medium clay"@en ;
.
<field-texture-ZMC>
  rdf:type skos:Concept ;
  dct:description "Behaviour of moist bolus: smooth plastic bolus; handles like plasticine and can be moulded into rods without fracture; has moderate resistance to ribboning shear; will form ribbon of 75 mm or more." ;
  rdfs:comment "Approximate clay content (%): 45 - 55%" ;
  rdfs:label "Silty medium clay" ;
  skos:broader <field-texture-MC> ;
  skos:definition "Behaviour of moist bolus: smooth plastic bolus; handles like plasticine and can be moulded into rods without fracture; has moderate resistance to ribboning shear; will form ribbon of 75 mm or more." ;
  skos:inScheme <> ;
  skos:narrower <field-texture-ZMC-A> ;
  skos:narrower <field-texture-ZMC-I> ;
  skos:notation "ZMC" ;
  skos:prefLabel "Silty medium clay"@en ;
.
<field-texture-ZMC-A>
  rdf:type skos:Concept ;
  dct:description "Behaviour of moist bolus: smooth plastic bolus; handles like plasticine and can be moulded into rods without fracture; has moderate resistance to ribboning shear; will form ribbon of 75 mm or more." ;
  rdfs:comment "Approximate clay content (%): 45 - 55%" ;
  rdfs:label "Sapric silty medium clay" ;
  skos:broader <field-texture-MC-A> ;
  skos:broader <field-texture-ZMC> ;
  skos:definition "Behaviour of moist bolus: smooth plastic bolus; handles like plasticine and can be moulded into rods without fracture; has moderate resistance to ribboning shear; will form ribbon of 75 mm or more." ;
  skos:inScheme <> ;
  skos:notation "ZMCA" ;
  skos:prefLabel "Sapric silty medium clay"@en ;
.
<field-texture-ZMC-I>
  rdf:type skos:Concept ;
  dct:description "Behaviour of moist bolus: smooth plastic bolus; handles like plasticine and can be moulded into rods without fracture; has moderate resistance to ribboning shear; will form ribbon of 75 mm or more." ;
  rdfs:comment "Approximate clay content (%): 45 - 55%" ;
  rdfs:label "Fibric silty medium clay" ;
  skos:broader <field-texture-MC-I> ;
  skos:broader <field-texture-ZMC> ;
  skos:definition "Behaviour of moist bolus: smooth plastic bolus; handles like plasticine and can be moulded into rods without fracture; has moderate resistance to ribboning shear; will form ribbon of 75 mm or more." ;
  skos:inScheme <> ;
  skos:notation "ZMCI" ;
  skos:prefLabel "Fibric silty medium clay"@en ;
.
<field-texture-ZMHC>
  rdf:type skos:Concept ;
  dct:description "Behaviour of moist bolus: smooth plastic bolus; handles like plasticine; can be moulded into rods without fracture; has moderate to firm resistance to ribboning shear; will form ribbon of 75 mm or more." ;
  rdfs:comment "Approximate clay content (%): 50% or more" ;
  rdfs:label "Silty medium heavy clay" ;
  skos:broader <field-texture-MHC> ;
  skos:definition "Behaviour of moist bolus: smooth plastic bolus; handles like plasticine; can be moulded into rods without fracture; has moderate to firm resistance to ribboning shear; will form ribbon of 75 mm or more." ;
  skos:inScheme <> ;
  skos:narrower <field-texture-ZMHC-A> ;
  skos:narrower <field-texture-ZMHC-I> ;
  skos:notation "ZMHC" ;
  skos:prefLabel "Silty medium heavy clay"@en ;
.
<field-texture-ZMHC-A>
  rdf:type skos:Concept ;
  dct:description "Behaviour of moist bolus: smooth plastic bolus; handles like plasticine; can be moulded into rods without fracture; has moderate to firm resistance to ribboning shear; will form ribbon of 75 mm or more." ;
  rdfs:comment "Approximate clay content (%): 50% or more" ;
  rdfs:label "Sapric silty medium heavy clay" ;
  skos:broader <field-texture-MHC-A> ;
  skos:broader <field-texture-ZMHC> ;
  skos:definition "Behaviour of moist bolus: smooth plastic bolus; handles like plasticine; can be moulded into rods without fracture; has moderate to firm resistance to ribboning shear; will form ribbon of 75 mm or more." ;
  skos:inScheme <> ;
  skos:notation "ZMHCA" ;
  skos:prefLabel "Sapric silty medium heavy clay"@en ;
.
<field-texture-ZMHC-I>
  rdf:type skos:Concept ;
  dct:description "Behaviour of moist bolus: smooth plastic bolus; handles like plasticine; can be moulded into rods without fracture; has moderate to firm resistance to ribboning shear; will form ribbon of 75 mm or more." ;
  rdfs:comment "Approximate clay content (%): 50% or more" ;
  rdfs:label "Fibric silty medium heavy clay" ;
  skos:broader <field-texture-MHC-I> ;
  skos:broader <field-texture-ZMHC> ;
  skos:definition "Behaviour of moist bolus: smooth plastic bolus; handles like plasticine; can be moulded into rods without fracture; has moderate to firm resistance to ribboning shear; will form ribbon of 75 mm or more." ;
  skos:inScheme <> ;
  skos:notation "ZMHCI" ;
  skos:prefLabel "Fibric silty medium heavy clay"@en ;
.
<field-texture-mineral>
  rdf:type skos:Collection ;
  ui:isMemberOf <field-texture> ;
  rdfs:label "Mineral field texture grades" ;
  skos:member <field-texture-CL> ;
  skos:member <field-texture-CLS> ;
  skos:member <field-texture-CS> ;
  skos:member <field-texture-HC> ;
  skos:member <field-texture-L> ;
  skos:member <field-texture-LC> ;
  skos:member <field-texture-LMC> ;
  skos:member <field-texture-LS> ;
  skos:member <field-texture-MC> ;
  skos:member <field-texture-MHC> ;
  skos:member <field-texture-S> ;
  skos:member <field-texture-SCL> ;
  skos:member <field-texture-SL> ;
  skos:member <field-texture-ZCL> ;
  skos:member <field-texture-ZL> ;
.
<field-texture-organic>
  rdf:type skos:Collection ;
  dct:description "Organic soils do not have textural grades, as soil texture is determined by the size of mineral particles finer than 2 mm (NCST). In a sense, organic soils do have a texture related to the plant materials from which they formed and the degree of decomposition, exposure and drying. These field texture names may be used to characterise materials that on field examination are considered to be clearly dominated by organic matter. Peats may be assessed by examining the degree of decomposition and distinctness of plant remains. This work is adapted from Soil Survey Staff (1975) and Avery (1980)." ;
  ui:isMemberOf <field-texture> ;
  rdfs:label "Organic field textures" ;
  skos:definition "Organic soils do not have textural grades, as soil texture is determined by the size of mineral particles finer than 2 mm (NCST). In a sense, organic soils do have a texture related to the plant materials from which they formed and the degree of decomposition, exposure and drying. These field texture names may be used to characterise materials that on field examination are considered to be clearly dominated by organic matter. Peats may be assessed by examining the degree of decomposition and distinctness of plant remains. This work is adapted from Soil Survey Staff (1975) and Avery (1980)." ;
  skos:member <field-texture-AP> ;
  skos:member <field-texture-CP> ;
  skos:member <field-texture-GP> ;
  skos:member <field-texture-HP> ;
  skos:member <field-texture-IP> ;
  skos:member <field-texture-LP> ;
  skos:member <field-texture-SP> ;
.
<horizon-a>
  rdf:type skos:Concept ;
  dct:description "Horizons either consisting of one or more surface mineral horizons with some organic accumulation and usually darker in colour than the underlying horizons, or consisting of surface and subsurface horizons that are lighter in colour but have a lower content of silicate clay and/or sesquioxides than the underlying horizons." ;
  ui:isMemberOf <horizons> ;
  rdfs:label "A Horizon" ;
  skos:definition "Horizons either consisting of one or more surface mineral horizons with some organic accumulation and usually darker in colour than the underlying horizons, or consisting of surface and subsurface horizons that are lighter in colour but have a lower content of silicate clay and/or sesquioxides than the underlying horizons." ;
  skos:narrower <horizon-a1> ;
  skos:narrower <horizon-a2> ;
  skos:narrower <horizon-a3> ;
  skos:notation "A" ;
  skos:prefLabel "A Horizon" ;
  skos:topConceptOf <> ;
.
<horizon-a1>
  rdf:type skos:Concept ;
  dct:description "Mineral horizon at or near the soil surface with some accumulation of humified organic matter, usually darker in colour than underlying horizons and with maximum biologic activity for any given soil profile. It may be divided into subhorizons and of these the A11 horizon is usually the more organic, or darker coloured uppermost portion. The A12 differs in either hue, value or chroma from the A11, usually being lighter in colour. It is not pale enough to qualify as an A2 horizon. The A1 may be further divided into subhorizons if necessary, for example A13, A14, etc." ;
  rdfs:label "A1 horizon" ;
  skos:broader <horizon-a> ;
  skos:definition "Mineral horizon at or near the soil surface with some accumulation of humified organic matter, usually darker in colour than underlying horizons and with maximum biologic activity for any given soil profile. It may be divided into subhorizons and of these the A11 horizon is usually the more organic, or darker coloured uppermost portion. The A12 differs in either hue, value or chroma from the A11, usually being lighter in colour. It is not pale enough to qualify as an A2 horizon. The A1 may be further divided into subhorizons if necessary, for example A13, A14, etc." ;
  skos:inScheme <> ;
  skos:notation "A1" ;
  skos:prefLabel "A1 horizon"@en ;
.
<horizon-a2>
  rdf:type skos:Concept ;
  dct:description "Mineral horizon having, either alone or in combination, less organic matter, sesquioxides, or silicate clay than immediately adjacent horizons. It is usually differentiated from the A1 horizon by its paler colour, that is, by having colour value at least one unit higher and usually less organic matter. It is usually differentiated from the B horizon by having colour value at least one unit higher and chroma at least two units lower, by coarser texture or by a combination of these attributes." ;
  rdfs:label "A2 horizon" ;
  skos:broader <horizon-a> ;
  skos:definition "Mineral horizon having, either alone or in combination, less organic matter, sesquioxides, or silicate clay than immediately adjacent horizons. It is usually differentiated from the A1 horizon by its paler colour, that is, by having colour value at least one unit higher and usually less organic matter. It is usually differentiated from the B horizon by having colour value at least one unit higher and chroma at least two units lower, by coarser texture or by a combination of these attributes." ;
  skos:inScheme <> ;
  skos:notation "A2" ;
  skos:prefLabel "A2 horizon"@en ;
.
<horizon-a3>
  rdf:type skos:Concept ;
  dct:description "Transitional horizon between A and B, which is dominated by properties characteristic of an overlying A1 or A2." ;
  rdfs:label "A3 horizon" ;
  skos:broader <horizon-a> ;
  skos:definition "Transitional horizon between A and B, which is dominated by properties characteristic of an overlying A1 or A2." ;
  skos:inScheme <> ;
  skos:notation "A3" ;
  skos:prefLabel "A3 horizon"@en ;
.
<horizon-b>
  rdf:type skos:Concept ;
  dct:description "Horizons consisting of one or more mineral soil layers characterised by one or more of the following: a concentration of silicate clay, iron, aluminium, organic material or several of these; a structure and/or consistence unlike that of the A horizons above or of any horizons immediately below; stronger colours, usually expressed as higher chroma and/or redder hue, than those of the A horizons above or those of the horizons below." ;
  ui:isMemberOf <horizons> ;
  rdfs:label "B Horizon" ;
  skos:definition "Horizons consisting of one or more mineral soil layers characterised by one or more of the following: a concentration of silicate clay, iron, aluminium, organic material or several of these; a structure and/or consistence unlike that of the A horizons above or of any horizons immediately below; stronger colours, usually expressed as higher chroma and/or redder hue, than those of the A horizons above or those of the horizons below." ;
  skos:narrower <horizon-b1> ;
  skos:narrower <horizon-b2> ;
  skos:narrower <horizon-b3> ;
  skos:notation "B" ;
  skos:prefLabel "B Horizon" ;
  skos:topConceptOf <> ;
.
<horizon-b1>
  rdf:type skos:Concept ;
  dct:description "Transitional horizon between A and B, which is dominated by properties characteristic of an underlying B2." ;
  rdfs:label "B1 horizon" ;
  skos:broader <horizon-b> ;
  skos:definition "Transitional horizon between A and B, which is dominated by properties characteristic of an underlying B2." ;
  skos:inScheme <> ;
  skos:notation "B1" ;
  skos:prefLabel "B1 horizon"@en ;
.
<horizon-b2>
  rdf:type skos:Concept ;
  dct:description """Horizon in which the dominant feature is one or more of the following:
•	an illuvial, residual or other concentration of silicate clay, or iron, aluminium or humus, either alone or in combination
•	maximum development of pedologic organisation* as evidenced by a different structure and/or consistence, and/or stronger colours than the A horizons above or any horizon immediately below.
It may be divided into subhorizons, for example B21, B22, B23.""" ;
  rdfs:comment "Pedologic organisation is a broad term used to include all changes in soil material resulting from the effect of physical, chemical and biologic processes, that is, soil formation. Results of these processes include horizonation, colour differences, presence of pedality, and texture and/or consistence changes" ;
  rdfs:label "B2 horizon" ;
  skos:broader <horizon-b> ;
  skos:definition """Horizon in which the dominant feature is one or more of the following:
•	an illuvial, residual or other concentration of silicate clay, or iron, aluminium or humus, either alone or in combination
•	maximum development of pedologic organisation* as evidenced by a different structure and/or consistence, and/or stronger colours than the A horizons above or any horizon immediately below.
It may be divided into subhorizons, for example B21, B22, B23.
""" ;
  skos:inScheme <> ;
  skos:notation "B2" ;
  skos:prefLabel "B2 horizon"@en ;
.
<horizon-b3>
  rdf:type skos:Concept ;
  dct:description "Transitional horizon between B and C or other subsolum material in which properties characteristic of an overlying B2 dominate, but intergrade to those of the underlying material." ;
  rdfs:label "B3 horizon" ;
  skos:broader <horizon-b> ;
  skos:definition """Transitional horizon between B and C or other subsolum material in which properties characteristic of an overlying B2 dominate, but intergrade to those of the underlying material.
""" ;
  skos:inScheme <> ;
  skos:notation "B3" ;
  skos:prefLabel "B3 horizon"@en ;
.
<horizon-bleached>
  rdf:type skos:Concept ;
  dct:description """Some horizons are white, near white or much paler than adjacent horizons. Bleached horizons most commonly occur as A2 horizons but are not restricted to them.

Bleached horizons are defined in terms of Munsell notations for dry soil:
•	for all hues, value 7 or greater with chroma 4 or less
•	where adjacent horizons have hues 5YR or redder, value 6 or greater with chroma 4 or less.

Two kinds of bleached horizons are recognised:
Conspicuously bleached: 80% or more of the horizon is bleached.
Sporadically bleached: bleach occurs:
•	irregularly through the horizon
•	as blotches, often less than 6 mm thick, at the interface of horizons, most commonly A and B horizons
•	as nests of bleached grains of soil material at the interface of horizons, most commonly A and B horizons, when no other evidence of a bleached horizon may occur.""" ;
  ui:isMemberOf <horizons> ;
  rdfs:label "Bleached horizon" ;
  skos:definition """Some horizons are white, near white or much paler than adjacent horizons. Bleached horizons most commonly occur as A2 horizons but are not restricted to them.

Bleached horizons are defined in terms of Munsell notations for dry soil:
•	for all hues, value 7 or greater with chroma 4 or less
•	where adjacent horizons have hues 5YR or redder, value 6 or greater with chroma 4 or less.

Two kinds of bleached horizons are recognised:
Conspicuously bleached: 80% or more of the horizon is bleached.
Sporadically bleached: bleach occurs:
•	irregularly through the horizon
•	as blotches, often less than 6 mm thick, at the interface of horizons, most commonly A and B horizons
•	as nests of bleached grains of soil material at the interface of horizons, most commonly A and B horizons, when no other evidence of a bleached horizon may occur.""" ;
  skos:prefLabel "Bleached horizon" ;
  skos:topConceptOf <> ;
.
<horizon-boundary>
  rdf:type skos:Concept ;
  ui:isMemberOf <horizons> ;
  rdfs:label "Boundaries between horizons" ;
  skos:narrower <horizon-boundary-distinctness> ;
  skos:narrower <horizon-boundary-shape> ;
  skos:prefLabel "Boundaries between horizons" ;
  skos:topConceptOf <> ;
.
<horizon-boundary-distinctness>
  rdf:type skos:Collection ;
  ui:isMemberOf <boundaries-between-horizons> ;
  rdfs:comment "N_H_BOUND_DISTINCT" ;
  rdfs:label "Boundary distinctness" ;
  skos:broader <horizon-boundary> ;
  skos:member <horizon-boundary-distinctness-A> ;
  skos:member <horizon-boundary-distinctness-C> ;
  skos:member <horizon-boundary-distinctness-D> ;
  skos:member <horizon-boundary-distinctness-G> ;
  skos:member <horizon-boundary-distinctness-S> ;
  skos:prefLabel "Boundary distinctness" ;
.
<horizon-boundary-distinctness-A>
  rdf:type skos:Concept ;
  dct:description "Width of boundary is 5-20 mm" ;
  ui:isMemberOf <horizon-boundary-distinctness> ;
  rdfs:label "Abrupt" ;
  skos:definition "Width of boundary is 5-20 mm" ;
  skos:notation "A" ;
  skos:prefLabel "Abrupt" ;
  skos:topConceptOf <> ;
.
<horizon-boundary-distinctness-C>
  rdf:type skos:Concept ;
  dct:description "Width of boundary is 20-50 mm" ;
  ui:isMemberOf <horizon-boundary-distinctness> ;
  rdfs:label "Clear" ;
  skos:definition "Width of boundary is 20-50 mm" ;
  skos:notation "C" ;
  skos:prefLabel "Clear" ;
  skos:topConceptOf <> ;
.
<horizon-boundary-distinctness-D>
  rdf:type skos:Concept ;
  dct:description "Width of boundary is >100 mm" ;
  ui:isMemberOf <horizon-boundary-distinctness> ;
  rdfs:label "Diffuse" ;
  skos:definition "Width of boundary is >100 mm" ;
  skos:notation "D" ;
  skos:prefLabel "Diffuse" ;
  skos:topConceptOf <> ;
.
<horizon-boundary-distinctness-G>
  rdf:type skos:Concept ;
  dct:description "Width of boundary is 50-100 mm" ;
  ui:isMemberOf <horizon-boundary-distinctness> ;
  rdfs:label "Gradual" ;
  skos:definition "Width of boundary is 50-100 mm" ;
  skos:notation "G" ;
  skos:prefLabel "Gradual" ;
  skos:topConceptOf <> ;
.
<horizon-boundary-distinctness-S>
  rdf:type skos:Concept ;
  dct:description "Width of boundary is <5 mm" ;
  ui:isMemberOf <horizon-boundary-distinctness> ;
  rdfs:label "Sharp" ;
  skos:definition "Width of boundary is <5 mm" ;
  skos:notation "S" ;
  skos:prefLabel "Sharp" ;
  skos:topConceptOf <> ;
.
<horizon-boundary-shape>
  rdf:type skos:Collection ;
  ui:isMemberOf <boundaries-between-horizons> ;
  rdfs:comment "H_BOUND_SHAPE" ;
  rdfs:label "Boundary shape" ;
  skos:broader <horizon-boundary> ;
  skos:member <horizon-boundary-shape-B> ;
  skos:member <horizon-boundary-shape-I> ;
  skos:member <horizon-boundary-shape-S> ;
  skos:member <horizon-boundary-shape-T> ;
  skos:member <horizon-boundary-shape-W> ;
  skos:prefLabel "Boundary shape" ;
.
<horizon-boundary-shape-B>
  rdf:type skos:Concept ;
  dct:description "Discontinuous" ;
  ui:isMemberOf <horizon-boundary-shape> ;
  rdfs:label "Broken" ;
  skos:definition "Discontinuous" ;
  skos:notation "B" ;
  skos:prefLabel "Broken" ;
  skos:topConceptOf <> ;
.
<horizon-boundary-shape-I>
  rdf:type skos:Concept ;
  dct:description "Undulations with depressions deeper than they are wide" ;
  ui:isMemberOf <horizon-boundary-shape> ;
  rdfs:label "Irregular" ;
  skos:definition "Undulations with depressions deeper than they are wide" ;
  skos:notation "I" ;
  skos:prefLabel "Irregular" ;
  skos:topConceptOf <> ;
.
<horizon-boundary-shape-S>
  rdf:type skos:Concept ;
  dct:description "Almost a plane surface" ;
  ui:isMemberOf <horizon-boundary-shape> ;
  rdfs:label "Smooth" ;
  skos:definition "Almost a plane surface" ;
  skos:notation "S" ;
  skos:prefLabel "Smooth" ;
  skos:topConceptOf <> ;
.
<horizon-boundary-shape-T>
  rdf:type skos:Concept ;
  dct:description "Depressions considerably deeper than they are wide" ;
  ui:isMemberOf <horizon-boundary-shape> ;
  rdfs:label "Tongued" ;
  skos:definition "Depressions considerably deeper than they are wide" ;
  skos:notation "T" ;
  skos:prefLabel "Tongued" ;
  skos:topConceptOf <> ;
.
<horizon-boundary-shape-W>
  rdf:type skos:Concept ;
  dct:description "Undulations with depressions wider than they are deep" ;
  ui:isMemberOf <horizon-boundary-shape> ;
  rdfs:label "Wavy" ;
  skos:definition "Undulations with depressions wider than they are deep" ;
  skos:notation "W" ;
  skos:prefLabel "Wavy" ;
  skos:topConceptOf <> ;
.
<horizon-c>
  rdf:type skos:Concept ;
  dct:description "These are layers below the solum (AB profile) of consolidated or unconsolidated material, usually partially weathered, little affected by pedogenic processes, and either like or unlike the material from which the solum presumably formed. The C horizon lacks properties characteristic of O, P, A, B or D horizons. It is recognised by its lack of pedological development and/or the presence of geologic organisation frequently expressed as sedimentary laminae or as ghost rock structure as in saprolite. C horizons include consolidated rock and sediments that, when moist, can be dug with hand tools. Rock strength is generally weak or weaker. Because of their nature, C horizons may alternatively be described as substrate." ;
  ui:isMemberOf <horizons> ;
  rdfs:label "C Horizon" ;
  skos:definition "These are layers below the solum (AB profile) of consolidated or unconsolidated material, usually partially weathered, little affected by pedogenic processes, and either like or unlike the material from which the solum presumably formed. The C horizon lacks properties characteristic of O, P, A, B or D horizons. It is recognised by its lack of pedological development and/or the presence of geologic organisation frequently expressed as sedimentary laminae or as ghost rock structure as in saprolite. C horizons include consolidated rock and sediments that, when moist, can be dug with hand tools. Rock strength is generally weak or weaker. Because of their nature, C horizons may alternatively be described as substrate." ;
  skos:notation "C" ;
  skos:prefLabel "C Horizon" ;
  skos:topConceptOf <> ;
.
<horizon-d>
  rdf:type skos:Concept ;
  dct:description "Considered to be any soil material below the solum that is unlike the solum in its general character, is not C horizon, and cannot be given reliable horizon designation as with ‘Buried soils’ or ‘Lithologic discontinuities’. Thus a D horizon may be recognised by the contrast in pedologic organisation between it and the overlying horizons." ;
  ui:isMemberOf <horizons> ;
  rdfs:label "D Horizon" ;
  skos:definition "Considered to be any soil material below the solum that is unlike the solum in its general character, is not C horizon, and cannot be given reliable horizon designation as with ‘Buried soils’ or ‘Lithologic discontinuities’. Thus a D horizon may be recognised by the contrast in pedologic organisation between it and the overlying horizons." ;
  skos:notation "D" ;
  skos:prefLabel "D Horizon" ;
  skos:topConceptOf <> ;
.
<horizon-o>
  rdf:type skos:Concept ;
  dct:description "Horizons dominated by organic materials in varying stages of decomposition that have accumulated on the mineral soil surface. They are usually divided into O1 and O2 horizons." ;
  ui:isMemberOf <horizons> ;
  rdfs:label "O Horizon" ;
  skos:definition "Horizons dominated by organic materials in varying stages of decomposition that have accumulated on the mineral soil surface. They are usually divided into O1 and O2 horizons." ;
  skos:narrower <horizon-o1> ;
  skos:narrower <horizon-o2> ;
  skos:notation "O" ;
  skos:prefLabel "O Horizon" ;
  skos:topConceptOf <> ;
.
<horizon-o1>
  rdf:type skos:Concept ;
  dct:description "Consists of undecomposed organic debris, usually dominated by leaves and twigs. The original form of the debris can be recognised with the naked eye." ;
  rdfs:label "O1 horizon" ;
  skos:broader <horizon-o> ;
  skos:definition "Consists of undecomposed organic debris, usually dominated by leaves and twigs. The original form of the debris can be recognised with the naked eye." ;
  skos:inScheme <> ;
  skos:notation "O1" ;
  skos:prefLabel "O1 horizon"@en ;
.
<horizon-o2>
  rdf:type skos:Concept ;
  dct:description "Consists of organic debris in various stages of decomposition. The original form of most of the debris cannot be recognised with the naked eye." ;
  rdfs:label "O2 horizon" ;
  skos:broader <horizon-o> ;
  skos:definition "Consists of organic debris in various stages of decomposition. The original form of most of the debris cannot be recognised with the naked eye." ;
  skos:inScheme <> ;
  skos:notation "O2" ;
  skos:prefLabel "O2 horizon"@en ;
.
<horizon-p>
  rdf:type skos:Concept ;
  dct:description "These are horizons dominated by organic materials in various stages of decomposition that have accumulated either under water or in conditions of excessive wetness. They have long been known as peat. The organic material consists of the remains of plants that have been growing in place. " ;
  ui:isMemberOf <horizons> ;
  rdfs:comment "When such horizons are buried, they may be designated in a manner similar to designations for buried mineral soils, for example 2P1, 3P2, etc." ;
  rdfs:label "P Horizon" ;
  skos:definition "These are horizons dominated by organic materials in various stages of decomposition that have accumulated either under water or in conditions of excessive wetness. They have long been known as peat. The organic material consists of the remains of plants that have been growing in place." ;
  skos:narrower <horizon-p1> ;
  skos:narrower <horizon-p2> ;
  skos:notation "P" ;
  skos:prefLabel "P Horizon" ;
  skos:topConceptOf <> ;
.
<horizon-p1>
  rdf:type skos:Concept ;
  dct:description "Consists primarily of undecomposed or weakly decomposed organic material (fibric peat). Plant remains are distinct and readily identifiable." ;
  rdfs:label "P1 horizon" ;
  skos:broader <horizon-p> ;
  skos:definition "Consists primarily of undecomposed or weakly decomposed organic material (fibric peat). Plant remains are distinct and readily identifiable." ;
  skos:inScheme <> ;
  skos:notation "P1" ;
  skos:prefLabel "P1 horizon"@en ;
.
<horizon-p2>
  rdf:type skos:Concept ;
  dct:description "Consists primarily of moderately to completely decomposed organic material (hemic to sapric peat). Plant remains vary from being difficult to identify to completely amorphous." ;
  rdfs:label "P2 horizon" ;
  skos:broader <horizon-p> ;
  skos:definition "Consists primarily of moderately to completely decomposed organic material (hemic to sapric peat). Plant remains vary from being difficult to identify to completely amorphous." ;
  skos:inScheme <> ;
  skos:notation "P2" ;
  skos:prefLabel "P2 horizon"@en ;
.
<horizon-prefix>
  rdf:type skos:Collection ;
  dct:description """Where obvious contrasts in lithology exist between different horizons in the soil profile, or between the soil profile and the underlying lithology, the different lithologic layers are given a numeric prefix (Figure 13).
Each layer may consist of one or more horizons. The different layers are numbered from the top downward. The upper layer is not numbered 1, this being understood. Numbering starts with the second layer, which is designated 2. Even though a layer below material 3, for example, is similar to material 2, it is designated 4 in the sequence (see Profiles C and D in Figure 13). Discrimination of lithological discontinuities from soil horizon boundaries will depend in each case upon the degree of pedological organisation and the contrast between lithological units (see, for example, Profiles C and D in Figure 13).
Where lithologic discontinuities are suspected in the profile but there is no clear evidence, either the numeric prefix should not be used or a query should be added to indicate doubt. It is better used only where there is clear evidence. Whether the numeric prefix is used or not, the horizon naming, with appropriate suffixes, remains the same, as illustrated in the examples in Figure 13.""" ;
  ui:isMemberOf <horizons> ;
  rdfs:label "Lithologic discontinuity" ;
  skos:definition """Where obvious contrasts in lithology exist between different horizons in the soil profile, or between the soil profile and the underlying lithology, the different lithologic layers are given a numeric prefix (Figure 13).
Each layer may consist of one or more horizons. The different layers are numbered from the top downward. The upper layer is not numbered 1, this being understood. Numbering starts with the second layer, which is designated 2. Even though a layer below material 3, for example, is similar to material 2, it is designated 4 in the sequence (see Profiles C and D in Figure 13). Discrimination of lithological discontinuities from soil horizon boundaries will depend in each case upon the degree of pedological organisation and the contrast between lithological units (see, for example, Profiles C and D in Figure 13).
Where lithologic discontinuities are suspected in the profile but there is no clear evidence, either the numeric prefix should not be used or a query should be added to indicate doubt. It is better used only where there is clear evidence. Whether the numeric prefix is used or not, the horizon naming, with appropriate suffixes, remains the same, as illustrated in the examples in Figure 13.""" ;
  skos:prefLabel "Lithologic discontinuity" ;
.
<horizon-r>
  rdf:type skos:Concept ;
  dct:description "These horizons consist of continuous masses (not boulders) of moderately strong to very strong rock (excluding pans) such as bedrock. R horizons may have cracks but these are few enough and/or fine enough that few roots penetrate and there is no significant displacement of rock. It is usually too strong to dig with hand tools, even when moist." ;
  ui:isMemberOf <horizons> ;
  rdfs:label "R Horizon" ;
  skos:definition "These horizons consist of continuous masses (not boulders) of moderately strong to very strong rock (excluding pans) such as bedrock. R horizons may have cracks but these are few enough and/or fine enough that few roots penetrate and there is no significant displacement of rock. It is usually too strong to dig with hand tools, even when moist." ;
  skos:notation "R" ;
  skos:prefLabel "R Horizon" ;
  skos:topConceptOf <> ;
.
<horizon-subdivision>
  rdf:type skos:Collection ;
  dct:description """All horizon subdivisions are numbered consecutively from the top of each horizon downward, as in A11, A12, A2, B21, B22, B23. The numeric suffix always precedes the alphabetic suffix except with the alphabetic suffix ‘p’ where the number always follows the letter.
The above horizon nomenclature will cover most soils, but there will be instances where there are buried soils (pedologic discontinuities) (Figure 14) and also where a profile has formed on what are obviously different parent materials (lithologic discontinuities) (Figure 13). Where there are buried soils and it is not possible to identify reliably the horizon as A or B, then these are D horizons, for example Profile E, Figure 13.
""" ;
  ui:isMemberOf <horizons> ;
  rdfs:label "Subdivision of horizons" ;
  skos:definition """All horizon subdivisions are numbered consecutively from the top of each horizon downward, as in A11, A12, A2, B21, B22, B23. The numeric suffix always precedes the alphabetic suffix except with the alphabetic suffix ‘p’ where the number always follows the letter.
The above horizon nomenclature will cover most soils, but there will be instances where there are buried soils (pedologic discontinuities) (Figure 14) and also where a profile has formed on what are obviously different parent materials (lithologic discontinuities) (Figure 13). Where there are buried soils and it is not possible to identify reliably the horizon as A or B, then these are D horizons, for example Profile E, Figure 13.
""" ;
  skos:prefLabel "Subdivision of horizons" ;
.
<horizon-suffix-b>
  rdf:type skos:Concept ;
  dct:description "Used for buried soil horizons. Used in mineral soils only. The suffix is written last, for example 2B2b." ;
  ui:isMemberOf <horizon-suffixes> ;
  rdfs:comment "Where there are buried soils, and it is possible to designate reliably the horizon nomenclature in the buried profiles, the buried horizons are given the suffix ‘b’ which is written last. Number the different soils from the top downward. The upper soil, or modern soil, is not numbered 1, this being understood. Two examples are given in Figure 14" ;
  rdfs:label "Horizon suffix b" ;
  skos:definition "Used for buried soil horizons. Used in mineral soils only. The suffix is written last, for example 2B2b." ;
  skos:notation "b" ;
  skos:prefLabel "Horizon suffix b"@en ;
  skos:topConceptOf <> ;
.
<horizon-suffix-c>
  rdf:type skos:Concept ;
  dct:description "Used for horizons with accumulation of concretions or nodules of iron and/or aluminium and/or manganese, as in B2c." ;
  ui:isMemberOf <horizon-suffixes> ;
  rdfs:label "Horizon suffix c" ;
  skos:definition "Used for horizons with accumulation of concretions or nodules of iron and/or aluminium and/or manganese, as in B2c." ;
  skos:notation "c" ;
  skos:prefLabel "Horizon suffix c"@en ;
  skos:topConceptOf <> ;
.
<horizon-suffix-d>
  rdf:type skos:Concept ;
  dct:description "Used for densipans. Very fine, sandy, earthy pan." ;
  ui:isMemberOf <horizon-suffixes> ;
  rdfs:label "Horizon suffix d" ;
  skos:definition "Used for densipans. Very fine, sandy, earthy pan." ;
  skos:notation "d" ;
  skos:prefLabel "Horizon suffix d"@en ;
  skos:topConceptOf <> ;
.
<horizon-suffix-e>
  rdf:type skos:Concept ;
  dct:description "Used for conspicuously bleached horizons, for example A2e." ;
  ui:isMemberOf <horizon-suffixes> ;
  rdfs:label "Horizon suffix e" ;
  skos:definition "Used for conspicuously bleached horizons, for example A2e." ;
  skos:notation "e" ;
  skos:prefLabel "Horizon suffix e"@en ;
  skos:topConceptOf <> ;
.
<horizon-suffix-f>
  rdf:type skos:Concept ;
  dct:description "Used when faunal accumulation, such as worm casts, dominates certain A1 horizons, for example A1f in some soils under rainforest." ;
  ui:isMemberOf <horizon-suffixes> ;
  rdfs:label "Horizon suffix f" ;
  skos:definition "Used when faunal accumulation, such as worm casts, dominates certain A1 horizons, for example A1f in some soils under rainforest." ;
  skos:notation "f" ;
  skos:prefLabel "Horizon suffix f"@en ;
  skos:topConceptOf <> ;
.
<horizon-suffix-g>
  rdf:type skos:Concept ;
  dct:description "Indicates strong gleying, as in B2g. Gleying is indicative of permanent or periodic intense reduction due to wetness; it is characterised by greyish, bluish or greenish colours, generally of low chroma. Mottling may be prominent; mottles may have reddish hues and higher chromas if oxidising conditions occur periodically. Roots may have rusty or yellowish outlines; hence horizons such as A1g can occur." ;
  ui:isMemberOf <horizon-suffixes> ;
  rdfs:label "Horizon suffix g" ;
  skos:definition "Indicates strong gleying, as in B2g. Gleying is indicative of permanent or periodic intense reduction due to wetness; it is characterised by greyish, bluish or greenish colours, generally of low chroma. Mottling may be prominent; mottles may have reddish hues and higher chromas if oxidising conditions occur periodically. Roots may have rusty or yellowish outlines; hence horizons such as A1g can occur." ;
  skos:notation "g" ;
  skos:prefLabel "Horizon suffix g"@en ;
  skos:topConceptOf <> ;
.
<horizon-suffix-h>
  rdf:type skos:Concept ;
  dct:description "Used where horizons contain accumulation of amorphous, organic matter – aluminium complexes in which iron contents are very low. The dominantly organic matter – aluminium  complexes occur as discrete pellets between clean sand grains or completely fill the voids; occasionally they may coat sand grains. Such horizons may be soft or cemented and form the characteristic B horizon of poorly drained soils known as podzols or Podosols." ;
  ui:isMemberOf <horizon-suffixes> ;
  rdfs:label "Horizon suffix h" ;
  skos:definition "Used where horizons contain accumulation of amorphous, organic matter – aluminium complexes in which iron contents are very low. The dominantly organic matter – aluminium  complexes occur as discrete pellets between clean sand grains or completely fill the voids; occasionally they may coat sand grains. Such horizons may be soft or cemented and form the characteristic B horizon of poorly drained soils known as podzols or Podosols." ;
  skos:notation "h" ;
  skos:prefLabel "Horizon suffix h"@en ;
  skos:topConceptOf <> ;
.
<horizon-suffix-j>
  rdf:type skos:Concept ;
  dct:description "Used for sporadically bleached horizons, for example A2j." ;
  ui:isMemberOf <horizon-suffixes> ;
  rdfs:label "Horizon suffix j" ;
  skos:definition "Used for sporadically bleached horizons, for example A2j." ;
  skos:notation "j" ;
  skos:prefLabel "Horizon suffix j"@en ;
  skos:topConceptOf <> ;
.
<horizon-suffix-k>
  rdf:type skos:Concept ;
  dct:description "Used for horizons with accumulation of carbonates, commonly calcium carbonate, as in B2k." ;
  ui:isMemberOf <horizon-suffixes> ;
  rdfs:comment "This suffix is usually recorded only if there is a common or larger abundance of these segregations. Horizons with few (2–10%) or very few (<2%) segregations are not usually given these horizon notations. This suffix indicates relative accumulations compared with other horizons. Thus in a soil with no carbonate except for one horizon with few segregations, this horizon could be designated with a suffix ‘k’, for example B22tk. However, in a soil with few segregations of carbonate throughout, no horizon would be given the suffix ‘k’ unless it had common or more segregations, that is, a relatively larger amount than adjacent horizons." ;
  rdfs:label "Horizon suffix k" ;
  skos:definition "Used for horizons with accumulation of carbonates, commonly calcium carbonate, as in B2k." ;
  skos:notation "k" ;
  skos:prefLabel "Horizon suffix k"@en ;
  skos:topConceptOf <> ;
.
<horizon-suffix-m>
  rdf:type skos:Concept ;
  dct:description "Used for horizons with strong cementation or induration. It is confined to irreversibly cemented horizons that are essentially continuous (more than 90%) though they may be fractured." ;
  ui:isMemberOf <horizon-suffixes> ;
  rdfs:label "Horizon suffix m" ;
  skos:definition "Used for horizons with strong cementation or induration. It is confined to irreversibly cemented horizons that are essentially continuous (more than 90%) though they may be fractured." ;
  skos:notation "m" ;
  skos:prefLabel "Horizon suffix m"@en ;
  skos:topConceptOf <> ;
.
<horizon-suffix-p>
  rdf:type skos:Concept ;
  dct:description """Used for horizons where ploughing, tillage practices or other disturbance by humans has occurred, for example deep ripping. This suffix is used only with A, as in Ap2. Where the plough layer clearly includes what was once B horizon and it is no longer possible to infer with any reliability what the texture and depth of the A horizon was, the plough layer is designated Ap.
An Ap horizon may be subdivided into subhorizons (e.g. Ap1, Ap2).""" ;
  ui:isMemberOf <horizon-suffixes> ;
  rdfs:comment "An Ap2 horizon is not the same as an A2 horizon but a subdivision equivalent to A12." ;
  rdfs:label "Horizon suffix p" ;
  skos:definition """Used for horizons where ploughing, tillage practices or other disturbance by humans has occurred, for example deep ripping. This suffix is used only with A, as in Ap2. Where the plough layer clearly includes what was once B horizon and it is no longer possible to infer with any reliability what the texture and depth of the A horizon was, the plough layer is designated Ap.
An Ap horizon may be subdivided into subhorizons (e.g. Ap1, Ap2).""" ;
  skos:notation "p" ;
  skos:prefLabel "Horizon suffix p"@en ;
  skos:topConceptOf <> ;
.
<horizon-suffix-q>
  rdf:type skos:Concept ;
  dct:description "Used for horizons with accumulation of secondary silica. If silica cementation is continuous or nearly continuous, ‘qm’ is used." ;
  ui:isMemberOf <horizon-suffixes> ;
  rdfs:label "Horizon suffix q" ;
  skos:definition "Used for horizons with accumulation of secondary silica. If silica cementation is continuous or nearly continuous, ‘qm’ is used." ;
  skos:notation "q" ;
  skos:prefLabel "Horizon suffix q"@en ;
  skos:topConceptOf <> ;
.
<horizon-suffix-r>
  rdf:type skos:Concept ;
  dct:description "Used for horizons with layers of weathered rock (including saprolite) that, although consolidated, can be dug with hand tools." ;
  ui:isMemberOf <horizon-suffixes> ;
  rdfs:label "Horizon suffix r" ;
  skos:definition "Used for horizons with layers of weathered rock (including saprolite) that, although consolidated, can be dug with hand tools." ;
  skos:notation "r" ;
  skos:prefLabel "Horizon suffix r"@en ;
  skos:topConceptOf <> ;
.
<horizon-suffix-s>
  rdf:type skos:Concept ;
  dct:description "Used for horizons with an accumulation of sesquioxide – organic matter complexes in which iron is dominant relative to aluminium. These complexes coat sand grains, occur as discrete pellets, or, with moderate amounts of iron, may fill voids forming cemented patches. The content of organic matter is variable and its distribution is often irregular. The suffix ‘s’ is often used in combination with ‘h’ (as in Bhs) where both organic and iron components are significant; s or Bhs horizons may be soft or hard and form the characteristic B horizon of free-draining podzols or Podosols." ;
  ui:isMemberOf <horizon-suffixes> ;
  rdfs:label "Horizon suffix s" ;
  skos:definition "Used for horizons with an accumulation of sesquioxide – organic matter complexes in which iron is dominant relative to aluminium. These complexes coat sand grains, occur as discrete pellets, or, with moderate amounts of iron, may fill voids forming cemented patches. The content of organic matter is variable and its distribution is often irregular. The suffix ‘s’ is often used in combination with ‘h’ (as in Bhs) where both organic and iron components are significant; s or Bhs horizons may be soft or hard and form the characteristic B horizon of free-draining podzols or Podosols." ;
  skos:notation "s" ;
  skos:prefLabel "Horizon suffix s"@en ;
  skos:topConceptOf <> ;
.
<horizon-suffix-t>
  rdf:type skos:Concept ;
  dct:description "Used for horizons with accumulation of silicate clay (from German ton, clay). Different mechanisms (such as illuviation, formation in situ) may be responsible for the clay accumulation, but these may be difficult to confirm. This suffix is used only with the B, for example B2t, to indicate the nature of the B." ;
  ui:isMemberOf <horizon-suffixes> ;
  rdfs:label "Horizon suffix t" ;
  skos:definition "Used for horizons with accumulation of silicate clay (from German ton, clay). Different mechanisms (such as illuviation, formation in situ) may be responsible for the clay accumulation, but these may be difficult to confirm. This suffix is used only with the B, for example B2t, to indicate the nature of the B." ;
  skos:notation "t" ;
  skos:prefLabel "Horizon suffix t"@en ;
  skos:topConceptOf <> ;
.
<horizon-suffix-w>
  rdf:type skos:Concept ;
  dct:description "Used where development of colour and/or structure, or both, in the B horizon is observed, with little or no accumulation of sesquioxide – organic matter complexes." ;
  ui:isMemberOf <horizon-suffixes> ;
  rdfs:label "Horizon suffix w" ;
  skos:definition "Used where development of colour and/or structure, or both, in the B horizon is observed, with little or no accumulation of sesquioxide – organic matter complexes." ;
  skos:notation "w" ;
  skos:prefLabel "Horizon suffix w"@en ;
  skos:topConceptOf <> ;
.
<horizon-suffix-x>
  rdf:type skos:Concept ;
  dct:description "Used for fragipans or earthy pans. A horizon with high bulk density relative to the horizon above, seemingly cemented when dry, but showing a moderate to weak cementation when moist." ;
  ui:isMemberOf <horizon-suffixes> ;
  rdfs:label "Horizon suffix x" ;
  skos:definition "Used for fragipans or earthy pans. A horizon with high bulk density relative to the horizon above, seemingly cemented when dry, but showing a moderate to weak cementation when moist." ;
  skos:notation "x" ;
  skos:prefLabel "Horizon suffix x"@en ;
  skos:topConceptOf <> ;
.
<horizon-suffix-y>
  rdf:type skos:Concept ;
  dct:description "Used for horizons with accumulation of calcium sulphate (gypsum), as in B21, B22." ;
  ui:isMemberOf <horizon-suffixes> ;
  rdfs:comment "This suffix is usually recorded only if there is a common or larger abundance of these segregations. Horizons with few (2–10%) or very few (<2%) segregations are not usually given these horizon notations. This suffix indicates relative accumulations compared with other horizons. Thus in a soil with no carbonate except for one horizon with few segregations, this horizon could be designated with a suffix ‘k’, for example B22tk. However, in a soil with few segregations of carbonate throughout, no horizon would be given the suffix ‘k’ unless it had common or more segregations, that is, a relatively larger amount than adjacent horizons." ;
  rdfs:label "Horizon suffix y" ;
  skos:definition "Used for horizons with accumulation of calcium sulphate (gypsum), as in B21, B22." ;
  skos:notation "y" ;
  skos:prefLabel "Horizon suffix y"@en ;
  skos:topConceptOf <> ;
.
<horizon-suffix-z>
  rdf:type skos:Concept ;
  dct:description "Used for horizons with accumulation of salts more soluble than calcium sulphate and calcium carbonate." ;
  ui:isMemberOf <horizon-suffixes> ;
  rdfs:label "Horizon suffix z" ;
  skos:definition "Used for horizons with accumulation of salts more soluble than calcium sulphate and calcium carbonate." ;
  skos:notation "z" ;
  skos:prefLabel "Horizon suffix z"@en ;
  skos:topConceptOf <> ;
.
<horizon-suffixes>
  rdf:type skos:Collection ;
  dct:description "The horizon's alphabetic suffix is used to further define the horizon. It always comes after the numeric subdivision except for suffix p, where the number always follows the letter (e.g. Ap2)." ;
  ui:isMemberOf <horizons> ;
  rdfs:label "Horizon suffixes" ;
  skos:definition "The horizon's alphabetic suffix is used to further define the horizon. It always comes after the numeric subdivision except for suffix p, where the number always follows the letter (e.g. Ap2)." ;
  skos:member <horizon-suffix-b> ;
  skos:member <horizon-suffix-c> ;
  skos:member <horizon-suffix-d> ;
  skos:member <horizon-suffix-e> ;
  skos:member <horizon-suffix-f> ;
  skos:member <horizon-suffix-g> ;
  skos:member <horizon-suffix-h> ;
  skos:member <horizon-suffix-j> ;
  skos:member <horizon-suffix-k> ;
  skos:member <horizon-suffix-m> ;
  skos:member <horizon-suffix-p> ;
  skos:member <horizon-suffix-q> ;
  skos:member <horizon-suffix-r> ;
  skos:member <horizon-suffix-s> ;
  skos:member <horizon-suffix-t> ;
  skos:member <horizon-suffix-w> ;
  skos:member <horizon-suffix-x> ;
  skos:member <horizon-suffix-y> ;
  skos:member <horizon-suffix-z> ;
  skos:prefLabel "Horizon suffixes" ;
.
<horizon-transitional>
  rdf:type skos:Collection ;
  dct:description """Two main kinds are distinguished:
•	transitional horizons that have subordinate properties of both horizons but are not dominated by properties characteristic of either horizon. For example, AB, AC, BC horizons.
•	transitional horizons in which distinct parts have recognisable properties of two kinds of horizons indicated by capital letters (Soil Survey Staff 1990).

The two capital letters are separated by a virgule (/) as A/B, A/C, B/C. Most of the individual parts of at least one of the components are surrounded by the other. The first symbol is that of the horizon that makes up the greater volume.""" ;
  ui:isMemberOf <horizons> ;
  rdfs:label "Transitional horizon" ;
  skos:definition """Two main kinds are distinguished:
•	transitional horizons that have subordinate properties of both horizons but are not dominated by properties characteristic of either horizon. For example, AB, AC, BC horizons.
•	transitional horizons in which distinct parts have recognisable properties of two kinds of horizons indicated by capital letters (Soil Survey Staff 1990).

The two capital letters are separated by a virgule (/) as A/B, A/C, B/C. Most of the individual parts of at least one of the components are surrounded by the other. The first symbol is that of the horizon that makes up the greater volume.""" ;
  skos:prefLabel "Transitional horizon" ;
.
<horizons>
  rdf:type skos:Collection ;
  dct:description "A soil horizon is a layer of soil, approximately parallel to the land surface, with morphological properties different from layers below and/or above it. Tongues of material from one horizon may penetrate into adjacent horizons." ;
  ui:topMemberOf <> ;
  rdfs:comment """As horizon notation is deduced from the profile description data (Northcote 1979) and in some instances laboratory data, record it after the profile is described. Horizons may be difficult to name, but should be named in the field. Opinions formed at the time of description are useful for later reference.
Cracking clays
The A and B horizons in cracking clays are defined and recognised on the basis of structure rather than colour (McDonald 1977).
The A horizon in cracking clays may be structured or massive. The structural A horizon is the granular, subangular blocky, angular blocky or polyhedral surface horizon where ped faces are not accommodated and have irregular coarse voids between them. This is exemplified in soils with a self-mulching surface. The A horizon structure is unstable only in the sense that relatively rapid wetting and drying continually creates new peds and voids.
The B horizon is the coarse angular blocky and/or lenticular horizon where ped faces are all accommodated and usually have only narrow planar voids between them. The B horizon structure is stable because of relatively slow wetting and drying. The B horizon will usually occur within 200 mm of the surface, but the structural change must be confirmed using a spade or exposure to examine the soil. The boundary may often be gradual or diffuse, but can be clear or abrupt.""" ;
  rdfs:label "Horizons" ;
  skos:definition "A soil horizon is a layer of soil, approximately parallel to the land surface, with morphological properties different from layers below and/or above it. Tongues of material from one horizon may penetrate into adjacent horizons." ;
  skos:member <horizon-a> ;
  skos:member <horizon-b> ;
  skos:member <horizon-bleached> ;
  skos:member <horizon-boundary> ;
  skos:member <horizon-c> ;
  skos:member <horizon-d> ;
  skos:member <horizon-o> ;
  skos:member <horizon-p> ;
  skos:member <horizon-prefix> ;
  skos:member <horizon-r> ;
  skos:member <horizon-subdivision> ;
  skos:member <horizon-suffixes> ;
  skos:member <horizon-transitional> ;
  skos:prefLabel "Horizons" ;
.
<mottle-abundance>
  rdf:type skos:Collection ;
  dct:description "The percentage of mottles is estimated by eye using the chart in Figure 11 (ASLSFH3Ed) for comparison. " ;
  ui:isMemberOf <mottles-and-other-colour-patterns> ;
  rdfs:comment "N_MOTT_ABUN" ;
  rdfs:label "Mottle abundance" ;
  skos:definition "The percentage of mottles is estimated by eye using the chart in Figure 11 (ASLSFH3Ed) for comparison. " ;
  skos:member <mottle-abundance-0> ;
  skos:member <mottle-abundance-1> ;
  skos:member <mottle-abundance-2> ;
  skos:member <mottle-abundance-3> ;
  skos:member <mottle-abundance-4> ;
.
<mottle-abundance-0>
  rdf:type skos:Concept ;
  dct:description "0%" ;
  ui:isMemberOf <mottle-abundance> ;
  rdfs:comment "N_MOTT_ABUN" ;
  rdfs:label "No mottles or other colour patterns" ;
  skos:definition "0%" ;
  skos:notation "0" ;
  skos:prefLabel "No mottles or other colour patterns"@en ;
  skos:topConceptOf <> ;
.
<mottle-abundance-1>
  rdf:type skos:Concept ;
  dct:description "<2%" ;
  ui:isMemberOf <mottle-abundance> ;
  rdfs:comment "N_MOTT_ABUN" ;
  rdfs:label "Very few" ;
  skos:definition "<2%" ;
  skos:notation "1" ;
  skos:prefLabel "Very few"@en ;
  skos:topConceptOf <> ;
.
<mottle-abundance-2>
  rdf:type skos:Concept ;
  dct:description "2-10%" ;
  ui:isMemberOf <mottle-abundance> ;
  rdfs:comment "N_MOTT_ABUN" ;
  rdfs:label "Few" ;
  skos:definition "2-10%" ;
  skos:notation "2" ;
  skos:prefLabel "Few"@en ;
  skos:topConceptOf <> ;
.
<mottle-abundance-3>
  rdf:type skos:Concept ;
  dct:description "10-20%" ;
  ui:isMemberOf <mottle-abundance> ;
  rdfs:comment "N_MOTT_ABUN" ;
  rdfs:label "Common" ;
  skos:definition "10-20%" ;
  skos:notation "3" ;
  skos:prefLabel "Common"@en ;
  skos:topConceptOf <> ;
.
<mottle-abundance-4>
  rdf:type skos:Concept ;
  dct:description "20-50%" ;
  ui:isMemberOf <mottle-abundance> ;
  rdfs:comment "N_MOTT_ABUN" ;
  rdfs:label "Many" ;
  skos:definition "20-50%" ;
  skos:notation "4" ;
  skos:prefLabel "Many"@en ;
  skos:topConceptOf <> ;
.
<mottle-boundary-C>
  rdf:type skos:Concept ;
  dct:description "colour transition over less than 2 mm" ;
  ui:isMemberOf <mottle-boundary-distinctness> ;
  rdfs:comment "C_MOTT_BOUN_DISTINCT" ;
  rdfs:label "Clear" ;
  skos:definition "colour transition over less than 2 mm" ;
  skos:notation "C" ;
  skos:prefLabel "Clear"@en ;
  skos:topConceptOf <> ;
.
<mottle-boundary-D>
  rdf:type skos:Concept ;
  dct:description "colour transition over 2 mm or more" ;
  ui:isMemberOf <mottle-boundary-distinctness> ;
  rdfs:comment "C_MOTT_BOUN_DISTINCT" ;
  rdfs:label "Diffuse" ;
  skos:definition "colour transition over 2 mm or more" ;
  skos:notation "D" ;
  skos:prefLabel "Diffuse"@en ;
  skos:topConceptOf <> ;
.
<mottle-boundary-S>
  rdf:type skos:Concept ;
  dct:description "knife-edge boundary between colours" ;
  ui:isMemberOf <mottle-boundary-distinctness> ;
  rdfs:comment "C_MOTT_BOUN_DISTINCT" ;
  rdfs:label "Sharp" ;
  skos:definition "knife-edge boundary between colours" ;
  skos:notation "S" ;
  skos:prefLabel "Sharp"@en ;
  skos:topConceptOf <> ;
.
<mottle-boundary-distinctness>
  rdf:type skos:Collection ;
  dct:description "Mottle boundary distinctness" ;
  ui:isMemberOf <mottles-and-other-colour-patterns> ;
  rdfs:comment "C_MOTT_BOUN_DISTINCT" ;
  rdfs:label "Mottle boundary distinctness" ;
  skos:definition "Mottle boundary distinctness" ;
  skos:member <mottle-boundary-C> ;
  skos:member <mottle-boundary-D> ;
  skos:member <mottle-boundary-S> ;
.
<mottle-colour-B>
  rdf:type skos:Concept ;
  dct:description "Brown" ;
  ui:isMemberOf <mottle-colours> ;
  rdfs:comment "C_MOTT_COLOUR" ;
  rdfs:label "Brown" ;
  skos:definition "Brown" ;
  skos:notation "B" ;
  skos:prefLabel "Brown"@en ;
  skos:topConceptOf <> ;
.
<mottle-colour-D>
  rdf:type skos:Concept ;
  dct:description "values 3 or less and chromas 2 or less for all hues" ;
  ui:isMemberOf <mottle-colours> ;
  rdfs:comment "C_MOTT_COLOUR" ;
  rdfs:label "Dark" ;
  skos:definition "values 3 or less and chromas 2 or less for all hues" ;
  skos:notation "D" ;
  skos:prefLabel "Dark"@en ;
  skos:topConceptOf <> ;
.
<mottle-colour-G>
  rdf:type skos:Concept ;
  dct:description "Grey" ;
  ui:isMemberOf <mottle-colours> ;
  rdfs:comment "C_MOTT_COLOUR" ;
  rdfs:label "Grey" ;
  skos:definition "Grey" ;
  skos:notation "G" ;
  skos:prefLabel "Grey"@en ;
  skos:topConceptOf <> ;
.
<mottle-colour-L>
  rdf:type skos:Concept ;
  dct:description "gley charts only" ;
  ui:isMemberOf <mottle-colours> ;
  rdfs:comment "C_MOTT_COLOUR" ;
  rdfs:label "Gley" ;
  skos:definition "gley charts only" ;
  skos:notation "L" ;
  skos:prefLabel "Gley"@en ;
  skos:topConceptOf <> ;
.
<mottle-colour-O>
  rdf:type skos:Concept ;
  dct:description "Orange" ;
  ui:isMemberOf <mottle-colours> ;
  rdfs:comment "C_MOTT_COLOUR" ;
  rdfs:label "Orange" ;
  skos:definition "Orange" ;
  skos:notation "O" ;
  skos:prefLabel "Orange"@en ;
  skos:topConceptOf <> ;
.
<mottle-colour-P>
  rdf:type skos:Concept ;
  dct:description "values 7 or more and chromas 2 or less for all hues" ;
  ui:isMemberOf <mottle-colours> ;
  rdfs:comment "C_MOTT_COLOUR" ;
  rdfs:label "Pale" ;
  skos:definition "values 7 or more and chromas 2 or less for all hues" ;
  skos:notation "P" ;
  skos:prefLabel "Pale"@en ;
  skos:topConceptOf <> ;
.
<mottle-colour-R>
  rdf:type skos:Concept ;
  dct:description "Red" ;
  ui:isMemberOf <mottle-colours> ;
  rdfs:comment "C_MOTT_COLOUR" ;
  rdfs:label "Red" ;
  skos:definition "Red" ;
  skos:notation "R" ;
  skos:prefLabel "Red"@en ;
  skos:topConceptOf <> ;
.
<mottle-colour-Y>
  rdf:type skos:Concept ;
  dct:description "Yellow" ;
  ui:isMemberOf <mottle-colours> ;
  rdfs:comment "C_MOTT_COLOUR" ;
  rdfs:label "Yellow" ;
  skos:definition "Yellow" ;
  skos:notation "Y" ;
  skos:prefLabel "Yellow"@en ;
  skos:topConceptOf <> ;
.
<mottle-colours>
  rdf:type skos:Collection ;
  dct:description "This should be described in terms of Munsell or Revised Standard Soil colours, but abbreviated forms can be used" ;
  ui:isMemberOf <mottles-and-other-colour-patterns> ;
  rdfs:comment "C_MOTT_COLOUR" ;
  rdfs:label "Mottle colour" ;
  skos:definition "This should be described in terms of Munsell or Revised Standard Soil colours, but abbreviated forms can be used" ;
  skos:member <mottle-colour-B> ;
  skos:member <mottle-colour-D> ;
  skos:member <mottle-colour-G> ;
  skos:member <mottle-colour-L> ;
  skos:member <mottle-colour-O> ;
  skos:member <mottle-colour-P> ;
  skos:member <mottle-colour-R> ;
  skos:member <mottle-colour-Y> ;
.
<mottle-constrasts>
  rdf:type skos:Collection ;
  dct:description "Mottle contrast" ;
  ui:isMemberOf <mottles-and-other-colour-patterns> ;
  rdfs:comment "C_CONTRAST" ;
  rdfs:label "Mottle contrast" ;
  skos:definition "Mottle contrast" ;
  skos:member <mottle-contrast-D> ;
  skos:member <mottle-contrast-F> ;
  skos:member <mottle-contrast-P> ;
  skos:prefLabel "Mottle contrast"@en ;
.
<mottle-contrast-D>
  rdf:type skos:Concept ;
  dct:description "readily evident although not striking" ;
  ui:isMemberOf <mottle-constrasts> ;
  rdfs:comment "C_CONTRAST" ;
  rdfs:label "Distinct" ;
  skos:definition "readily evident although not striking" ;
  skos:notation "D" ;
  skos:prefLabel "Distinct"@en ;
  skos:topConceptOf <> ;
.
<mottle-contrast-F>
  rdf:type skos:Concept ;
  dct:description "indistinct; evident only on close examination" ;
  ui:isMemberOf <mottle-constrasts> ;
  rdfs:comment "C_CONTRAST" ;
  rdfs:label "Faint" ;
  skos:definition "indistinct; evident only on close examination" ;
  skos:notation "F" ;
  skos:prefLabel "Faint"@en ;
  skos:topConceptOf <> ;
.
<mottle-contrast-P>
  rdf:type skos:Concept ;
  dct:description "striking and conspicuous" ;
  ui:isMemberOf <mottle-constrasts> ;
  rdfs:comment "C_CONTRAST" ;
  rdfs:label "Prominent" ;
  skos:definition "striking and conspicuous" ;
  skos:notation "P" ;
  skos:prefLabel "Prominent"@en ;
  skos:topConceptOf <> ;
.
<mottle-size-1>
  rdf:type skos:Concept ;
  dct:description "<5 mm" ;
  ui:isMemberOf <mottle-sizes> ;
  rdfs:comment "N_MOTT_SIZE" ;
  rdfs:label "Fine" ;
  skos:definition "<5 mm" ;
  skos:notation "1" ;
  skos:prefLabel "Fine"@en ;
  skos:topConceptOf <> ;
.
<mottle-size-2>
  rdf:type skos:Concept ;
  dct:description "5-15 mm" ;
  ui:isMemberOf <mottle-sizes> ;
  rdfs:comment "N_MOTT_SIZE" ;
  rdfs:label "Medium" ;
  skos:definition "5-15 mm" ;
  skos:notation "2" ;
  skos:prefLabel "Medium"@en ;
  skos:topConceptOf <> ;
.
<mottle-size-3>
  rdf:type skos:Concept ;
  dct:description "15-30 mm" ;
  ui:isMemberOf <mottle-sizes> ;
  rdfs:comment "N_MOTT_SIZE" ;
  rdfs:label "Coarse" ;
  skos:definition "15-30 mm" ;
  skos:notation "3" ;
  skos:prefLabel "Coarse"@en ;
  skos:topConceptOf <> ;
.
<mottle-size-4>
  rdf:type skos:Concept ;
  dct:description ">30 mm" ;
  ui:isMemberOf <mottle-sizes> ;
  rdfs:comment "N_MOTT_SIZE" ;
  rdfs:label "Very coarse" ;
  skos:definition ">30 mm" ;
  skos:notation "4" ;
  skos:prefLabel "Very coarse"@en ;
  skos:topConceptOf <> ;
.
<mottle-sizes>
  rdf:type skos:Collection ;
  dct:description "Measure mottle size (mm) along the greatest dimension, except in streaks or linear forms where width is measured." ;
  ui:isMemberOf <mottles-and-other-colour-patterns> ;
  rdfs:comment "N_MOTT_SIZE" ;
  rdfs:label "Mottle size" ;
  skos:definition "Measure mottle size (mm) along the greatest dimension, except in streaks or linear forms where width is measured." ;
  skos:member <mottle-size-1> ;
  skos:member <mottle-size-2> ;
  skos:member <mottle-size-3> ;
  skos:member <mottle-size-4> ;
.
<mottle-type-M>
  rdf:type skos:Concept ;
  dct:description "Mottles" ;
  ui:isMemberOf <mottle-types> ;
  rdfs:comment "C_MOTT_TYPE" ;
  rdfs:label "Mottles" ;
  skos:definition "Mottles" ;
  skos:notation "M" ;
  skos:prefLabel "Mottles"@en ;
  skos:topConceptOf <> ;
.
<mottle-type-X>
  rdf:type skos:Concept ;
  dct:description "Colour patterns due to biological mixing of soil material from other horizons, for example worm casts" ;
  ui:isMemberOf <mottle-types> ;
  rdfs:comment "C_MOTT_TYPE" ;
  rdfs:label "Mottle type X" ;
  skos:definition "Colour patterns due to biological mixing of soil material from other horizons, for example worm casts" ;
  skos:notation "X" ;
  skos:prefLabel "Mottle type X"@en ;
  skos:topConceptOf <> ;
.
<mottle-type-Y>
  rdf:type skos:Concept ;
  dct:description "Colour patterns due to mechanical mixing of soil material from other horizons, for example inclusions of B horizon material in Ap horizons" ;
  ui:isMemberOf <mottle-types> ;
  rdfs:comment "C_MOTT_TYPE" ;
  rdfs:label "Mottle type Y" ;
  skos:definition "Colour patterns due to mechanical mixing of soil material from other horizons, for example inclusions of B horizon material in Ap horizons" ;
  skos:notation "Y" ;
  skos:prefLabel "Mottle type Y"@en ;
  skos:topConceptOf <> ;
.
<mottle-type-Z>
  rdf:type skos:Concept ;
  dct:description "Colour patterns due to inclusions of weathered substrate material" ;
  ui:isMemberOf <mottle-types> ;
  rdfs:comment "C_MOTT_TYPE" ;
  rdfs:label "Mottle type Z" ;
  skos:definition "Colour patterns due to inclusions of weathered substrate material" ;
  skos:notation "Z" ;
  skos:prefLabel "Mottle type Z"@en ;
  skos:topConceptOf <> ;
.
<mottle-types>
  rdf:type skos:Collection ;
  dct:description "The type of mottle can suggest the origin of the mottles." ;
  dct:title "Mottle type" ;
  ui:isMemberOf <mottles-and-other-colour-patterns> ;
  rdfs:comment "C_MOTT_TYPE" ;
  rdfs:label "Mottle type" ;
  skos:definition "The type of mottle can suggest the origin of the mottles." ;
  skos:member <mottle-type-M> ;
  skos:member <mottle-type-X> ;
  skos:member <mottle-type-Y> ;
  skos:member <mottle-type-Z> ;
  skos:prefLabel "Mottle type"@en ;
.
<mottles-and-other-colour-patterns>
  rdf:type skos:Collection ;
  dct:description "Mottles are spots, blotches or streaks of subdominant colours different from the matrix colour and also different from the colour of the ped surface. Segregations of pedogenic origin are not considered to be mottles and are recorded elsewhere (page 146). Colour patterns due to biological or mechanical mixing and inclusions of weathered substrate material are described separately." ;
  ui:topMemberOf <> ;
  rdfs:label "Mottles and other colour patterns" ;
  skos:definition "Mottles are spots, blotches or streaks of subdominant colours different from the matrix colour and also different from the colour of the ped surface. Segregations of pedogenic origin are not considered to be mottles and are recorded elsewhere (page 146). Colour patterns due to biological or mechanical mixing and inclusions of weathered substrate material are described separately." ;
  skos:member <mottle-abundance> ;
  skos:member <mottle-boundary-distinctness> ;
  skos:member <mottle-colours> ;
  skos:member <mottle-constrasts> ;
  skos:member <mottle-sizes> ;
  skos:member <mottle-types> ;
  skos:prefLabel "Mottles and other colour patterns" ;
.
<observation-type-A>
  rdf:type skos:Concept ;
  dct:description "Auger boring is used to describe the soil profile." ;
  ui:isMemberOf <types-of-soil-observation> ;
  rdfs:comment "C_O_TYPE" ;
  rdfs:label "Auger boring" ;
  skos:definition "Auger boring is used to describe the soil profile." ;
  skos:notation "A" ;
  skos:prefLabel "Auger boring" ;
  skos:topConceptOf <> ;
.
<observation-type-C>
  rdf:type skos:Concept ;
  dct:description "The profile is described from a soil core that it relatively undisturbed." ;
  ui:isMemberOf <types-of-soil-observation> ;
  rdfs:comment "C_O_TYPE" ;
  rdfs:label "Relatively undisturbed soil core" ;
  skos:definition "The profile is described from a soil core that it relatively undisturbed." ;
  skos:notation "C" ;
  skos:prefLabel "Relatively undisturbed soil core" ;
  skos:topConceptOf <> ;
.
<observation-type-E>
  rdf:type skos:Concept ;
  dct:description "An existing vertical exposure (e.g. road cutting) can be used to describe the soil profile." ;
  ui:isMemberOf <types-of-soil-observation> ;
  rdfs:comment "C_O_TYPE" ;
  rdfs:label "Existing vertical exposure" ;
  skos:definition "An existing vertical exposure (e.g. road cutting) can be used to describe the soil profile." ;
  skos:notation "E" ;
  skos:prefLabel "Existing vertical exposure" ;
  skos:topConceptOf <> ;
.
<observation-type-P>
  rdf:type skos:Concept ;
  dct:description "The soil pit is one of several types of observation used to describe the soil profile." ;
  ui:isMemberOf <types-of-soil-observation> ;
  rdfs:comment "C_O_TYPE" ;
  rdfs:label "Soil pit" ;
  skos:definition "The soil pit is one of several types of observation used to describe the soil profile." ;
  skos:notation "P" ;
  skos:prefLabel "Soil pit" ;
  skos:topConceptOf <> ;
.
<pans>
  rdf:type skos:Collection ;
  dct:description "A pan is an indurated and/or cemented soil horizon" ;
  ui:topMemberOf <> ;
  rdfs:label "Pans" ;
  skos:definition "A pan is an indurated and/or cemented soil horizon" ;
  skos:member <pans-cementation> ;
  skos:member <pans-continuity> ;
  skos:member <pans-structure> ;
  skos:member <pans-type> ;
  skos:prefLabel "Pans" ;
.
<pans-cementation>
  rdf:type skos:Collection ;
  dct:description "Place a 30 mm diameter piece of the pan in water for 1 hour. If it slakes, it is uncemented; if not, it is cemented. The degree of cementation is assessed on the following scale after the 1 hour soaking in water." ;
  ui:isMemberOf <pans> ;
  rdfs:comment "C_PAN_CEMENTATION" ;
  rdfs:label "Cementation of pan" ;
  skos:definition "Place a 30 mm diameter piece of the pan in water for 1 hour. If it slakes, it is uncemented; if not, it is cemented. The degree of cementation is assessed on the following scale after the 1 hour soaking in water." ;
  skos:member <pans-cementation-0> ;
  skos:member <pans-cementation-1> ;
  skos:member <pans-cementation-2> ;
  skos:member <pans-cementation-3> ;
  skos:member <pans-cementation-4> ;
  skos:prefLabel "Cementation of pan" ;
.
<pans-cementation-0>
  rdf:type skos:Concept ;
  dct:description "Slakes" ;
  ui:isMemberOf <pans-cementation> ;
  rdfs:label "Uncemented" ;
  skos:definition "Slakes" ;
  skos:notation "0" ;
  skos:prefLabel "Uncemented" ;
  skos:topConceptOf <> ;
.
<pans-cementation-1>
  rdf:type skos:Concept ;
  dct:description "can be crushed between thumb and forefinger" ;
  ui:isMemberOf <pans-cementation> ;
  rdfs:label "Weakly cemented" ;
  skos:definition "can be crushed between thumb and forefinger" ;
  skos:notation "1" ;
  skos:prefLabel "Weakly cemented" ;
  skos:topConceptOf <> ;
.
<pans-cementation-2>
  rdf:type skos:Concept ;
  dct:description "beyond power of thumb and forefinger. Crushes underfoot on hard, flat surface with weight of average person (80 kg) applied slowly." ;
  ui:isMemberOf <pans-cementation> ;
  rdfs:label "Moderately cemented" ;
  skos:definition "beyond power of thumb and forefinger. Crushes underfoot on hard, flat surface with weight of average person (80 kg) applied slowly." ;
  skos:notation "2" ;
  skos:prefLabel "Moderately cemented" ;
  skos:topConceptOf <> ;
.
<pans-cementation-3>
  rdf:type skos:Concept ;
  dct:description "cannot be crushed underfoot by weight of average man applied slowly. Can be broken by hammer." ;
  ui:isMemberOf <pans-cementation> ;
  rdfs:label "Strongly cemented" ;
  skos:definition "cannot be crushed underfoot by weight of average man applied slowly. Can be broken by hammer." ;
  skos:notation "3" ;
  skos:prefLabel "Strongly cemented" ;
  skos:topConceptOf <> ;
.
<pans-cementation-4>
  rdf:type skos:Concept ;
  dct:description "cannot be broken by hammer, or only with extreme difficulty" ;
  ui:isMemberOf <pans-cementation> ;
  rdfs:label "Very strongly cemented" ;
  skos:definition "cannot be broken by hammer, or only with extreme difficulty" ;
  skos:notation "4" ;
  skos:prefLabel "Very strongly cemented" ;
  skos:topConceptOf <> ;
.
<pans-continuity>
  rdf:type skos:Collection ;
  dct:description "Continuity of pan" ;
  ui:isMemberOf <pans> ;
  rdfs:comment "C_PAN_CONTINUITY" ;
  rdfs:label "Continuity of pan" ;
  skos:definition "Continuity of pan" ;
  skos:member <pans-continuity-B> ;
  skos:member <pans-continuity-C> ;
  skos:member <pans-continuity-D> ;
  skos:prefLabel "Continuity of pan" ;
.
<pans-continuity-B>
  rdf:type skos:Concept ;
  dct:description "broken by cracks and fragments are disoriented" ;
  ui:isMemberOf <pans-continuity> ;
  rdfs:label "Broken" ;
  skos:definition "broken by cracks and fragments are disoriented" ;
  skos:notation "B" ;
  skos:prefLabel "Broken" ;
  skos:topConceptOf <> ;
.
<pans-continuity-C>
  rdf:type skos:Concept ;
  dct:description "extends as a layer with little or no break across 1 m or more" ;
  ui:isMemberOf <pans-continuity> ;
  rdfs:label "Continuous" ;
  skos:definition "extends as a layer with little or no break across 1 m or more" ;
  skos:notation "C" ;
  skos:prefLabel "Continuous" ;
  skos:topConceptOf <> ;
.
<pans-continuity-D>
  rdf:type skos:Concept ;
  dct:description "broken by cracks but original orientation of fragments is preserved" ;
  ui:isMemberOf <pans-continuity> ;
  rdfs:label "Discontinuous" ;
  skos:definition "broken by cracks but original orientation of fragments is preserved" ;
  skos:notation "D" ;
  skos:prefLabel "Discontinuous" ;
  skos:topConceptOf <> ;
.
<pans-structure>
  rdf:type skos:Collection ;
  dct:description "Structure of pan" ;
  ui:isMemberOf <pans> ;
  rdfs:comment "C_PAN_STRUCTURE" ;
  rdfs:label "Structure of pan" ;
  skos:definition "Structure of pan" ;
  skos:member <pans-structure-C> ;
  skos:member <pans-structure-L> ;
  skos:member <pans-structure-N> ;
  skos:member <pans-structure-R> ;
  skos:member <pans-structure-S> ;
  skos:member <pans-structure-V> ;
  skos:prefLabel "Structure of pan" ;
.
<pans-structure-C>
  rdf:type skos:Concept ;
  dct:description "spheroidal concretions cemented together" ;
  ui:isMemberOf <pans-structure> ;
  rdfs:label "Concretionary" ;
  skos:definition "spheroidal concretions cemented together" ;
  skos:notation "C" ;
  skos:prefLabel "Concretionary" ;
  skos:topConceptOf <> ;
.
<pans-structure-L>
  rdf:type skos:Concept ;
  dct:description "plate-like units cemented together" ;
  ui:isMemberOf <pans-structure> ;
  rdfs:label "Platy" ;
  skos:definition "plate-like units cemented together" ;
  skos:notation "L" ;
  skos:prefLabel "Platy" ;
  skos:topConceptOf <> ;
.
<pans-structure-N>
  rdf:type skos:Concept ;
  dct:description "nodules of irregular shape cemented together" ;
  ui:isMemberOf <pans-structure> ;
  rdfs:label "Nodular" ;
  skos:definition "nodules of irregular shape cemented together" ;
  skos:notation "N" ;
  skos:prefLabel "Nodular" ;
  skos:topConceptOf <> ;
.
<pans-structure-R>
  rdf:type skos:Concept ;
  dct:description "worm-like structure and/or cavities" ;
  ui:isMemberOf <pans-structure> ;
  rdfs:label "Vermicular" ;
  skos:definition "worm-like structure and/or cavities" ;
  skos:notation "R" ;
  skos:prefLabel "Vermicular" ;
  skos:topConceptOf <> ;
.
<pans-structure-S>
  rdf:type skos:Concept ;
  dct:description "sponge-like structure having large pores, which may or may not be filled with softer material" ;
  ui:isMemberOf <pans-structure> ;
  rdfs:label "Vesicular" ;
  skos:definition "sponge-like structure having large pores, which may or may not be filled with softer material" ;
  skos:notation "S" ;
  skos:prefLabel "Vesicular" ;
  skos:topConceptOf <> ;
.
<pans-structure-V>
  rdf:type skos:Concept ;
  dct:description "no recognisable structure" ;
  ui:isMemberOf <pans-structure> ;
  rdfs:label "Massive" ;
  skos:definition "no recognisable structure" ;
  skos:notation "V" ;
  skos:prefLabel "Massive" ;
  skos:topConceptOf <> ;
.
<pans-type>
  rdf:type skos:Collection ;
  dct:description "Type of pan" ;
  ui:isMemberOf <pans> ;
  rdfs:comment "C_PAN_TYPE" ;
  rdfs:label "Type of pan" ;
  skos:definition "Type of pan" ;
  skos:member <pans-type-A> ;
  skos:member <pans-type-C> ;
  skos:member <pans-type-D> ;
  skos:member <pans-type-E> ;
  skos:member <pans-type-F> ;
  skos:member <pans-type-I> ;
  skos:member <pans-type-K> ;
  skos:member <pans-type-L> ;
  skos:member <pans-type-M> ;
  skos:member <pans-type-N> ;
  skos:member <pans-type-O> ;
  skos:member <pans-type-R> ;
  skos:member <pans-type-T> ;
  skos:member <pans-type-V> ;
  skos:member <pans-type-Z> ;
  skos:prefLabel "Type of pan" ;
.
<pans-type-A>
  rdf:type skos:Concept ;
  dct:description "indurated material rich in aluminium hydroxides. Commonly consists of cemented pisoliths and usually known as bauxite" ;
  ui:isMemberOf <pans-type> ;
  rdfs:label "Alcrete" ;
  skos:altLabel "Bauxite" ;
  skos:definition "indurated material rich in aluminium hydroxides. Commonly consists of cemented pisoliths and usually known as bauxite" ;
  skos:notation "A" ;
  skos:prefLabel "Alcrete" ;
  skos:topConceptOf <> ;
.
<pans-type-C>
  rdf:type skos:Concept ;
  dct:description "horizon relatively high in organic matter but low in iron. It is relatively thick and weakly to strongly cemented by aluminium and usually becomes progressively more cemented with depth. It is usually relatively uniform in appearance laterally. It is commonly the B horizon of humus podzols, where it is often known as coffee rock or sandrock" ;
  ui:isMemberOf <pans-type> ;
  rdfs:label "Organic pan" ;
  skos:definition "horizon relatively high in organic matter but low in iron. It is relatively thick and weakly to strongly cemented by aluminium and usually becomes progressively more cemented with depth. It is usually relatively uniform in appearance laterally. It is commonly the B horizon of humus podzols, where it is often known as coffee rock or sandrock" ;
  skos:notation "C" ;
  skos:prefLabel "Organic pan" ;
  skos:topConceptOf <> ;
.
<pans-type-D>
  rdf:type skos:Concept ;
  dct:description "earthy pan so cemented by silica that dry fragments do not slake in water and are always brittle, even after prolonged wetting. (Described by Soil Survey Staff (1975).)" ;
  ui:isMemberOf <pans-type> ;
  rdfs:label "Duripan" ;
  skos:definition "earthy pan so cemented by silica that dry fragments do not slake in water and are always brittle, even after prolonged wetting. (Described by Soil Survey Staff (1975).)" ;
  skos:notation "D" ;
  skos:prefLabel "Duripan" ;
  skos:topConceptOf <> ;
.
<pans-type-E>
  rdf:type skos:Concept ;
  dct:description "indurated material rich in hydrated oxides of iron (usually goethite and hematite) occurring as cemented nodules and/or concretions, or as massive sheets. This material has been commonly referred to in local usage around Australia as laterite, duricrust or ironstone" ;
  ui:isMemberOf <pans-type> ;
  rdfs:label "Ferricrete" ;
  skos:definition "indurated material rich in hydrated oxides of iron (usually goethite and hematite) occurring as cemented nodules and/or concretions, or as massive sheets. This material has been commonly referred to in local usage around Australia as laterite, duricrust or ironstone" ;
  skos:notation "E" ;
  skos:prefLabel "Ferricrete" ;
  skos:topConceptOf <> ;
.
<pans-type-F>
  rdf:type skos:Concept ;
  dct:description "earthy pan, which is usually loamy. A dry fragment slakes in water. A wet fragment does not slake in water but has moderate or weak brittleness. Fragipans are more stable on exposure than overlying or underlying horizons. (Described by Soil Survey Staff (1975).)" ;
  ui:isMemberOf <pans-type> ;
  rdfs:label "Fragipan" ;
  skos:definition "earthy pan, which is usually loamy. A dry fragment slakes in water. A wet fragment does not slake in water but has moderate or weak brittleness. Fragipans are more stable on exposure than overlying or underlying horizons. (Described by Soil Survey Staff (1975).)" ;
  skos:notation "F" ;
  skos:prefLabel "Fragipan" ;
  skos:topConceptOf <> ;
.
<pans-type-I>
  rdf:type skos:Concept ;
  dct:description "commonly thin (2–10 mm), black to dark reddish pan cemented by iron, iron and manganese, or iron – organic matter complexes. Rarely 40 mm thick. Has wavy or convolute form and usually occurs as a single pan. This is a placic horizon (described by Soil Survey Staff (1975))" ;
  ui:isMemberOf <pans-type> ;
  rdfs:label "Thin ironpan" ;
  skos:definition "commonly thin (2–10 mm), black to dark reddish pan cemented by iron, iron and manganese, or iron – organic matter complexes. Rarely 40 mm thick. Has wavy or convolute form and usually occurs as a single pan. This is a placic horizon (described by Soil Survey Staff (1975))" ;
  skos:notation "I" ;
  skos:prefLabel "Thin ironpan" ;
  skos:topConceptOf <> ;
.
<pans-type-K>
  rdf:type skos:Concept ;
  dct:description "any cemented, terrestrial carbonate accumulation that may vary significantly in morphology and degree of cementation. Also known as carbonate pan, calcareous pan, caliche, kunkar, secondary limestone, travertine. All show slight to strong effervescence with 1-molar HCl" ;
  ui:isMemberOf <pans-type> ;
  rdfs:label "Calcrete" ;
  skos:definition "any cemented, terrestrial carbonate accumulation that may vary significantly in morphology and degree of cementation. Also known as carbonate pan, calcareous pan, caliche, kunkar, secondary limestone, travertine. All show slight to strong effervescence with 1-molar HCl" ;
  skos:notation "K" ;
  skos:prefLabel "Calcrete" ;
  skos:topConceptOf <> ;
.
<pans-type-L>
  rdf:type skos:Concept ;
  dct:description "strongly indurated siliceous material cemented by, and largely composed of, forms of silica, including quartz, chalcedony, opal and chert" ;
  ui:isMemberOf <pans-type> ;
  rdfs:label "Silcrete" ;
  skos:definition "strongly indurated siliceous material cemented by, and largely composed of, forms of silica, including quartz, chalcedony, opal and chert" ;
  skos:notation "L" ;
  skos:prefLabel "Silcrete" ;
  skos:topConceptOf <> ;
.
<pans-type-M>
  rdf:type skos:Concept ;
  dct:description "indurated material dominated by oxides of manganese" ;
  ui:isMemberOf <pans-type> ;
  rdfs:label "Manganiferous pan" ;
  skos:definition "indurated material dominated by oxides of manganese" ;
  skos:notation "M" ;
  skos:prefLabel "Manganiferous pan" ;
  skos:topConceptOf <> ;
.
<pans-type-N>
  rdf:type skos:Concept ;
  dct:description "earthy pan, which is very fine sandy (0.02–0.05 mm). Fragments, both wet and dry, slake in water. Densipans are less stable on exposure than overlying or underlying horizons. (Described by Smith et al. (1975).)" ;
  ui:isMemberOf <pans-type> ;
  rdfs:label "Densipan" ;
  skos:definition "earthy pan, which is very fine sandy (0.02–0.05 mm). Fragments, both wet and dry, slake in water. Densipans are less stable on exposure than overlying or underlying horizons. (Described by Smith et al. (1975).)" ;
  skos:notation "N" ;
  skos:prefLabel "Densipan" ;
  skos:topConceptOf <> ;
.
<pans-type-O>
  rdf:type skos:Concept ;
  dct:description "Other pans" ;
  ui:isMemberOf <pans-type> ;
  rdfs:label "Other pans" ;
  skos:definition "Other pans" ;
  skos:notation "O" ;
  skos:prefLabel "Other pans" ;
  skos:topConceptOf <> ;
.
<pans-type-R>
  rdf:type skos:Concept ;
  dct:description "earthy pan, which is normally reddish brown to red with dense yet porous appearance; it is very hard, has an irregular laminar cleavage and some vertical cracks, and varies from less than 0.3 m to over 30 m thick. Other variable features are bedded and unsorted sand and gravel lenses; wavy black veinings, probably manganiferous; and, less commonly, off-white veins of calcium carbonate. (The presence of calcium carbonate is not common and the red-brown hardpan in which it occurs may be relatively brittle and finely laminar.) The red-brown hardpan is usually present below the soil profile and is not a feature of any particular soil group. (It has some similarity with other silica pans such as duripans of arid climates). In many instances, it is not known if the red-brown hardpan is a paleosol or a cemented sediment (Wright 1983). If thought to be the latter, it may be described as a substrate material " ;
  ui:isMemberOf <pans-type> ;
  rdfs:label "Red-brown hardpan" ;
  skos:definition "earthy pan, which is normally reddish brown to red with dense yet porous appearance; it is very hard, has an irregular laminar cleavage and some vertical cracks, and varies from less than 0.3 m to over 30 m thick. Other variable features are bedded and unsorted sand and gravel lenses; wavy black veinings, probably manganiferous; and, less commonly, off-white veins of calcium carbonate. (The presence of calcium carbonate is not common and the red-brown hardpan in which it occurs may be relatively brittle and finely laminar.) The red-brown hardpan is usually present below the soil profile and is not a feature of any particular soil group. (It has some similarity with other silica pans such as duripans of arid climates). In many instances, it is not known if the red-brown hardpan is a paleosol or a cemented sediment (Wright 1983). If thought to be the latter, it may be described as a substrate material " ;
  skos:notation "R" ;
  skos:prefLabel "Red-brown hardpan" ;
  skos:topConceptOf <> ;
.
<pans-type-T>
  rdf:type skos:Concept ;
  dct:description "horizon strongly cemented by iron and organic matter. It has marked local variability in colour, both laterally and vertically. It may occur in the B horizon of podzols" ;
  ui:isMemberOf <pans-type> ;
  rdfs:label "Ortstein" ;
  skos:definition "horizon strongly cemented by iron and organic matter. It has marked local variability in colour, both laterally and vertically. It may occur in the B horizon of podzols" ;
  skos:notation "T" ;
  skos:prefLabel "Ortstein" ;
  skos:topConceptOf <> ;
.
<pans-type-V>
  rdf:type skos:Concept ;
  dct:description "subsurface soil horizon having higher bulk density, lower total porosity, and lower permeability to both air and water than horizons directly above and below as a result of cultivation practices. (After Morse et al. 1987.)" ;
  ui:isMemberOf <pans-type> ;
  rdfs:label "Cultivation pan" ;
  skos:definition "subsurface soil horizon having higher bulk density, lower total porosity, and lower permeability to both air and water than horizons directly above and below as a result of cultivation practices. (After Morse et al. 1987.)" ;
  skos:notation "V" ;
  skos:prefLabel "Cultivation pan" ;
  skos:topConceptOf <> ;
.
<pans-type-Z>
  rdf:type skos:Concept ;
  dct:description "Zero of no pan" ;
  ui:isMemberOf <pans-type> ;
  rdfs:label "Zero of no pan" ;
  skos:definition "Zero of no pan" ;
  skos:notation "Z" ;
  skos:prefLabel "Zero of no pan" ;
  skos:topConceptOf <> ;
.
<roots>
  rdf:type skos:Collection ;
  dc:description "Record the presence of roots observed in each horizon in areas 100 mm square on a cleaned exposure face." ;
  dct:description "Record the presence of roots observed in each horizon in areas 100 mm square on a cleaned exposure face." ;
  ui:topMemberOf <> ;
  rdfs:label "Roots" ;
  skos:definition "Record the presence of roots observed in each horizon in areas 100 mm square on a cleaned exposure face." ;
  skos:member <roots-abundance> ;
  skos:member <roots-size> ;
  skos:prefLabel "Roots" ;
.
<roots-abundance>
  rdf:type skos:Collection ;
  dct:description "<p>Number of roots per 0.01 m<sup>2</sup> (100 mm × 100 mm)</p>"^^rdf:HTML ;
  ui:isMemberOf <roots> ;
  rdfs:comment "N_ROOT_ABUN" ;
  rdfs:label "Root abundance" ;
  skos:definition "Number of roots per 0.01 m2 (100 mm × 100 mm)" ;
  skos:member <roots-abundance-0> ;
  skos:member <roots-abundance-1> ;
  skos:member <roots-abundance-2> ;
  skos:member <roots-abundance-3> ;
  skos:member <roots-abundance-4> ;
  skos:prefLabel "Root abundance" ;
.
<roots-abundance-0>
  rdf:type skos:Concept ;
  dct:description "0" ;
  ui:isMemberOf <roots-abundance> ;
  rdfs:label "No roots" ;
  skos:definition "0" ;
  skos:notation "0" ;
  skos:prefLabel "No roots"@en ;
  skos:topConceptOf <> ;
.
<roots-abundance-1>
  rdf:type skos:Concept ;
  dct:description """1 - 10 very fine and fine roots
Or
1 - 2 medium and coarse roots""" ;
  ui:isMemberOf <roots-abundance> ;
  rdfs:label "Few" ;
  skos:definition """1 - 10 very fine and fine roots
Or
1 - 2 medium and coarse roots""" ;
  skos:notation "1" ;
  skos:prefLabel "Few"@en ;
  skos:topConceptOf <> ;
.
<roots-abundance-2>
  rdf:type skos:Concept ;
  dct:description """10 - 25 very fine and fine roots
Or
2 - 5 medium and coarse roots""" ;
  ui:isMemberOf <roots-abundance> ;
  rdfs:label "Common" ;
  skos:definition """10 - 25 very fine and fine roots
Or
2 - 5 medium and coarse roots""" ;
  skos:notation "2" ;
  skos:prefLabel "Common"@en ;
  skos:topConceptOf <> ;
.
<roots-abundance-3>
  rdf:type skos:Concept ;
  dct:description """25 - 200 very fine and fine roots
Or
> 5 medium and coarse roots""" ;
  ui:isMemberOf <roots-abundance> ;
  rdfs:label "Many" ;
  skos:definition """25 - 200 very fine and fine roots
Or
> 5 medium and coarse roots""" ;
  skos:notation "3" ;
  skos:prefLabel "Many"@en ;
  skos:topConceptOf <> ;
.
<roots-abundance-4>
  rdf:type skos:Concept ;
  dct:description """> 200 very fine and fine roots
Or
> 5 medium and coarse roots""" ;
  ui:isMemberOf <roots-abundance> ;
  rdfs:label "Abundant" ;
  skos:definition """> 200 very fine and fine roots
Or
> 5 medium and coarse roots""" ;
  skos:notation "4" ;
  skos:prefLabel "Abundant"@en ;
  skos:topConceptOf <> ;
.
<roots-size>
  rdf:type skos:Collection ;
  dct:description "The size (diameter) of roots observed in the horizon in mm" ;
  ui:isMemberOf <roots> ;
  rdfs:comment "N_ROOT_SIZE" ;
  rdfs:label "Root size" ;
  skos:definition "The size (diameter) of roots observed in the horizon in mm" ;
  skos:member <roots-size-1> ;
  skos:member <roots-size-2> ;
  skos:member <roots-size-3> ;
  skos:member <roots-size-4> ;
  skos:prefLabel "Root size" ;
.
<roots-size-1>
  rdf:type skos:Concept ;
  dct:description "<1 mm" ;
  ui:isMemberOf <roots-size> ;
  rdfs:label "Very fine" ;
  skos:definition "<1 mm" ;
  skos:notation "1" ;
  skos:prefLabel "Very fine"@en ;
  skos:topConceptOf <> ;
.
<roots-size-2>
  rdf:type skos:Concept ;
  dct:description "1 - 2 mm" ;
  ui:isMemberOf <roots-size> ;
  rdfs:label "Fine" ;
  skos:definition "1 - 2 mm" ;
  skos:notation "2" ;
  skos:prefLabel "Fine"@en ;
  skos:topConceptOf <> ;
.
<roots-size-3>
  rdf:type skos:Concept ;
  dct:description "2 - 5 mm" ;
  ui:isMemberOf <roots-size> ;
  rdfs:label "Medium" ;
  skos:definition "2 - 5 mm" ;
  skos:notation "3" ;
  skos:prefLabel "Medium"@en ;
  skos:topConceptOf <> ;
.
<roots-size-4>
  rdf:type skos:Concept ;
  dct:description ">5 mm" ;
  ui:isMemberOf <roots-size> ;
  rdfs:label "Coarse" ;
  skos:definition ">5 mm" ;
  skos:notation "4" ;
  skos:prefLabel "Coarse"@en ;
  skos:topConceptOf <> ;
.
<segregations-abundance>
  rdf:type skos:Collection ;
  dct:description "Abundance of segregations. Use figure 11 as a guide" ;
  ui:isMemberOf <segregations-of-pedogenic-origin> ;
  rdfs:comment "N_SEG_ABUN" ;
  rdfs:label "Abundance of segregations" ;
  skos:definition "Abundance of segregations. Use figure 11 as a guide" ;
  skos:member <segregations-abundance-0> ;
  skos:member <segregations-abundance-1> ;
  skos:member <segregations-abundance-2> ;
  skos:member <segregations-abundance-3> ;
  skos:member <segregations-abundance-4> ;
  skos:member <segregations-abundance-5> ;
  skos:prefLabel "Abundance of segregations" ;
.
<segregations-abundance-0>
  rdf:type skos:Concept ;
  dct:description "0" ;
  ui:isMemberOf <segregations-abundance> ;
  rdfs:label "No segregations" ;
  skos:definition "0" ;
  skos:notation "0" ;
  skos:prefLabel "No segregations"@en ;
  skos:topConceptOf <> ;
.
<segregations-abundance-1>
  rdf:type skos:Concept ;
  dct:description "< 2%" ;
  ui:isMemberOf <segregations-abundance> ;
  rdfs:label "Very few" ;
  skos:definition "< 2%" ;
  skos:notation "1" ;
  skos:prefLabel "Very few"@en ;
  skos:topConceptOf <> ;
.
<segregations-abundance-2>
  rdf:type skos:Concept ;
  dct:description "2 - 10%" ;
  ui:isMemberOf <segregations-abundance> ;
  rdfs:label "Few" ;
  skos:definition "2 - 10%" ;
  skos:notation "2" ;
  skos:prefLabel "Few"@en ;
  skos:topConceptOf <> ;
.
<segregations-abundance-3>
  rdf:type skos:Concept ;
  dct:description "10 - 20%" ;
  ui:isMemberOf <segregations-abundance> ;
  rdfs:label "Common" ;
  skos:definition "10 - 20%" ;
  skos:notation "3" ;
  skos:prefLabel "Common"@en ;
  skos:topConceptOf <> ;
.
<segregations-abundance-4>
  rdf:type skos:Concept ;
  dct:description "20 - 50%" ;
  ui:isMemberOf <segregations-abundance> ;
  rdfs:label "Many" ;
  skos:definition "20 - 50%" ;
  skos:notation "4" ;
  skos:prefLabel "Many"@en ;
  skos:topConceptOf <> ;
.
<segregations-abundance-5>
  rdf:type skos:Concept ;
  dct:description "> 50%" ;
  ui:isMemberOf <segregations-abundance> ;
  rdfs:label "Very many" ;
  skos:definition "> 50%" ;
  skos:notation "5" ;
  skos:prefLabel "Very many"@en ;
  skos:topConceptOf <> ;
.
<segregations-form>
  rdf:type skos:Collection ;
  dct:description "Form of segregations" ;
  ui:isMemberOf <segregations-of-pedogenic-origin> ;
  rdfs:comment "C_SEG_FORM" ;
  rdfs:label "Form of segregations" ;
  skos:definition "Form of segregations" ;
  skos:member <segregations-form-C> ;
  skos:member <segregations-form-F> ;
  skos:member <segregations-form-L> ;
  skos:member <segregations-form-N> ;
  skos:member <segregations-form-R> ;
  skos:member <segregations-form-S> ;
  skos:member <segregations-form-T> ;
  skos:member <segregations-form-V> ;
  skos:member <segregations-form-X> ;
  skos:prefLabel "Form of segregations" ;
.
<segregations-form-C>
  rdf:type skos:Concept ;
  dct:description "Spheroidal mineral aggregates. Crudely concentric internal fabric can be seen with naked eye. Includes pisoliths and ooliths" ;
  ui:isMemberOf <segregations-form> ;
  rdfs:label "Concretions" ;
  skos:definition "Spheroidal mineral aggregates. Crudely concentric internal fabric can be seen with naked eye. Includes pisoliths and ooliths" ;
  skos:notation "C" ;
  skos:prefLabel "Concretions"@en ;
  skos:topConceptOf <> ;
.
<segregations-form-F>
  rdf:type skos:Concept ;
  dct:description "broken pieces of segregations" ;
  ui:isMemberOf <segregations-form> ;
  rdfs:label "Fragments" ;
  skos:definition "broken pieces of segregations" ;
  skos:notation "F" ;
  skos:prefLabel "Fragments"@en ;
  skos:topConceptOf <> ;
.
<segregations-form-L>
  rdf:type skos:Concept ;
  dct:description "planar, plate-like or sheet-like segregations" ;
  ui:isMemberOf <segregations-form> ;
  rdfs:label "Laminae" ;
  skos:definition "planar, plate-like or sheet-like segregations" ;
  skos:notation "L" ;
  skos:prefLabel "Laminae"@en ;
  skos:topConceptOf <> ;
.
<segregations-form-N>
  rdf:type skos:Concept ;
  dct:description "irregular, rounded mineral aggregates. No concentric or symmetric internal fabric. Can have hollow interior" ;
  ui:isMemberOf <segregations-form> ;
  rdfs:label "Nodules" ;
  skos:definition "irregular, rounded mineral aggregates. No concentric or symmetric internal fabric. Can have hollow interior" ;
  skos:notation "N" ;
  skos:prefLabel "Nodules"@en ;
  skos:topConceptOf <> ;
.
<segregations-form-R>
  rdf:type skos:Concept ;
  dct:description "linings of former or current root channels" ;
  ui:isMemberOf <segregations-form> ;
  rdfs:label "Root linings" ;
  skos:definition "linings of former or current root channels" ;
  skos:notation "R" ;
  skos:prefLabel "Root linings"@en ;
  skos:topConceptOf <> ;
.
<segregations-form-S>
  rdf:type skos:Concept ;
  dct:description "finely divided soft segregations. They contrast with surrounding soil in colour and composition but are not easily separated as discrete bodies. Boundaries may be clearly defined or diffuse" ;
  ui:isMemberOf <segregations-form> ;
  rdfs:label "Soft segregations" ;
  skos:definition "finely divided soft segregations. They contrast with surrounding soil in colour and composition but are not easily separated as discrete bodies. Boundaries may be clearly defined or diffuse" ;
  skos:notation "S" ;
  skos:prefLabel "Soft segregations"@en ;
  skos:topConceptOf <> ;
.
<segregations-form-T>
  rdf:type skos:Concept ;
  dct:description "medium or coarser (>2 mm wide) tube-like segregations, which may or may not be hollow" ;
  ui:isMemberOf <segregations-form> ;
  rdfs:label "Tubules" ;
  skos:definition "medium or coarser (>2 mm wide) tube-like segregations, which may or may not be hollow" ;
  skos:notation "T" ;
  skos:prefLabel "Tubules"@en ;
  skos:topConceptOf <> ;
.
<segregations-form-V>
  rdf:type skos:Concept ;
  dct:description "fine (<2 mm wide) linear segregations" ;
  ui:isMemberOf <segregations-form> ;
  rdfs:label "Veins" ;
  skos:definition "fine (<2 mm wide) linear segregations" ;
  skos:notation "V" ;
  skos:prefLabel "Veins"@en ;
  skos:topConceptOf <> ;
.
<segregations-form-X>
  rdf:type skos:Concept ;
  dct:description "single or complex clusters of crystals visible with naked eye or ×10 hand lens" ;
  ui:isMemberOf <segregations-form> ;
  rdfs:label "Crystals" ;
  skos:definition "single or complex clusters of crystals visible with naked eye or ×10 hand lens" ;
  skos:notation "X" ;
  skos:prefLabel "Crystals"@en ;
  skos:topConceptOf <> ;
.
<segregations-magnetic>
  rdf:type skos:Collection ;
  dct:description "attraction onto surface of hand-held magnet" ;
  ui:isMemberOf <segregations-of-pedogenic-origin> ;
  rdfs:comment "C_SEG_MAGNETIC_ATTR" ;
  rdfs:label "Magnetic attributes of segregations" ;
  skos:definition "attraction onto surface of hand-held magnet" ;
  skos:member <segregations-magnetic-M> ;
  skos:member <segregations-magnetic-N> ;
  skos:prefLabel "Magnetic attributes of segregations" ;
.
<segregations-magnetic-M>
  rdf:type skos:Concept ;
  dct:description "attracted onto surface of hand-held magnet" ;
  ui:isMemberOf <segregations-magnetic> ;
  rdfs:label "Magnetic" ;
  skos:definition "attracted onto surface of hand-held magnet" ;
  skos:notation "M" ;
  skos:prefLabel "Magnetic"@en ;
  skos:topConceptOf <> ;
.
<segregations-magnetic-N>
  rdf:type skos:Concept ;
  dct:description "not attracted onto surface of hand-held magnet" ;
  ui:isMemberOf <segregations-magnetic> ;
  rdfs:label "Non-magnetic" ;
  skos:definition "not attracted onto surface of hand-held magnet" ;
  skos:notation "N" ;
  skos:prefLabel "Non-magnetic"@en ;
  skos:topConceptOf <> ;
.
<segregations-nature>
  rdf:type skos:Collection ;
  dct:description "Nature of segregations" ;
  ui:isMemberOf <segregations-of-pedogenic-origin> ;
  rdfs:comment "C_SEG_NATURE" ;
  rdfs:label "Nature of segregations" ;
  skos:definition "Nature of segregations" ;
  skos:member <segregations-nature-A> ;
  skos:member <segregations-nature-E> ;
  skos:member <segregations-nature-F> ;
  skos:member <segregations-nature-G> ;
  skos:member <segregations-nature-H> ;
  skos:member <segregations-nature-K> ;
  skos:member <segregations-nature-L> ;
  skos:member <segregations-nature-M> ;
  skos:member <segregations-nature-N> ;
  skos:member <segregations-nature-O> ;
  skos:member <segregations-nature-S> ;
  skos:member <segregations-nature-U> ;
  skos:member <segregations-nature-Y> ;
  skos:member <segregations-nature-Z> ;
  skos:prefLabel "Nature of segregations" ;
.
<segregations-nature-A>
  rdf:type skos:Concept ;
  dct:description "Aluminous (aluminium)" ;
  ui:isMemberOf <segregations-nature> ;
  rdfs:label "Aluminous" ;
  skos:definition "Aluminous (aluminium)" ;
  skos:notation "A" ;
  skos:prefLabel "Aluminous"@en ;
  skos:topConceptOf <> ;
.
<segregations-nature-E>
  rdf:type skos:Concept ;
  dct:description "Earthy (dominantly non-clayey)" ;
  ui:isMemberOf <segregations-nature> ;
  rdfs:label "Earthy" ;
  skos:definition "Earthy (dominantly non-clayey)" ;
  skos:notation "E" ;
  skos:prefLabel "Earthy"@en ;
  skos:topConceptOf <> ;
.
<segregations-nature-F>
  rdf:type skos:Concept ;
  dct:description "Ferruginous (iron)" ;
  ui:isMemberOf <segregations-nature> ;
  rdfs:label "Ferruginous" ;
  skos:definition "Ferruginous (iron)" ;
  skos:notation "F" ;
  skos:prefLabel "Ferruginous"@en ;
  skos:topConceptOf <> ;
.
<segregations-nature-G>
  rdf:type skos:Concept ;
  dct:description "Ferruginous–organic (iron – organic matter)" ;
  ui:isMemberOf <segregations-nature> ;
  rdfs:label "Ferruginous–organic" ;
  skos:definition "Ferruginous–organic (iron – organic matter)" ;
  skos:notation "G" ;
  skos:prefLabel "Ferruginous–organic"@en ;
  skos:topConceptOf <> ;
.
<segregations-nature-H>
  rdf:type skos:Concept ;
  dct:description "Organic (humified, well-decomposed organic matter)" ;
  ui:isMemberOf <segregations-nature> ;
  rdfs:label "Organic" ;
  skos:definition "Organic (humified, well-decomposed organic matter)" ;
  skos:notation "H" ;
  skos:prefLabel "Organic"@en ;
  skos:topConceptOf <> ;
.
<segregations-nature-K>
  rdf:type skos:Concept ;
  dct:description "Calcareous (carbonate)" ;
  ui:isMemberOf <segregations-nature> ;
  rdfs:label "Calcareous" ;
  skos:definition "Calcareous (carbonate)" ;
  skos:notation "K" ;
  skos:prefLabel "Calcareous"@en ;
  skos:topConceptOf <> ;
.
<segregations-nature-L>
  rdf:type skos:Concept ;
  dct:description "Argillaceous (clayey)" ;
  ui:isMemberOf <segregations-nature> ;
  rdfs:label "Argillaceous" ;
  skos:definition "Argillaceous (clayey)" ;
  skos:notation "L" ;
  skos:prefLabel "Argillaceous"@en ;
  skos:topConceptOf <> ;
.
<segregations-nature-M>
  rdf:type skos:Concept ;
  dct:description "Manganiferous (manganese)" ;
  ui:isMemberOf <segregations-nature> ;
  rdfs:label "Manganiferous" ;
  skos:definition "Manganiferous (manganese)" ;
  skos:notation "M" ;
  skos:prefLabel "Manganiferous"@en ;
  skos:topConceptOf <> ;
.
<segregations-nature-N>
  rdf:type skos:Concept ;
  dct:description "Ferromanganiferous (iron–manganese)" ;
  ui:isMemberOf <segregations-nature> ;
  rdfs:label "Ferromanganiferous" ;
  skos:definition "Ferromanganiferous (iron–manganese)" ;
  skos:notation "N" ;
  skos:prefLabel "Ferromanganiferous"@en ;
  skos:topConceptOf <> ;
.
<segregations-nature-O>
  rdf:type skos:Concept ;
  dct:description "Other" ;
  ui:isMemberOf <segregations-nature> ;
  rdfs:label "Other" ;
  skos:definition "Other" ;
  skos:notation "O" ;
  skos:prefLabel "Other"@en ;
  skos:topConceptOf <> ;
.
<segregations-nature-S>
  rdf:type skos:Concept ;
  dct:description "Sulphurous (sulphur), for example in acid sulphate soils" ;
  ui:isMemberOf <segregations-nature> ;
  rdfs:label "Sulphurous" ;
  skos:definition "Sulphurous (sulphur), for example in acid sulphate soils" ;
  skos:notation "S" ;
  skos:prefLabel "Sulphurous"@en ;
  skos:topConceptOf <> ;
.
<segregations-nature-U>
  rdf:type skos:Concept ;
  dct:description "Unidentified" ;
  ui:isMemberOf <segregations-nature> ;
  rdfs:label "Unidentified" ;
  skos:definition "Unidentified" ;
  skos:notation "U" ;
  skos:prefLabel "Unidentified"@en ;
  skos:topConceptOf <> ;
.
<segregations-nature-Y>
  rdf:type skos:Concept ;
  dct:description "Gypseous (gypsum)" ;
  ui:isMemberOf <segregations-nature> ;
  rdfs:label "Gypseous" ;
  skos:definition "Gypseous (gypsum)" ;
  skos:notation "Y" ;
  skos:prefLabel "Gypseous"@en ;
  skos:topConceptOf <> ;
.
<segregations-nature-Z>
  rdf:type skos:Concept ;
  dct:description "Saline (visible salt)" ;
  ui:isMemberOf <segregations-nature> ;
  rdfs:label "Saline" ;
  skos:definition "Saline (visible salt)" ;
  skos:notation "Z" ;
  skos:prefLabel "Saline" ;
  skos:topConceptOf <> ;
.
<segregations-of-pedogenic-origin>
  rdf:type skos:Collection ;
  dct:description """Discrete segregations that have accumulated in the soil because of the concentration of some constituent, usually by chemical or biological action.
Segregations may be relict or formed in situ by current pedogenic processes.""" ;
  ui:topMemberOf <> ;
  rdfs:label "Segregations of pedogenic origin" ;
  skos:definition """Discrete segregations that have accumulated in the soil because of the concentration of some constituent, usually by chemical or biological action.
Segregations may be relict or formed in situ by current pedogenic processes.""" ;
  skos:member <segregations-abundance> ;
  skos:member <segregations-form> ;
  skos:member <segregations-magnetic> ;
  skos:member <segregations-nature> ;
  skos:member <segregations-size> ;
  skos:member <segregations-strength> ;
  skos:prefLabel "Segregations of pedogenic origin" ;
.
<segregations-size>
  rdf:type skos:Collection ;
  dct:description "Approximately equidimensional segregations (concretions, nodules) are measured in the greatest dimension. Segregations where one dimension is much greater than the other two (tubules, root linings, veins, laminae) are measured in the least dimension" ;
  ui:isMemberOf <segregations-of-pedogenic-origin> ;
  rdfs:comment "N_SEG_SIZE" ;
  rdfs:label "Size of segregations" ;
  skos:definition "Approximately equidimensional segregations (concretions, nodules) are measured in the greatest dimension. Segregations where one dimension is much greater than the other two (tubules, root linings, veins, laminae) are measured in the least dimension" ;
  skos:member <segregations-size-1> ;
  skos:member <segregations-size-2> ;
  skos:member <segregations-size-3> ;
  skos:member <segregations-size-4> ;
  skos:member <segregations-size-5> ;
  skos:prefLabel "Size of segregations" ;
.
<segregations-size-1>
  rdf:type skos:Concept ;
  dct:description "< 2mm" ;
  ui:isMemberOf <segregations-size> ;
  rdfs:label "Fine" ;
  skos:definition "< 2mm" ;
  skos:notation "1" ;
  skos:prefLabel "Fine"@en ;
  skos:topConceptOf <> ;
.
<segregations-size-2>
  rdf:type skos:Concept ;
  dct:description "2 - 6mm" ;
  ui:isMemberOf <segregations-size> ;
  rdfs:label "Medium" ;
  skos:definition "2 - 6mm" ;
  skos:notation "2" ;
  skos:prefLabel "Medium"@en ;
  skos:topConceptOf <> ;
.
<segregations-size-3>
  rdf:type skos:Concept ;
  dct:description "6 - 20mm" ;
  ui:isMemberOf <segregations-size> ;
  rdfs:label "Coarse" ;
  skos:definition "6 - 20mm" ;
  skos:notation "3" ;
  skos:prefLabel "Coarse"@en ;
  skos:topConceptOf <> ;
.
<segregations-size-4>
  rdf:type skos:Concept ;
  dct:description "20 - 60mm" ;
  ui:isMemberOf <segregations-size> ;
  rdfs:label "Very coarse" ;
  skos:definition "20 - 60mm" ;
  skos:notation "4" ;
  skos:prefLabel "Very coarse"@en ;
  skos:topConceptOf <> ;
.
<segregations-size-5>
  rdf:type skos:Concept ;
  dct:description "> 60mm" ;
  ui:isMemberOf <segregations-size> ;
  rdfs:label "Extremely coarse" ;
  skos:definition "> 60mm" ;
  skos:notation "5" ;
  skos:prefLabel "Extremely coarse"@en ;
  skos:topConceptOf <> ;
.
<segregations-strength>
  rdf:type skos:Collection ;
  dct:description "Strength may be recorded where appropriate" ;
  ui:isMemberOf <segregations-of-pedogenic-origin> ;
  rdfs:comment "C_SEG_STRENGTH" ;
  rdfs:label "Strength of segregations" ;
  skos:definition "Strength may be recorded where appropriate" ;
  skos:member <segregations-strength-1> ;
  skos:member <segregations-strength-2> ;
  skos:prefLabel "Strength of segregations" ;
.
<segregations-strength-1>
  rdf:type skos:Concept ;
  dct:description "can be broken between thumb and forefinger" ;
  ui:isMemberOf <segregations-strength> ;
  rdfs:label "Weak" ;
  skos:definition "can be broken between thumb and forefinger" ;
  skos:notation "1" ;
  skos:prefLabel "Weak"@en ;
  skos:topConceptOf <> ;
.
<segregations-strength-2>
  rdf:type skos:Concept ;
  dct:description "cannot be broken between thumb and forefinger" ;
  ui:isMemberOf <segregations-strength> ;
  rdfs:label "Strong" ;
  skos:definition "cannot be broken between thumb and forefinger" ;
  skos:notation "2" ;
  skos:prefLabel "Strong"@en ;
  skos:topConceptOf <> ;
.
<soil-water-regime>
  rdf:type skos:Collection ;
  dct:description """Traditional approaches to soil drainage do not adequately differentiate between hydrological setting and permeability of the material of the profile. For example, a very permeable, coarse-textured soil occurring in a wet depression would have to be classed as very poorly drained. Hence there is a need to consider permeability, which refers to the potential of a soil to transmit water internally, and drainage, which refers to the rapidity and extent of water removal from the soil profile or site. Both these aspects of internal drainage may be difficult to assess in the field, and cannot be based solely on profile morphology. Mottling may, but not always, reflect drainage status, since mottling may be a relict feature. Vegetation and topography may be useful guides.
These concepts of permeability and drainage are largely based on Canada Soil Survey Committee (1978).""" ;
  ui:topMemberOf <> ;
  rdfs:label "Soil water regime" ;
  skos:definition """Traditional approaches to soil drainage do not adequately differentiate between hydrological setting and permeability of the material of the profile. For example, a very permeable, coarse-textured soil occurring in a wet depression would have to be classed as very poorly drained. Hence there is a need to consider permeability, which refers to the potential of a soil to transmit water internally, and drainage, which refers to the rapidity and extent of water removal from the soil profile or site. Both these aspects of internal drainage may be difficult to assess in the field, and cannot be based solely on profile morphology. Mottling may, but not always, reflect drainage status, since mottling may be a relict feature. Vegetation and topography may be useful guides.
These concepts of permeability and drainage are largely based on Canada Soil Survey Committee (1978).
""" ;
  skos:member <soilwater-drainage> ;
  skos:member <soilwater-permeability> ;
  skos:member <soilwater-status> ;
  skos:prefLabel "Soil water regime" ;
.
<soilwater-drainage>
  rdf:type skos:Collection ;
  dct:description "Drainage is a useful term to summarise local soil wetness conditions, that is, it provides a statement about soil and site drainage likely to occur in most years. It is affected by a number of attributes, both internal and external, that may act separately or together. Internal attributes include soil structure, texture, porosity, hydraulic conductivity, and water-holding capacity, while external attributes are source and quality of water, evapotranspiration, gradient and length of slope, and position in the landscape." ;
  ui:isMemberOf <soil-water-regime> ;
  rdfs:comment "C_O_DRAINAGE" ;
  rdfs:label "Drainage" ;
  skos:definition "Drainage is a useful term to summarise local soil wetness conditions, that is, it provides a statement about soil and site drainage likely to occur in most years. It is affected by a number of attributes, both internal and external, that may act separately or together. Internal attributes include soil structure, texture, porosity, hydraulic conductivity, and water-holding capacity, while external attributes are source and quality of water, evapotranspiration, gradient and length of slope, and position in the landscape." ;
  skos:member <soilwater-drainage-1> ;
  skos:member <soilwater-drainage-2> ;
  skos:member <soilwater-drainage-3> ;
  skos:member <soilwater-drainage-4> ;
  skos:member <soilwater-drainage-5> ;
  skos:member <soilwater-drainage-6> ;
  skos:prefLabel "Drainage" ;
.
<soilwater-drainage-1>
  rdf:type skos:Concept ;
  dct:description "Water is removed from the soil so slowly that the water table remains at or near the surface for most of the year. Surface flow, groundwater and subsurface flow are major sources of water, although precipitation may be important where there is a perched water table and precipitation exceeds evapotranspiration. Soils have a wide range in texture and depth, and often occur in depressed sites. Strong gleying and accumulation of surface organic matter are usually features of most soils." ;
  ui:isMemberOf <soilwater-drainage> ;
  rdfs:label "Very poorly drained" ;
  skos:definition "Water is removed from the soil so slowly that the water table remains at or near the surface for most of the year. Surface flow, groundwater and subsurface flow are major sources of water, although precipitation may be important where there is a perched water table and precipitation exceeds evapotranspiration. Soils have a wide range in texture and depth, and often occur in depressed sites. Strong gleying and accumulation of surface organic matter are usually features of most soils." ;
  skos:notation "1" ;
  skos:prefLabel "Very poorly drained"@en ;
  skos:topConceptOf <> ;
.
<soilwater-drainage-2>
  rdf:type skos:Concept ;
  dct:description "Water is removed very slowly in relation to supply. Subsurface and/or groundwater flow, as well as precipitation, may be a significant water source. Seasonal ponding, resulting from runon and insufficient outfall, also occurs. A perched water table may be present. Soils have a wide range in texture and depth; many have horizons that are gleyed, mottled, or possess orange or rusty linings of root channels. All horizons remain wet for periods of several months." ;
  ui:isMemberOf <soilwater-drainage> ;
  rdfs:label "Poorly drained" ;
  skos:definition "Water is removed very slowly in relation to supply. Subsurface and/or groundwater flow, as well as precipitation, may be a significant water source. Seasonal ponding, resulting from runon and insufficient outfall, also occurs. A perched water table may be present. Soils have a wide range in texture and depth; many have horizons that are gleyed, mottled, or possess orange or rusty linings of root channels. All horizons remain wet for periods of several months." ;
  skos:notation "2" ;
  skos:prefLabel "Poorly drained"@en ;
  skos:topConceptOf <> ;
.
<soilwater-drainage-3>
  rdf:type skos:Concept ;
  dct:description "Water is removed only slowly in relation to supply. Precipitation is the main source if available water storage capacity is high, but subsurface flow and/or groundwater contribute as available water storage capacity decreases. Soils have a wide range in texture and depth. Some horizons may be mottled and/or have orange or rusty linings of root channels, and are wet for several weeks." ;
  ui:isMemberOf <soilwater-drainage> ;
  rdfs:label "Imperfectly drained" ;
  skos:definition "Water is removed only slowly in relation to supply. Precipitation is the main source if available water storage capacity is high, but subsurface flow and/or groundwater contribute as available water storage capacity decreases. Soils have a wide range in texture and depth. Some horizons may be mottled and/or have orange or rusty linings of root channels, and are wet for several weeks." ;
  skos:notation "3" ;
  skos:prefLabel "Imperfectly drained"@en ;
  skos:topConceptOf <> ;
.
<soilwater-drainage-4>
  rdf:type skos:Concept ;
  dct:description "Water is removed from the soil somewhat slowly in relation to supply, due to low permeability, shallow water table, lack of gradient, or some combination of these. Soils are usually medium to fine in texture. Significant additions of water by subsurface flow are necessary in coarse-textured soils. Some horizons may remain wet for as long as one week after water addition." ;
  ui:isMemberOf <soilwater-drainage> ;
  rdfs:label "Moderately well drained" ;
  skos:definition "Water is removed from the soil somewhat slowly in relation to supply, due to low permeability, shallow water table, lack of gradient, or some combination of these. Soils are usually medium to fine in texture. Significant additions of water by subsurface flow are necessary in coarse-textured soils. Some horizons may remain wet for as long as one week after water addition." ;
  skos:notation "4" ;
  skos:prefLabel "Moderately well drained"@en ;
  skos:topConceptOf <> ;
.
<soilwater-drainage-5>
  rdf:type skos:Concept ;
  dct:description "Water is removed from the soil readily but not rapidly. Excess water flows downward readily into underlying, moderately permeable material or laterally as subsurface flow. The soils are often medium in texture. Some horizons may remain wet for several days after water addition." ;
  ui:isMemberOf <soilwater-drainage> ;
  rdfs:label "Well drained" ;
  skos:definition "Water is removed from the soil readily but not rapidly. Excess water flows downward readily into underlying, moderately permeable material or laterally as subsurface flow. The soils are often medium in texture. Some horizons may remain wet for several days after water addition." ;
  skos:notation "5" ;
  skos:prefLabel "Well drained"@en ;
  skos:topConceptOf <> ;
.
<soilwater-drainage-6>
  rdf:type skos:Concept ;
  dct:description "Water is removed from the soil rapidly in relation to supply. Excess water flows downward rapidly if underlying material is highly permeable. There may be rapid subsurface lateral flow during heavy rainfall provided there is a steep gradient. Soils are usually coarse-textured, or shallow, or both. No horizon is normally wet for more than several hours after water addition." ;
  ui:isMemberOf <soilwater-drainage> ;
  rdfs:label "Rapidly drained" ;
  skos:definition "Water is removed from the soil rapidly in relation to supply. Excess water flows downward rapidly if underlying material is highly permeable. There may be rapid subsurface lateral flow during heavy rainfall provided there is a steep gradient. Soils are usually coarse-textured, or shallow, or both. No horizon is normally wet for more than several hours after water addition." ;
  skos:notation "6" ;
  skos:prefLabel "Rapidly drained"@en ;
  skos:topConceptOf <> ;
.
<soilwater-permeability>
  rdf:type skos:Collection ;
  dct:description "Permeability is independent of climate and drainage, and – as applied to a soil – is controlled by the potential to transmit water (saturated hydraulic conductivity, Ks) of the least permeable layer in the soil. Therefore it is inferred from attributes of the soil such as structure, texture, porosity, cracks and shrink–swell properties. The rate of transmission of water in the profile is based on the assumption that loss by evapotranspiration is minimal. The Ks ranges are compatible with those of Nowland in Canada, as reported by McKeague et al. (1982)." ;
  ui:isMemberOf <soil-water-regime> ;
  rdfs:comment "C_PERMEABILITY" ;
  rdfs:label "Permeability" ;
  skos:definition "Permeability is independent of climate and drainage, and – as applied to a soil – is controlled by the potential to transmit water (saturated hydraulic conductivity, Ks) of the least permeable layer in the soil. Therefore it is inferred from attributes of the soil such as structure, texture, porosity, cracks and shrink–swell properties. The rate of transmission of water in the profile is based on the assumption that loss by evapotranspiration is minimal. The Ks ranges are compatible with those of Nowland in Canada, as reported by McKeague et al. (1982)." ;
  skos:member <soilwater-permeability-1> ;
  skos:member <soilwater-permeability-2> ;
  skos:member <soilwater-permeability-3> ;
  skos:member <soilwater-permeability-4> ;
  skos:prefLabel "Permeability" ;
.
<soilwater-permeability-1>
  rdf:type skos:Concept ;
  dct:description "Vertical transmission of water in the least permeable horizon is very slow; the profile would take periods of a month or more after thorough wetting to reach field capacity if there were no obstructions to movement from the profile. Structure may vary, but cracks or spaces between peds when dry close on wetting. Texture is usually clay or silty clay, and there are no pores visible (with a hand lens) that could conduct water when wet." ;
  ui:isMemberOf <soilwater-permeability> ;
  rdfs:comment """Ks range: <5 mm/day
Drainage time: months""" ;
  rdfs:label "Very slowly permeable" ;
  skos:definition "Vertical transmission of water in the least permeable horizon is very slow; the profile would take periods of a month or more after thorough wetting to reach field capacity if there were no obstructions to movement from the profile. Structure may vary, but cracks or spaces between peds when dry close on wetting. Texture is usually clay or silty clay, and there are no pores visible (with a hand lens) that could conduct water when wet." ;
  skos:notation "1" ;
  skos:prefLabel "Very slowly permeable"@en ;
  skos:topConceptOf <> ;
.
<soilwater-permeability-2>
  rdf:type skos:Concept ;
  dct:description "Vertical transmission of water in the least permeable horizon is slow; the profile would take periods of a week or more after thorough wetting to reach field capacity if there were no obstructions to movement from the profile. Structure may vary, usually from massive to moderate grade. Texture is usually clay or silty clay, and there will be few pores visible (with a hand lens) that conduct water when wet. If texture is coarser, the interparticle voids are filled with fine mineral." ;
  ui:isMemberOf <soilwater-permeability> ;
  rdfs:comment """Ks range: 5-50 mm/day
Drainage time: weeks""" ;
  rdfs:label "Slowly permeable" ;
  skos:definition "Vertical transmission of water in the least permeable horizon is slow; the profile would take periods of a week or more after thorough wetting to reach field capacity if there were no obstructions to movement from the profile. Structure may vary, usually from massive to moderate grade. Texture is usually clay or silty clay, and there will be few pores visible (with a hand lens) that conduct water when wet. If texture is coarser, the interparticle voids are filled with fine mineral." ;
  skos:notation "2" ;
  skos:prefLabel "Slowly permeable"@en ;
  skos:topConceptOf <> ;
.
<soilwater-permeability-3>
  rdf:type skos:Concept ;
  dct:description "Vertical transmission of water in the least permeable horizon is such that the profile would take no more than a number (1–5) of days after a thorough wetting to reach field capacity if there were no obstructions to water movement from the profile. The soil may vary in structure but grade is usually at least moderate, and blocky or polyhedral peds are common. If massive, the soil material is always porous. The pores and channels that remain open when wet are clearly visible with a hand lens." ;
  ui:isMemberOf <soilwater-permeability> ;
  rdfs:comment """Ks range: 50-500 mm/day
Drainage time: days""" ;
  rdfs:label "Moderately permeable" ;
  skos:definition "Vertical transmission of water in the least permeable horizon is such that the profile would take no more than a number (1–5) of days after a thorough wetting to reach field capacity if there were no obstructions to water movement from the profile. The soil may vary in structure but grade is usually at least moderate, and blocky or polyhedral peds are common. If massive, the soil material is always porous. The pores and channels that remain open when wet are clearly visible with a hand lens." ;
  skos:notation "3" ;
  skos:prefLabel "Moderately permeable"@en ;
  skos:topConceptOf <> ;
.
<soilwater-permeability-4>
  rdf:type skos:Concept ;
  dct:description "Vertical transmission of water in the least permeable horizon is such that the profile would take no more than a number (1–12) of hours after a thorough wetting to reach field capacity if there were no obstructions to water movement from the profile. Horizons have large, continuous and clearly visible connecting pores and cracks that do not close with wetting. Texture is usually sandy and nodules or gravel are commonly present. Soil horizons are usually apedal, but some medium- to fine-textured soils with strong granular structure or cementation of aggregates can be highly permeable." ;
  ui:isMemberOf <soilwater-permeability> ;
  rdfs:comment """Ks range: >500 mm/day
Drainage time: hours""" ;
  rdfs:label "Highly permeable" ;
  skos:definition "Vertical transmission of water in the least permeable horizon is such that the profile would take no more than a number (1–12) of hours after a thorough wetting to reach field capacity if there were no obstructions to water movement from the profile. Horizons have large, continuous and clearly visible connecting pores and cracks that do not close with wetting. Texture is usually sandy and nodules or gravel are commonly present. Soil horizons are usually apedal, but some medium- to fine-textured soils with strong granular structure or cementation of aggregates can be highly permeable." ;
  skos:notation "4" ;
  skos:prefLabel "Highly permeable"@en ;
  skos:topConceptOf <> ;
.
<soilwater-status>
  rdf:type skos:Collection ;
  dct:description """Give soil water status of the soil at the time of description (see Table 30).
It may also be relevant to note the weather conditions immediately prior to examination of the soil if these are known, for example a soil may be wet because of local rain or from seepage.
The following guidelines may be used as a crude approximation of soil water status:

Dry is below wilting point. Material becomes darker or has lower colour value when moistened.
Moderately moist is the drier half of the available moisture range.
Moist is the wetter half of the available moisture range.
Wet is at, or exceeding, field capacity. Will wet and/or stick to fingers when moulded.""" ;
  ui:isMemberOf <soil-water-regime> ;
  rdfs:label "Soil water status" ;
  skos:definition """Give soil water status of the soil at the time of description (see Table 30).
It may also be relevant to note the weather conditions immediately prior to examination of the soil if these are known, for example a soil may be wet because of local rain or from seepage.
The following guidelines may be used as a crude approximation of soil water status:

Dry is below wilting point. Material becomes darker or has lower colour value when moistened.
Moderately moist is the drier half of the available moisture range.
Moist is the wetter half of the available moisture range.
Wet is at, or exceeding, field capacity. Will wet and/or stick to fingers when moulded.""" ;
  skos:member <soilwater-status-D> ;
  skos:member <soilwater-status-M> ;
  skos:member <soilwater-status-T> ;
  skos:member <soilwater-status-W> ;
  skos:prefLabel "Soil water status" ;
.
<soilwater-status-D>
  rdf:type skos:Concept ;
  dct:description "Dry is below wilting point. Material becomes darker or has lower colour value when moistened" ;
  ui:isMemberOf <soilwater-status> ;
  rdfs:comment """See table 30 - behaviour of soils subjected to field test
These guidelines may not apply with sodic 2:1 clays, as, for example, they may be moderately moist but below wilting point.""" ;
  rdfs:label "Dry" ;
  skos:definition "Dry is below wilting point. Material becomes darker or has lower colour value when moistened" ;
  skos:notation "D" ;
  skos:prefLabel "Dry"@en ;
  skos:topConceptOf <> ;
.
<soilwater-status-M>
  rdf:type skos:Concept ;
  dct:description "Moist is the wetter half of the available moisture range." ;
  ui:isMemberOf <soilwater-status> ;
  rdfs:comment """See table 30 - behaviour of soils subjected to field test
These guidelines may not apply with sodic 2:1 clays, as, for example, they may be moderately moist but below wilting point.""" ;
  rdfs:label "Moist" ;
  skos:definition "Moist is the wetter half of the available moisture range." ;
  skos:notation "M" ;
  skos:prefLabel "Moist"@en ;
  skos:topConceptOf <> ;
.
<soilwater-status-T>
  rdf:type skos:Concept ;
  dct:description "Moderately moist is the drier half of the available moisture range" ;
  ui:isMemberOf <soilwater-status> ;
  rdfs:comment """See table 30 - behaviour of soils subjected to field test
These guidelines may not apply with sodic 2:1 clays, as, for example, they may be moderately moist but below wilting point.""" ;
  rdfs:label "Moderately moist" ;
  skos:definition "Moderately moist is the drier half of the available moisture range" ;
  skos:notation "T" ;
  skos:prefLabel "Moderately moist"@en ;
  skos:topConceptOf <> ;
.
<soilwater-status-W>
  rdf:type skos:Concept ;
  dct:description "Wet is at, or exceeding, field capacity. Will wet and/or stick to fingers when moulded." ;
  ui:isMemberOf <soilwater-status> ;
  rdfs:comment """See table 30 - behaviour of soils subjected to field test
These guidelines may not apply with sodic 2:1 clays, as, for example, they may be moderately moist but below wilting point.""" ;
  rdfs:label "Wet" ;
  skos:definition "Wet is at, or exceeding, field capacity. Will wet and/or stick to fingers when moulded." ;
  skos:notation "W" ;
  skos:prefLabel "Wet"@en ;
  skos:topConceptOf <> ;
.
<structure>
  rdf:type skos:Collection ;
  dc:description """Soil structure refers to the distinctness, size and shape of peds. A ped is an individual natural soil aggregate consisting of a cluster of primary particles. Peds are separated from adjoining peds by surfaces of weakness that are recognisable as natural voids or by the occurrence of cutans (Brewer 1960).
Soil structure can only be described reliably in a relatively fresh vertical exposure or relatively undisturbed soil core, not from an auger boring. Vertical exposures that have been exposed for a long time (road cuttings, gullies) are unsuitable for the determination of structure that may alter due to daily or seasonal changes in moisture and temperature.""" ;
  dct:description """Soil structure refers to the distinctness, size and shape of peds. A ped is an individual natural soil aggregate consisting of a cluster of primary particles. Peds are separated from adjoining peds by surfaces of weakness that are recognisable as natural voids or by the occurrence of cutans (Brewer 1960).
Soil structure can only be described reliably in a relatively fresh vertical exposure or relatively undisturbed soil core, not from an auger boring. Vertical exposures that have been exposed for a long time (road cuttings, gullies) are unsuitable for the determination of structure that may alter due to daily or seasonal changes in moisture and temperature.""" ;
  ui:topMemberOf <> ;
  rdfs:label "Structure" ;
  skos:definition """Soil structure refers to the distinctness, size and shape of peds. A ped is an individual natural soil aggregate consisting of a cluster of primary particles. Peds are separated from adjoining peds by surfaces of weakness that are recognisable as natural voids or by the occurrence of cutans (Brewer 1960).
Soil structure can only be described reliably in a relatively fresh vertical exposure or relatively undisturbed soil core, not from an auger boring. Vertical exposures that have been exposed for a long time (road cuttings, gullies) are unsuitable for the determination of structure that may alter due to daily or seasonal changes in moisture and temperature.""" ;
  skos:member <structure-artificial> ;
  skos:member <structure-pedality-compound> ;
  skos:member <structure-pedality-grade> ;
  skos:member <structure-pedality-size> ;
  skos:member <structure-pedality-type> ;
  skos:prefLabel "Structure" ;
.
<structure-artificial>
  rdf:type skos:Collection ;
  dct:description "Cultivated horizons (Ap horizons) often consist of artificial aggregates formed by cultivation or work being done on the soil. The distinction between artificial aggregates and peds can be difficult. In cultivated horizons, where the pedologist is confident the aggregates are natural peds they should be recorded as such. If the pedologist is doubtful, or the aggregates are obviously artificial, they should be recorded as clods or fragments." ;
  ui:isMemberOf <structure> ;
  rdfs:label "Artificial aggregates" ;
  skos:definition "Cultivated horizons (Ap horizons) often consist of artificial aggregates formed by cultivation or work being done on the soil. The distinction between artificial aggregates and peds can be difficult. In cultivated horizons, where the pedologist is confident the aggregates are natural peds they should be recorded as such. If the pedologist is doubtful, or the aggregates are obviously artificial, they should be recorded as clods or fragments." ;
  skos:member <structure-artificial-CL> ;
  skos:member <structure-artificial-FR> ;
  skos:prefLabel "Artificial aggregates" ;
.
<structure-artificial-CL>
  rdf:type skos:Concept ;
  dct:description "artificial aggregate with diameter 100 mm or more" ;
  ui:isMemberOf <structure-artificial> ;
  rdfs:label "Clod" ;
  skos:definition "artificial aggregate with diameter 100 mm or more" ;
  skos:notation "CL" ;
  skos:prefLabel "Clod" ;
  skos:topConceptOf <> ;
.
<structure-artificial-FR>
  rdf:type skos:Concept ;
  dct:description "artificial aggregate with diameter less than 100 mm" ;
  ui:isMemberOf <structure-artificial> ;
  rdfs:label "Fragment" ;
  skos:definition "artificial aggregate with diameter less than 100 mm" ;
  skos:notation "FR" ;
  skos:prefLabel "Fragment" ;
  skos:topConceptOf <> ;
.
<structure-pedality-compound>
  rdf:type skos:Collection ;
  dct:description """Compound pedality occurs where large peds part along natural planes of weakness to form smaller peds, which may again part to smaller peds, and so on to the smallest or primary peds.
Primary peds are the simplest peds occurring in soil material; they cannot be divided into smaller peds, but may be packed together to form compound peds of a higher level of organisation (Brewer 1964).
The order of peds and relationship of one to the other is important and may be described as the larger peds parting to the smaller and further where necessary. For example, strong 50100 mm columnar, parting to moderate 2050 mm prismatic, parting to moderate
1020 mm angular blocky. The word parting and not breaking is used. The term breaking is used when soil is fractured along planes other than natural planes of weakness.
1	Largest peds (in the type of soil observation described), parting to
2	Next size peds, parting to
3	Next size peds, ... and further, if required, to the primary ped.""" ;
  ui:isMemberOf <structure> ;
  rdfs:label "Compound pedality" ;
  skos:definition """Compound pedality occurs where large peds part along natural planes of weakness to form smaller peds, which may again part to smaller peds, and so on to the smallest or primary peds.
Primary peds are the simplest peds occurring in soil material; they cannot be divided into smaller peds, but may be packed together to form compound peds of a higher level of organisation (Brewer 1964).
The order of peds and relationship of one to the other is important and may be described as the larger peds parting to the smaller and further where necessary. For example, strong 50100 mm columnar, parting to moderate 2050 mm prismatic, parting to moderate
1020 mm angular blocky. The word parting and not breaking is used. The term breaking is used when soil is fractured along planes other than natural planes of weakness.
1	Largest peds (in the type of soil observation described), parting to
2	Next size peds, parting to
3	Next size peds, ... and further, if required, to the primary ped.""" ;
  skos:prefLabel "Compound pedality" ;
.
<structure-pedality-grade>
  rdf:type skos:Collection ;
  dct:description "Grade of pedality is the degree of development and distinctness of peds. In virtually all material that has structure, the surface of individual peds will differ in some way from the interior of peds. The degree of development expresses the relative difference between the strength of cohesion within peds and the strength of adhesion between adjacent peds. Determination of grade of structure in the field depends on the proportion of peds that hold together as entire peds when displaced and also on the ease with which the soil separates into discrete peds. Grade of pedality varies with the soil water status. It is important to record the soil water status of the described profile, and it is desirable that the grade of pedality be described at the soil water status most common for the horizon." ;
  ui:isMemberOf <structure> ;
  rdfs:comment "C_STR_PED_GRADE" ;
  rdfs:label "Grade of pedality" ;
  skos:definition "Grade of pedality is the degree of development and distinctness of peds. In virtually all material that has structure, the surface of individual peds will differ in some way from the interior of peds. The degree of development expresses the relative difference between the strength of cohesion within peds and the strength of adhesion between adjacent peds. Determination of grade of structure in the field depends on the proportion of peds that hold together as entire peds when displaced and also on the ease with which the soil separates into discrete peds. Grade of pedality varies with the soil water status. It is important to record the soil water status of the described profile, and it is desirable that the grade of pedality be described at the soil water status most common for the horizon." ;
  skos:member <structure-pedality-grade-G> ;
  skos:member <structure-pedality-grade-M> ;
  skos:member <structure-pedality-grade-S> ;
  skos:member <structure-pedality-grade-V> ;
  skos:member <structure-pedality-grade-W> ;
  skos:prefLabel "Grade of pedality" ;
.
<structure-pedality-grade-G>
  rdf:type skos:Concept ;
  dct:description "loose, incoherent* mass of individual particles. When displaced, soil separates into ultimate particles." ;
  ui:isMemberOf <structure-pedality-grade> ;
  rdfs:comment """Apedal soil (no observable peds)
*Incoherent means that less than two-thirds of the soil material will remain united at the given moisture state without very small force (force 1, see ‘Consistence’ on page 138) having been applied""" ;
  rdfs:label "Single grain" ;
  skos:definition "loose, incoherent* mass of individual particles. When displaced, soil separates into ultimate particles." ;
  skos:notation "G" ;
  skos:prefLabel "Single grain" ;
  skos:topConceptOf <> ;
.
<structure-pedality-grade-M>
  rdf:type skos:Concept ;
  dct:description "peds well-formed and evident but not distinct in undisplaced soil. Adhesion between peds is usually firm or stronger. When displaced, more than one-third of the soil material consists of entire peds, the remainder consisting of broken peds, fragments and ultimate particles." ;
  ui:isMemberOf <structure-pedality-grade> ;
  rdfs:comment "Pedal soil (observable peds)" ;
  rdfs:label "Moderate" ;
  skos:definition "peds well-formed and evident but not distinct in undisplaced soil. Adhesion between peds is usually firm or stronger. When displaced, more than one-third of the soil material consists of entire peds, the remainder consisting of broken peds, fragments and ultimate particles." ;
  skos:notation "M" ;
  skos:prefLabel "Moderate" ;
  skos:topConceptOf <> ;
.
<structure-pedality-grade-S>
  rdf:type skos:Concept ;
  dct:description "peds quite distinct in undisplaced soil. Adhesion between peds is usually firm or weaker. When displaced, more than two-thirds of the soil material consists of entire peds." ;
  ui:isMemberOf <structure-pedality-grade> ;
  rdfs:comment "Pedal soil (observable peds)" ;
  rdfs:label "Strong" ;
  skos:definition "peds quite distinct in undisplaced soil. Adhesion between peds is usually firm or weaker. When displaced, more than two-thirds of the soil material consists of entire peds." ;
  skos:notation "S" ;
  skos:prefLabel "Strong" ;
  skos:topConceptOf <> ;
.
<structure-pedality-grade-V>
  rdf:type skos:Concept ;
  dct:description "coherent. When displaced, soil separates into fragments (see page 133), which may be crushed to ultimate particles." ;
  ui:isMemberOf <structure-pedality-grade> ;
  rdfs:comment """Apedal soil (no observable peds)
*Coherent means that two-thirds or more of the soil material will remain united at the given moisture state unless force is applied""" ;
  rdfs:label "Massive" ;
  skos:definition "coherent*. When displaced, soil separates into fragments (see page 133), which may be crushed to ultimate particles." ;
  skos:notation "V" ;
  skos:prefLabel "Massive" ;
  skos:topConceptOf <> ;
.
<structure-pedality-grade-W>
  rdf:type skos:Concept ;
  dct:description "peds indistinct and barely observable in undisplaced soil. When displaced, up to one-third of the soil material consists of peds, the remainder consisting of variable amounts of fragments and ultimate particles." ;
  ui:isMemberOf <structure-pedality-grade> ;
  rdfs:comment "Pedal soil (observable peds)" ;
  rdfs:label "Weak" ;
  skos:definition "peds indistinct and barely observable in undisplaced soil. When displaced, up to one-third of the soil material consists of peds, the remainder consisting of variable amounts of fragments and ultimate particles." ;
  skos:notation "W" ;
  skos:prefLabel "Weak" ;
  skos:topConceptOf <> ;
.
<structure-pedality-size>
  rdf:type skos:Collection ;
  dct:description "The average least dimension of peds is used to determine the class interval. The least dimension is the vertical dimension for platy structure; the horizontal dimension for prismatic, columnar, blocky and polyhedral peds; the maximum separation of convex faces for lenticular peds; and the diameter for granular peds." ;
  ui:isMemberOf <structure> ;
  rdfs:comment "N_STR_PED_SIZE" ;
  rdfs:label "Size of peds" ;
  skos:definition "Figure 17" ;
  skos:member <structure-pedality-size-1> ;
  skos:member <structure-pedality-size-2> ;
  skos:member <structure-pedality-size-3> ;
  skos:member <structure-pedality-size-4> ;
  skos:member <structure-pedality-size-5> ;
  skos:member <structure-pedality-size-6> ;
  skos:member <structure-pedality-size-7> ;
  skos:member <structure-pedality-size-8> ;
  skos:member <structure-pedality-size-9> ;
  skos:prefLabel "Size of peds" ;
.
<structure-pedality-size-1>
  rdf:type skos:Concept ;
  dc:description "<2 mm" ;
  dct:description "<2 mm" ;
  ui:isMemberOf <structure-pedality-size> ;
  rdfs:label "less than 2 mm" ;
  skos:definition "<2 mm" ;
  skos:notation "1" ;
  skos:prefLabel "less than 2 mm" ;
  skos:topConceptOf <> ;
.
<structure-pedality-size-2>
  rdf:type skos:Concept ;
  dc:description "2-5 mm" ;
  dct:description "2-5 mm" ;
  ui:isMemberOf <structure-pedality-size> ;
  rdfs:label "2-5 mm" ;
  skos:definition "2-5 mm" ;
  skos:notation "2" ;
  skos:prefLabel "2-5 mm" ;
  skos:topConceptOf <> ;
.
<structure-pedality-size-3>
  rdf:type skos:Concept ;
  dc:description "5-10 mm" ;
  dct:description "5-10 mm" ;
  ui:isMemberOf <structure-pedality-size> ;
  rdfs:label "5-10 mm" ;
  skos:definition "5-10 mm" ;
  skos:notation "3" ;
  skos:prefLabel "5-10 mm" ;
  skos:topConceptOf <> ;
.
<structure-pedality-size-4>
  rdf:type skos:Concept ;
  dc:description "10-20 mm" ;
  dct:description "10-20 mm" ;
  ui:isMemberOf <structure-pedality-size> ;
  rdfs:label "10-20 mm" ;
  skos:definition "10-20 mm" ;
  skos:notation "4" ;
  skos:prefLabel "10-20 mm" ;
  skos:topConceptOf <> ;
.
<structure-pedality-size-5>
  rdf:type skos:Concept ;
  dc:description "20-50 mm" ;
  dct:description "20-50 mm" ;
  ui:isMemberOf <structure-pedality-size> ;
  rdfs:label "20-50 mm" ;
  skos:definition "20-50 mm" ;
  skos:notation "5" ;
  skos:prefLabel "20-50 mm" ;
  skos:topConceptOf <> ;
.
<structure-pedality-size-6>
  rdf:type skos:Concept ;
  dc:description "50-100 mm" ;
  dct:description "50-100 mm" ;
  ui:isMemberOf <structure-pedality-size> ;
  rdfs:label "50-100 mm" ;
  skos:definition "50-100 mm" ;
  skos:notation "6" ;
  skos:prefLabel "50-100 mm" ;
  skos:topConceptOf <> ;
.
<structure-pedality-size-7>
  rdf:type skos:Concept ;
  dc:description "100-200 mm" ;
  dct:description "100-200 mm" ;
  ui:isMemberOf <structure-pedality-size> ;
  rdfs:label "100-200 mm" ;
  skos:definition "100-200 mm" ;
  skos:notation "7" ;
  skos:prefLabel "100-200 mm" ;
  skos:topConceptOf <> ;
.
<structure-pedality-size-8>
  rdf:type skos:Concept ;
  dc:description "200-500 mm" ;
  dct:description "200-500 mm" ;
  ui:isMemberOf <structure-pedality-size> ;
  rdfs:label "200-500 mm" ;
  skos:definition "200-500 mm" ;
  skos:notation "8" ;
  skos:prefLabel "200-500 mm" ;
  skos:topConceptOf <> ;
.
<structure-pedality-size-9>
  rdf:type skos:Concept ;
  dc:description ">500 mm" ;
  dct:description ">500 mm" ;
  ui:isMemberOf <structure-pedality-size> ;
  rdfs:label "more than 500 mm" ;
  skos:definition ">500 mm" ;
  skos:notation "9" ;
  skos:prefLabel "more than 500 mm" ;
  skos:topConceptOf <> ;
.
<structure-pedality-type>
  rdf:type skos:Collection ;
  dct:description "The types of structure are illustrated in diagrammatic form." ;
  ui:isMemberOf <structure> ;
  rdfs:comment "C_STR_PED_TYPE" ;
  rdfs:label "Type of pedality" ;
  skos:definition "Figure 17" ;
  skos:member <structure-pedality-type-AB> ;
  skos:member <structure-pedality-type-CA> ;
  skos:member <structure-pedality-type-CO> ;
  skos:member <structure-pedality-type-GR> ;
  skos:member <structure-pedality-type-LE> ;
  skos:member <structure-pedality-type-PL> ;
  skos:member <structure-pedality-type-PO> ;
  skos:member <structure-pedality-type-PR> ;
  skos:member <structure-pedality-type-SB> ;
  skos:prefLabel "Type of pedality" ;
.
<structure-pedality-type-AB>
  rdf:type skos:Concept ;
  dct:description "Soil particles arranged around a point and bounded by six relatively flat, roughly equal faces. Re-entrant angles between adjoining faces are few or absent. There is usually much accommodation of ped faces to the faces of surrounding peds. Most vertices between adjoining faces are angular.	Angular blocky	Soil particles arranged around a point and bounded by six relatively flat, roughly equal faces. Re-entrant angles between adjoining faces are few or absent. There is usually much accommodation of ped faces to the faces of surrounding peds. Most vertices between adjoining faces are angular." ;
  ui:isMemberOf <structure-pedality-type> ;
  rdfs:label "Angular blocky" ;
  skos:definition "Soil particles arranged around a point and bounded by six relatively flat, roughly equal faces. Re-entrant angles between adjoining faces are few or absent. There is usually much accommodation of ped faces to the faces of surrounding peds. Most vertices between adjoining faces are angular.	Angular blocky	Soil particles arranged around a point and bounded by six relatively flat, roughly equal faces. Re-entrant angles between adjoining faces are few or absent. There is usually much accommodation of ped faces to the faces of surrounding peds. Most vertices between adjoining faces are angular." ;
  skos:notation "AB" ;
  skos:prefLabel "Angular blocky" ;
  skos:topConceptOf <> ;
.
<structure-pedality-type-CA>
  rdf:type skos:Concept ;
  dct:description "Faunal casts are strictly not peds, but they are described in a similar manner. They are formed from, or are deposited in, the O horizons or the soil solum and include: excreta of soil fauna which may be discrete particles, for example insect faeces or the dense, coherent, globular forms of earthworm excreta. They are generally spherical or ovate in shape and have a strong conchoidal fracture; soil masticated with salivary secretions into globular forms, for example, by ants, crickets, wasps.	Cast	Faunal casts are strictly not peds, but they are described in a similar manner. They are formed from, or are deposited in, the O horizons or the soil solum and include: excreta of soil fauna which may be discrete particles, for example insect faeces or the dense, coherent, globular forms of earthworm excreta. They are generally spherical or ovate in shape and have a strong conchoidal fracture; soil masticated with salivary secretions into globular forms, for example, by ants, crickets, wasps." ;
  ui:isMemberOf <structure-pedality-type> ;
  rdfs:label "Cast" ;
  skos:definition "Faunal casts are strictly not peds, but they are described in a similar manner. They are formed from, or are deposited in, the O horizons or the soil solum and include: excreta of soil fauna which may be discrete particles, for example insect faeces or the dense, coherent, globular forms of earthworm excreta. They are generally spherical or ovate in shape and have a strong conchoidal fracture; soil masticated with salivary secretions into globular forms, for example, by ants, crickets, wasps.	Cast	Faunal casts are strictly not peds, but they are described in a similar manner. They are formed from, or are deposited in, the O horizons or the soil solum and include: excreta of soil fauna which may be discrete particles, for example insect faeces or the dense, coherent, globular forms of earthworm excreta. They are generally spherical or ovate in shape and have a strong conchoidal fracture; soil masticated with salivary secretions into globular forms, for example, by ants, crickets, wasps." ;
  skos:notation "CA" ;
  skos:prefLabel "Cast" ;
  skos:topConceptOf <> ;
.
<structure-pedality-type-CO>
  rdf:type skos:Concept ;
  dct:description "Soil particles arranged around a vertical axis and bounded by well-defined, relatively flat faces with much accommodation to the faces of surrounding peds. Vertices between adjoining faces are usually angular with domed tops.	Columnar	Soil particles arranged around a vertical axis and bounded by well-defined, relatively flat faces with much accommodation to the faces of surrounding peds. Vertices between adjoining faces are usually angular with domed tops." ;
  ui:isMemberOf <structure-pedality-type> ;
  rdfs:label "Columnar" ;
  skos:definition "Soil particles arranged around a vertical axis and bounded by well-defined, relatively flat faces with much accommodation to the faces of surrounding peds. Vertices between adjoining faces are usually angular with domed tops.	Columnar	Soil particles arranged around a vertical axis and bounded by well-defined, relatively flat faces with much accommodation to the faces of surrounding peds. Vertices between adjoining faces are usually angular with domed tops." ;
  skos:notation "CO" ;
  skos:prefLabel "Columnar" ;
  skos:topConceptOf <> ;
.
<structure-pedality-type-GR>
  rdf:type skos:Concept ;
  dct:description "Spheroidal with limited accommodation to the faces of surrounding peds.	Granular	Spheroidal with limited accommodation to the faces of surrounding peds." ;
  ui:isMemberOf <structure-pedality-type> ;
  rdfs:label "Granular" ;
  skos:definition "Spheroidal with limited accommodation to the faces of surrounding peds.	Granular	Spheroidal with limited accommodation to the faces of surrounding peds." ;
  skos:notation "GR" ;
  skos:prefLabel "Granular" ;
  skos:topConceptOf <> ;
.
<structure-pedality-type-LE>
  rdf:type skos:Concept ;
  dct:description "Soil particles arranged around an elliptical or circular plane and bounded by curved faces with much accommodation to the faces of surrounding peds. Most vertices are angular and acute.	Lenticular	Soil particles arranged around an elliptical or circular plane and bounded by curved faces with much accommodation to the faces of surrounding peds. Most vertices are angular and acute." ;
  ui:isMemberOf <structure-pedality-type> ;
  rdfs:label "Lenticular" ;
  skos:definition "Soil particles arranged around an elliptical or circular plane and bounded by curved faces with much accommodation to the faces of surrounding peds. Most vertices are angular and acute.	Lenticular	Soil particles arranged around an elliptical or circular plane and bounded by curved faces with much accommodation to the faces of surrounding peds. Most vertices are angular and acute." ;
  skos:notation "LE" ;
  skos:prefLabel "Lenticular" ;
  skos:topConceptOf <> ;
.
<structure-pedality-type-PL>
  rdf:type skos:Concept ;
  dct:description "Soil particles arranged around a horizontal plane and bounded by relatively flat horizontal faces with much accommodation to the faces of surrounding peds.	Platy	Soil particles arranged around a horizontal plane and bounded by relatively flat horizontal faces with much accommodation to the faces of surrounding peds." ;
  ui:isMemberOf <structure-pedality-type> ;
  rdfs:label "Platy" ;
  skos:definition "Soil particles arranged around a horizontal plane and bounded by relatively flat horizontal faces with much accommodation to the faces of surrounding peds.	Platy	Soil particles arranged around a horizontal plane and bounded by relatively flat horizontal faces with much accommodation to the faces of surrounding peds." ;
  skos:notation "PL" ;
  skos:prefLabel "Platy" ;
  skos:topConceptOf <> ;
.
<structure-pedality-type-PO>
  rdf:type skos:Concept ;
  dct:description "Soil particles arranged around a point and bounded by more than six relatively flat, unequal, dissimilar faces. Re-entrant angles between adjoining faces are a feature. There is usually much accommodation of ped faces to the faces of surrounding peds. Most vertices are angular.	Polyhedral	Soil particles arranged around a point and bounded by more than six relatively flat, unequal, dissimilar faces. Re-entrant angles between adjoining faces are a feature. There is usually much accommodation of ped faces to the faces of surrounding peds. Most vertices are angular." ;
  ui:isMemberOf <structure-pedality-type> ;
  rdfs:label "Polyhedral" ;
  skos:definition "Soil particles arranged around a point and bounded by more than six relatively flat, unequal, dissimilar faces. Re-entrant angles between adjoining faces are a feature. There is usually much accommodation of ped faces to the faces of surrounding peds. Most vertices are angular.	Polyhedral	Soil particles arranged around a point and bounded by more than six relatively flat, unequal, dissimilar faces. Re-entrant angles between adjoining faces are a feature. There is usually much accommodation of ped faces to the faces of surrounding peds. Most vertices are angular." ;
  skos:notation "PO" ;
  skos:prefLabel "Polyhedral" ;
  skos:topConceptOf <> ;
.
<structure-pedality-type-PR>
  rdf:type skos:Concept ;
  dct:description "Soil particles arranged around a vertical axis and bounded by well-defined, relatively flat faces with much accommodation to the faces of surrounding peds. Vertices between adjoining faces are usually angular.	Prismatic	Soil particles arranged around a vertical axis and bounded by well-defined, relatively flat faces with much accommodation to the faces of surrounding peds. Vertices between adjoining faces are usually angular." ;
  ui:isMemberOf <structure-pedality-type> ;
  rdfs:label "Prismatic" ;
  skos:definition "Soil particles arranged around a vertical axis and bounded by well-defined, relatively flat faces with much accommodation to the faces of surrounding peds. Vertices between adjoining faces are usually angular.	Prismatic	Soil particles arranged around a vertical axis and bounded by well-defined, relatively flat faces with much accommodation to the faces of surrounding peds. Vertices between adjoining faces are usually angular." ;
  skos:notation "PR" ;
  skos:prefLabel "Prismatic" ;
  skos:topConceptOf <> ;
.
<structure-pedality-type-SB>
  rdf:type skos:Concept ;
  dct:description "Soil particles arranged around a point and bounded by flat and rounded faces with limited accommodation to the faces of surrounding peds. Many vertices are rounded.	Subangular blocky	Soil particles arranged around a point and bounded by flat and rounded faces with limited accommodation to the faces of surrounding peds. Many vertices are rounded." ;
  ui:isMemberOf <structure-pedality-type> ;
  rdfs:label "Subangular blocky" ;
  skos:definition "Soil particles arranged around a point and bounded by flat and rounded faces with limited accommodation to the faces of surrounding peds. Many vertices are rounded.	Subangular blocky	Soil particles arranged around a point and bounded by flat and rounded faces with limited accommodation to the faces of surrounding peds. Many vertices are rounded." ;
  skos:notation "SB" ;
  skos:prefLabel "Subangular blocky" ;
  skos:topConceptOf <> ;
.
<surfacecondition-C>
  rdf:type skos:Concept ;
  dct:description "distinct surface layer, often laminated, ranging in thickness from a few millimetres to a few tens of millimetres, which is hard and brittle when dry and cannot be readily separated from, and lifted off, the underlying soil material" ;
  ui:isMemberOf <condition-of-surface-soil-when-dry> ;
  rdfs:label "Surface crust" ;
  skos:definition "distinct surface layer, often laminated, ranging in thickness from a few millimetres to a few tens of millimetres, which is hard and brittle when dry and cannot be readily separated from, and lifted off, the underlying soil material" ;
  skos:notation "C" ;
  skos:prefLabel "Surface crust"@en ;
  skos:topConceptOf <> ;
.
<surfacecondition-F>
  rdf:type skos:Concept ;
  dct:description "coherent mass of individual particles or aggregates. Surface disturbed or indented by moderate pressure of forefinger" ;
  ui:isMemberOf <condition-of-surface-soil-when-dry> ;
  rdfs:label "Firm" ;
  skos:definition "coherent mass of individual particles or aggregates. Surface disturbed or indented by moderate pressure of forefinger" ;
  skos:notation "F" ;
  skos:note "Coherent means that two-thirds of the soil material, whether composed of peds or not, will remain united at the given moisture state unless force is applied" ;
  skos:prefLabel "Firm"@en ;
  skos:topConceptOf <> ;
.
<surfacecondition-G>
  rdf:type skos:Concept ;
  dct:description "cracks at least 5 mm wide and extending upwards to the surface or to the base of any plough layer or thin (<0.03 m) surface horizon" ;
  ui:isMemberOf <condition-of-surface-soil-when-dry> ;
  rdfs:label "Cracking" ;
  skos:definition "cracks at least 5 mm wide and extending upwards to the surface or to the base of any plough layer or thin (<0.03 m) surface horizon" ;
  skos:notation "G" ;
  skos:prefLabel "Cracking"@en ;
  skos:topConceptOf <> ;
.
<surfacecondition-H>
  rdf:type skos:Concept ;
  dct:description "compact, hard, apparently apedal condition forms on drying but softens on wetting. When dry, the material is hard below any surface crust or flake that may occur, and is not disturbed or indented by pressure of forefinger" ;
  ui:isMemberOf <condition-of-surface-soil-when-dry> ;
  rdfs:label "Hard setting" ;
  skos:definition "compact, hard, apparently apedal condition forms on drying but softens on wetting. When dry, the material is hard below any surface crust or flake that may occur, and is not disturbed or indented by pressure of forefinger" ;
  skos:notation "H" ;
  skos:prefLabel "Hard setting"@en ;
  skos:topConceptOf <> ;
.
<surfacecondition-L>
  rdf:type skos:Concept ;
  dct:description "incoherent mass of individual particles or aggregates. Surface easily disturbed by pressure of forefinger" ;
  ui:isMemberOf <condition-of-surface-soil-when-dry> ;
  rdfs:label "Loose" ;
  skos:definition "incoherent mass of individual particles or aggregates. Surface easily disturbed by pressure of forefinger" ;
  skos:notation "L" ;
  skos:note "Incoherent means that less than two-thirds of the soil material, whether composed of peds or not, will remain united at the given moisture state without very small force (force 1, see ‘Consistence’) having been applied" ;
  skos:prefLabel "Loose"@en ;
  skos:topConceptOf <> ;
.
<surfacecondition-M>
  rdf:type skos:Concept ;
  dct:description "strongly pedal loose surface mulch forms on wetting and drying. Peds commonly less than 5 mm in least dimension" ;
  ui:isMemberOf <condition-of-surface-soil-when-dry> ;
  rdfs:label "Self-mulching" ;
  skos:definition "strongly pedal loose surface mulch forms on wetting and drying. Peds commonly less than 5 mm in least dimension" ;
  skos:notation "M" ;
  skos:prefLabel "Self-mulching"@en ;
  skos:topConceptOf <> ;
.
<surfacecondition-O>
  rdf:type skos:Concept ;
  dct:description "Other" ;
  ui:isMemberOf <condition-of-surface-soil-when-dry> ;
  rdfs:label "Other" ;
  skos:definition "Other" ;
  skos:notation "O" ;
  skos:prefLabel "Other"@en ;
  skos:topConceptOf <> ;
.
<surfacecondition-P>
  rdf:type skos:Concept ;
  dct:description "soil that has been extensively trampled under wet conditions by hoofed animals" ;
  ui:isMemberOf <condition-of-surface-soil-when-dry> ;
  rdfs:label "Poached" ;
  skos:definition "soil that has been extensively trampled under wet conditions by hoofed animals" ;
  skos:notation "P" ;
  skos:prefLabel "Poached"@en ;
  skos:topConceptOf <> ;
.
<surfacecondition-R>
  rdf:type skos:Concept ;
  dct:description "effect of cultivation is obvious" ;
  ui:isMemberOf <condition-of-surface-soil-when-dry> ;
  rdfs:label "Recently cultivated" ;
  skos:definition "effect of cultivation is obvious" ;
  skos:notation "R" ;
  skos:prefLabel "Recently cultivated"@en ;
  skos:topConceptOf <> ;
.
<surfacecondition-S>
  rdf:type skos:Concept ;
  dct:description "coherent mass of individual particles or aggregates. Surface easily disturbed by pressure of forefinger" ;
  ui:isMemberOf <condition-of-surface-soil-when-dry> ;
  rdfs:label "Soft" ;
  skos:definition "coherent mass of individual particles or aggregates. Surface easily disturbed by pressure of forefinger" ;
  skos:notation "S" ;
  skos:note "Coherent means that two-thirds of the soil material, whether composed of peds or not, will remain united at the given moisture state unless force is applied" ;
  skos:prefLabel "Soft"@en ;
  skos:topConceptOf <> ;
.
<surfacecondition-T>
  rdf:type skos:Concept ;
  dct:description "soil that has been extensively trampled under dry conditions by hoofed animals" ;
  ui:isMemberOf <condition-of-surface-soil-when-dry> ;
  rdfs:label "Trampled" ;
  skos:definition "soil that has been extensively trampled under dry conditions by hoofed animals" ;
  skos:notation "T" ;
  skos:prefLabel "Trampled"@en ;
  skos:topConceptOf <> ;
.
<surfacecondition-X>
  rdf:type skos:Concept ;
  dct:description "thin, massive surface layer, usually less than 10 mm thick, which on drying separates from, and can be readily lifted off, the soil below. It usually consists mainly of dispersed clay, and may become increasingly fragile as the soil dries" ;
  ui:isMemberOf <condition-of-surface-soil-when-dry> ;
  rdfs:label "Surface flake" ;
  skos:definition "thin, massive surface layer, usually less than 10 mm thick, which on drying separates from, and can be readily lifted off, the soil below. It usually consists mainly of dispersed clay, and may become increasingly fragile as the soil dries" ;
  skos:notation "X" ;
  skos:prefLabel "Surface flake"@en ;
  skos:topConceptOf <> ;
.
<surfacecondition-Y>
  rdf:type skos:Concept ;
  dct:description "thin, more or less continuous crust of biologically stabilised soil material usually due to algae, liverworts and mosses" ;
  ui:isMemberOf <condition-of-surface-soil-when-dry> ;
  rdfs:label "Cryptogam surface" ;
  skos:definition "thin, more or less continuous crust of biologically stabilised soil material usually due to algae, liverworts and mosses" ;
  skos:notation "Y" ;
  skos:prefLabel "Cryptogam surface"@en ;
  skos:topConceptOf <> ;
.
<surfacecondition-Z>
  rdf:type skos:Concept ;
  dct:description "surface has visible salt, or salinity is evident from the absence or nature of the vegetation or from soil consistence. These conditions are characterised by their notable difference from adjacent non-saline areas" ;
  ui:isMemberOf <condition-of-surface-soil-when-dry> ;
  rdfs:label "Saline" ;
  skos:definition "surface has visible salt, or salinity is evident from the absence or nature of the vegetation or from soil consistence. These conditions are characterised by their notable difference from adjacent non-saline areas" ;
  skos:notation "Z" ;
  skos:prefLabel "Saline"@en ;
  skos:topConceptOf <> ;
.
<types-of-soil-observation>
  rdf:type skos:Collection ;
  dct:description "The soil profile may be described using several types of observation." ;
  ui:topMemberOf <> ;
  rdfs:comment "C_O_TYPE" ;
  rdfs:label "ype of soil observation" ;
  skos:definition "The soil profile may be described using several types of observation." ;
  skos:member <observation-type-A> ;
  skos:member <observation-type-C> ;
  skos:member <observation-type-E> ;
  skos:member <observation-type-P> ;
  skos:prefLabel "Observation type" ;
.
<voids>
  rdf:type skos:Collection ;
  dc:description "This is a general term for pore space and other openings in soils not occupied by solid mineral matter. The most important are cracks (planar voids) and pores, which are approximately circular in cross-section" ;
  dct:description "This is a general term for pore space and other openings in soils not occupied by solid mineral matter. The most important are cracks (planar voids) and pores, which are approximately circular in cross-section" ;
  ui:topMemberOf <> ;
  rdfs:label "Voids" ;
  skos:definition "This is a general term for pore space and other openings in soils not occupied by solid mineral matter. The most important are cracks (planar voids) and pores, which are approximately circular in cross-section" ;
  skos:member <voids-cracks> ;
  skos:member <voids-macropores> ;
  skos:member <voids-micropores> ;
  skos:prefLabel "Voids" ;
.
<voids-cracks>
  rdf:type skos:Collection ;
  dct:description "Planar voids" ;
  ui:isMemberOf <voids> ;
  rdfs:label "Cracks" ;
  skos:definition "Planar voids" ;
  skos:member <voids-cracks-1> ;
  skos:member <voids-cracks-2> ;
  skos:member <voids-cracks-3> ;
  skos:member <voids-cracks-4> ;
  skos:member <voids-cracks-5> ;
  skos:prefLabel "Cracks" ;
.
<voids-cracks-1>
  rdf:type skos:Concept ;
  dc:description "<5 mm" ;
  dct:description "<5 mm" ;
  ui:isMemberOf <voids-cracks> ;
  rdfs:label "Fine" ;
  skos:definition "<5 mm" ;
  skos:notation "1" ;
  skos:prefLabel "Fine" ;
  skos:topConceptOf <> ;
.
<voids-cracks-2>
  rdf:type skos:Concept ;
  dc:description "5 - 10 mm" ;
  dct:description "5 - 10 mm" ;
  ui:isMemberOf <voids-cracks> ;
  rdfs:label "Medium" ;
  skos:definition "5 - 10 mm" ;
  skos:notation "2" ;
  skos:prefLabel "Medium" ;
  skos:topConceptOf <> ;
.
<voids-cracks-3>
  rdf:type skos:Concept ;
  dc:description "10–20 mm" ;
  dct:description "10–20 mm" ;
  ui:isMemberOf <voids-cracks> ;
  rdfs:label "Coarse" ;
  skos:definition "10–20 mm" ;
  skos:notation "3" ;
  skos:prefLabel "Coarse" ;
  skos:topConceptOf <> ;
.
<voids-cracks-4>
  rdf:type skos:Concept ;
  dc:description "20–50 mm" ;
  dct:description "20–50 mm" ;
  ui:isMemberOf <voids-cracks> ;
  rdfs:label "Very coarse" ;
  skos:definition "20–50 mm" ;
  skos:notation "4" ;
  skos:prefLabel "Very coarse" ;
  skos:topConceptOf <> ;
.
<voids-cracks-5>
  rdf:type skos:Concept ;
  dc:description "20–50 mm" ;
  dct:description "20–50 mm" ;
  ui:isMemberOf <voids-cracks> ;
  rdfs:label "Extremely coarse" ;
  skos:definition "20–50 mm" ;
  skos:notation "5" ;
  skos:prefLabel "Extremely coarse" ;
  skos:topConceptOf <> ;
.
<voids-macropores>
  rdf:type skos:Collection ;
  dct:description "voids that are approximately circular in cross-section and greater than 0.075 mm diameter" ;
  ui:isMemberOf <voids> ;
  rdfs:label "Macropores" ;
  skos:definition "voids that are approximately circular in cross-section and greater than 0.075 mm diameter" ;
  skos:member <voids-macropores-abundance> ;
  skos:member <voids-macropores-diameter> ;
  skos:note "Only macropores can be seen with the naked eye" ;
  skos:prefLabel "Macropores" ;
.
<voids-macropores-abundance>
  rdf:type skos:Collection ;
  dct:description "abundance of macropores based relevant to the diameter of the macropores" ;
  ui:isMemberOf <voids-macropores> ;
  rdfs:comment "N_PORE_ABUN" ;
  rdfs:label "Abundance of macropores" ;
  skos:definition "abundance of macropores based relevant to the diameter of the macropores" ;
  skos:member <voids-macropores-abundance-0> ;
  skos:member <voids-macropores-abundance-1> ;
  skos:member <voids-macropores-abundance-2> ;
  skos:member <voids-macropores-abundance-3> ;
  skos:member <voids-macropores-abundance-4> ;
  skos:member <voids-macropores-abundance-5> ;
  skos:member <voids-macropores-abundance-6> ;
  skos:prefLabel "Abundance of macropores" ;
.
<voids-macropores-abundance-0>
  rdf:type skos:Concept ;
  dc:description "No fine, very fine, medium or coarse macropores" ;
  dct:description "No fine, very fine, medium or coarse macropores" ;
  ui:isMemberOf <voids-macropores-abundance> ;
  rdfs:label "No fine, very fine, medium or coarse macropores" ;
  skos:definition "No fine, very fine, medium or coarse macropores" ;
  skos:notation "0" ;
  skos:prefLabel "No fine, very fine, medium or coarse macropores" ;
  skos:topConceptOf <> ;
.
<voids-macropores-abundance-1>
  rdf:type skos:Concept ;
  dc:description "<1 per 100 mm2 of diameter less than 2mm" ;
  dct:description "<1 per 100 mm2 of diameter less than 2mm" ;
  ui:isMemberOf <voids-macropores-abundance> ;
  rdfs:label "Few fine or very fine macropores" ;
  skos:definition "<1 per 100 mm2 of diameter less than 2mm" ;
  skos:notation "1" ;
  skos:prefLabel "Few fine or very fine macropores" ;
  skos:topConceptOf <> ;
.
<voids-macropores-abundance-2>
  rdf:type skos:Concept ;
  dc:description "1–5 per 100 mm2 of diameter less than 2mm" ;
  dct:description "1–5 per 100 mm2 of diameter less than 2mm" ;
  ui:isMemberOf <voids-macropores-abundance> ;
  rdfs:label "Common fine or very fine macropores" ;
  skos:definition "1–5 per 100 mm2 of diameter less than 2mm" ;
  skos:notation "2" ;
  skos:prefLabel "Common fine or very fine macropores" ;
  skos:topConceptOf <> ;
.
<voids-macropores-abundance-3>
  rdf:type skos:Concept ;
  dc:description ">5 per 100 mm2 of diameter less than 2mm" ;
  dct:description ">5 per 100 mm2 of diameter less than 2mm" ;
  ui:isMemberOf <voids-macropores-abundance> ;
  rdfs:label "Many fine or very fine macropores" ;
  skos:definition ">5 per 100 mm2 of diameter less than 2mm" ;
  skos:notation "3" ;
  skos:prefLabel "Many fine or very fine macropores" ;
  skos:topConceptOf <> ;
.
<voids-macropores-abundance-4>
  rdf:type skos:Concept ;
  dc:description "<1 per 0.01 m2 of diameter greater than 2mm" ;
  dct:description "<1 per 0.01 m2 of diameter greater than 2mm" ;
  ui:isMemberOf <voids-macropores-abundance> ;
  rdfs:label "Few medium or coarse macropores" ;
  skos:definition "<1 per 0.01 m2 of diameter greater than 2mm" ;
  skos:notation "4" ;
  skos:prefLabel "Few medium or coarse macropores" ;
  skos:topConceptOf <> ;
.
<voids-macropores-abundance-5>
  rdf:type skos:Concept ;
  dc:description "1–5 per 0.01 m2 of diameter greater than 2mm" ;
  dct:description "1–5 per 0.01 m2 of diameter greater than 2mm" ;
  ui:isMemberOf <voids-macropores-abundance> ;
  rdfs:label "Common medium or coarse macropores" ;
  skos:definition "1–5 per 0.01 m2 of diameter greater than 2mm" ;
  skos:notation "5" ;
  skos:prefLabel "Common medium or coarse macropores" ;
  skos:topConceptOf <> ;
.
<voids-macropores-abundance-6>
  rdf:type skos:Concept ;
  dc:description ">5 per 0.01 m2 of diameter greater than 2mm" ;
  dct:description ">5 per 0.01 m2 of diameter greater than 2mm" ;
  ui:isMemberOf <voids-macropores-abundance> ;
  rdfs:label "Many medium or coarse macropores" ;
  skos:definition ">5 per 0.01 m2 of diameter greater than 2mm" ;
  skos:notation "6" ;
  skos:prefLabel "Many medium or coarse macropores" ;
  skos:topConceptOf <> ;
.
<voids-macropores-diameter>
  rdf:type skos:Collection ;
  dct:description "Diameter of macropores Use Figure 18 as a guide to average diameter" ;
  ui:isMemberOf <voids-macropores> ;
  rdfs:comment "N_PORE_DIAMETER" ;
  rdfs:label "Diameter of macropores" ;
  skos:definition "Diameter of macropores Use Figure 18 as a guide to average diameter" ;
  skos:member <voids-macropores-diameter-1> ;
  skos:member <voids-macropores-diameter-2> ;
  skos:member <voids-macropores-diameter-3> ;
  skos:member <voids-macropores-diameter-4> ;
  skos:prefLabel "Diameter of macropores" ;
.
<voids-macropores-diameter-1>
  rdf:type skos:Concept ;
  dc:description "0.075–1 mm" ;
  dct:description "0.075–1 mm" ;
  ui:isMemberOf <voids-macropores-diameter> ;
  rdfs:label "Very fine" ;
  skos:definition "0.075–1 m" ;
  skos:notation "1" ;
  skos:note "Use Figure 18 as a guide to average diameter" ;
  skos:prefLabel "Very fine" ;
  skos:topConceptOf <> ;
.
<voids-macropores-diameter-2>
  rdf:type skos:Concept ;
  dc:description "1–2 mm" ;
  dct:description "1–2 mm" ;
  ui:isMemberOf <voids-macropores-diameter> ;
  rdfs:label "Fine" ;
  skos:definition "1–2 mm" ;
  skos:notation "2" ;
  skos:note "Use Figure 18 as a guide to average diameter" ;
  skos:prefLabel "Fine" ;
  skos:topConceptOf <> ;
.
<voids-macropores-diameter-3>
  rdf:type skos:Concept ;
  dc:description "2–5 mm" ;
  dct:description "2–5 mm" ;
  ui:isMemberOf <voids-macropores-diameter> ;
  rdfs:label "Medium" ;
  skos:definition "2–5 mm" ;
  skos:notation "3" ;
  skos:note "Use Figure 18 as a guide to average diameter" ;
  skos:prefLabel "Medium" ;
  skos:topConceptOf <> ;
.
<voids-macropores-diameter-4>
  rdf:type skos:Concept ;
  dc:description ">5 mm" ;
  dct:description ">5 mm" ;
  ui:isMemberOf <voids-macropores-diameter> ;
  rdfs:label "Coarse" ;
  skos:definition ">5 mm" ;
  skos:notation "4" ;
  skos:note "Use Figure 18 as a guide to average diameter" ;
  skos:prefLabel "Coarse" ;
  skos:topConceptOf <> ;
.
<voids-micropores>
  rdf:type skos:Concept ;
  dct:description "voids that are approximately circular in cross-section and less than 0.075 mm diameter" ;
  ui:isMemberOf <voids> ;
  rdfs:label "Micropores" ;
  skos:definition "voids that are approximately circular in cross-section and less than 0.075 mm diameter" ;
  skos:note "Only macropores can be seen with the naked eye" ;
  skos:prefLabel "Micropores" ;
  skos:topConceptOf <> ;
.
<water-repellence>
  rdf:type skos:Collection ;
  dct:description "Water repellence of some soils, usually sandy, is caused by a series of long-chain polymethylene waxes, made up of acids, alcohols and esters, attached to the sand grains (Ma’shum et al. 1988). These soils occur Australia-wide but are more widespread in southern Australia (Wetherby 1984, McGhie and Posner 1980). Degree of repellence is assessed by determining the concentration of ethanol required to wet the sand in 10 seconds (King 1981). An abbreviated form of this method is recommended for routine field situations" ;
  ui:topMemberOf <> ;
  rdfs:label "Water repellence" ;
  skos:definition "Water repellence of some soils, usually sandy, is caused by a series of long-chain polymethylene waxes, made up of acids, alcohols and esters, attached to the sand grains (Ma’shum et al. 1988). These soils occur Australia-wide but are more widespread in southern Australia (Wetherby 1984, McGhie and Posner 1980). Degree of repellence is assessed by determining the concentration of ethanol required to wet the sand in 10 seconds (King 1981). An abbreviated form of this method is recommended for routine field situations" ;
  skos:member <waterrepellence-N> ;
  skos:member <waterrepellence-R> ;
  skos:member <waterrepellence-S> ;
  skos:note "Soil temperature at testing should be between 15ºC and 25ºC. Higher temperatures will increase, and lower decrease, rates of absorption. Industrial-grade methylated spirits, available from chemists, at a concentration of 23.9 ml per 200 ml water can be substituted for the 2-molar ethanol to obtain approximate values" ;
  skos:prefLabel "Water repellence" ;
.
<waterrepellence-N>
  rdf:type skos:Concept ;
  dct:description "water is absorbed into soil in 10 seconds or less" ;
  ui:isMemberOf <water-repellence> ;
  rdfs:label "Non water repellent" ;
  skos:definition "water is absorbed into soil in 10 seconds or less" ;
  skos:notation "N" ;
  skos:prefLabel "Non water repellent"@en ;
  skos:topConceptOf <> ;
.
<waterrepellence-R>
  rdf:type skos:Concept ;
  dct:description "water takes greater than 10 seconds and 2-molar ethanol takes 10 seconds or less to be absorbed into soil" ;
  ui:isMemberOf <water-repellence> ;
  rdfs:label "Water repellent" ;
  skos:definition "water takes greater than 10 seconds and 2-molar ethanol takes 10 seconds or less to be absorbed into soil" ;
  skos:notation "R" ;
  skos:prefLabel "Water repellent"@en ;
  skos:topConceptOf <> ;
.
<waterrepellence-S>
  rdf:type skos:Concept ;
  dct:description "2-molar ethanol takes greater than 10 seconds to be absorbed into soil" ;
  ui:isMemberOf <water-repellence> ;
  rdfs:label "Strongly water repellent" ;
  skos:definition "2-molar ethanol takes greater than 10 seconds to be absorbed into soil" ;
  skos:notation "S" ;
  skos:prefLabel "Strongly water repellent"@en ;
  skos:topConceptOf <> ;
.
