# baseURI: http://registry.it.csiro.au/def/soils/technical-reference/
# imports: http://purl.org/dc/elements/1.1/
# imports: http://www.w3.org/2004/02/skos/core

@prefix dc: <http://purl.org/dc/elements/1.1/> .
@prefix dct: <http://purl.org/dc/terms/> .
@prefix owl: <http://www.w3.org/2002/07/owl#> .
@prefix rdf: <http://www.w3.org/1999/02/22-rdf-syntax-ns#> .
@prefix rdf123: <http://rdf123.umbc.edu/ns/> .
@prefix rdfs: <http://www.w3.org/2000/01/rdf-schema#> .
@prefix skos: <http://www.w3.org/2004/02/skos/core#> .
@prefix tech_ref: <http://registry.it.csiro.au/def/soils/technical-reference/> .
@prefix xsd: <http://www.w3.org/2001/XMLSchema#> .

tech_ref:
  rdf:type owl:Ontology ;
  dc:source "natsoil CSIRO database - Technical Reference table"^^xsd:string ;
  dct:created "2015-12-04"^^xsd:date ;
  dct:creator <mailto:xavier.butcher@csiro.au> ;
  rdfs:comment "This table shows the 3 editions of the Soil and Terrain handbook."^^xsd:string ;
  rdfs:label "Technical Reference"^^xsd:string ;
  rdfs:seeAlso "National Committee on Soil and Terrain (2009), 'Australian soil and land survey field handbook (3rd edn).' (CSIRO Publishing: Melbourne)"^^xsd:string ;
  owl:imports dc: ;
  owl:imports <http://www.w3.org/2004/02/skos/core> ;
.
tech_ref:first-edition
  rdf:type skos:Concept ;
  dct:description "Australian Soil and Land Survey, Field Handbook First Edition" ;
  rdfs:label "'First Edition'@en" ;
  skos:definition "Australian Soil and Land Survey, Field Handbook First Edition" ;
  skos:notation "1" ;
  skos:prefLabel "'First Edition'@en" ;
.
tech_ref:second-edition
  rdf:type skos:Concept ;
  dct:description "Australian Soil and Land Survey, Field Handbook Second Edition" ;
  rdfs:label "'Second Edition'@en" ;
  skos:definition "Australian Soil and Land Survey, Field Handbook Second Edition" ;
  skos:notation "2" ;
  skos:prefLabel "'Second Edition'@en" ;
.
tech_ref:third-edition
  rdf:type skos:Concept ;
  dct:description "Australian Soil and Land Survey, Field Handbook Third Edition" ;
  rdfs:label "'Third Edition'@en" ;
  skos:definition "Australian Soil and Land Survey, Field Handbook Third Edition" ;
  skos:notation "3" ;
  skos:prefLabel "'Third Edition'@en" ;
.
