@prefix dc: <http://purl.org/dc/elements/1.1/> .
@prefix dct: <http://purl.org/dc/terms/> .
@prefix owl: <http://www.w3.org/2002/07/owl#> .
@prefix rdf: <http://www.w3.org/1999/02/22-rdf-syntax-ns#> .
@prefix rdfs: <http://www.w3.org/2000/01/rdf-schema#> .
@prefix skos: <http://www.w3.org/2004/02/skos/core#> .
@prefix tech_ref: <http://registry.it.csiro.au/def/soils/technical-reference/> .
@prefix xsd: <http://www.w3.org/2001/XMLSchema#> .

<first-edition>
  rdf:type skos:Concept ;
  dct:description "Australian Soil and Land Survey, Field Handbook First Edition" ;
  rdfs:label 'First Edition'@en ;
  skos:definition "Australian Soil and Land Survey, Field Handbook First Edition" ;
  skos:notation "1" ;
  skos:prefLabel 'First Edition'@en ;
.
<second-edition>
  rdf:type skos:Concept ;
  dct:description "Australian Soil and Land Survey, Field Handbook Second Edition" ;
  rdfs:label 'Second Edition'@en ;
  skos:definition "Australian Soil and Land Survey, Field Handbook Second Edition" ;
  skos:notation "2" ;
  skos:prefLabel 'Second Edition'@en ;
.
<third-edition>
  rdf:type skos:Concept ;
  dct:description "Australian Soil and Land Survey, Field Handbook Third Edition" ;
  rdfs:label 'Third Edition'@en ;
  skos:definition "Australian Soil and Land Survey, Field Handbook Third Edition" ;
  skos:notation "3" ;
  skos:prefLabel 'Third Edition'@en ;
.
