# baseURI: http://registry.it.csiro.au/sandbox/soil/observation-method/
# imports: http://purl.org/dc/elements/1.1/
# imports: http://www.w3.org/2004/02/skos/core
# prefix: observation-method

@prefix dc: <http://purl.org/dc/elements/1.1/> .
@prefix dct: <http://purl.org/dc/terms/> .
@prefix observation-method: <http://registry.it.csiro.au/sandbox/soil/observation-method/> .
@prefix owl: <http://www.w3.org/2002/07/owl#> .
@prefix rdf: <http://www.w3.org/1999/02/22-rdf-syntax-ns#> .
@prefix rdf123: <http://rdf123.umbc.edu/ns/> .
@prefix rdfs: <http://www.w3.org/2000/01/rdf-schema#> .
@prefix skos: <http://www.w3.org/2004/02/skos/core#> .
@prefix xsd: <http://www.w3.org/2001/XMLSchema#> .

dc:
  dct:description "This version has been modified for use in TopBraid: it defines the dc namespace prefix and imports SKOS and DCTerms."^^xsd:string ;
  rdfs:label "Dublin Core Metadata Element Set, Version 1.1" ;
.
observation-method:
  rdf:type owl:Ontology ;
  dc:source "National Committee on Soil and Terrain (2009), 'Australian soil and land survey field handbook (3rd edn).' (CSIRO Publishing: Melbourne)"^^xsd:string ;
  dct:created "2016-07-05"^^xsd:date ;
  dct:creator <mailto:asris@csiro.au> ;
  dct:description "Observing the soil body at a particular location is done using a variety of methods, depending on access and the scale of the information required."^^xsd:string ;
  dct:license <http://creativecommons.org/licences/by/4.0> ;
  dct:rights "copyright CSIRO 2009, 2016. All rights reserved." ;
  rdfs:label "Observation Method"^^xsd:string ;
  owl:imports dc: ;
  owl:imports <http://www.w3.org/2004/02/skos/core> ;
.
observation-method:auger-boring
  rdf:type skos:Concept ;
  dct:description "--"^^xsd:string ;
  rdfs:label "Auger boring"^^xsd:string ;
  skos:definition "--"^^xsd:string ;
  skos:notation "A"^^xsd:string ;
  skos:prefLabel "Auger boring"@en ;
.
observation-method:existing-vertical-exposure
  rdf:type skos:Concept ;
  dct:description "--."^^xsd:string ;
  rdfs:label "Existing vertical exposure"^^xsd:string ;
  skos:definition "--"^^xsd:string ;
  skos:notation "E"^^xsd:string ;
  skos:prefLabel "Existing vertical exposure"@en ;
.
observation-method:soil-pit
  rdf:type skos:Concept ;
  dct:description "--."^^xsd:string ;
  rdfs:label "Soil pit"^^xsd:string ;
  skos:definition "--."^^xsd:string ;
  skos:notation "P"^^xsd:string ;
  skos:prefLabel "Soil pit"@en ;
.
observation-method:undisturbed-soil-core
  rdf:type skos:Concept ;
  dct:description "--"^^xsd:string ;
  rdfs:label "Undisturbed soil core"^^xsd:string ;
  skos:definition "--"^^xsd:string ;
  skos:notation "C"^^xsd:string ;
  skos:prefLabel "Undisturbed soil core"@en ;
.
<http://www.w3.org/2002/07/owl>
  dct:description """
  This ontology partially describes the built-in classes and
  properties that together form the basis of the RDF/XML syntax of OWL 2.
  The content of this ontology is based on Tables 6.1 and 6.2
  in Section 6.4 of the OWL 2 RDF-Based Semantics specification,
  available at http://www.w3.org/TR/owl2-rdf-based-semantics/.
  Please note that those tables do not include the different annotations
  (labels, comments and rdfs:isDefinedBy links) used in this file.  
  Also note that the descriptions provided in this ontology do not
  provide a complete and correct formal description of either the syntax
  or the semantics of the introduced terms (please see the OWL 2
  recommendations for the complete and normative specifications).
  Furthermore, the information provided by this ontology may be
  misleading if not used with care. This ontology SHOULD NOT be imported
  into OWL ontologies. Importing this file into an OWL 2 DL ontology
  will cause it to become an OWL 2 Full ontology and may have other,
  unexpected, consequences.
   """ ;
  rdfs:label "owl" ;
.
