# baseURI: http://www.anzsoil.org/def/asc
# imports: http://www.anzsoil.org/schema/soil-classification

@prefix afn: <http://jena.hpl.hp.com/ARQ/function#> .
@prefix asc: <http://www.anzsoil.org/def/asc/> .
@prefix backspin: <http://topbraid.org/backspin#> .
@prefix corpus: <http://topbraid.org/corpus#> .
@prefix crosswalk: <http://topbraid.org/crosswalk#> .
@prefix crosswalkprojects: <http://teamwork.topbraidlive.org/crosswalkprojects#> .
@prefix dc: <http://purl.org/dc/elements/1.1/> .
@prefix dcam: <http://purl.org/dc/dcam/> .
@prefix dcat: <http://www.w3.org/ns/dcat#> .
@prefix dct: <http://purl.org/dc/terms/> .
@prefix dcterms: <http://purl.org/dc/terms/> .
@prefix edg: <http://edg.topbraid.solutions/model/> .
@prefix evnconstraints: <http://topbraid.org/spin/evnconstraints#> .
@prefix evnui: <http://evn.topbraidlive.org/ui#> .
@prefix fn: <http://www.w3.org/2005/xpath-functions#> .
@prefix html: <http://uispin.org/html#> .
@prefix jfn: <java:org.apache.jena.sparql.function.library.> .
@prefix lfunctions: <http://example.org/lfunctions#> .
@prefix lib-importer: <http://edg.topbraid.solutions/importer/lib#> .
@prefix metadata: <http://topbraid.org/metadata#> .
@prefix ontologyprojects: <http://teamwork.topbraidlive.org/ontologyprojects#> .
@prefix owl: <http://www.w3.org/2002/07/owl#> .
@prefix owlrl: <http://topbraid.org/spin/owlrl#> .
@prefix pf: <http://jena.hpl.hp.com/ARQ/property#> .
@prefix raci: <http://topbraid.org/raci#> .
@prefix rdf: <http://www.w3.org/1999/02/22-rdf-syntax-ns#> .
@prefix rdfs: <http://www.w3.org/2000/01/rdf-schema#> .
@prefix search: <http://topbraid.org/search#> .
@prefix shaclify: <http://topbraid.org/shacl/shaclify#> .
@prefix sharepoint: <http://topbraid.org/sharepoint#> .
@prefix skos: <http://www.w3.org/2004/02/skos/core#> .
@prefix skosspin: <http://topbraid.org/spin/skosspin#> .
@prefix skostemplate: <http://topbraid.org/spin/skostemplates#> .
@prefix sm: <http://topbraid.org/sparqlmotion#> .
@prefix sm2wsdl: <http://topbraid.org/sparqlmotion/sm2wsdl.sms#> .
@prefix smf: <http://topbraid.org/sparqlmotionfunctions#> .
@prefix sml: <http://topbraid.org/sparqlmotionlib#> .
@prefix softwareprojects: <http://teamwork.topbraidlive.org/software/softwareprojects#> .
@prefix soil: <http://www.anzsoil.org/schema/soil-classification#> .
@prefix sp: <http://spinrdf.org/sp#> .
@prefix spif: <http://spinrdf.org/spif#> .
@prefix spin: <http://spinrdf.org/spin#> .
@prefix spinmap: <http://spinrdf.org/spinmap#> .
@prefix spinmapl: <http://topbraid.org/spin/spinmapl#> .
@prefix spl: <http://spinrdf.org/spl#> .
@prefix spr: <http://spinrdf.org/spr#> .
@prefix spra: <http://spinrdf.org/spra#> .
@prefix swa: <http://topbraid.org/swa#> .
@prefix swaclasses: <http://topbraid.org/swaclasses#> .
@prefix swaeditor: <http://topbraid.org/swaeditor#> .
@prefix swauml: <http://topbraid.org/swauml#> .
@prefix swon: <http://uispin.org/swon#> .
@prefix tables: <http://topbraid.org/tables#> .
@prefix tablesmap: <http://topbraid.org/spin/tablesmap#> .
@prefix tagger: <http://evn.topbraidlive.org/tagger#> .
@prefix tasks: <http://topbraid.org/tasks#> .
@prefix taxonomies: <http://evn.topbraidlive.org/evnprojects#> .
@prefix tbladmin: <http://server.topbraidlive.org/system-applications/tbladmin#> .
@prefix teamwork: <http://topbraid.org/teamwork#> .
@prefix teamworkconstraints: <http://topbraid.org/teamworkconstraints#> .
@prefix tops: <http://www.topbraid.org/tops#> .
@prefix tosh.ui: <http://topbraid.org/tosh.ui#> .
@prefix tracker: <http://teamwork.topbraidlive.org/ui/tracker#> .
@prefix ui: <http://uispin.org/ui#> .
@prefix uix: <http://topbraidlive.org/uix#> .
@prefix xsd: <http://www.w3.org/2001/XMLSchema#> .

<http://www.anzsoil.org/def/asc>
  rdf:type owl:Ontology ;
  rdf:type dcat:Dataset ;
  dcterms:creator <https://www.directory.gov.au/portfolios/agriculture-and-water-resources/department-agriculture-and-water-resources/national-committee-soil-and-terrain> ;
  dcterms:license <https://creativecommons.org/licenses/by/4.0/> ;
  dcterms:publisher <http://www.publish.csiro.au/> ;
  dcterms:source <http://www.publish.csiro.au/book/7428> ;
  rdfs:comment "This extract has been made available by the copyright holder for use in the context of the ENVO ontology, on condition that the information is attributed to CSIRO Publishing and the National Committee on Soil and Terrain. " ;
  rdfs:comment "This is an extract from the Australian Soil Classification, comprising only the top-level soil orders." ;
  rdfs:label "Soil orders from the Australian Soil Classification" ;
  owl:imports <http://www.anzsoil.org/schema/soil-classification> ;
  dcat:contactPoint <https://people.csiro.au/Simon-Cox> ;
.
asc:AN
  rdf:type soil:Order ;
  rdf:type skos:Concept ;
  rdfs:comment """These soils result from human activities which have caused a profound modification, mixing, truncation or burial of the original soil horizons, or the creation of new soil parent materials. Note that the concept of soil used in this classification of Australian soils (see Background) also applies to the Anthroposols, and hence sealed and semi-sealed surfaces such as streets, roads etc. are regarded as 'non-soil'. Also, in depositional situations, the anthropic material must be 0.3 m or more thick where it overlies buried soils. Anthropic materials < 0.3 m thick will identify an anthropic phase of the soil below.

To qualify as soil an Anthroposol needs to possess some pedogenic features, as noted below. Key criteria in the identification of an Anthroposol are the presence of artefacts in the profile or knowledge that the soils or their parent materials have been made or altered by human action.

Anthroposols differ from other soils in that we normally know their origin with a degree of certainty, and hence we can invoke a knowledge of process rather than defined pedogenic attributes to initially classify the soil. We can then subdivide at the higher levels on the basis of type of process and nature of the product which forms the parent material of the new soil. At lower levels in the classification, conventional soil properties could be used when available, although obviously these will be limited in very young soils.

It is difficult to quantify ‘profound modification, mixing and truncation’ but this would normally exclude the usual agricultural operations (including land planning) which may change a soil from say a Chromosol to a Dermosol by mixing or removal of the upper horizons. Similarly, soils that are artificially drained or flooded are not Anthroposols but may classify as different soil orders following a permanent change in water status (see also Comment in Hydrosols).

There will also be instances where the question is how much truncation results in ‘profound modification’ or merely a truncated phase. It is difficult to give guidelines that will cover all circumstances, and inevitably judgement is required. Similarly, there will be instances where land reclamation and restoration in the past have been so successful that little evidence of a prior disturbance remains, and soil development gives no clue to past history. A good example of this is Podosol development on restored and revegetated coastal dunes following sand mining.""" ;
  owl:versionInfo "Version 1 (1996)" ;
  skos:definition "Soils resulting from human activities which have led to a profound modification, truncation or burial of the original soil horizons, or the creation of new soil parent materials by a variety of mechanical means. Where burial of a pre-existing soil is involved, the anthropic materials must be 0.3 m or more thick. Pedogenic features may be the result of in situ processes (usually the minimal development of an A1 horizon, sometimes the stronger development of typical soil horizons) or the result of pedogenic processes prior to modification or placement (ie. the presence of identifiable pre-existing soil material)." ;
  skos:inScheme asc: ;
  skos:notation "AN" ;
  skos:note "Soils resulting from human activity" ;
  skos:prefLabel "Anthroposols" ;
.
asc:CA
  rdf:type soil:Order ;
  rdf:type skos:Concept ;
  dcterms:description """As the name suggests, the soils in this order are usually calcareous throughout the profile, often highly so. They constitute one of the most widespread and important groups of soils in southern Australia.
Soils that are calcareous throughout the solum - or calcareous at least directly below the A1 or Ap horizon, or a depth of 0.2 m (whichever is shallower). Carbonate accumulations must be judged to be pedogenic1 (either current or relict), and the soils do not have clear or abrupt textural B horizons. Hydrosols, Organosols and Vertosols are excluded.""" ;
  rdfs:comment """As the name suggests, the soils in this order are usually calcareous throughout the profile, often highly so. They constitute one of the most widespread and important groups of soils in southern Australia.

A difficulty may arise in separating those Calcarosols that are not calcareous throughout from calcareous Kandosols and from Tenosols containing pedogenic carbonate. However, in the latter two soils it is usual for the carbonate to occur in the lower part of the B horizon, and not immediately below the A horizon. Even so, transitional cases will arise where it becomes a matter of judgement in to which order the particular soil is best placed. Similar transitions might occur between shallow Calcarosols and Arenic Rudosols overlying a layer of calcrete or limestone. Again, Calcareous Arenic Rudosols will occur where recent aeolian calcareous material has been deposited.

In dune landscapes, where these soils frequently occur, it is common to find evidence of post-European settlement deflation and layering of soil profiles caused by wind erosion and consequent deposition. Unless the surface depositional material is 0.3 m or more thick, it is ignored in the classification and treated as a phase.""" ;
  owl:versionInfo "Version 1 (1996)" ;
  skos:definition "Soils that are calcareous throughout the solum - or calcareous at least directly below the A1 or Ap horizon, or a depth of 0.2 m (whichever is shallower). Carbonate accumulations must be judged to be pedogenic1 (either current or relict), and the soils do not have clear or abrupt textural B horizons. Hydrosols, Organosols and Vertosols are excluded." ;
  skos:inScheme asc: ;
  skos:notation "CA" ;
  skos:note "Soils with calcium carbonate" ;
  skos:prefLabel "Calcarosols" ;
.
asc:CH
  rdf:type soil:Order ;
  rdf:type skos:Concept ;
  rdfs:comment """Soils with strong texture contrast between A horizons and B horizons. The latter are not strongly acid and are not sodic. The soils of this order are among the most widespread soils used for agriculture in Australia, particularly those with red subsoils.

In the case of those soils with strongly subplastic B horizons, care needs to be taken to ensure if they qualify for the clear or abrupt textural B horizon. As far as is presently known, such soils appear to be largely confined to the Riverine Plain of south eastern Australia.""" ;
  owl:versionInfo "Version 1 (1996)" ;
  skos:definition "Soils other than Hydrosols with a clear or abrupt textural B horizon and in which the major part of the upper 0.2 m of the B2 horizon (or the major part of the entire B2 horizon if it is less than 0.2 m thick) is not sodic and not strongly acid. Soils with strongly subplastic upper B2 horizons are also included even if they are sodic." ;
  skos:inScheme asc: ;
  skos:notation "CH" ;
  skos:note "Soils with an abrupt increase in clay" ;
  skos:prefLabel "Chromosols" ;
.
asc:DE
  rdf:type soil:Order ;
  rdf:type skos:Concept ;
  dcterms:description """Structured soils

Soils with structured B2 horizons and lacking strong texture contrast between A and B horizons. Although there is some diversity within the order, it brings together a range of soils with some important properties in common.

Soils other than Vertosols, Hydrosols, Calcarosols and Ferrosols which:
(i) Have B2 horizons with structure more developed than weak1 throughout the major part of the horizon, and
(ii) Do not have clear or abrupt textural B horizons.""" ;
  rdfs:comment """Soils with structured B2 horizons and lacking strong texture contrast between A and B horizons. Although there is some diversity within the order, it brings together a range of soils with some important properties in common.

Some clayey soils in the arid zone which are relatively high in salt tend to have strong, fine blocky structure. It may be difficult to decide if they are Vertosols or Dermosols because of an apparent lack of cracking and slickensides or lenticular structure. The use of shrinkage measurements such as those discussed under vertic properties will help to resolve this situation.""" ;
  owl:versionInfo "Version 1 (1996)" ;
  skos:definition """Soils other than Vertosols, Hydrosols, Calcarosols and Ferrosols which:
(i) Have B2 horizons with structure more developed than weak1 throughout the major part of the horizon, and
(ii) Do not have clear or abrupt textural B horizons.""" ;
  skos:inScheme asc: ;
  skos:notation "DE" ;
  skos:note "Structured soils" ;
  skos:prefLabel "Dermosols" ;
.
asc:FE
  rdf:type soil:Order ;
  rdf:type skos:Concept ;
  dcterms:description """Iron rich soils

Soils with B2 horizons which are high in free iron oxide, and which lack strong texture contrast between A and B horizons.

Soils other than Vertosols, Hydrosols, and Calcarosols that:
(i) Have B2 horizons in which the major part has a free iron oxide free iron oxide1 content greater than 5% Fe in the fine earth fraction (<2 mm), and
(ii) Do not have clear or abrupt textural B horizons or a B2 horizon in which at least 0.3m has vertic properties.""" ;
  rdfs:comment """Soils with B2 horizons which are high in free iron oxide, and which lack strong texture contrast between A and B horizons.

These soils are almost entirely formed on either basic or ultrabasic igneous rocks, their metamorphic equivalents, or alluvium derived therefrom. Although these soils do not occupy large areas in Australia, they are widely recognised and often intensively used because of their favourable physical properties. The most common forms have B2 horizons with strong polyhedral compound peds up to 10-15 mm, usually with smooth and often shiny faces. These break down readily to primary peds about 5 mm or less in size. However forms also occur with a very fine granular structure which may appear massive in place.""" ;
  owl:versionInfo "Version 1 (1996)" ;
  skos:definition """Soils other than Vertosols, Hydrosols, and Calcarosols that:
(i) Have B2 horizons in which the major part has a free iron oxide free iron oxide1 content greater than 5% Fe in the fine earth fraction (<2 mm), and
(ii) Do not have clear or abrupt textural B horizons or a B2 horizon in which at least 0.3m has vertic properties.""" ;
  skos:inScheme asc: ;
  skos:notation "FE" ;
  skos:note "Iron rich soils" ;
  skos:prefLabel "Ferrosols" ;
.
asc:HY
  rdf:type soil:Order ;
  rdf:type skos:Concept ;
  rdfs:comment """This order is designed to accommodate a range of seasonally or permanently wet soils and thus there is some diversity within the order. The key criterion is saturation of the greater part of the profile for prolonged periods (2-3 months) in most years. The soils may or may not experience reducing conditions for all or part of the period of saturation, and thus manifestations of reduction and oxidation such as 'gley' colours and ochrous mottles may or may not be present.

Saturation by a water table may not necessarily be caused by low soil permeability. Often site drainage will be the most important factor, while in other well-known cases tidal influence is dominant. The relevant Field Handbook drainage classes are very poorly and poorly drained.

Several major classes of soils are excluded because it is considered their other profile characteristics are of greater significance than wetness. These are the Organosols, Podosols and Vertosols. Although some Hydrosols are dominated by organic materials (see Intertidal Hydrosols below), it is thought that because of their unique nature (ie. largely consisting of mangrove debris that is regularly inundated by saline tidal waters), it is more appropriate to classify them as organic Hydrosols rather than as a class of Organosols that occur in a mangrove environment.

The approach taken in this concept of 'wet' soils differs from more traditional usage in that reducing conditions are not emphasised. The rationale for the present approach is based on the assumption that saturation affects soil properties irrespective of whether or not reducing conditions are present. Obvious examples are those relating to certain physical and engineering properties, which result in limitations to the use of a soil eg. trafficability, etc.

A further reason for not making reducing conditions mandatory is the well-known difficulty in identifying such conditions, which are often of a temporal nature and sporadic in spatial distribution. It is widely recognised that the traditional use of 'gley' colours and particular kinds of mottling are not universally indicative of a saturated condition or its duration. In particular, mottles or other segregations can be relict. Another problem in identification of reducing conditions, is the experience that various indicator dyes such as a,a-dipyridyl (Childs & Clayden 1986) may be unreliable.

It will also be apparent that the concept adopted for Hydrosols will normally exclude the pseudo (or surface water) gley class commonly distinguished in several European classification schemes. These soils have a perched water table usually caused by a slowly permeable horizon or layer within the soil profile.

A difficult question arises as to how artificially drained soils are best treated. In many cases drainage will merely lower the water table to depths which permit the successful growth of particular plants. Such depths may still be relatively shallow eg. 0.5 - 1 m, and capillary rise may result in wet soil conditions to variable heights above the new water table. Additionally, the topographic situation and/or the climatic environment may mean that drainage merely reduces the period of saturation. If drainage is such that saturation no longer occurs for appropriate periods in the relevant parts of the profile, the soil can strictly no longer be considered a Hydrosol. Possibly a 'drained' phase may be appropriate in some such circumstances.

In the case of irrigated soils, the main example is when more or less permanent flood irrigation is employed to grow rice. This would be expected to change, for example, a Chromosol to a Chromosolic Hydrosol. It should be noted that the definition of the order is deliberately somewhat equivocal in that the duration and frequency of saturation of a precise section of the profile are not specifically defined. Lack of water table data is one reason, but it is also thought that a degree of flexibility is required for the definition. It is recognised that the extent of soil wetness can seldom be assessed by a single inspection of a particular site. However, in the author's experience judicious questioning of people with local knowledge, together with the soil scientist's assessment of soil and site drainage and climatic environment, can usually achieve a satisfactory resolution of the problem.""" ;
  owl:versionInfo "Version 1 (1996)" ;
  skos:definition "Soils other than Organosols, Podosols and Vertosols in which the greater part of the profile is saturated for at least 2-3 months in most years." ;
  skos:inScheme asc: ;
  skos:notation "HY" ;
  skos:note "Seasonally or permanently wet soils" ;
  skos:prefLabel "Hydrosols" ;
.
asc:KA
  rdf:type soil:Order ;
  rdf:type skos:Concept ;
  dcterms:description """Structureless soils

This order accommodates those soils which lack strong texture contrast, have massive or only weakly structured B horizons, and are not calcareous throughout. The soils of this order range throughout the continent, often occurring locally as very large areas.

Soils other than Hydrosols which have all of the following:
(i) B2 horizons in which the major part is massive or has only a weak grade of structure.
(ii) A maximum clay content in some part of the B2 horizon which exceeds 15% (ie. heavy sandy loam, SL+).
(iii) Do not have a tenic B horizon.
(iv) Do not have clear or abrupt textural B horizons.
(v) Are not calcareous throughout the solum, or below the A1 or Ap horizon or to a depth of 0.2m if the A1 horizon is only weakly developed.""" ;
  rdfs:comment """This order accommodates those soils which lack strong texture contrast, have massive or only weakly structured B horizons, and are not calcareous throughout. The soils of this order range throughout the continent, often occurring locally as very large areas.

Because of the lack of clearly defined horizons in some of these soils (particularly the red forms) with thick sola, there can be argument as to how to identify the limits of the B2 horizon.

As noted under Tenosols (see Comment following Definition), there may also be difficulty in deciding whether B horizon development is strong enough for the soil to be classed as a Kandosol, or is only weak and better classed as a tenic B horizon.""" ;
  owl:versionInfo "Version 1 (1996)" ;
  skos:definition """Soils other than Hydrosols which have all of the following:
(i) B2 horizons in which the major part is massive or has only a weak grade of structure.
(ii) A maximum clay content in some part of the B2 horizon which exceeds 15% (ie. heavy sandy loam, SL+).
(iii) Do not have a tenic B horizon.
(iv) Do not have clear or abrupt textural B horizons.
(v) Are not calcareous throughout the solum, or below the A1 or Ap horizon or to a depth of 0.2m if the A1 horizon is only weakly developed.""" ;
  skos:inScheme asc: ;
  skos:notation "KA" ;
  skos:note "Structureless soils" ;
  skos:prefLabel "Kandosols" ;
.
asc:KU
  rdf:type soil:Order ;
  rdf:type skos:Concept ;
  dcterms:description "Soils with strong texture contrast between A horizons and strongly acid B horizons. Many of these soils have some unusual subsoil chemical features (high magnesium, sodium and aluminium)." ;
  rdfs:comment """Soils with strong texture contrast between A horizons and strongly acid B horizons. Many of these soils have some unusual subsoil chemical features (high magnesium, sodium and aluminium).

The relevance of sodicity in strongly acid soils is open to question as in theory the presence of aluminium in such soils should counterbalance the usual deleterious effect of sodium (via dispersion) on soil physical properties. Unpublished data from many localities in Australia imply that for B horizons the critical limits of pH 5.5 and ESP of 6 to distinguish dispersive and non-dispersive soils seems to generally work in practice, although as might be expected, some soils do not behave as predicted. For this reason, sodicity is also used in Kurosols, but at a lower hierarchical level, to cater for those soils which have an ESP > 6 and may disperse in spite of having a pH less than 5.5. The role of the high exchangeable magnesium in many Kurosols is largely unknown.""" ;
  owl:versionInfo "Version 1 (1996)" ;
  skos:definition "Soils other than Hydrosols with a clear or abrupt textural B horizon and in which the major part of the upper 0.2 m of the B2 horizon (or the major part of the entire B2 horizon if it is less than 0.2 m thick) is strongly acid." ;
  skos:inScheme asc: ;
  skos:notation "KU" ;
  skos:note "Acidic soils with an abrupt increase in clay" ;
  skos:prefLabel "Kurosols" ;
.
asc:OR
  rdf:type soil:Order ;
  rdf:type skos:Concept ;
  dcterms:description """Soils that are not regularly inundated by saline tidal waters and either:(i) Have more than 0.4 m of organic materials within the upper 0.8 m. The required thickness may either extend down from the surface or be taken cumulatively within the upper 0.8 m. or
(ii) Have organic materials extending from the surface to a minimum depth of 0.1 m; these either directly overlie rock or other hard layers, partially weathered or decomposed rock or saprolite, or overlie fragmental material such as gravel, cobbles or stones in which the interstices are filled or partially filled with organic material. In some soils there may be layers of humose and/or melacic horizon material underlying the organic materials and overlying the substrate.""" ;
  rdfs:comment """This class caters for most soils dominated by organic materials. Although they are found from the wet tropics to the alpine regions, areas are mostly small except in south west Tasmania. There have been few previous attempts to subdivide these soils and data are limited in Australia.

The above definition is similar to definitions of organic soils in Soil Taxonomy (1975) and in Canada (Canada Soil Survey Committee 1978).""" ;
  owl:versionInfo "Version 1 (1996)" ;
  skos:definition """Soils that are not regularly inundated by saline tidal waters and either:
(i) Have more than 0.4 m of organic materials within the upper 0.8 m. The required thickness may either extend down from the surface or be taken cumulatively within the upper 0.8 m. or
(ii) Have organic materials extending from the surface to a minimum depth of 0.1 m; these either directly overlie rock or other hard layers, partially weathered or decomposed rock or saprolite, or overlie fragmental material such as gravel, cobbles or stones in which the interstices are filled or partially filled with organic material. In some soils there may be layers of humose and/or melacic horizon material underlying the organic materials and overlying the substrate.""" ;
  skos:inScheme asc: ;
  skos:notation "OR" ;
  skos:note "Organic soils" ;
  skos:prefLabel "Organosols" ;
.
asc:PO
  rdf:type soil:Order ;
  rdf:type skos:Concept ;
  rdfs:comment """Soils with B horizons dominated by the accumulation of compounds of organic matter, aluminium and/or iron. These soils are recognised world-wide, and Australia is particularly noted for its 'giant' forms.

Extensive revisions of the classification of Spodosols and podzols have recently taken place in the USA (with world-wide input) and New Zealand. It is clear that there is considerable diversity of opinion on the desirability, nature and efficacy of chemical criteria to define Spodosols/podzols. For this reason the present proposal for Australian 'podzols' has deliberately avoided the use of chemical diagnostic criteria. It is realised that problems may arise in distinguishing a Bs horizon from a tenic B horizon; the diagnostic feature of the former is the presence of discontinuous patches or a thin band of darker organic accumulations.""" ;
  owl:versionInfo "Version 1 (1996)" ;
  skos:definition "Soils which possess either a Bs horizon (visible dominance of iron compounds), a Bhs horizon (organic-aluminium and iron compounds), or a Bh horizon (organic-aluminium compounds). These horizons may occur singly in a profile or in combination (see Podosol diagnostic horizons)." ;
  skos:inScheme asc: ;
  skos:notation "PO" ;
  skos:note "Organic materials and aluminium, with or without iron" ;
  skos:prefLabel "Podosols" ;
.
asc:RU
  rdf:type soil:Order ;
  rdf:type skos:Concept ;
  rdfs:comment """This order is designed to accommodate soils that have negligible pedologic organisation. They are usually young soils in the sense that soil forming factors have had little time to pedologically modify parent rocks or sediments. The component soils can obviously vary widely in terms of texture and depth; many are stratified and some are highly saline. Data on some of them are very limited.

By definition, these soils will grade to Tenosols, so before deciding on the order check the Tenosol definition as it will often be a matter of judgement as to which order a particular soil is best placed. Hydrosols are excluded on the basis that these will normally show some pedological development eg. mottling. A particular problem with the definition and subdivision of Rudosols is the difficulty in distinguishing between soil and 'non-soil', (see also 'What do we classify?'). In many instances they are classified on the basis of the nature of AC or C horizon materials or other substrates because these are the dominating features of the profile. It also follows that there may be difficulties in deciding if a soil is best classified as an Anthroposol or be regarded as an ‘anthropic’ Rudosol because the little-altered soil parent material may be human-made.""" ;
  rdfs:label "RU" ;
  owl:versionInfo "Version 1 (1996)" ;
  skos:definition "Soil with negligible (rudimentary) pedologic organisation apart from (a) minimal development of an Al horizon or (b) the presence of less than 10% of B horizon material (including pedogenic carbonate) in fissures in the parent rock or saprolite. The soils are apedal or only weakly structured in the A1 horizon and show no pedological colour changes apart from the darkening of an A1 horizon. There is little or no texture or colour change with depth unless stratified or buried soils are present." ;
  skos:inScheme asc: ;
  skos:note "Minimal soil development" ;
  skos:prefLabel "Rudosols" ;
.
asc:SO
  rdf:type soil:Order ;
  rdf:type skos:Concept ;
  dcterms:description """Soils with strong texture contrast between A horizons and sodicB horizons which are not strongly acid. Australia is noteworthy for the extent and diversity of sodic soils and the use of sodicity in Australian soil classification systems has recently been reviewed (Isbell, 1995).

Soils with a clear or abrupt textural B horizon and in which the major part of the upper 0.2 m of the B2 horizon (or the major part of the entire B2 horizon if it is less than 0.2m thick) is sodic and not strongly acid. Hydrosols and soils with strongly subplastic upper B2 horizons are excluded.""" ;
  rdfs:comment """Soils with strong texture contrast between A horizons and sodicB horizons which are not strongly acid. Australia is noteworthy for the extent and diversity of sodic soils and the use of sodicity in Australian soil classification systems has recently been reviewed (Isbell, 1995).

There is convincing evidence from the Riverine Plain of south eastern Australia that soils with sodic clay B horizons (ESP 25-30) which are strongly subplastic behave very differently in terms of permeability to the more commonly found plastic sodic clay B horizons which are characterised by low to very low saturated hydraulic conductivity (McIntyre 1979). It is on this basis that subplastic sodic soils are excluded from Sodosols, because of their very different land use properties.

Strongly acid sodic soils are also excluded from Sodosols because they usually contain appreciable exchangeable aluminium (KC1 extractable) and thus should be unlikely to disperse.

It is usually possible to assess, in the field, the likelihood of a soil possessing a sodic B2 horizon. Such a criterion as the presence of a bleached A2 horizon with an abrupt change to a B2 horizon which has columnar or prismatic structure is a useful but not universal guide. A high pH value (>8.5) suggests sodicity, but the converse is not true. The soapy nature of the bolus produced in field texturing will also often suggest appreciable sodium (and/or magnesium) on the clay exchange complex.

Increasing experience in many parts of Australia is confirming that the Emerson dispersion test (Emerson 1967) and the modified version of Loveday and Pyle (1973) is a reliable guide to sodicity. It can be carried out as a preliminary test in the field, but should always be repeated under the better controlled conditions of the laboratory. In the initial test at least several fragments (each about 0.2 g or about 4 -5 mm diameter) are immersed in 100 ml of distilled water. The large water:soil ratio is necessary to remove any salt present in the aggregate. Also for this reason Emerson (1991) suggests that the classification for each test be made after 24 hours. For the remoulded test, use a 5 mm cube which can be obtained from the bolus used for determining field texture. This will be approximately in the plastic limit condition. Note that distilled water should be used to prepare the bolus.

Data from Loveday and Pyle (1973) and unpublished data available to the author suggest that a dispersive soil will usually indicate sodicity, ie. ESP of 6 or greater. The data of Murphy (1995) indicate that whereas Emerson class 1 and the more strongly dispersive soils of class 2 are a reliable indicator of sodicity, class 3 is a more variable predictor. Emerson classes of 5 or greater or a Loveday and Pyle score of zero strongly suggest soils are non-sodic. There is less evidence that the dispersion tests give a reliable indication of the degree of sodicity; factors such as extent of initial slaking and initial salt content in the aggregates, and the amount of magnesium and amount and form of aluminium on the exchange complex (Emerson 1994), can also influence the rapidity of dispersion. Nevertheless, the data of Loveday and Pyle measuring dispersion after 2 hours and 20 hours showed that the rate of dispersion could be used as a guide to ESP. This relationship does not apply to the subplastic soils of the Riverine Plain where subsoils with an ESP of 25-30 do not disperse unless remoulded (Blackmore 1976). Other anomalous results occur in a small minority of normal plastic soils in which dispersion will not occur even after remoulding in spite of an ESP much greater than 6 and a pH as high as neutral. In at least some of these non-dispersive soils the typical sodic soil morphology is present, ie. a conspicuously bleached A2 horizon abruptly overlying a B2 horizon with prismatic or columnar structure, suggesting the low hydraulic conductivity expected of a sodicB horizon.""" ;
  owl:versionInfo "Version 1 (1996)" ;
  skos:definition "Soils with a clear or abrupt textural B horizon and in which the major part of the upper 0.2 m of the B2 horizon (or the major part of the entire B2 horizon if it is less than 0.2m thick) is sodic and not strongly acid. Hydrosols and soils with strongly subplastic upper B2 horizons are excluded." ;
  skos:inScheme asc: ;
  skos:notation "SO" ;
  skos:note "Soils high in sodium and an abrupt increase in clay" ;
  skos:prefLabel "Sodosols" ;
.
asc:TE
  rdf:type soil:Order ;
  rdf:type skos:Concept ;
  dcterms:description """Weakly developed soils

This order is designed to embrace soils with generally only weak pedologic organisation apart from the A horizons. It encompasses a rather diverse range of soils, which are nevertheless widespread in many parts of Australia.

Soils that do not fit the requirements of any other soil orders and generally with one or more of the following:
(i) A peaty horizon.
(ii) A humose, melacic or melanic horizon, or conspicuously bleached A2 horizon, which overlies a calcrete pan, hard unweathered rock or other hard materials; or partially weathered or decomposed rock or saprolite, or unconsolidated mineral materials.
(iii) A horizons which meet all the conditions for a peaty, humose, melacic or melanic horizon except the depth requirement, and directly overlie a calcrete pan, hard unweathered rock or other hard materials; or partially weathered or decomposed rock or saprolite, or unconsolidated mineral materials.
(iv) A1 horizons which have more than a weak development of structure and directly overlie a calcrete pan, hard unweathered rock or other hard materials; or partially weathered or decomposed rock or saprolite, or unconsolidated mineral materials.
(v) An A2 horizon which overlies a calcrete pan, hard unweathered rock or other hard materials; or partially weathered or decomposed rock or saprolite, or unconsolidated mineral materials.
(vi) Either a tenic B horizon, or a B2 horizon with 15% clay (SL) or less1 , or a transitional horizon (C/B) occurring in fissures in the parent rock or saprolite which contains between 10 and 50% of B horizon material (including pedogenic carbonate).
(vii) A ferric or bauxitic horizon >0.2 m thick.
(viii) A calcareous horizon >0.2 m thick.with one or more of the following""" ;
  rdfs:comment """This order is designed to embrace soils with generally only weak pedologic organisation apart from the A horizons. It encompasses a rather diverse range of soils, which are nevertheless widespread in many parts of Australia.

It may be desirable to specify a minimum thickness for those A1 horizons which do not meet the requirements for a peaty, humose, melacic or melanic horizon. The inclusion of certain soils with conspicuously bleached A2 horizons may be questioned by some, but it is difficult to find a more appropriate place for them.

The Tenosols will differ from Rudosols by virtue of having either a more than weakly developed A1 horizon, an A2, or a weakly developed B horizon. As B horizons are difficult to identify consistently in some Tenosols, specific mention of a B horizon is omitted from some Suborders. They will obviously grade to Kandosols, and some difficulty may be experienced in separating medium-textured Tenosols from Kandosols. Here again, B horizon development is the key; Kandosols must have a clearly distinguishable, well-developed B2 horizon with more than 15% clay. Tenosols will also grade to Podosols, but the latter must have a Podosol diagnostic B horizon. In cold, wet environments, some Tenosols with peaty A horizons will grade to Organosols.

This revised edition of the Australian Soil Classification includes three major changes to the Tenosol order. First, the Calcenic suborder has been added to cover soils with non-calcareous A horizons, more than 0.2m thick, with highly calcareous sub-surface horizons, which fail to classify as Kandosols due to insufficient clay content (>15% clay is needed for Kandosols). Second, the former Orthic suborder has been split to include soil colour. Finally, the Sesqui-Nodular suborder has been added to bring together soils dominated by bauxitic or ferric nodules or concretions.""" ;
  owl:versionInfo "Version 1 (1996)" ;
  skos:definition """Soils that do not fit the requirements of any other soil orders and generally with one or more of the following:
(i) A peaty horizon.
(ii) A humose, melacic or melanic horizon, or conspicuously bleached A2 horizon, which overlies a calcrete pan, hard unweathered rock or other hard materials; or partially weathered or decomposed rock or saprolite, or unconsolidated mineral materials.
(iii) A horizons which meet all the conditions for a peaty, humose, melacic or melanic horizon except the depth requirement, and directly overlie a calcrete pan, hard unweathered rock or other hard materials; or partially weathered or decomposed rock or saprolite, or unconsolidated mineral materials.
(iv) A1 horizons which have more than a weak development of structure and directly overlie a calcrete pan, hard unweathered rock or other hard materials; or partially weathered or decomposed rock or saprolite, or unconsolidated mineral materials.
(v) An A2 horizon which overlies a calcrete pan, hard unweathered rock or other hard materials; or partially weathered or decomposed rock or saprolite, or unconsolidated mineral materials.
(vi) Either a tenic B horizon, or a B2 horizon with 15% clay (SL) or less1 , or a transitional horizon (C/B) occurring in fissures in the parent rock or saprolite which contains between 10 and 50% of B horizon material (including pedogenic carbonate).
(vii) A ferric or bauxitic horizon >0.2 m thick.
(viii) A calcareous horizon >0.2 m thick.with one or more of the following""" ;
  skos:inScheme asc: ;
  skos:notation "TE" ;
  skos:note "Weakly developed soils" ;
  skos:prefLabel "Tenosols" ;
.
asc:VE
  rdf:type soil:Order ;
  rdf:type skos:Concept ;
  rdfs:comment """Clay soils with shrink-swell properties that exhibit strong cracking when dry and at depth have slickensides and/or lenticular structural aggregates. Although many soils exhibit gilgai microrelief, this feature is not used in their definition. Australia has the greatest area and diversity of cracking clay soils of any country in the world.

In some clay soils it may be difficult to decide if sufficient cracks are present, or at the time of inspection the soil may be too moist to exhibit cracking. Also, in arid zone clay soils which commonly have high salt contents, the soil structure may be so fine and strong granular, or 'puffy', that it is difficult to decide if cracks are present or not. In such soils it is also obviously difficult to discern slickensides or lenticular peds. In yet other clay soils (up to 50% clay or more) cracks may develop but slickensides and lenticular peds are apparently not present.

Because cracking, slickensides and lenticular peds are essentially used as evidence to indicate shrink-swell behaviour, it is desirable that surrogate measurements be available if the morphological evidence is lacking or cannot be determined. See Vertic properties.""" ;
  owl:versionInfo "Version 1 (1996)" ;
  skos:definition """Soils with the following:
(i) A clay field texture or 35% or more clay throughout the solum except for thin, surface crusty horizons 0.03 m or less thick and.
(ii) When dry, open cracks occur at some time in most years1. These are at least 5 mm wide and extend upward to the surface or to the base of any plough layer, peaty horizon, self-mulching horizon, or thin, surface crusty horizon; and
(iii) Slickensides and/or lenticular peds occur at some depth in the solum. See Comment.""" ;
  skos:inScheme asc: ;
  skos:notation "VE" ;
  skos:note "Shrink and swell clay soils" ;
  skos:prefLabel "Vertosols" ;
.
